@prefix : <https://w3id.org/italia/onto/HER/> .
@prefix dc: <http://purl.org/dc/elements/1.1/> .
@prefix l0: <https://w3id.org/italia/onto/l0/> .
@prefix ti: <https://w3id.org/italia/onto/TI/> .
@prefix dct: <http://purl.org/dc/terms/> .
@prefix owl: <http://www.w3.org/2002/07/owl#> .
@prefix rdf: <http://www.w3.org/1999/02/22-rdf-syntax-ns#> .
@prefix xml: <http://www.w3.org/XML/1998/namespace> .
@prefix xsd: <http://www.w3.org/2001/XMLSchema#> .
@prefix dcat: <http://www.w3.org/ns/dcat#> .
@prefix foaf: <http://xmlns.com/foaf/0.1/> .
@prefix prov: <http://www.w3.org/ns/prov#> .
@prefix rdfs: <http://www.w3.org/2000/01/rdf-schema#> .
@prefix skos: <http://www.w3.org/2004/02/skos/core#> .
@prefix vcard: <http://www.w3.org/2006/vcard/ns#> .
@prefix covapit: <https://w3id.org/italia/onto/COV/> .
@prefix admsapit: <https://w3id.org/italia/onto/ADMS/> .
@prefix dcatapit: <http://dati.gov.it/onto/dcatapit#> .
@base <https://w3id.org/italia/onto/HER> .

<https://w3id.org/italia/onto/HER> rdf:type owl:Ontology ;
                                    owl:versionIRI <https://w3id.org/italia/onto/HER/0.3> ;
                                    owl:imports <https://w3id.org/italia/onto/CPV> ,
                                                <https://w3id.org/italia/onto/Project> ,
                                                <https://w3id.org/italia/onto/l0> ;
                                    dct:accrualPeriodicity <http://publications.europa.eu/resource/authority/frequency/IRREG> ;
                                    dct:creator <https://w3id.org/italia/data/public-organization/agid> ,
                                                <https://w3id.org/italia/data/public-organization/r_toscan> ,
                                                <https://w3id.org/italia/datq/private-organization/siris> ,
                                                <https://w3id.org/italia/datq/private-organization/03033080213> ;
                                    dct:description "Questa è l'ontologia del profilo di italiano sull'alta formazione, ricerca e innovazione. Essa nasce come versione per OntoPiA dell'ontologia sviluppata nell'ambito del progetto Toscana Open Research (http://www.toscanaopenresearch.it/) disponibile in https://ontology-documentation-toscana-public.s3-eu-west-1.amazonaws.com/index.html#unics_miur_scholars"@it ,
                                                    "This is the ontology of the Italian application profile for Higher Education and Research. It is born as the OntoPiA's version of the ontology already developed in the context of Toscana Open Research Project (http://www.toscanaopenresearch.it/en/) and available in https://ontology-documentation-toscana-public.s3-eu-west-1.amazonaws.com/index.html#unics_miur_scholars"@en ;
                                    dct:issued "2020-04-02"^^xsd:date ;
                                    dct:language <http://publications.europa.eu/resource/authority/language/ENG> ,
                                                 <http://publications.europa.eu/resource/authority/language/ITA> ;
                                    dct:modified "2020-10-14"@en ;
                                    dct:publisher <https://w3id.org/italia/data/public-organization/agid> ;
                                    dct:rightsHolder <https://w3id.org/italia/data/public-organization/r_toscan> ;
                                    dct:title "Higher Education and Research Ontology"@en ,
                                              "Ontologia sull'Alta Formazione, Ricerca e Innovazione"@it ;
                                    rdfs:comment "Questa è l'ontologia del profilo di italiano sull'alta formazione, ricerca e innovazione. Essa nasce come versione per OntoPiA dell'ontologia sviluppata nell'ambito del progetto Toscana Open Research (http://www.toscanaopenresearch.it/) disponibile in https://ontology-documentation-toscana-public.s3-eu-west-1.amazonaws.com/index.html#unics_miur_scholars"@it ,
                                                 "This is the ontology of the Italian application profile for Higher Education and Research. It is born as the OntoPiA's version of the ontology already developed in the context of Toscana Open Research Project (http://www.toscanaopenresearch.it/en/) and available in https://ontology-documentation-toscana-public.s3-eu-west-1.amazonaws.com/index.html#unics_miur_scholars"@en ;
                                    rdfs:isDefinedBy <https://w3id.org/italia/onto/HER> ;
                                    rdfs:label "Higher Education and Research Ontology"@en ,
                                               "Ontologia dell'Alta Formazione, Ricerca e Innovazione"@it ;
                                    owl:versionInfo "Version 0.3 in OntoPiA"@en ,
                                                    "Versione 0.3 in OntoPiA"@it ;
                                    dcat:contactPoint <https://w3id.org/italia/data/contact-point/onto-agid> ;
                                    dcat:keyword "Peronale universitario"@it ,
                                                 "Progetti di ricerca"@it ,
                                                 "Public Research"@en ,
                                                 "Research Projects"@en ,
                                                 "Ricerca pubblica"@it ,
                                                 "Student"@en ,
                                                 "Studenti"@it ;
                                    dcat:theme <http://publications.europa.eu/resource/authority/data-theme/EDUC> ;
                                    prov:wasDerivedFrom <https://w3id.org/italia/onto/HER/0.1> ;
                                    admsapit:acronym "HER-AP_IT" ;
                                    admsapit:hasFormalityLevel admsapit:Formal ;
                                    admsapit:hasKeyClass :PublicResearchProject ;
                                    admsapit:hasOntologyLanguage admsapit:OWL ;
                                    admsapit:hasSemanticAssetDistribution <https://w3id.org/italia/data/distribution/HERAPIT-JSON-LD> ,
                                                                          <https://w3id.org/italia/data/distribution/HERAPIT-RDF-TURTLE> ,
                                                                          <https://w3id.org/italia/data/distribution/HERAPIT-RDF-XML> ;
                                    admsapit:hasTask admsapit:AnnotationTask ,
                                                     admsapit:QueryFormulationTask ,
                                                     admsapit:SearchTask ;
                                    admsapit:last <https://w3id.org/italia/onto/CLV/1.0> ,
                                                  <https://w3id.org/italia/onto/HER/0.2> ;
                                    admsapit:officialURI "https://w3id.org/italia/onto/HER"^^xsd:anyURI ;
                                    admsapit:prefix "herapit" ;
                                    admsapit:semanticAssetInUse <https://w3id.org/italia/data/project/OntoPiA> ,
                                                                <https://w3id.org/italia/data/project/toscana-open-research> ;
                                    admsapit:status "draft" ;
                                    admsapit:target "Imprese" ,
                                                    "Pubbliche Amministrazioni" ;
                                    admsapit:type admsapit:DomainOntology .

#################################################################
#    Annotation properties
#################################################################

###  http://purl.org/dc/terms/accrualPeriodicity
dct:accrualPeriodicity rdf:type owl:AnnotationProperty .


###  http://purl.org/dc/terms/language
dct:language rdf:type owl:AnnotationProperty .


###  http://purl.org/dc/terms/publisher
dct:publisher rdf:type owl:AnnotationProperty .


###  http://purl.org/dc/terms/rightsHolder
dct:rightsHolder rdf:type owl:AnnotationProperty .


###  http://www.w3.org/2002/07/owl#maxQualifiedCardinality
owl:maxQualifiedCardinality rdf:type owl:AnnotationProperty .


###  http://www.w3.org/ns/dcat#contactPoint
dcat:contactPoint rdf:type owl:AnnotationProperty .


###  http://www.w3.org/ns/dcat#keyword
dcat:keyword rdf:type owl:AnnotationProperty .


###  http://www.w3.org/ns/dcat#theme
dcat:theme rdf:type owl:AnnotationProperty .


###  https://w3id.org/italia/onto/ADMS/acronym
admsapit:acronym rdf:type owl:AnnotationProperty .


###  https://w3id.org/italia/onto/ADMS/hasFormalityLevel
admsapit:hasFormalityLevel rdf:type owl:AnnotationProperty .


###  https://w3id.org/italia/onto/ADMS/hasKeyClass
admsapit:hasKeyClass rdf:type owl:AnnotationProperty .


###  https://w3id.org/italia/onto/ADMS/hasOntologyLanguage
admsapit:hasOntologyLanguage rdf:type owl:AnnotationProperty .


###  https://w3id.org/italia/onto/ADMS/hasSemanticAssetDistribution
admsapit:hasSemanticAssetDistribution rdf:type owl:AnnotationProperty .


###  https://w3id.org/italia/onto/ADMS/hasTask
admsapit:hasTask rdf:type owl:AnnotationProperty .


###  https://w3id.org/italia/onto/ADMS/last
admsapit:last rdf:type owl:AnnotationProperty .


###  https://w3id.org/italia/onto/ADMS/officialURI
admsapit:officialURI rdf:type owl:AnnotationProperty .


###  https://w3id.org/italia/onto/ADMS/prefix
admsapit:prefix rdf:type owl:AnnotationProperty .


###  https://w3id.org/italia/onto/ADMS/semanticAssetInUse
admsapit:semanticAssetInUse rdf:type owl:AnnotationProperty .


###  https://w3id.org/italia/onto/ADMS/target
admsapit:target rdf:type owl:AnnotationProperty .


###  https://w3id.org/italia/onto/ADMS/type
admsapit:type rdf:type owl:AnnotationProperty .


#################################################################
#    Object Properties
#################################################################

###  https://w3id.org/italia/onto/COV/hasOrganization
covapit:hasOrganization rdf:type owl:ObjectProperty .


###  https://w3id.org/italia/onto/COV/hasPublicOrganization
covapit:hasPublicOrganization rdf:type owl:ObjectProperty .


###  https://w3id.org/italia/onto/CPV/hasSex
<https://w3id.org/italia/onto/CPV/hasSex> rdf:type owl:ObjectProperty .


###  https://w3id.org/italia/onto/HER/IsPrincipalInvestigatorOf
:IsPrincipalInvestigatorOf rdf:type owl:ObjectProperty ;
                           owl:inverseOf :hasPrincipalInvestigator ;
                           rdfs:domain <https://w3id.org/italia/onto/CPV/Person> ;
                           rdfs:range <https://w3id.org/italia/onto/Project/PublicResearchProject> ;
                           rdfs:comment "Inverse property of hasPrincipalInvestigator"@en ,
                                        "Proprietà inversa di ha esaminatore principale"@it ;
                           rdfs:isDefinedBy <https://w3id.org/italia/onto/HER> ;
                           rdfs:label "is principal investigator of"@en ,
                                      "è esaminatore principale di"@it ;
                           owl:versionInfo "provvisoria - da verificare bene la descrizione"@it ,
                                           "unstable"@en .


###  https://w3id.org/italia/onto/HER/allocatesFundsTo
:allocatesFundsTo rdf:type owl:ObjectProperty ;
                  rdfs:domain :CTNPRINOperation ;
                  rdfs:range :CTNPRINEntity ;
                  rdfs:comment "Indica i soggetti beneficiari dell'iniziativa."@it ,
                               "Indicates the subjects benefiting from the initiative."@en ;
                  rdfs:isDefinedBy <https://w3id.org/italia/onto/HER> ;
                  rdfs:label "allocates funds to"@en ,
                             "fondi stanziati a"@it ;
                  owl:versionInfo "provvisoria"@it ,
                                  "unstable"@en .


###  https://w3id.org/italia/onto/HER/definedIn
:definedIn rdf:type owl:ObjectProperty ;
           rdfs:domain :AcademicAffiliation ;
           rdfs:range covapit:Organization ;
           rdfs:comment "Collega l'affiliazione accademica con l'organizzazione corrispondente"@it ,
                        "Connects the academic affiliation with the corresponding organization"@en ;
           rdfs:isDefinedBy <https://w3id.org/italia/onto/HER> ;
           rdfs:label "defined in"@en ,
                      "definito in"@it ;
           owl:versionInfo "stabile"@it ,
                           "stable"@en .


###  https://w3id.org/italia/onto/HER/distributedInErasumplusFile
:distributedInErasumplusFile rdf:type owl:ObjectProperty ;
                             rdfs:domain :ErasmusPlusProjectResult ;
                             rdfs:range :ErasmusPlusFile ;
                             rdfs:comment "It is used to link the output result of an erasmus plus project to the associated file."@en ,
                                          "Viene utilizzato per collegare il risultato di un progetto erasmus plus al file associato."@it ;
                             rdfs:isDefinedBy <https://w3id.org/italia/onto/HER> ;
                             rdfs:label "distribuito in un file eramsus+"@it ,
                                        "distributed in erasmus+ file"@en ;
                             owl:versionInfo "stabile"@it ,
                                             "stable"@en .


###  https://w3id.org/italia/onto/HER/forChafeaProject
:forChafeaProject rdf:type owl:ObjectProperty ;
                  rdfs:subPropertyOf <https://w3id.org/italia/onto/RO/forEntity> ;
                  rdfs:domain :CHAFEAParticipant ;
                  rdfs:range :CHAFEAProject ;
                  rdfs:comment "Questa proprietà si collega ad una delle corrispondenti attività finanziate."@it ,
                               "This property links to one of the corresponding funded activities."@en ;
                  rdfs:isDefinedBy <https://w3id.org/italia/onto/HER> ;
                  rdfs:label "ha un progetto chafea"@it ,
                             "has chafea project"@en .


###  https://w3id.org/italia/onto/HER/forECProject
:forECProject rdf:type owl:ObjectProperty ;
              rdfs:subPropertyOf <https://w3id.org/italia/onto/RO/forEntity> ;
              rdfs:domain :ECParticipant ;
              rdfs:range [ rdf:type owl:Class ;
                           owl:unionOf ( :ECProject
                                         :ERCProject
                                       )
                         ] ;
              rdfs:comment "Questa proprietà si collega ad un corrispondente progetto della CE."@it ,
                           "This property links to a corresponding EC project."@en ;
              rdfs:isDefinedBy <https://w3id.org/italia/onto/HER> ;
              rdfs:label "ha un progetto CE"@it ,
                         "has ec project"@en .


###  https://w3id.org/italia/onto/HER/forEurekaProject
:forEurekaProject rdf:type owl:ObjectProperty ;
                  rdfs:subPropertyOf <https://w3id.org/italia/onto/RO/forEntity> ;
                  rdfs:domain :EUREKAParticipant ;
                  rdfs:range :EUREKAProject ;
                  rdfs:comment "Questa proprietà collega un partecipante al corrispondente progetto EUREKA."@it ,
                               "This property connects a participant with the corresponding EUREKA project."@en ;
                  rdfs:isDefinedBy <https://w3id.org/italia/onto/HER> ;
                  rdfs:label "partecipa in progetto eureka"@it ,
                             "participates in eureka project"@en ;
                  owl:versionInfo "provvisoria"@it ,
                                  "unstable"@en .


###  https://w3id.org/italia/onto/HER/foundedBy
:foundedBy rdf:type owl:ObjectProperty ;
           rdfs:domain :Spinoff ;
           rdfs:range covapit:Organization ;
           rdfs:comment "It is used to link the spin-off to the research institution or university of origin, to which its foundation is linked."@en ,
                        "Viene utilizzato per collegare lo spin-off all'ente di ricerca o ateneo di origine, a cui è collegata la sua fondazione."@it ;
           rdfs:isDefinedBy <https://w3id.org/italia/onto/HER> ;
           rdfs:label "fondata da"@it ,
                      "founded by"@en ;
           owl:versionInfo "stabile"@it ,
                           "stable"@en .


###  https://w3id.org/italia/onto/HER/hasAACTCondition
:hasAACTCondition rdf:type owl:ObjectProperty ;
                  rdfs:domain :AACTStudy ;
                  rdfs:range :AACTCondition ;
                  rdfs:comment "La malattia, il disturbo, la sindrome, la malattia o la lesione che si sta studiando. Su ClinicalTrials.gov, le condizioni possono includere anche altre questioni relative alla salute, come la durata della vita, la qualità della vita e i rischi per la salute."@it ,
                               "The disease, disorder, syndrome, illness, or injury that is being studied. On ClinicalTrials.gov, conditions may also include other health-related issues, such as lifespan, quality of life, and health risks."@en ;
                  rdfs:isDefinedBy <https://w3id.org/italia/onto/HER> ;
                  rdfs:label "ha condizione AACT"@it ,
                             "has AACT condition"@en ;
                  owl:versionInfo "stabile"@it ,
                                  "stable"@en .


###  https://w3id.org/italia/onto/HER/hasAACTConditionMeshTerm
:hasAACTConditionMeshTerm rdf:type owl:ObjectProperty ;
                          rdfs:subPropertyOf :hasAACTMeshTerm ;
                          rdfs:domain :AACTStudy ;
                          rdfs:range :AACTConditionMeshTerm ;
                          rdfs:comment "Il nome o i nomi della malattia o della condizione o delle condizioni studiate nello studio clinico, o il focus dello studio clinico descrittori appropriati da NLM's Medical Subject Headings (MeSH) - thesaurus vocabolario controllato da NLM's Medical Subject Headings (MeSH) - o termini da un altro vocabolario, come la Systematized Nomenclature of Medicine-Clinical Terms (SNOMED CT), che è stato mappato a MeSH all'interno del Metathesaurus Unified Medical Language System (UMLS)."@it ,
                                       "The name(s) of the disease(s) or condition(s) studied in the clinical study, or the focus of the clinical study appropriate descriptors from NLM's Medical Subject Headings (MeSH)-controlled vocabulary thesaurus or terms from another vocabulary, such as the Systematized Nomenclature of Medicine—Clinical Terms (SNOMED CT), that has been mapped to MeSH within the Unified Medical Language System (UMLS) Metathesaurus."@en ;
                          rdfs:isDefinedBy <https://w3id.org/italia/onto/HER> ;
                          rdfs:label "ha termine MeSH di condizione AACT"@it ,
                                     "has AACT condition MeSH term"@en ;
                          owl:versionInfo "stabile"@it ,
                                          "stable"@en .


###  https://w3id.org/italia/onto/HER/hasAACTDesign
:hasAACTDesign rdf:type owl:ObjectProperty ;
               rdfs:domain :AACTStudy ;
               rdfs:range :AACTDesign ;
               rdfs:comment "I metodi di indagine e le strategie utilizzate nello studio clinico. Una descrizione delle modalità di conduzione dello studio clinico"@it ,
                            "The investigative methods and strategies used in the clinical study. A description of the manner in which the clinical trial will be conducted"@en ;
               rdfs:isDefinedBy <https://w3id.org/italia/onto/HER> ;
               rdfs:label "ha sviluppo AACT"@it ,
                          "has AACT design"@en ;
               owl:versionInfo "stabile"@it ,
                               "stable"@en .


###  https://w3id.org/italia/onto/HER/hasAACTEligibility
:hasAACTEligibility rdf:type owl:ObjectProperty ;
                    rdfs:domain :AACTStudy ;
                    rdfs:range :AACTEligibility ;
                    rdfs:comment "I requisiti chiave che le persone che vogliono partecipare a uno studio clinico devono soddisfare o le caratteristiche che devono avere."@it ,
                                 "The key requirements that people who want to participate in a clinical study must meet or the characteristics they must have."@en ;
                    rdfs:isDefinedBy <https://w3id.org/italia/onto/HER> ;
                    rdfs:label "ha idoneitá AACT"@it ,
                               "has AACT eligibility"@en ;
                    owl:versionInfo "stabile"@it ,
                                    "stable"@en .


###  https://w3id.org/italia/onto/HER/hasAACTFacility
:hasAACTFacility rdf:type owl:ObjectProperty ;
                 rdfs:domain :AACTStudy ;
                 rdfs:range :AACTFacility ;
                 rdfs:comment "conduzione del sito/partecipazione ad uno studio"@it ,
                              "site conducting/participating in a study"@en ;
                 rdfs:isDefinedBy <https://w3id.org/italia/onto/HER> ;
                 rdfs:label "ha struttura per sperimentazione clinica"@it ,
                            "has clinical trial facility"@en ;
                 owl:versionInfo "provvisoria - da verificare"@it ,
                                 "unstable - to be verified"@en .


###  https://w3id.org/italia/onto/HER/hasAACTIntervention
:hasAACTIntervention rdf:type owl:ObjectProperty ;
                     rdfs:domain :AACTStudy ;
                     rdfs:range :AACTIntervention ;
                     rdfs:comment "A process or action that is the focus of a clinical study. Interventions include drugs, medical devices, procedures, vaccines, and other products that are either investigational or already available. Interventions can also include noninvasive approaches, such as education or modifying diet and exercise."@en ,
                                  "Un processo o un'azione che è il fulcro di uno studio clinico. Gli interventi comprendono farmaci, dispositivi medici, procedure, vaccini e altri prodotti che sono in fase di sperimentazione o già disponibili. Gli interventi possono anche includere approcci non invasivi, come l'educazione o la modifica della dieta e dell'esercizio fisico."@it ;
                     rdfs:isDefinedBy <https://w3id.org/italia/onto/HER> ;
                     rdfs:label "ha intervento AACT"@it ,
                                "has AACT intervention"@en ;
                     owl:versionInfo "stabile"@it ,
                                     "stable"@en .


###  https://w3id.org/italia/onto/HER/hasAACTInterventionMeshTerm
:hasAACTInterventionMeshTerm rdf:type owl:ObjectProperty ;
                             rdfs:subPropertyOf :hasAACTMeshTerm ;
                             rdfs:domain :AACTStudy ;
                             rdfs:range :AACTInterventionMeshTerm ;
                             rdfs:comment "Clinical study intervention appropriate descriptors from NLM's Medical Subject Headings (MeSH)-controlled vocabulary thesaurus"@en ,
                                          "interventi di studio clinico descritti da NLM's Medical Subject Headings (MeSH) - thesaurus del vocabolario controllato da NLM's Medical Subject Headings (MeSH) - thesaurus del vocabolario"@it ;
                             rdfs:isDefinedBy <https://w3id.org/italia/onto/HER> ;
                             rdfs:label "ha termine MeSH di intervento AACT"@it ,
                                        "has AACT intervention MeSH term"@en ;
                             owl:versionInfo "stabile"@it ,
                                             "stable"@en .


###  https://w3id.org/italia/onto/HER/hasAACTMeshTerm
:hasAACTMeshTerm rdf:type owl:ObjectProperty ;
                 rdfs:domain :AACTStudy ;
                 rdfs:range :AACTMeshTerm ;
                 rdfs:isDefinedBy <https://w3id.org/italia/onto/HER> ;
                 rdfs:label "ha termine MeSH riportato da AACT"@it ,
                            "has AACT reported MeSH term"@en ;
                 owl:versionInfo "provvisoria"@it ,
                                 "unstable"@en .


###  https://w3id.org/italia/onto/HER/hasAACTResponsible
:hasAACTResponsible rdf:type owl:ObjectProperty ;
                    rdfs:domain :AACTStudy ;
                    rdfs:range <https://w3id.org/italia/onto/CPV/Person> ;
                    rdfs:comment "La persona responsabile dell'invio di informazioni su uno studio clinico a ClinicalTrials.gov e dell'aggiornamento di tali informazioni. Di solito lo sponsor dello studio o lo sperimentatore."@it ,
                                 "The person responsible for submitting information about a clinical study to ClinicalTrials.gov and updating that information. Usually the study sponsor or investigator."@en ;
                    rdfs:isDefinedBy <https://w3id.org/italia/onto/HER> ;
                    rdfs:label "ha responsabile AACT"@it ,
                               "has AACT responsible"@en ;
                    owl:versionInfo "stabile"@it ,
                                    "stable"@en .


###  https://w3id.org/italia/onto/HER/hasAACTSponsor
:hasAACTSponsor rdf:type owl:ObjectProperty ;
                rdfs:domain :AACTStudy ;
                rdfs:range :AACTSponsor ;
                rdfs:comment "L'organizzazione o la persona che avvia lo studio e che ha autorità e controllo sullo studio."@it ,
                             "The organization or person who initiates the study and who has authority and control over the study."@en ;
                rdfs:isDefinedBy <https://w3id.org/italia/onto/HER> ;
                rdfs:label "ha sponsor AACT"@it ,
                           "has AACT sponsor"@en ;
                owl:versionInfo "stabile"@it ,
                                "stable"@en .


###  https://w3id.org/italia/onto/HER/hasAACTStudy
:hasAACTStudy rdf:type owl:ObjectProperty ;
              rdfs:domain [ rdf:type owl:Class ;
                            owl:unionOf ( :AACTCondition
                                          :AACTDesign
                                          :AACTEligibility
                                          :AACTMeshTerm
                                          :CountryInvolvement
                                        )
                          ] ;
              rdfs:range :AACTStudy ;
              rdfs:comment "Questa proprietà si collega allo studio corrispondente."@it ,
                           "This property links to the corresponding study."@en ;
              rdfs:isDefinedBy <https://w3id.org/italia/onto/HER> ;
              rdfs:label "ha studio AACT"@it ,
                         "has AACT study"@en ;
              owl:versionInfo "stabile"@it ,
                              "stable"@en .


###  https://w3id.org/italia/onto/HER/hasAcademicDegree
:hasAcademicDegree rdf:type owl:ObjectProperty ;
                   rdfs:domain [ rdf:type owl:Class ;
                                 owl:unionOf ( :ISCEDFClassification
                                               :MIURStudentsByCitizenshipDegreeAggregate
                                               :MIURStudentsByCitizenshipDegreeDegreeClassAggregate
                                               :MIURStudentsByDegreeDegreeClassAggregate
                                               :MIURStudentsByDiplomaDegreeDegreeClassAggregate
                                               :MIURStudentsByProvinceOfResidenceDegreeDegreeClassAggregate
                                               :MIURStudentsByRegionOfResidenceDegreeDegreeClassAggregate
                                             )
                               ] ;
                   rdfs:range :AcademicDegree ;
                   rdfs:comment "Questa proprietà è collegata a un titolo accademico."@it ,
                                "This property links to an academic degree."@en ;
                   rdfs:isDefinedBy <https://w3id.org/italia/onto/HER> ;
                   rdfs:label "ha una laurea"@it ,
                              "has academic degree"@en ;
                   owl:versionInfo "stabile"@it ,
                                   "stable"@en .


###  https://w3id.org/italia/onto/HER/hasAcademicDiscipline
:hasAcademicDiscipline rdf:type owl:ObjectProperty ;
                       rdfs:domain owl:Thing ;
                       rdfs:range :AcademicDiscipline ;
                       rdfs:comment "Questa proprietà consente di collegare qualunque cosa del dominio a discipline accademiche (definite nell'ambito del relativo vocabolario controllato)."@it ,
                                    "This property allows one to link any thing of the domain with the academic disciplines (defined in the context of the related controlled vocabulary)."@en ;
                       rdfs:isDefinedBy <https://w3id.org/italia/onto/HER> ;
                       rdfs:label "ha discipline accademiche"@it ,
                                  "has Academic Discipline"@en ;
                       owl:versionInfo "stabile"@it ,
                                       "stable"@en .


###  https://w3id.org/italia/onto/HER/hasAcademicOrg
:hasAcademicOrg rdf:type owl:ObjectProperty ;
                rdfs:subPropertyOf covapit:hasPublicOrganization ;
                rdfs:domain [ rdf:type owl:Class ;
                              owl:unionOf ( :ItalianPhDCourseByCycle
                                            :MIURStudentsAggregate
                                            :MIURStudentsByCitizenshipAggregate
                                            :MIURStudentsByCitizenshipDegreeAggregate
                                            :MIURStudentsByCitizenshipDegreeClassAggregate
                                            :MIURStudentsByCitizenshipDegreeDegreeClassAggregate
                                            :MIURStudentsByDegreeDegreeClassAggregate
                                            :MIURStudentsByDiplomaAggregate
                                            :MIURStudentsByDiplomaDegreeDegreeClassAggregate
                                            :MIURStudentsByProvinceOfResidenceAggregate
                                            :MIURStudentsByProvinceOfResidenceDegreeDegreeClassAggregate
                                            :MIURStudentsByRegionOfResidenceAggregate
                                            :MIURStudentsByRegionOfResidenceDegreeDegreeClassAggregate
                                          )
                            ] ;
                rdfs:range covapit:PublicOrganization ;
                rdfs:comment "Questa proprietà si collega diversi dati statistici a un'organizzazione accademica."@it ,
                             "This property links different statistical data to an academic Organization."@en ;
                rdfs:isDefinedBy <https://w3id.org/italia/onto/HER> ;
                rdfs:label "ha organizzazione accademica"@it ,
                           "has academic organization"@en ;
                owl:versionInfo "provvisoria"@it ,
                                "unstable"@en .


###  https://w3id.org/italia/onto/HER/hasAcademicRole
:hasAcademicRole rdf:type owl:ObjectProperty ;
                 rdfs:domain :ResearcherSeniorityGrade ;
                 rdfs:range [ rdf:type owl:Class ;
                              owl:unionOf ( :AcademicRole
                                            :ItalianAcademicRole
                                          )
                            ] ;
                 rdfs:comment "Connects a ReseacherSeniorityGrade with the corresponding AcademicRole."@en ,
                              "Connette un ReseacherSeniorityGrade al corrispondente AcademicRole."@it ;
                 rdfs:isDefinedBy <https://w3id.org/italia/onto/HER> ;
                 rdfs:label "ha ruolo accademico"@it ,
                            "has academic role"@en ;
                 owl:versionInfo "stabile"@it ,
                                 "stable"@en .


###  https://w3id.org/italia/onto/HER/hasArea
:hasArea rdf:type owl:ObjectProperty ;
         rdfs:subPropertyOf :hasAcademicDiscipline ;
         rdfs:domain [ rdf:type owl:Class ;
                       owl:unionOf ( :AcademicDegree
                                     :ItalianPhDCourseByCycle
                                   )
                     ] ;
         rdfs:range :Area ;
         rdfs:comment "Property that links some statistical aggregated data and the academic degree to the CUN area."@en ,
                      "Proprietà che collega alcuni dati statistici e la laurea all'area CUN di riferimento della classificazione sulle discipline accademiche."@it ;
         rdfs:isDefinedBy <https://w3id.org/italia/onto/HER> ;
         rdfs:label "ha area CUN"@it ,
                    "has CUN area"@en ;
         owl:versionInfo "stabile"@it ,
                         "stable"@en .


###  https://w3id.org/italia/onto/HER/hasCHAFEAOutput
:hasCHAFEAOutput rdf:type owl:ObjectProperty ;
                 rdfs:subPropertyOf :hasResult ;
                 rdfs:domain :CHAFEAProject ;
                 rdfs:range :CHAFEAOutput ;
                 rdfs:comment "Questa proprietà collega un'attività finanziata con uno dei suoi risultati."@it ,
                              "This property connects a funded activity with one of its outputs."@en ;
                 rdfs:isDefinedBy <https://w3id.org/italia/onto/HER> ;
                 rdfs:label "ha risultato CHAFEA"@it ,
                            "has CHAFEA output"@en ;
                 owl:versionInfo "provvisoria"@it ,
                                 "unstable"@en .


###  https://w3id.org/italia/onto/HER/hasCHAFEAParticipant
:hasCHAFEAParticipant rdf:type owl:ObjectProperty ;
                      rdfs:subPropertyOf <https://w3id.org/italia/onto/RO/hasRiT> ;
                      rdfs:domain :CHAFEAProject ;
                      rdfs:range :CHAFEAParticipant ;
                      rdfs:comment "Questa proprietà collega un'attività finanziata con le istituzioni coinvolte."@it ,
                                   "This property connects a funded activity with the institutions involved."@en ;
                      rdfs:isDefinedBy <https://w3id.org/italia/onto/HER> ;
                      rdfs:label "ha partecipante CHAFEA"@it ,
                                 "has CHAFEA participant"@en ;
                      owl:versionInfo "stabile"@it ,
                                      "stable"@en .


###  https://w3id.org/italia/onto/HER/hasCHAFEAProgramme
:hasCHAFEAProgramme rdf:type owl:ObjectProperty ;
                    rdfs:subPropertyOf :hasProgramme ;
                    rdfs:domain :CHAFEAProject ;
                    rdfs:range :CHAFEAProgramme ;
                    rdfs:comment "Questa proprietà collega un progetto CHAFEA con un programma."@it ,
                                 "This property connects a CHAFEA project with a programme."@en ;
                    rdfs:isDefinedBy <https://w3id.org/italia/onto/HER> ;
                    rdfs:label "ha programma CHAFEA"@it ,
                               "has CHAFEA programme"@en ;
                    owl:versionInfo "stabile"@it ,
                                    "stable"@en .


###  https://w3id.org/italia/onto/HER/hasCTNPRINAmount
:hasCTNPRINAmount rdf:type owl:ObjectProperty ;
                  rdfs:domain :CTNPRINOperation ;
                  rdfs:range :CTNPRINAmount ;
                  rdfs:comment "Questa proprietà collega l'operazione con gli importi."@it ,
                               "This property links the operation with the amounts."@en ;
                  rdfs:isDefinedBy <https://w3id.org/italia/onto/HER> ;
                  rdfs:label "ha importo riportato da CTN/PRIN"@it ,
                             "has CTN/PRIN amount"@en ;
                  owl:versionInfo "provvisoria"@it ,
                                  "unstable"@en .


###  https://w3id.org/italia/onto/HER/hasCTNPRINFinancingFund
:hasCTNPRINFinancingFund rdf:type owl:ObjectProperty ;
                         rdfs:domain :CTNPRINInitiative ;
                         rdfs:range :CTNPRINFinancingFund ;
                         rdfs:comment "Collega un'iniziativa al fondo di finanziamento da cui l'iniziativa attinge le sue risorse economiche"@it ,
                                      "Connects an initiative to the financing fund from which the initiative draws its economic resources"@en ;
                         rdfs:isDefinedBy <https://w3id.org/italia/onto/HER> ;
                         rdfs:label "ha CTN/PRIN financing fund"@en ,
                                    "ha fondo di finanziamento CTN/PRIN"@it ;
                         owl:versionInfo "provvisoria"@it ,
                                         "unstable"@en .


###  https://w3id.org/italia/onto/HER/hasCall
:hasCall rdf:type owl:ObjectProperty ;
         rdfs:domain <https://w3id.org/italia/onto/Project/PublicResearchProject> ;
         rdfs:range :Call ;
         rdfs:comment "Questa proprietà collega un progetto di ricerca con una chiamata."@it ,
                      "This property connects a research project with a call."@en ;
         rdfs:isDefinedBy <https://w3id.org/italia/onto/HER> ;
         rdfs:label "ha bando"@it ,
                    "has call"@en ;
         owl:versionInfo "provvisoria"@it ,
                         "unstable"@en .


###  https://w3id.org/italia/onto/HER/hasCessationYear
:hasCessationYear rdf:type owl:ObjectProperty ;
                  rdfs:subPropertyOf ti:hasYear ;
                  rdfs:domain :Spinoff ;
                  rdfs:range ti:Year ;
                  rdfs:comment "Indica l'anno di cessazione dell'attività dello spin-off, se applicabile."@it ,
                               "It indicates the year of cessation of the spin-off activity, if applicable."@en ;
                  rdfs:isDefinedBy <https://w3id.org/italia/onto/HER> ;
                  rdfs:label "ha anno di cessazione"@it ,
                             "has cessation year"@en ;
                  owl:versionInfo "stabile"@it ,
                                  "stable"@en .


###  https://w3id.org/italia/onto/HER/hasCoordinator
:hasCoordinator rdf:type owl:ObjectProperty ;
                owl:inverseOf :isCoordinatorOf ;
                rdfs:domain <https://w3id.org/italia/onto/Project/PublicResearchProject> ;
                rdfs:range covapit:Organization ;
                rdfs:comment "Beneficiario principale in un gruppo di beneficiari. Punto di contatto principale per il progetto."@it ,
                             "Lead beneficiary in a group of beneficiaries. Main contact point for the project."@en ;
                rdfs:isDefinedBy <https://w3id.org/italia/onto/HER> ;
                rdfs:label "ha coordinatore"@it ,
                           "has coordinator"@en ;
                owl:versionInfo "provvisoria"@it ,
                                "unstable"@en .


###  https://w3id.org/italia/onto/HER/hasCountryInvolvement
:hasCountryInvolvement rdf:type owl:ObjectProperty ;
                       rdfs:domain :AACTStudy ;
                       rdfs:range :CountryInvolvement ;
                       rdfs:comment "Country where the facility conducting a clinical protocol is located"@en ,
                                    "Paese in cui si trova la struttura che conduce un protocollo clinico"@it ;
                       rdfs:isDefinedBy <https://w3id.org/italia/onto/HER> ;
                       rdfs:label "ha coinvolgimento del paese"@it ,
                                  "has country involvement"@en ;
                       owl:versionInfo "stabile"@it ,
                                       "stable"@en .


###  https://w3id.org/italia/onto/HER/hasDSUInterventionType
:hasDSUInterventionType rdf:type owl:ObjectProperty ;
                        rdfs:domain :DSURightToUniversityStudiesAggregate ;
                        rdfs:range :DSUInterventionType ;
                        rdfs:comment "Questa proprietà collega l'informazione sui dati relativi agli interventi a favore degli studenti alla tipologia di intervento corrispondente."@it ,
                                     "This property links the information on student intervention data to the corresponding type of intervention."@en ;
                        rdfs:isDefinedBy <https://w3id.org/italia/onto/HER> ;
                        rdfs:label "ha tipo/classe di intervento DSU"@it ,
                                   "has DSU intervention type"@en ;
                        owl:versionInfo "stabile"@it ,
                                        "stable"@en .


###  https://w3id.org/italia/onto/HER/hasDiploma
:hasDiploma rdf:type owl:ObjectProperty ;
            rdfs:domain [ rdf:type owl:Class ;
                          owl:unionOf ( :MIURStudentsByDiplomaAggregate
                                        :MIURStudentsByDiplomaDegreeDegreeClassAggregate
                                      )
                        ] ;
            rdfs:range :Diploma ;
            rdfs:comment "Questa proprietà si collega a un diploma accademico."@it ,
                         "This property links to an academic diploma."@en ;
            rdfs:isDefinedBy <https://w3id.org/italia/onto/HER> ;
            rdfs:label "ha  diploma"@it ,
                       "has diploma"@en ;
            owl:versionInfo "stabile"@it ,
                            "stable"@en .


###  https://w3id.org/italia/onto/HER/hasECActivityType
:hasECActivityType rdf:type owl:ObjectProperty ;
                   rdfs:domain :ECParticipant ;
                   rdfs:range :ECActivityType ;
                   rdfs:comment "Tipologia di organizzazione che partecipa ad un progetto CE. Le seguenti descrizioni e codici di convenzione sono utilizzati per distinguere tra i diversi tipi di organizzazioni: società private a scopo di lucro (PRC), enti pubblici (esclusi ricerca e istruzione) (PUB), organizzazioni di ricerca (esclusa l'istruzione) (REC), istituti di istruzione secondaria e superiore (HES) e altri enti (OTH)."@it ,
                                "Type of organisation participating in a EC project. The following descriptions and convention codes are used for distinguishing between different types of organisations: private for profit companies (PRC), public bodies (excluding research and education) (PUB), research organisations (excluding education) (REC), secondary and higher education establishments (HES), and other entities (OTH)."@en ;
                   rdfs:isDefinedBy <https://w3id.org/italia/onto/HER> ;
                   rdfs:label "ha tipo di attivitá CE"@it ,
                              "has EC activity type"@en ;
                   owl:versionInfo "provvisoria"@it ,
                                   "unstable"@en .


###  https://w3id.org/italia/onto/HER/hasECCall
:hasECCall rdf:type owl:ObjectProperty ;
           rdfs:subPropertyOf :hasCall ;
           rdfs:domain [ rdf:type owl:Class ;
                         owl:unionOf ( :ECProject
                                       :ERCProject
                                     )
                       ] ;
           rdfs:range :ECCall ;
           rdfs:comment "Questa proprietà collega un progetto EC con la relativa chiamata EC corrispondente."@it ,
                        "This property connects an EC project with its corresponding EC call."@en ;
           rdfs:isDefinedBy <https://w3id.org/italia/onto/HER> ;
           rdfs:label "ha un bando CE"@it ,
                      "has EC call"@en ;
           owl:versionInfo "stabile"@it ,
                           "stable"@en .


###  https://w3id.org/italia/onto/HER/hasECFrameworkProgramme
:hasECFrameworkProgramme rdf:type owl:ObjectProperty ;
                         rdfs:domain [ rdf:type owl:Class ;
                                       owl:unionOf ( :ECProject
                                                     :ERCProject
                                                   )
                                     ] ;
                         rdfs:range :ECFrameworkProgramme ;
                         rdfs:comment "Questa proprietà collega un progetto CE con il corrispondente programma quadro."@it ,
                                      "This property links an EC project with the corresponding framework programme."@en ;
                         rdfs:isDefinedBy <https://w3id.org/italia/onto/HER> ;
                         rdfs:label "ha struttura di lavoro CE"@it ,
                                    "has EC framework programme"@en ;
                         owl:versionInfo "stabile"@it ,
                                         "stable"@en .


###  https://w3id.org/italia/onto/HER/hasECParticipant
:hasECParticipant rdf:type owl:ObjectProperty ;
                  rdfs:subPropertyOf <https://w3id.org/italia/onto/RO/hasRiT> ;
                  rdfs:domain [ rdf:type owl:Class ;
                                owl:unionOf ( :ECProject
                                              :ERCProject
                                            )
                              ] ;
                  rdfs:range :ECParticipant ;
                  rdfs:comment "Questa proprietà collega un progetto CE con uno dei suoi partecipanti."@it ,
                               "This property connects an EC project with one of its participants."@en ;
                  rdfs:isDefinedBy <https://w3id.org/italia/onto/HER> ;
                  rdfs:label "ha partecipante CE"@it ,
                             "has EC participant"@en ;
                  owl:versionInfo "stabile"@it ,
                                  "stable"@en .


###  https://w3id.org/italia/onto/HER/hasECProgramme
:hasECProgramme rdf:type owl:ObjectProperty ;
                rdfs:subPropertyOf :hasProgramme ;
                rdfs:domain [ rdf:type owl:Class ;
                              owl:unionOf ( :ECProject
                                            :ERCProject
                                            :ErasmusPlusProject
                                          )
                            ] ;
                rdfs:range :ECProgramme ;
                rdfs:comment "Questa proprietà collega un progetto con il corrispondente programma di finanziamento."@it ,
                             "This property connects a project with the corresponding funding programme."@en ;
                rdfs:isDefinedBy <https://w3id.org/italia/onto/HER> ;
                rdfs:label "ha programma CE"@it ,
                           "has EC programme"@en ;
                owl:versionInfo "stabile"@it ,
                                "stable"@en .


###  https://w3id.org/italia/onto/HER/hasECTopic
:hasECTopic rdf:type owl:ObjectProperty ;
            rdfs:subPropertyOf l0:hasTopic ;
            rdfs:domain [ rdf:type owl:Class ;
                          owl:unionOf ( :ECProject
                                        :ERCProject
                                      )
                        ] ;
            rdfs:range :ECTopic ;
            rdfs:comment "Questa proprietà collega un progetto CE con l'argomento corrispondente all'interno del suo invito a presentare proposte."@it ,
                         "This property connects an EC project with the corresponding topic within its call for proposals."@en ;
            rdfs:isDefinedBy <https://w3id.org/italia/onto/HER> ;
            rdfs:label "ha argomento CE"@it ,
                       "has EC topic"@en ;
            owl:versionInfo "stabile"@it ,
                            "stable"@en .


###  https://w3id.org/italia/onto/HER/hasERCGrantType
:hasERCGrantType rdf:type owl:ObjectProperty ;
                 rdfs:domain [ rdf:type owl:Class ;
                               owl:unionOf ( :ECProject
                                             :ERCProject
                                           )
                             ] ;
                 rdfs:range :ERCGrantType ;
                 rdfs:comment "Questa proprietà collega un progetto del CER con il tipo di sovvenzione corrispondente."@it ,
                              "This property connects an EC or ERC project with the corresponding type of grant."@en ;
                 rdfs:isDefinedBy <https://w3id.org/italia/onto/HER> ;
                 rdfs:label "ha tipo contributo ERC"@it ,
                            "has ERC grant type"@en ;
                 owl:versionInfo "stabile"@it ,
                                 "stable"@en .


###  https://w3id.org/italia/onto/HER/hasERCPanel
:hasERCPanel rdf:type owl:ObjectProperty ;
             rdfs:subPropertyOf l0:hasTopic ;
             rdfs:domain [ rdf:type owl:Class ;
                           owl:unionOf ( :ECProject
                                         :ERCProject
                                       )
                         ] ;
             rdfs:range :ERCPanel ;
             rdfs:comment "Questa proprietà si collega al corrispondente pannello del CER."@it ,
                          "This property links to the corresponding ERC panel."@en ;
             rdfs:isDefinedBy <https://w3id.org/italia/onto/HER> ;
             rdfs:label "ha pannello ERC"@it ,
                        "has ERC panel"@en ;
             owl:versionInfo "stabile"@it ,
                             "stable"@en .


###  https://w3id.org/italia/onto/HER/hasEUREKAParticipant
:hasEUREKAParticipant rdf:type owl:ObjectProperty ;
                      rdfs:subPropertyOf <https://w3id.org/italia/onto/RO/hasRiT> ;
                      rdfs:domain :EUREKAProject ;
                      rdfs:range :EUREKAParticipant ;
                      rdfs:comment "Questa proprietà collega un progetto EUREKA con uno dei suoi partecipanti."@it ,
                                   "This property connects an EUREKA project with one of its participants."@en ;
                      rdfs:isDefinedBy <https://w3id.org/italia/onto/HER> ;
                      rdfs:label "ha partecipant EUREKA"@it ,
                                 "has EUREKA participant"@en ;
                      owl:versionInfo "stabile"@it ,
                                      "stable"@en .


###  https://w3id.org/italia/onto/HER/hasEnrollment
:hasEnrollment rdf:type owl:ObjectProperty ;
               rdfs:domain :USTATEnrolledStudentsAggregate ;
               rdfs:range :USTATEnrollment ;
               rdfs:comment "Questa proprietà collega l'informazione sugli studenti iscritti degli atenei in regola con il pagamento delle tasse universitarie all'informazione sulle tipologie di iscrizione."@it ,
                            "This property links information on enrolled students of universities in good standing with the payment of tuition fees to information on the types of enrollment."@en ;
               rdfs:isDefinedBy <https://w3id.org/italia/onto/HER> ;
               rdfs:label "ha  iscrizione"@it ,
                          "has enrollment"@en .


###  https://w3id.org/italia/onto/HER/hasErasmusPlusParticipant
:hasErasmusPlusParticipant rdf:type owl:ObjectProperty ;
                           rdfs:subPropertyOf <https://w3id.org/italia/onto/RO/hasRiT> ;
                           rdfs:domain :ErasmusPlusProject ;
                           rdfs:range :ErasmusPlusParticipant ;
                           rdfs:comment "It is used to link Erasmus+ projects to the entities which partecipate in the project."@en ,
                                        "Viene utilizzato per collegare i progetti Erasmus+ alle entità che partecipano al progetto."@it ;
                           rdfs:isDefinedBy <https://w3id.org/italia/onto/HER> ;
                           rdfs:label "ha partecipante Erasmus+"@it ,
                                      "has Erasmus+ participant"@en ;
                           owl:versionInfo "stabile"@it ,
                                           "stable"@en .


###  https://w3id.org/italia/onto/HER/hasErasmusplusActionType
:hasErasmusplusActionType rdf:type owl:ObjectProperty ;
                          rdfs:domain :ErasmusPlusProject ;
                          rdfs:range :ErasmusPlusActionType ;
                          rdfs:comment "It is used to link Erasmus+ projects to the action types."@en ,
                                       "Viene utilizzato per collegare i progetti Erasmus+ ai tipi di azione."@it ;
                          rdfs:isDefinedBy <https://w3id.org/italia/onto/HER> ;
                          rdfs:label "ha tipologia di azione Erasmus+"@it ,
                                     "has Erasmus+ action type"@en ;
                          owl:versionInfo "stabile"@it ,
                                          "stable"@en .


###  https://w3id.org/italia/onto/HER/hasErasmusplusKeyAction
:hasErasmusplusKeyAction rdf:type owl:ObjectProperty ;
                         rdfs:domain :ErasmusPlusProject ;
                         rdfs:range :ErasmusPlusKeyAction ;
                         rdfs:comment "It is used to link Erasmus+ projects to the key actions."@en ,
                                      "Viene utilizzato per collegare i progetti Erasmus+ alle azioni chiave."@it ;
                         rdfs:isDefinedBy <https://w3id.org/italia/onto/HER> ;
                         rdfs:label "ha azione chiave Erasmus+"@it ,
                                    "has Erasmus+ key action"@en ;
                         owl:versionInfo "stabile"@it ,
                                         "stable"@en .


###  https://w3id.org/italia/onto/HER/hasErasmusplusProjectResult
:hasErasmusplusProjectResult rdf:type owl:ObjectProperty ;
                             rdfs:subPropertyOf :hasResult ;
                             rdfs:domain :ErasmusPlusProject ;
                             rdfs:range :ErasmusPlusProjectResult ;
                             rdfs:comment "It is used to link Erasmus+ projects to the output results."@en ,
                                          "Viene utilizzato per collegare i progetti Erasmus+ ai risultati ottenuti."@it ;
                             rdfs:isDefinedBy <https://w3id.org/italia/onto/HER> ;
                             rdfs:label "ha un risultato del progetto Erasmus+"@it ,
                                        "has Erasmus+ project result"@en ;
                             owl:versionInfo "stabile"@it ,
                                             "stable"@en .


###  https://w3id.org/italia/onto/HER/hasErasmusplusTopic
:hasErasmusplusTopic rdf:type owl:ObjectProperty ;
                     rdfs:subPropertyOf l0:hasTopic ;
                     rdfs:domain :ErasmusPlusProject ;
                     rdfs:range :ErasmusPlusTopic ;
                     rdfs:comment "It is used to link Erasmus+ projects to Topics."@en ,
                                  "Viene utilizzato per collegare i progetti Erasmus+ agli argomenti."@it ;
                     rdfs:isDefinedBy <https://w3id.org/italia/onto/HER> ;
                     rdfs:label "ha argomento Erasmus+"@it ,
                                "has Erasmus+ topic"@en ;
                     owl:versionInfo "stabile"@it ,
                                     "stable"@en .


###  https://w3id.org/italia/onto/HER/hasEurekaCluster
:hasEurekaCluster rdf:type owl:ObjectProperty ;
                  rdfs:domain :EUREKAProject ;
                  rdfs:range :EUREKACluster ;
                  rdfs:comment "Questa proprietà collega un progetto EUREKA con il cluster corrispondente."@it ,
                               "This property connects an EUREKA project with the corresponding cluster."@en ;
                  rdfs:isDefinedBy <https://w3id.org/italia/onto/HER> ;
                  rdfs:label "ha gruppo EUREKA"@it ,
                             "has EUREKA cluster"@en ;
                  owl:versionInfo "stabile"@it ,
                                  "stable"@en .


###  https://w3id.org/italia/onto/HER/hasEurekaInstrument
:hasEurekaInstrument rdf:type owl:ObjectProperty ;
                     rdfs:domain :EUREKAProject ;
                     rdfs:range :EUREKAInstrument ;
                     rdfs:comment "Questa proprietà collega un progetto EUREKA con lo strumento corrispondente."@it ,
                                  "This property connects an EUREKA project with the corresponding instrument."@en ;
                     rdfs:isDefinedBy <https://w3id.org/italia/onto/HER> ;
                     rdfs:label "ha strumento EUREKA"@it ,
                                "has EUREKA instrument"@en ;
                     owl:versionInfo "stabile"@it ,
                                     "stable"@en .


###  https://w3id.org/italia/onto/HER/hasEurekaMarketArea
:hasEurekaMarketArea rdf:type owl:ObjectProperty ;
                     rdfs:subPropertyOf l0:hasTopic ;
                     rdfs:domain :EUREKAProject ;
                     rdfs:range :EUREKAMarketArea ;
                     rdfs:comment "Questa proprietà collega un progetto EUREKA con la corrispondente area di mercato."@it ,
                                  "This property connects an EUREKA projects with the corresponding market area."@en ;
                     rdfs:isDefinedBy <https://w3id.org/italia/onto/HER> ;
                     rdfs:label "ha area di mercato EUREKA"@it ,
                                "has EUREKA market area"@en ;
                     owl:versionInfo "stabile"@it ,
                                     "stable"@en .


###  https://w3id.org/italia/onto/HER/hasEurekaTechArea
:hasEurekaTechArea rdf:type owl:ObjectProperty ;
                   rdfs:subPropertyOf l0:hasTopic ;
                   rdfs:domain :EUREKAProject ;
                   rdfs:range :EUREKATechArea ;
                   rdfs:comment "Questa proprietà collega un progetto EUREKA con l'area tecnologica corrispondente."@it ,
                                "This property connects an EUREKA project with the corresponding tech area."@en ;
                   rdfs:isDefinedBy <https://w3id.org/italia/onto/HER> ;
                   rdfs:label "ha un area tecnica EUREKA"@it ,
                              "has EUREKA tech area"@en ;
                   owl:versionInfo "stabile"@it ,
                                   "stable"@en .


###  https://w3id.org/italia/onto/HER/hasFORDClassification
:hasFORDClassification rdf:type owl:ObjectProperty ;
                       rdfs:subPropertyOf l0:hasTopic ;
                       rdfs:domain :USTATStaffByGender ;
                       rdfs:range :FORDClassification ;
                       rdfs:comment "Questa proprietà si collega alla classificazione dei Campi di ricerca e sviluppo (FORD) dell'UNESCO."@it ,
                                    "This property links to the UNESCO's Fields of research and development (FORD) classification."@en ;
                       rdfs:isDefinedBy <https://w3id.org/italia/onto/HER> ;
                       rdfs:label "ha una classificazione FORD"@it ,
                                  "has FORD classification"@en ;
                       owl:versionInfo "stabile"@it ,
                                       "stable"@en .


###  https://w3id.org/italia/onto/HER/hasFoundationYear
:hasFoundationYear rdf:type owl:ObjectProperty ;
                   rdfs:subPropertyOf ti:hasYear ;
                   rdfs:domain :Spinoff ;
                   rdfs:range ti:Year ;
                   rdfs:comment "Indica l'anno di fondazione dello spin-off."@it ,
                                "It indicates the year of foundation of the spin-off."@en ;
                   rdfs:isDefinedBy <https://w3id.org/italia/onto/HER> ;
                   rdfs:label "ha anno di fondazione"@it ,
                              "has foundation year"@en ;
                   owl:versionInfo "stabile"@it ,
                                   "stable"@en .


###  https://w3id.org/italia/onto/HER/hasFundingDSUOrg
:hasFundingDSUOrg rdf:type owl:ObjectProperty ;
                  rdfs:domain owl:Thing ;
                  rdfs:range [ rdf:type owl:Class ;
                               owl:unionOf ( covapit:PublicOrganization
                                             covapit:SupportUnit
                                           )
                             ] ;
                  rdfs:comment "Questa proprietà collega qualunque cosa nel dominio inclusi gli interventi a favore degli studenti all'Ente o ufficio per il Diritto allo Studio Universitario (DSU) corrispondente."@it ,
                               "This property links things including the interventions in favour of students to the corresponding Institution or Office for the Right to University Studies (DSU)."@en ;
                  rdfs:isDefinedBy <https://w3id.org/italia/onto/HER> ;
                  rdfs:label "ha ente finanziatore di diritto allo studio"@it ,
                             "has funding DSU organisation"@en ;
                  owl:versionInfo "stabile"@it ,
                                  "stable"@en .


###  https://w3id.org/italia/onto/HER/hasFundingScheme
:hasFundingScheme rdf:type owl:ObjectProperty ;
                  rdfs:domain [ rdf:type owl:Class ;
                                owl:unionOf ( :ECProject
                                              :ERCProject
                                            )
                              ] ;
                  rdfs:range :ECFundingScheme ;
                  rdfs:comment "Questa proprietà collega un progetto CE con il corrispondente schema di finanziamento"@it ,
                               "This property links an EC project with the corresponding funding scheme."@en ;
                  rdfs:isDefinedBy <https://w3id.org/italia/onto/HER> ;
                  rdfs:label "ha piano di finanziamento CE"@it ,
                             "has EC funding scheme"@en ;
                  owl:versionInfo "stabile"@it ,
                                  "stable"@en .


###  https://w3id.org/italia/onto/HER/hasIPC
:hasIPC rdf:type owl:ObjectProperty ;
        rdfs:subPropertyOf l0:hasTopic ;
        rdfs:domain :Result ;
        rdfs:range :InternationalPatentClassification ;
        rdfs:comment "Questa proprietà collega un brevetto con le corrispondenti etichette di classificazione IPC."@it ,
                     "This property connects a patent with the corresponding IPC classification labels."@en ;
        rdfs:isDefinedBy <https://w3id.org/italia/onto/HER> ;
        rdfs:label "ha una classificazione internazione dei brevetti"@it ,
                   "has International Patent Classification"@en ;
        owl:versionInfo "stabile"@it ,
                        "stable"@en .


###  https://w3id.org/italia/onto/HER/hasISCEDFClassification
:hasISCEDFClassification rdf:type owl:ObjectProperty ;
                         rdfs:subPropertyOf l0:hasTopic ;
                         rdfs:domain [ rdf:type owl:Class ;
                                       owl:unionOf ( :AcademicDegree
                                                     :USTATStudentsBySexAggregate
                                                   )
                                     ] ;
                         rdfs:range :ISCEDFClassification ;
                         rdfs:comment "Questa proprietà si collega alla classificazione internazionale standard dell'istruzione dell'UNESCO (ISCED)."@it ,
                                      "This property links to the UNESCO's International Standard Classification of Education (ISCED)."@en ;
                         rdfs:isDefinedBy <https://w3id.org/italia/onto/HER> ;
                         rdfs:label "ha classificazione ISCED-F"@it ,
                                    "has ISCED-F classification"@en ;
                         owl:versionInfo "stabile"@it ,
                                         "stable"@en .


###  https://w3id.org/italia/onto/HER/hasInitiative
:hasInitiative rdf:type owl:ObjectProperty ;
               rdfs:domain [ rdf:type owl:Class ;
                             owl:unionOf ( :CTNPRINOperation
                                           :CTNPRINProject
                                         )
                           ] ;
               rdfs:range :CTNPRINInitiative ;
               rdfs:comment "An initiative may be associated with a call for proposals, a notice, an invitation, a campaign, etc."@en ,
                            "Un'iniziativa può essere associata ad un bando, un avviso, un invito, una campagna, etc."@it ;
               rdfs:isDefinedBy <https://w3id.org/italia/onto/HER> ;
               rdfs:label "ha un'iniziativa CTN/PRIN"@it ,
                          "has CTN/PRIN initiative"@en ;
               owl:versionInfo "stabile"@it ,
                               "stable"@en .


###  https://w3id.org/italia/onto/HER/hasInstrument
:hasInstrument rdf:type owl:ObjectProperty ;
               rdfs:domain :CHAFEAProject ;
               rdfs:range :CHAFEAInstrument ;
               rdfs:comment "Questa proprietà collega un progetto CHAFEA finanziato con lo strumento corrispondente."@it ,
                            "This property connects a funded CHAFEA project with the corresponding instrument."@en ;
               rdfs:isDefinedBy <https://w3id.org/italia/onto/HER> ;
               rdfs:label "ha strumento CHAFEA"@it ,
                          "has CHAFEA instrument"@en ;
               owl:versionInfo "stabile"@it ,
                               "stable"@en .


###  https://w3id.org/italia/onto/HER/hasOperation
:hasOperation rdf:type owl:ObjectProperty ;
              rdfs:domain [ rdf:type owl:Class ;
                            owl:unionOf ( :CTNPRINAmount
                                          :CTNPRINProject
                                        )
                          ] ;
              rdfs:range :CTNPRINOperation ;
              rdfs:comment "Identifica un'operazione contabile. Si veda la proprietà \"operationIdentifier\" per informazioni sulla definizione."@it ,
                           "Identifies an accounting transaction. See the \"operationIdentifier\" property for definition information."@en ;
              rdfs:isDefinedBy <https://w3id.org/italia/onto/HER> ;
              rdfs:label "ha operazione CTN/PRIN"@it ,
                         "has CTN/PRIN operation"@en ;
              owl:versionInfo "stabile"@it ,
                              "stable"@en .


###  https://w3id.org/italia/onto/HER/hasOperationalSpinoffAddress
:hasOperationalSpinoffAddress rdf:type owl:ObjectProperty ;
                              rdfs:subPropertyOf <https://w3id.org/italia/onto/CLV/hasAddress> ;
                              rdfs:domain :Spinoff ;
                              rdfs:range <https://w3id.org/italia/onto/CLV/Address> ;
                              rdfs:comment "Collega lo spin-off alla sua sede operativa."@it ,
                                           "It connects the spin-off to its operational headquarters."@en ;
                              rdfs:isDefinedBy <https://w3id.org/italia/onto/HER> ;
                              rdfs:label "ha indirizzo operativo spinoff"@it ,
                                         "has operational spinoff address"@en ;
                              owl:versionInfo "stabile"@it ,
                                              "stable"@en .


###  https://w3id.org/italia/onto/HER/hasParticipationCountry
:hasParticipationCountry rdf:type owl:ObjectProperty ;
                         rdfs:domain [ rdf:type owl:Class ;
                                       owl:unionOf ( :CHAFEAParticipant
                                                     :ECParticipant
                                                     :EUREKAParticipant
                                                     :ErasmusPlusParticipant
                                                   )
                                     ] ;
                         rdfs:range <https://w3id.org/italia/onto/CLV/Country> ;
                         rdfs:comment "Questa proprietà si collega a un Paese."@it ,
                                      "This property links to a Country."@en ;
                         rdfs:isDefinedBy <https://w3id.org/italia/onto/HER> ;
                         rdfs:label "ha un pease"@it ,
                                    "has country"@en ;
                         owl:versionInfo "provvisoria - da verificare"@it ,
                                         "unstable"@en .


###  https://w3id.org/italia/onto/HER/hasPatentInventor
:hasPatentInventor rdf:type owl:ObjectProperty ;
                   rdfs:domain :Patent ;
                   rdfs:range <https://w3id.org/italia/onto/CPV/Person> ;
                   rdfs:comment "Questa proprietà collega un brevetto con le persone che lo hanno inventato."@it ,
                                "This property connects a patent with the persons that invented it."@en ;
                   rdfs:isDefinedBy <https://w3id.org/italia/onto/HER> ;
                   rdfs:label "ha inventore"@it ,
                              "has inventor"@en ;
                   owl:versionInfo "stabile"@it ,
                                   "stable"@en .


###  https://w3id.org/italia/onto/HER/hasPatentPriorityDetail
:hasPatentPriorityDetail rdf:type owl:ObjectProperty ;
                         rdfs:domain :Patent ;
                         rdfs:range :PatentPriorityDetail .


###  https://w3id.org/italia/onto/HER/hasPatentPublicationDetail
:hasPatentPublicationDetail rdf:type owl:ObjectProperty ;
                            rdfs:domain :Patent ;
                            rdfs:range :PatentPublicationDetail ;
                            rdfs:comment "Questa proprietà collega un brevetto con i suoi dettagli di pubblicazione."@it ,
                                         "This property connects a patent with its publication details."@en ;
                            rdfs:isDefinedBy <https://w3id.org/italia/onto/HER> ;
                            rdfs:label "ha dettagli sulla pubblicazione del brevetto"@it ,
                                       "has patent publication details"@en ;
                            owl:versionInfo "provvisoria"@it ,
                                            "unstable"@en .


###  https://w3id.org/italia/onto/HER/hasPatentPublicationStage
:hasPatentPublicationStage rdf:type owl:ObjectProperty ;
                           rdfs:domain :PatentPublicationDetail ;
                           rdfs:range :PatentPublicationStage ;
                           rdfs:comment "Questa proprietà collega i dettagli della pubblicazione del brevetto con l'attuale fase della pubblicazione."@it ,
                                        "This property connects the publication details of the patent with the current stage of the publication."@en ;
                           rdfs:isDefinedBy <https://w3id.org/italia/onto/HER> ;
                           rdfs:label "ha fase di pubblicazione del brevetto"@it ,
                                      "has patent publication stage"@en ;
                           owl:versionInfo "stabile"@it ,
                                           "stable"@en .


###  https://w3id.org/italia/onto/HER/hasPhdCourse
:hasPhdCourse rdf:type owl:ObjectProperty ;
              rdfs:domain :ItalianPhDCourseByCycle ;
              rdfs:range :ItalianPhDCourse ;
              rdfs:comment "Questa proprietà si collega ad un corso di dottorato di ricerca corrispondente."@it ,
                           "This property links to a corresponding PhD course."@en ;
              rdfs:isDefinedBy <https://w3id.org/italia/onto/HER> ;
              rdfs:label "ha  corso di dottorato di ricerca"@it ,
                         "has phd course"@en ;
              owl:versionInfo "stabile"@it ,
                              "stable"@en .


###  https://w3id.org/italia/onto/HER/hasPrincipalInvestigator
:hasPrincipalInvestigator rdf:type owl:ObjectProperty ;
                          rdfs:domain <https://w3id.org/italia/onto/Project/PublicResearchProject> ;
                          rdfs:range <https://w3id.org/italia/onto/CPV/Person> ;
                          rdfs:comment "Esaminatore principale del progetto"@it ,
                                       "Principal investigator of the project"@en ;
                          rdfs:isDefinedBy <https://w3id.org/italia/onto/HER> ;
                          rdfs:label "ha esaminatore principale"@it ,
                                     "has principal investigator"@en ;
                          owl:versionInfo "provvisoria - verificare la definizione"@it ,
                                          "unstable"@en .


###  https://w3id.org/italia/onto/HER/hasProgramme
:hasProgramme rdf:type owl:ObjectProperty ;
              rdfs:domain <https://w3id.org/italia/onto/Project/PublicInvestmentProject> ;
              rdfs:range :Programme ;
              rdfs:comment "Questa proprietà collega un progetto a un programma."@it ,
                           "This property links a project with a programme."@en ;
              rdfs:isDefinedBy <https://w3id.org/italia/onto/HER> ;
              rdfs:label "ha programma"@it ,
                         "has programme"@en ;
              owl:versionInfo "provvisoria"@it ,
                              "unstable"@en .


###  https://w3id.org/italia/onto/HER/hasReportedCitizenship
:hasReportedCitizenship rdf:type owl:ObjectProperty ;
                        rdfs:domain [ rdf:type owl:Class ;
                                      owl:unionOf ( :MIURStudentsByCitizenshipAggregate
                                                    :MIURStudentsByCitizenshipDegreeAggregate
                                                    :MIURStudentsByCitizenshipDegreeClassAggregate
                                                    :MIURStudentsByCitizenshipDegreeDegreeClassAggregate
                                                  )
                                    ] ;
                        rdfs:range :ReportedCitizenship ;
                        rdfs:comment "Questa proprietà si collega alla corrispondente cittadinanza segnalata dal sistema MIUR."@it ,
                                     "This property links to the corresponding citizenship reported by the MIUR system."@en ;
                        rdfs:isDefinedBy <https://w3id.org/italia/onto/HER> ;
                        rdfs:label "ha cittadinanza riportata"@it ,
                                   "has reported citizenship"@en ;
                        owl:versionInfo "provvisoria"@it ,
                                        "unstable"@en .


###  https://w3id.org/italia/onto/HER/hasResearcherSeniorityGrade
:hasResearcherSeniorityGrade rdf:type owl:ObjectProperty ;
                             rdfs:domain :USTATStaffByGender ;
                             rdfs:range :ResearcherSeniorityGrade ;
                             rdfs:comment "Codice identificativo della qualifica ricoperta dal personale docente/ricercatore secondo la classificazione del Manuale di Frascati 2015. La corrispondenza tra gradi e qualifica è la seguente: Grade A = Prof. I fascia (ordinario); Grade B = Prof. II fascia (associato); Grade C = Ricercatore a tempo indeterminato e determinato; Grade D = Titolare di assegno di ricerca."@it ,
                                          "Identification code of the qualification held by the teaching staff/researcher according to the classification of the Frascati Manual 2015. The correspondence between grades and qualification is as follows: Grade A = Prof. I category (ordinary); Grade B = Prof. II category (associated); Grade C = Permanent and temporary researcher; Grade D = Holder of research grant."@en ;
                             rdfs:isDefinedBy <https://w3id.org/italia/onto/HER> ;
                             rdfs:label "ha anzianità di servizio del ricercatore"@it ,
                                        "has researcher seniority grade"@en ;
                             owl:versionInfo "stabile"@it ,
                                             "stable"@en .


###  https://w3id.org/italia/onto/HER/hasResult
:hasResult rdf:type owl:ObjectProperty ;
           rdfs:domain owl:Thing ;
           rdfs:range :Result ;
           rdfs:comment "Property that links any thing in the modelled domain to the result or output."@en ,
                        "Proprietà che collega qualunque cosa nel dominio modellato a un risultato o output."@it ;
           rdfs:isDefinedBy <https://w3id.org/italia/onto/HER> ;
           rdfs:label "ha risultato"@it ,
                      "has result"@en ;
           owl:versionInfo "stabile"@it ,
                           "stable"@en .


###  https://w3id.org/italia/onto/HER/hasSSD
:hasSSD rdf:type owl:ObjectProperty ;
        rdfs:subPropertyOf :hasAcademicDiscipline ;
        rdfs:domain :ItalianPhDCourseByCycle ;
        rdfs:range :ScientificDisciplinarySector ;
        rdfs:comment "Property that links some statistical data to the scientific disciplinary sector of the academic disciplines classification."@en ,
                     "Proprietà che collega alcuni dati statistici al settore scientifico disciplinare della classificazione sulle discipline accademiche."@it ;
        rdfs:isDefinedBy <https://w3id.org/italia/onto/HER> ;
        rdfs:label "ha settore scientifico disciplinare"@it ,
                   "has scientific disciplinary sector"@en ;
        owl:versionInfo "stabile"@it ,
                        "stable"@en .


###  https://w3id.org/italia/onto/HER/hasSubjectArea
:hasSubjectArea rdf:type owl:ObjectProperty ;
                rdfs:subPropertyOf l0:hasTopic ;
                rdfs:domain [ rdf:type owl:Class ;
                              owl:unionOf ( :ECProject
                                            :ERCProject
                                          )
                            ] ;
                rdfs:range :ECSubjectArea ;
                rdfs:comment "Questa proprietà collega un progetto CE con la corrispondente categorizzazione tematica. Questa categorizzazione è disponibile per il programma quadro FP7, ma non per H2020."@it ,
                             "This property connects an EC project with the corresponding thematic categorisation. This categorisation is available for the FP7 framework programme, but not for H2020."@en ;
                rdfs:isDefinedBy <https://w3id.org/italia/onto/HER> ;
                rdfs:label "ha un'area tematica CE"@it ,
                           "has EC subject area"@en ;
                owl:versionInfo "stabile"@it ,
                                "stable"@en .


###  https://w3id.org/italia/onto/HER/hasSummary
:hasSummary rdf:type owl:ObjectProperty ;
            rdfs:domain :CHAFEAProject ;
            rdfs:range :CHAFEASummary ;
            rdfs:comment "Description of funded activity."@en ,
                         "Descrizione dell'attività finanziata."@it ;
            rdfs:isDefinedBy <https://w3id.org/italia/onto/HER> ;
            rdfs:label "ha sommario"@it ,
                       "has summary"@en .


###  https://w3id.org/italia/onto/HER/hasUSTATCateenService
:hasUSTATCateenService rdf:type owl:ObjectProperty ;
                       rdfs:domain :DSUCanteenAndAccomodationsAggregate ;
                       rdfs:range :USTATCanteenServiceClass ;
                       rdfs:comment "Questa proprietà collega l'informazione sul totale dei serivizi disponibili alla tipologia di servizio corrispondente."@it ,
                                    "This property links the information on the total number of services available to the corresponding type of service."@en ;
                       rdfs:isDefinedBy <https://w3id.org/italia/onto/HER> ;
                       rdfs:label "ha una classe di servizio ustat"@it ,
                                  "has ustat service class"@en .


###  https://w3id.org/italia/onto/HER/hasUSTATContributionClass
:hasUSTATContributionClass rdf:type owl:ObjectProperty ;
                           rdfs:domain :USTATContributionByClass ;
                           rdfs:range :USTATContributionClass ;
                           rdfs:comment """Code of the university student contribution class. Can take the values:
00: contribution not expected (excluding exemptions)
00a: contribution financed by external bodies
01 : from 0,01 to 100,00 (excluding exemptions)
02 : from 100,01 to 200,00
03 : from 200,01 to 300,00
04 : from 300,01 to 400,00
05 : from 400,01 to 500,00
06 : from 500,01 to 600,00
07 : from 600,01 to 700,00
08 : from 700,01 to 800,00
09 : from 800,01 to 900,00
10 : from 900.01 to 1,000.00
11a: from 1,000.01 to 1,100.00
11b: from 1.100,01 to 1.200,00
11c: from 1.200,01 to 1.300,00
11d: from 1.300,01 to 1.400,00
11e: from 1.400,01 to 1.500,00
12a: from 1.500,01 to 1.600,00
12b: from 1.600,01 to 1.700,00
12c: from 1.700,01 to 1.800,00
12d: from 1.800,01 to 1.900,00
12e: from 1,900.01 to 2,000.00
13 : from 2.000,01 to 2.500,00
14 : from 2,500.01 to 3,000.00
15 : from 3.000,01 to 3.500,00
16 : from 3.500,01 to 4.000,00
17 : from 4.000,01 to 4.500,00
18 : from 4.500,01 to 5.000,00
19 : from 5,000.01 to 6,000.00
20 : from 6,000.01 to 8,000.00
21a: from 8,000.01 to 10,000.00
21b: over 10,000.00"""@en ,
                                        """Codice della classe di contribuzione degli studenti universitari. Può assumere i valori:
00: contribuzione non prevista (esclusi esoneri)
00a: contribuzione finanziata da enti esterni
01 : da 0,01 a 100,00 (esclusi esoneri)
02 : da 100,01 a 200,00
03 : da 200,01 a 300,00
04 : da 300,01 a 400,00
05 : da 400,01 a 500,00
06 : da 500,01 a 600,00
07 : da 600,01 a 700,00
08 : da 700,01 a 800,00
09 : da 800,01 a 900,00
10 : da 900,01 a 1.000,00
11a: da 1.000,01 a 1.100,00
11b: da 1.100,01 a 1.200,00
11c: da 1.200,01 a 1.300,00
11d: da 1.300,01 a 1.400,00
11e: da 1.400,01 a 1.500,00
12a: da 1.500,01 a 1.600,00
12b: da 1.600,01 a 1.700,00
12c: da 1.700,01 a 1.800,00
12d: da 1.800,01 a 1.900,00
12e: da 1.900,01 a 2.000,00
13 : da 2.000,01 a 2.500,00
14 : da 2.500,01 a 3.000,00
15 : da 3.000,01 a 3.500,00
16 : da 3.500,01 a 4.000,00
17 : da 4.000,01 a 4.500,00
18 : da 4.500,01 a 5.000,00
19 : da 5.000,01 a 6.000,00
20 : da 6.000,01 a 8.000,00
21a: da 8.000,01 a 10.000,00
21b: oltre 10.000,00"""@it ;
                           rdfs:isDefinedBy <https://w3id.org/italia/onto/HER> ;
                           rdfs:label "ha un contributo per classe"@it ,
                                      "has contribution class"@en .


###  https://w3id.org/italia/onto/HER/hasUSTATContributionRevenueClass
:hasUSTATContributionRevenueClass rdf:type owl:ObjectProperty ;
                                  rdfs:domain :USTATContributionRevenue ;
                                  rdfs:range :USTATContributionRevenueClass ;
                                  rdfs:comment "Questa proprietà collega l'informazione sui dati relativi al gettito dalla contribuzione studentesca degli atenei alle informazioni sulla fonte del gettito."@it ,
                                               "This property links information on revenue data from student contributions to information on the source of the revenue."@en ;
                                  rdfs:isDefinedBy <https://w3id.org/italia/onto/HER> ;
                                  rdfs:label "ha un classe di contributo ricavante"@it ,
                                             "has contribution revenue class"@en .


###  https://w3id.org/italia/onto/HER/hasUSTATExonerationClass
:hasUSTATExonerationClass rdf:type owl:ObjectProperty ;
                          rdfs:domain [ rdf:type owl:Class ;
                                        owl:unionOf ( :USTATPartiallyExoneratedStudentsAggregate
                                                      :USTATTotallyExoneratedStudentsAggregate
                                                    )
                                      ] ;
                          rdfs:range :USTATExonerationType ;
                          rdfs:comment "Questa proprietà collega l'informazione sugli studenti esonerati (parzialmente o totalmente) alla classe di esonero corrispondente."@it ,
                                       "This property links information about exonerated students (partially or totally) to the corresponding exoneration class."@en ;
                          rdfs:isDefinedBy <https://w3id.org/italia/onto/HER> ;
                          rdfs:label "ha una classe di esonero"@it ,
                                     "has exoneration class"@en .


###  https://w3id.org/italia/onto/HER/hasUSTATExpenseClass
:hasUSTATExpenseClass rdf:type owl:ObjectProperty ;
                      rdfs:domain [ rdf:type owl:Class ;
                                    owl:unionOf ( :USTATInterventionExpensesAggregate
                                                  :USTATUniversityInterventionExpensesAggregate
                                                )
                                  ] ;
                      rdfs:range [ rdf:type owl:Class ;
                                   owl:unionOf ( :USTATExpenseClass
                                                 :USTATUniversityExpenseClass
                                               )
                                 ] ;
                      rdfs:comment "Questa proprietà collega l'informazione sui dati relativi alla spesa per interventi a favore degli studenti degli atenei (solo prestiti a studenti) alla tipologia di spesa corrispondente."@it ,
                                   "This property links the information on expenses for interventions in favour of university students (student loans only) to the corresponding type of expenses."@en ;
                      rdfs:isDefinedBy <https://w3id.org/italia/onto/HER> ;
                      rdfs:label "ha una classe di spesa"@it ,
                                 "has expense class"@en .


###  https://w3id.org/italia/onto/HER/hasUSTATFunctionalArea
:hasUSTATFunctionalArea rdf:type owl:ObjectProperty ;
                        rdfs:domain :USTATTAStaffByGender ;
                        rdfs:range :USTATFunctionalArea ;
                        rdfs:comment "It is used to link data on the number of technical-administrative staff by gender and year to the corresponding functional area."@en ,
                                     "Viene utilizzato per collegare i dati sul numero di personale tecnico-amministrativo per genere e per anno all'area funzionale corrispondente."@it ;
                        rdfs:isDefinedBy <https://w3id.org/italia/onto/HER> ;
                        rdfs:label "ha un area funzionale"@it ,
                                   "has functional area"@en .


###  https://w3id.org/italia/onto/HER/hasUSTATMeasureOfMealsProvided
:hasUSTATMeasureOfMealsProvided rdf:type owl:ObjectProperty ;
                                rdfs:domain :USTATMealsProvidedAggregate ;
                                rdfs:range :USTATMeasureOfMealsProvided ;
                                rdfs:comment "Questa proprietà collega l'informazione sui pasti erogati con la corrispondente tipologia."@it ,
                                             "This property links the information on the meals provided with the corresponding type."@en ;
                                rdfs:isDefinedBy <https://w3id.org/italia/onto/HER> ;
                                rdfs:label "measure of meals provided"@en ,
                                           "misure dei pasti forniti"@it .


###  https://w3id.org/italia/onto/HER/hasUSTATPostgraduateCourse
:hasUSTATPostgraduateCourse rdf:type owl:ObjectProperty ;
                            rdfs:domain [ rdf:type owl:Class ;
                                          owl:unionOf ( :USTATPostgraduateAggregateOfEnrolled
                                                        :USTATPostgraduateAggregateOfGraduated
                                                        :USTATPostgraduateAggregateOfRegistered
                                                      )
                                        ] ;
                            rdfs:range :USTATReportedPostgraduateCourse ;
                            rdfs:comment "Questa proprietà collega l'informazione sulla popolazione di studenti o diplomati di corsi di formazione post-laurea al corso corrispondente."@it ,
                                         "This property links information about the population of students or graduates of postgraduate training courses to the corresponding course."@en ;
                            rdfs:isDefinedBy <https://w3id.org/italia/onto/HER> ;
                            rdfs:label "ha un corso di perfezionamento"@it ,
                                       "has postgraduate course"@en .


###  https://w3id.org/italia/onto/HER/hasUSTATReportedHERInstitution
:hasUSTATReportedHERInstitution rdf:type owl:ObjectProperty ;
                                rdfs:domain [ rdf:type owl:Class ;
                                              owl:unionOf ( :DSURightToUniversityStudiesAggregate
                                                            :USTATInterventionExpensesAggregate
                                                          )
                                            ] ;
                                rdfs:range :USTATReportedHERInstitution ;
                                rdfs:comment "Questa proprietà collega l'informazione sui dati relativi agli interventi a favore degli studenti all'istituto per l'alta formazione (Ateneo, Istituto Alta Formazione Artistica e Musicale - AFAM, Scuola Superiore per Mediatori Linguistici, Altro) corrispondente."@it ,
                                             "This property links the information about the interventions in favour of the students to the corresponding Institute for Higher Education (Ateneo, Istituto Alta Formazione Artistica e Musicale - AFAM, Scuola Superiore per Mediatori Linguistici, Altro)."@en ;
                                rdfs:isDefinedBy <https://w3id.org/italia/onto/HER> ;
                                rdfs:label "ha un'istituzione di HER riportata da USTAT"@it ,
                                           "has USTAT reported HER institution"@en .


###  https://w3id.org/italia/onto/HER/hasUSTATReportedUniversityFacilityType
:hasUSTATReportedUniversityFacilityType rdf:type owl:ObjectProperty ;
                                        rdfs:domain :USTATUniversityFacilitiesAggregate ;
                                        rdfs:range :USTATReportedUniversityFacilityType ;
                                        rdfs:comment "Questa proprietà collega l'informazione sulle strutture universitarie (mense e residenze universitarie direttamente gestite dall'istituto) al codice e descrizione della struttura."@it ,
                                                     "This property links information on university facilities (canteens and university residences directly managed by the institute) to the code and description of the structure."@en ;
                                        rdfs:isDefinedBy <https://w3id.org/italia/onto/HER> ;
                                        rdfs:label "ha un tipo di struttura universitaria riportata da USTAT"@it ,
                                                   "has USTAT reported university facility type"@en ;
                                        owl:versionInfo "stabile"@it ,
                                                        "stable"@en .


###  https://w3id.org/italia/onto/HER/hasUSTATUniversityInterventionType
:hasUSTATUniversityInterventionType rdf:type owl:ObjectProperty ;
                                    rdfs:domain :USTATInterventionsForStudentsByUniversitiesAggregate ;
                                    rdfs:range :USTATUniversityInterventionType ;
                                    rdfs:comment "Property that links the aggregated data on the university intervention as defined by USTAT to the type of university intervention as defined by USTAT"@en ,
                                                 "Proprietà che collega i dati aggregati sui sugli interventi universitari come riportati da USTAT ai tipi di intervento universitari definiti nel contesto USTAT"@it ;
                                    rdfs:isDefinedBy <https://w3id.org/italia/onto/HER> ;
                                    rdfs:label "has USTAT university intervention type"@en ,
                                               "has tipo intervento universitario di USTAT"@it ;
                                    owl:versionInfo "stabile"@it ,
                                                    "stable"@en .


###  https://w3id.org/italia/onto/HER/hasWorkpackage
:hasWorkpackage rdf:type owl:ObjectProperty ;
                rdfs:domain :CHAFEAProject ;
                rdfs:range :CHAFEAWorkpackage ;
                rdfs:comment "Questa proprietà collega un'attività finanziata con uno dei suoi pacchetti di lavoro."@it ,
                             "This property connects a funded activity with one of its workpackages."@en ;
                rdfs:isDefinedBy <https://w3id.org/italia/onto/HER> ;
                rdfs:label "ha piano di lavoro"@it ,
                           "has workpackage"@en ;
                owl:versionInfo "provvisoria"@it ,
                                "unstable"@en .


###  https://w3id.org/italia/onto/HER/hsUSTATStaffType
:hsUSTATStaffType rdf:type owl:ObjectProperty ;
                  rdfs:domain [ rdf:type owl:Class ;
                                owl:unionOf ( :USTATPermanentStaff
                                              :USTATTemporaryStaff
                                            )
                              ] ;
                  rdfs:range :USTATStaffType ;
                  rdfs:comment "Questa proprietà collega l'informazione sul personale relativo all'ente o Ufficio per il Diritto allo Studio Universitario (DSU) considerato alla tipologia di contratto di assunzione."@it ,
                               "This property links the information on the personnel related to the institution or Office for the Right to University Studies (DSU) considered to the type of employment contract."@en ;
                  rdfs:isDefinedBy <https://w3id.org/italia/onto/HER> ;
                  rdfs:label "ha un ruolo di staff universitario italiano"@it ,
                             "has italian university staff role"@en .


###  https://w3id.org/italia/onto/HER/isCoordinatorOf
:isCoordinatorOf rdf:type owl:ObjectProperty ;
                 rdfs:domain covapit:Organization ;
                 rdfs:range <https://w3id.org/italia/onto/Project/PublicResearchProject> ;
                 rdfs:comment "Inverse property of hasCoordinator"@en ,
                              "Proprietà inversa di ha coordinatore"@it ;
                 rdfs:isDefinedBy <https://w3id.org/italia/onto/HER> ;
                 rdfs:label "is coordinator of"@en ,
                            "è coordinatore di"@it ;
                 owl:versionInfo "stabile"@it ,
                                 "stable"@en .


###  https://w3id.org/italia/onto/HER/isProducedBy
:isProducedBy rdf:type owl:ObjectProperty ;
              owl:inverseOf :producesPatent ;
              rdfs:domain :Patent ;
              rdfs:range covapit:Organization ;
              rdfs:comment "Questa proprietà collega un brevetto con l'organizzazione che lo produce"@it ,
                           "This property connects a patent with the organization that produces it"@en ;
              rdfs:isDefinedBy <https://w3id.org/italia/onto/HER> ;
              rdfs:label "brevetto prodotto da"@it ,
                         "patent is produced by"@en ;
              owl:versionInfo "stabile"@it ,
                              "stable"@en .


###  https://w3id.org/italia/onto/HER/producesPatent
:producesPatent rdf:type owl:ObjectProperty ;
                rdfs:subPropertyOf :hasResult ;
                rdfs:domain covapit:Organization ;
                rdfs:range :Patent ;
                rdfs:comment "Questa proprietà collega un'organizzazione con un brevetto."@it ,
                             "This property links an organization with a patent."@en ;
                rdfs:isDefinedBy <https://w3id.org/italia/onto/HER> ;
                rdfs:label "brevetto prodotto da"@it ,
                           "produces patent"@en ;
                owl:versionInfo "stabile"@it ,
                                "stable"@en .


###  https://w3id.org/italia/onto/HER/refersToProject
:refersToProject rdf:type owl:ObjectProperty ;
                 rdfs:domain :CTNPRINOperation ;
                 rdfs:range :CTNPRINProject ;
                 rdfs:comment "Questa proprietà  collega un'operazione CTN/PRIN con il progetto CTN/PRIN di riferimento"@it ,
                              "This property links a CTN/Prin opertion to the reference CTN/PRIN project."@en ;
                 rdfs:isDefinedBy <https://w3id.org/italia/onto/HER> ;
                 rdfs:label "refers to project"@en ,
                            "si riferisce a progetto"@it ;
                 owl:versionInfo "provissoria - da verificare"@it ,
                                 "unstable"@en .


###  https://w3id.org/italia/onto/HER/withAcademicRole
:withAcademicRole rdf:type owl:ObjectProperty ;
                  rdfs:subPropertyOf <https://w3id.org/italia/onto/RO/withRole> ;
                  rdfs:domain :AcademicAffiliation ;
                  rdfs:range [ rdf:type owl:Class ;
                               owl:unionOf ( :AcademicRole
                                             :ItalianAcademicRole
                                           )
                             ] ;
                  rdfs:comment "Questa proprietà collega un'affiliazione accademica con il ruolo accademico corrispondente."@it ,
                               "This property connects an Academic Affiliation with the corresponding Academic Role."@en ;
                  rdfs:isDefinedBy <https://w3id.org/italia/onto/HER> ;
                  rdfs:label "con ruolo accademico"@it ,
                             "with academic role"@en ;
                  owl:versionInfo "stabile"@it ,
                                  "stable"@en .


###  https://w3id.org/italia/onto/HER/withCountry
:withCountry rdf:type owl:ObjectProperty ;
             rdfs:domain :CountryInvolvement ;
             rdfs:range <https://w3id.org/italia/onto/CLV/Country> ;
             rdfs:comment "Questa proprietà collega un coinvolgimento del paese con il paese corrispondente"@it ,
                          "This property connects a country involvement with the corresponding country"@en ;
             rdfs:isDefinedBy <https://w3id.org/italia/onto/HER> ;
             rdfs:label "con paese"@it ,
                        "with country"@en .


###  https://w3id.org/italia/onto/RO/forEntity
<https://w3id.org/italia/onto/RO/forEntity> rdf:type owl:ObjectProperty .


###  https://w3id.org/italia/onto/RO/hasRiT
<https://w3id.org/italia/onto/RO/hasRiT> rdf:type owl:ObjectProperty .


###  https://w3id.org/italia/onto/RO/withRole
<https://w3id.org/italia/onto/RO/withRole> rdf:type owl:ObjectProperty .


###  https://w3id.org/italia/onto/l0/hasTopic
l0:hasTopic rdf:type owl:ObjectProperty .


#################################################################
#    Data properties
#################################################################

###  https://w3id.org/italia/onto/COV/VATnumber
covapit:VATnumber rdf:type owl:DatatypeProperty ;
                  rdfs:label "VAT number"@en ,
                             "codice fiscale"@it .


###  https://w3id.org/italia/onto/CPV/age
<https://w3id.org/italia/onto/CPV/age> rdf:type owl:DatatypeProperty .


###  https://w3id.org/italia/onto/CPV/altName
<https://w3id.org/italia/onto/CPV/altName> rdf:type owl:DatatypeProperty .


###  https://w3id.org/italia/onto/CPV/familyName
<https://w3id.org/italia/onto/CPV/familyName> rdf:type owl:DatatypeProperty .


###  https://w3id.org/italia/onto/CPV/givenName
<https://w3id.org/italia/onto/CPV/givenName> rdf:type owl:DatatypeProperty .


###  https://w3id.org/italia/onto/CPV/sexDesc
<https://w3id.org/italia/onto/CPV/sexDesc> rdf:type owl:DatatypeProperty .


###  https://w3id.org/italia/onto/CPV/sexID
<https://w3id.org/italia/onto/CPV/sexID> rdf:type owl:DatatypeProperty .


###  https://w3id.org/italia/onto/HER/DMC
:DMC rdf:type owl:DatatypeProperty ;
     rdfs:domain :AACTStudy ;
     rdfs:comment "Lo studio dispone di un Comitato di monitoraggio dei dati (DMC) (un gruppo di scienziati indipendenti che monitorano la sicurezza e l'integrità scientifica di uno studio clinico. Il DMC può raccomandare allo sponsor di interrompere la sperimentazione se non è efficace, se danneggia i partecipanti o se è improbabile che serva al suo scopo scientifico. I membri sono scelti in base alle competenze e alle conoscenze scientifiche necessarie per monitorare lo specifico studio. Chiamato anche scheda di sicurezza e monitoraggio dei dati, o DSMB)."@it ,
                  "Study has a Data Monitoring Committee (DMC) (a group of independent scientists who monitor the safety and scientific integrity of a clinical trial. The DMC can recommend to the sponsor that the trial be stopped if it is not effective, is harming participants, or is unlikely to serve its scientific purpose. Members are chosen based on the scientific skills and knowledge needed to monitor the particular trial. Also called a data safety and monitoring board, or DSMB.)"@en ;
     rdfs:isDefinedBy <https://w3id.org/italia/onto/HER> ;
     rdfs:label "DMC"@en ,
                "DMC"@it ;
     owl:versionInfo "provvisoria"@it ,
                     "unstable"@en .


###  https://w3id.org/italia/onto/HER/PHDCycle
:PHDCycle rdf:type owl:DatatypeProperty ;
          rdfs:domain [ rdf:type owl:Class ;
                        owl:unionOf ( :ItalianPhDCourseByCycle
                                      :USTATPostgraduateAggregateOfRegistered
                                    )
                      ] ;
          rdfs:comment "Numero del ciclo del Dottorato di Ricerca. Valido solo per i corsi di Dottorato di Ricerca."@it ,
                       "PhD cycle number. Only valid for PhD courses."@en ;
          rdfs:isDefinedBy <https://w3id.org/italia/onto/HER> ;
          rdfs:label "academic cycle"@en ,
                     "ciclo accademico"@it .


###  https://w3id.org/italia/onto/HER/aactCriterion
:aactCriterion rdf:type owl:DatatypeProperty ;
               rdfs:domain :AACTEligibility ;
               rdfs:range rdfs:Literal ;
               rdfs:comment "Criteri di ammissibilità nel contesto delle Aggregated Analysis for clininca trials. I criteri di ammissibilità consistono sia in criteri di inclusione (che sono richiesti per una persona per partecipare allo studio) sia in criteri di esclusione (che impediscono a una persona di partecipare). I tipi di criteri di ammissibilità si riferiscono a stabilire se uno studio accetta volontari sani, se ha requisiti di età o di gruppo d'età o se è limitato dal sesso."@it ,
                            "Eligibility criteria in the contest of Aggregated Analysis of Clinical Trials (AACT). Eligibility criteria consist of both inclusion criteria (which are required for a person to participate in the study) and exclusion criteria (which prevent a person from participating). Types of eligibility criteria include whether a study accepts healthy volunteers, has age or age group requirements, or is limited by sex."@en ;
               rdfs:isDefinedBy <https://w3id.org/italia/onto/HER> ;
               rdfs:label "AACT criterion"@en ,
                          "Criterio AACT"@it ;
               owl:versionInfo "stabile"@it ,
                               "stable"@en .


###  https://w3id.org/italia/onto/HER/aactEligibleSex
:aactEligibleSex rdf:type owl:DatatypeProperty ,
                          owl:FunctionalProperty ;
                 rdfs:domain :AACTEligibility ;
                 rdfs:range rdfs:Literal ;
                 rdfs:comment "Gender eligible for the corresponding study. Possible values are Male, Female and All."@en ,
                              "Sesso ammissibile per lo studio corrispondente. I valori possibili sono Maschio, Femmina e Tutti."@it ;
                 rdfs:isDefinedBy <https://w3id.org/italia/onto/HER> ;
                 rdfs:label "aact eligible sex"@en ,
                            "genere ammissibile secondo aact"@it ;
                 owl:versionInfo "stabile"@it ,
                                 "stable"@en .


###  https://w3id.org/italia/onto/HER/aactInterventionTypeName
:aactInterventionTypeName rdf:type owl:DatatypeProperty ;
                          rdfs:subPropertyOf l0:name ;
                          rdfs:domain :AACTIntervention ;
                          rdfs:range rdfs:Literal ;
                          rdfs:comment """For each intervention studied in the clinical study, the general type of intervention. They are:
Drug: Including placebo
Device: Including sham
Biological/Vaccine
Procedure/Surgery
Radiation
Behavioral: For example, psychotherapy, lifestyle counseling
Genetic: Including gene transfer, stem cell and recombinant DNA
Dietary Supplement: For example, vitamins, minerals
Combination Product: Combining a drug and device, a biological product and device; a drug and biological product; or a drug, biological product, and device
Diagnostic Test: For example, imaging, in-vitro
Other
"""@en ,
                                       """Per ogni intervento studiato nello studio clinico, il tipo generale di intervento. Di seguito descritti:
Farmaci: Compreso il placebo
Dispositivo: Inclusa la finzione
Biologico/Vaccino
Procedimento/chirurgia
Radiazioni
Comportamentale: per esempio, psicoterapia, consulenza sullo stile di vita
Genetico: incluso il trasferimento di geni, cellule staminali e DNA ricombinante
Integratore alimentare: Per esempio, vitamine, minerali
Prodotto combinato: Combinazione di un farmaco e dispositivo, un prodotto e dispositivo biologico; un farmaco e prodotto biologico; o un farmaco, prodotto biologico e dispositivo
Test diagnostico: Per esempio, imaging, in vitro
Altro
"""@it ;
                          rdfs:isDefinedBy <https://w3id.org/italia/onto/HER> ;
                          rdfs:label "Tipo di intervento AACT"@it ,
                                     "aact intervention type"@en .


###  https://w3id.org/italia/onto/HER/aactMaximumAge
:aactMaximumAge rdf:type owl:DatatypeProperty ;
                rdfs:subPropertyOf <https://w3id.org/italia/onto/CPV/age> ;
                rdfs:domain :AACTEligibility ;
                rdfs:range xsd:integer ;
                rdfs:comment "Il valore numerico, se presente, per l'età massima che un potenziale partecipante può avere per essere idoneo allo studio clinico."@it ,
                             "The numerical value, if any, for the maximum age a potential participant can be to be eligible for the clinical study."@en ;
                rdfs:isDefinedBy <https://w3id.org/italia/onto/HER> ;
                rdfs:label "AACT maximum age"@en ,
                           "etá massima AACT"@it ;
                owl:versionInfo "stabile"@it ,
                                "stable"@en .


###  https://w3id.org/italia/onto/HER/aactMinimumAge
:aactMinimumAge rdf:type owl:DatatypeProperty ;
                rdfs:subPropertyOf <https://w3id.org/italia/onto/CPV/age> ;
                rdfs:domain :AACTEligibility ;
                rdfs:range xsd:integer ;
                rdfs:comment "L'eventuale valore numerico per l'età minima che un potenziale partecipante deve soddisfare per essere idoneo allo studio clinico."@it ,
                             "The numerical value, if any, for the minimum age a potential participant must meet to be eligible for the clinical study."@en ;
                rdfs:isDefinedBy <https://w3id.org/italia/onto/HER> ;
                rdfs:label "AACT minimum age"@en ,
                           "etá minima AACT"@it ;
                owl:versionInfo "stabile"@it ,
                                "stable"@en .


###  https://w3id.org/italia/onto/HER/aactPopulation
:aactPopulation rdf:type owl:DatatypeProperty ;
                rdfs:domain :AACTEligibility ;
                rdfs:range rdfs:Literal ;
                rdfs:comment "A description of the population from which the groups or cohorts will be selected (for example, primary care clinic, community sample, residents of a certain town)."@en ,
                             "Una descrizione della popolazione da cui saranno selezionati i gruppi (ad esempio, clinica di assistenza primaria, campione della comunità, residenti di una certa città)."@it ;
                rdfs:isDefinedBy <https://w3id.org/italia/onto/HER> ;
                rdfs:label "AACT population"@en ,
                           "popolazione AACT"@it ;
                owl:versionInfo "stabile"@it ,
                                "stable"@en .


###  https://w3id.org/italia/onto/HER/aactResponsiblePartyTypeName
:aactResponsiblePartyTypeName rdf:type owl:DatatypeProperty ;
                              rdfs:subPropertyOf l0:name ;
                              rdfs:domain :AACTResponsibleParty ;
                              rdfs:range rdfs:Literal ;
                              rdfs:comment """Responsible Party type:
Sponsor: The entity (for example, corporation or agency) that initiates the study
Principal Investigator: The individual designated as responsible party by the sponsor (see Note)
Sponsor-Investigator: The individual who both initiates and conducts the study
"""@en ,
                                           """Tipologia di responsabile dello studio:
Sponsor: L'entità (per esempio, società o agenzia) che avvia lo studio
Investigatore principale: La persona designata come responsabile dallo sponsor (vedi nota)
Sponsor-Investigatore: L'individuo che inizia e conduce lo studio"""@it ;
                              rdfs:isDefinedBy <https://w3id.org/italia/onto/HER> ;
                              rdfs:label "responsible party type"@en ,
                                         "tipo di parte reponsabile"@it .


###  https://w3id.org/italia/onto/HER/abstract
:abstract rdf:type owl:DatatypeProperty ;
          rdfs:subPropertyOf l0:description ;
          rdfs:domain [ rdf:type owl:Class ;
                        owl:unionOf ( :CTNPRINOperation
                                      :Result
                                      <https://w3id.org/italia/onto/Project/PublicResearchProject>
                                    )
                      ] ;
          rdfs:range rdfs:Literal ;
          rdfs:comment "Testo dell'abstract di un progetto, di un risultato della ricerca, di un'operazione."@it ,
                       "Text of the abstract of a project, research output, accounting operation"@en ;
          rdfs:isDefinedBy <https://w3id.org/italia/onto/HER> ;
          rdfs:label "abstract"@en ,
                     "riassunto"@it ;
          owl:versionInfo "stabile"@it ,
                          "stable"@en .


###  https://w3id.org/italia/onto/HER/academicYear
:academicYear rdf:type owl:DatatypeProperty ;
              rdfs:subPropertyOf ti:year ;
              rdfs:domain [ rdf:type owl:Class ;
                            owl:unionOf ( :DSURightToUniversityStudiesAggregate
                                          :USTATAverageContributionsAggregate
                                          :USTATContributionByClass
                                          :USTATEnrolledStudentsAggregate
                                          :USTATInterventionsForStudentsByUniversitiesAggregate
                                          :USTATPartiallyExoneratedStudentsAggregate
                                          :USTATPostgraduateAggregateOfEnrolled
                                          :USTATPostgraduateAggregateOfRegistered
                                          :USTATTotallyExoneratedStudentsAggregate
                                        )
                          ] ;
              rdfs:range xsd:gYear ;
              rdfs:comment "Academic year of reference of the data. The academic year is defined as the period of the year in which a university or other higher education institution carries out its activities in accordance with the regulations in force."@en ,
                           "Anno Accademico di riferimento dei dati. L'anno accademico viene definito come il periodo dell'anno in cui un'università oppure un altro istituto competente in materia di istruzione superiore svolge la propria attività, in conformità con le normative vigenti."@it ;
              rdfs:isDefinedBy <https://w3id.org/italia/onto/HER> ;
              rdfs:label "academic year"@en ,
                         "anno accademico"@it .


###  https://w3id.org/italia/onto/HER/active
:active rdf:type owl:DatatypeProperty ,
                 owl:FunctionalProperty ;
        rdfs:domain :Spinoff ;
        rdfs:range xsd:boolean ;
        rdfs:comment "Definisce lo status dello spin-off come riportato nel dataset."@it ,
                     "It defines the status of the spin-off as reported in the dataset."@en ;
        rdfs:isDefinedBy <https://w3id.org/italia/onto/HER> ;
        rdfs:label "active"@en ,
                   "attiva"@it ;
        owl:versionInfo "stabile"@it ,
                        "stable"@en .


###  https://w3id.org/italia/onto/HER/actualCompletionDate
:actualCompletionDate rdf:type owl:DatatypeProperty ;
                      rdfs:subPropertyOf ti:date ;
                      rdfs:domain :AACTStudy ;
                      rdfs:range xsd:date ;
                      rdfs:comment "La data in cui l'ultimo partecipante a uno studio clinico è stato esaminato o ha ricevuto un intervento/trattamento per raccogliere i dati finali per le misure di esito primario, le misure di esito secondario e gli eventi avversi (cioè l'ultima visita dell'ultimo partecipante). La data \"stimata\" di completamento dello studio è la data che i ricercatori ritengono essere la data di completamento dello studio."@it ,
                                   "The date on which the last participant in a clinical study was examined or received an intervention/treatment to collect final data for the primary outcome measures, secondary outcome measures, and adverse events (that is, the last participant's last visit). The \"estimated\" study completion date is the date that the researchers think will be the study completion date."@en ;
                      rdfs:isDefinedBy <https://w3id.org/italia/onto/HER> ;
                      rdfs:label "actual completion date"@en ,
                                 "data effettiva di completamento"@it ;
                      owl:versionInfo "provvisoria"@it ,
                                      "unstable"@en .


###  https://w3id.org/italia/onto/HER/additionalInfo
:additionalInfo rdf:type owl:DatatypeProperty ;
                rdfs:domain :Spinoff ;
                rdfs:range rdfs:Literal ;
                rdfs:comment "It reports notes and additional information about the spin-off, if any."@en ,
                             "Riporta delle note e informazioni addizionali sullo spin-off, se presenti."@it ;
                rdfs:isDefinedBy <https://w3id.org/italia/onto/HER> ;
                rdfs:label "additional information"@en ,
                           "informazioni aggiuntive"@it ;
                owl:versionInfo "stabile"@it ,
                                "stable"@en .


###  https://w3id.org/italia/onto/HER/admissionDate
:admissionDate rdf:type owl:DatatypeProperty ;
               rdfs:subPropertyOf ti:date ;
               rdfs:domain :CTNPRINOperation ;
               rdfs:range xsd:date ;
               rdfs:comment "Data del decreto di ammissione al finanziamento del progetto associato all'operazione"@it ,
                            "Date of the decree of admission to the financing of the project associated with the operation"@en ;
               rdfs:isDefinedBy <https://w3id.org/italia/onto/HER> ;
               rdfs:label "admission date"@en ,
                          "data di ammissione"@it ;
               owl:versionInfo "stabile"@it ,
                               "stable"@en .


###  https://w3id.org/italia/onto/HER/ageClass
:ageClass rdf:type owl:DatatypeProperty ;
          rdfs:domain :USTATStaffByGender ;
          rdfs:range rdfs:Literal ;
          rdfs:comment "Age classes of teaching/researcher staff. Currently can take the following values: <35; 35 - 44; 45 -54; >=55"@en ,
                       "Età in classi del personale docente/ricercatore. Attualmente può assumere i seguenti valori: <35; 35 - 44; 45 -54; >=55"@it ;
          rdfs:isDefinedBy <https://w3id.org/italia/onto/HER> ;
          rdfs:label "age class"@en ,
                     "classe di etá"@it ;
          owl:versionInfo "stabile"@it ,
                          "stable"@en .


###  https://w3id.org/italia/onto/HER/allocation
:allocation rdf:type owl:DatatypeProperty ;
            rdfs:domain :AACTDesign ;
            rdfs:range rdfs:Literal ;
            rdfs:comment """A method used to assign participants to an arm of a clinical study. The types of allocation are:
N/A (not applicable): For a single-arm trial
Randomized: Participants are assigned to intervention groups by chance
Nonrandomized: Participants are expressly assigned to intervention groups through a non-random method, such as physician choice
"""@en ,
                         """Un metodo utilizzato per assegnare i partecipanti ad una branca di uno studio clinico. I tipi di assegnazione sono:
N/A (non applicabile): Per uno studio su una singola branca
Casuale: I partecipanti sono assegnati a gruppi d'intervento per caso
Non raro: I partecipanti sono espressamente assegnati ai gruppi di intervento attraverso un metodo non casuale, come la scelta del medico"""@it ;
            rdfs:isDefinedBy <https://w3id.org/italia/onto/HER> ;
            rdfs:label "allocation"@en ,
                       "assegnazione"@it ;
            owl:versionInfo "provvisoria"@it ,
                            "unstable"@en .


###  https://w3id.org/italia/onto/HER/availableSlot
:availableSlot rdf:type owl:DatatypeProperty ;
               rdfs:domain :USTATUniversityFacilitiesAggregate ;
               rdfs:range xsd:integer ;
               rdfs:comment """Numero di posti complessivamente disponibili nelle mense e residenze universitarie direttamente gestite dall'istituto all'1/11/(T).
Dalle \"Note sul dataset Contribuzione e interventi\":
I valori negativi hanno i seguenti significati:
-1: ateneo non rispondente/inadempiente
-2: dato non disponibile
-3: dato non pervenuto
-4: dato incluso in altra voce
-5: dato da definire
-6: dato non rilevabile

Gli spazi vuoti indicano un valore non esistente."""@it ,
                            """Total number of places available in canteens and university residences directly managed by the institute on 1/11/(T).
From \"Notes on the dataset Contribution and interventions\"\":
The negative values have the following meanings
-1: university not responding / non-compliant
-2: data not available
-3: data not received
-4: data included under another heading
-5: data to be defined
-6: data not detectable

Blanks indicate a non-existent value."""@en ;
               rdfs:isDefinedBy <https://w3id.org/italia/onto/HER> ;
               rdfs:label "available slot"@en ,
                          "slot disponibile"@it ;
               owl:versionInfo "stabile"@it ,
                               "stable"@en .


###  https://w3id.org/italia/onto/HER/averageTaxForPayingStudents
:averageTaxForPayingStudents rdf:type owl:DatatypeProperty ;
                             rdfs:subPropertyOf <https://w3id.org/italia/onto/MU/value> ;
                             rdfs:domain :USTATAverageContributionsAggregate ;
                             rdfs:comment "Average contribution for students enrolled in degree courses, master's degree courses, courses of the old system calculated on the basis of the fees actually paid (net of the regional tax for the Right to University Studies - DSU and stamp duty where applicable), EXCLUDED students totally exempted, students for whom the contribution is not expected or is financed by external bodies. The values are expressed in EURO. The average is calculated considering the central point of each contribution class."@en ,
                                          """Contribuzione media per gli studenti iscritti a corsi di laurea, corsi di laurea magistrale, corsi del vecchio ordinamento calcolata sulla base delle tasse realmente pagate (al netto della tassa regionale per il Diritto allo Studio Universitario - DSU e dell’imposta di bollo dove previste), ESCLUSI gli studenti esonerati totalmente, gli studenti per i quali la contribuzione non è prevista o è finanziata da enti esterni. I valori sono espressi in EURO. La media è calcolata considerando il punto centrale di ciascuna classe di contribuzione.
"""@it ;
                             rdfs:isDefinedBy <https://w3id.org/italia/onto/HER> ;
                             rdfs:label "average taxes for paying students"@en ,
                                        "spesa media delle tasse per pagare gli studenti"@it .


###  https://w3id.org/italia/onto/HER/averageTaxForTotalEnrolledStudents
:averageTaxForTotalEnrolledStudents rdf:type owl:DatatypeProperty ;
                                    rdfs:subPropertyOf <https://w3id.org/italia/onto/MU/value> ;
                                    rdfs:domain :USTATAverageContributionsAggregate ;
                                    rdfs:comment "Average contribution for students enrolled in degree courses, master's degree courses, courses of the old system calculated on the basis of the fees actually paid (net of the regional tax for the Right to University Studies - DSU and stamp duty where applicable), INCLUDING students totally exempted, students for whom the contribution is not expected or is financed by external bodies. Values are expressed in EURO. The average is calculated considering the central point of each contribution class."@en ,
                                                 "Contribuzione media per gli studenti iscritti a corsi di laurea, corsi di laurea magistrale, corsi del vecchio ordinamento calcolata sulla base delle tasse realmente pagate (al netto della tassa regionale per il DSU e dell’imposta di bollo dove previste), INCLUSI gli studenti esonerati totalmente, gli studenti per i quali la contribuzione non è prevista o è finanziata da enti esterni. I valori sono espressi in EURO. La media è calcolata considerando il punto centrale di ciascuna classe di contribuzione."@it ;
                                    rdfs:isDefinedBy <https://w3id.org/italia/onto/HER> ;
                                    rdfs:label "average taxes for total enrolled students"@en ,
                                               "spesa media delle tasse per pagare tutti gli studenti iscritti"@it .


###  https://w3id.org/italia/onto/HER/baselinePopulation
:baselinePopulation rdf:type owl:DatatypeProperty ;
                    rdfs:domain :AACTStudy ;
                    rdfs:range xsd:int ;
                    rdfs:comment "Data collected at the beginning of a clinical study for all participants and for each arm or comparison group. These data include demographics, such as age, sex/gender, race and ethnicity, and study-specific measures (for example, systolic blood pressure, prior antidepressant treatment)."@en ,
                                 "Dati raccolti all'inizio di uno studio clinico per tutti i partecipanti e per ogni braccio o gruppo di confronto. Questi dati includono dati demografici, come l'età, il sesso/genere, la razza e l'etnia, e misure specifiche dello studio (ad esempio, pressione sanguigna sistolica, trattamento antidepressivo preventivo)."@it ;
                    rdfs:isDefinedBy <https://w3id.org/italia/onto/HER> ;
                    rdfs:label "baseline population"@en ,
                               "popolazione di base"@it .


###  https://w3id.org/italia/onto/HER/biospecDescription
:biospecDescription rdf:type owl:DatatypeProperty ;
                    rdfs:subPropertyOf l0:description ;
                    rdfs:domain :AACTStudy ;
                    rdfs:range rdfs:Literal ;
                    rdfs:comment "Biological samples of material from study participants (e.g., whole blood, serum, white cells, urine, tissue)."@en ,
                                 "Descrizione dei campioni biologici di materiale proveniente dai partecipanti allo studio (ad esempio, sangue intero, siero, globuli bianchi, urine, tessuti)."@it ;
                    rdfs:isDefinedBy <https://w3id.org/italia/onto/HER> ;
                    rdfs:label "biospec description"@en ,
                               "descrizione biospec"@it ;
                    owl:versionInfo "stabile"@it ,
                                    "stable"@en .


###  https://w3id.org/italia/onto/HER/biospecRetention
:biospecRetention rdf:type owl:DatatypeProperty ;
                  rdfs:domain :AACTStudy ;
                  rdfs:range rdfs:Literal ;
                  rdfs:comment """Indica se i campioni di materiale dei partecipanti alla ricerca sono conservati in un biorepository. I valori ammessi sono:
Nessuno Conservato: Nessun campione conservato
Campioni con DNA: Campioni conservati, con possibilità di estrazione del DNA da almeno uno dei tipi di campioni conservati (ad esempio, tessuto congelato, sangue intero)
Campioni senza DNA: Campioni conservati, senza possibilità di estrazione del DNA da campioni conservati (ad esempio, tessuto fisso, plasma)"""@it ,
                               """Indicate whether samples of material from research participants are retained in a biorepository. They can be:
None Retained: No samples retained
Samples With DNA: Samples retained, with potential for extraction of DNA from at least one of the types of samples retained (e.g., frozen tissue, whole blood)
Samples Without DNA: Samples retained, with no potential for DNA extraction from any retained samples (e.g., fixed tissue, plasma)
"""@en ;
                  rdfs:isDefinedBy <https://w3id.org/italia/onto/HER> ;
                  rdfs:label "biospec retention"@en ,
                             "conservazione biospec"@it ;
                  owl:versionInfo "provvisoria"@it ,
                                  "unstable"@en .


###  https://w3id.org/italia/onto/HER/birthyear
:birthyear rdf:type owl:DatatypeProperty ;
           rdfs:subPropertyOf ti:year ;
           rdfs:domain <https://w3id.org/italia/onto/CPV/Person> ;
           rdfs:range xsd:gYear ;
           rdfs:comment "A person's year of birth."@en ,
                        "L'anno di nascita di una persona."@it ;
           rdfs:isDefinedBy <https://w3id.org/italia/onto/HER> ;
           rdfs:label "anno di nascita"@it ,
                      "birthyear"@en .


###  https://w3id.org/italia/onto/HER/caregiverMasked
:caregiverMasked rdf:type owl:DatatypeProperty ;
                 rdfs:domain :AACTDesign ;
                 rdfs:range xsd:boolean ;
                 rdfs:comment "Caregiver is the party or parties involved in the clinical trial who are prevented from having knowledge of the interventions assigned to individual participants."@en ,
                              "Il caregiver sono le parti coinvolte nello studio clinico a cui viene impedito di conoscere gli interventi assegnati ai singoli partecipanti."@it ;
                 rdfs:isDefinedBy <https://w3id.org/italia/onto/HER> ;
                 rdfs:label "caregiver masked"@en ,
                            "parti coinvolte conoscono interventi"@it ;
                 owl:versionInfo "provvisoria"@it ,
                                 "unstable"@en .


###  https://w3id.org/italia/onto/HER/completionMonthYear
:completionMonthYear rdf:type owl:DatatypeProperty ;
                     rdfs:subPropertyOf ti:month ;
                     rdfs:domain :AACTStudy ;
                     rdfs:range xsd:gMonth ;
                     rdfs:comment "Il valore della data di completamento esattamente come viene fornito da ClinicalTrials.gov. Alcuni studi hanno solo mese/anno definito la data di completamento (es. ottobre 2014). Questo valore è memorizzato in questa colonna e la colonna completion_date converte questo valore in una data assegnandogli il primo giorno del mese."@it ,
                                  "The value of the completion date exactly as it is provided by ClinicalTrials.gov. Some studies have only month/year defined for the completion date (ie. October, 2014). That value is stored in this column and the completion_date column converts this value to a date by assigning it the first day of the month."@en ;
                     rdfs:isDefinedBy <https://w3id.org/italia/onto/HER> ;
                     rdfs:label "completion month-year"@en ,
                                "mese-anno di completamento"@it .


###  https://w3id.org/italia/onto/HER/contribution
:contribution rdf:type owl:DatatypeProperty ;
              rdfs:domain :EUREKAParticipant ;
              rdfs:range xsd:float ;
              rdfs:comment "Contributo finanziario"@it ,
                           "Financial contribution"@en ;
              rdfs:isDefinedBy <https://w3id.org/italia/onto/HER> ;
              rdfs:label "contribution"@en ,
                         "contributo"@it ;
              owl:versionInfo "provvisoria"@it ,
                              "unstable"@en .


###  https://w3id.org/italia/onto/HER/cooperativeClassificationLabel
:cooperativeClassificationLabel rdf:type owl:DatatypeProperty .


###  https://w3id.org/italia/onto/HER/cordisRef
:cordisRef rdf:type owl:DatatypeProperty ;
           rdfs:subPropertyOf l0:identifier ;
           rdfs:domain [ rdf:type owl:Class ;
                         owl:unionOf ( :ECProject
                                       :ERCProject
                                     )
                       ] ;
           rdfs:range rdfs:Literal ;
           rdfs:comment "Numero record di un progetto CE all'interno di CORDIS."@it ,
                        "Record number of an EC project within CORDIS."@en ;
           rdfs:isDefinedBy <https://w3id.org/italia/onto/HER> ;
           rdfs:label "cordis reference number"@en ,
                      "numero di riferimento cordis"@it ;
           owl:versionInfo "stabile"@it ,
                           "stable"@en .


###  https://w3id.org/italia/onto/HER/ctnprinAmountAdmittedCost
:ctnprinAmountAdmittedCost rdf:type owl:DatatypeProperty ;
                           rdfs:subPropertyOf <https://w3id.org/italia/onto/MU/value> ;
                           rdfs:domain :CTNPRINAmount ;
                           rdfs:comment "Cost admitted by decree after the evaluation of the costs indicated in the project proposal for each item of expenditure"@en ,
                                        "Costo ammesso da decreto dopo la valutazione dei costo indicato nella proposta di progetto  per singola voce di spesa"@it ;
                           rdfs:label "admitted cost of CTN/PRIN amount"@en ,
                                      "costo ammesso dell'importo CTN/PRIN"@it .


###  https://w3id.org/italia/onto/HER/ctnprinAmountApprovedCost
:ctnprinAmountApprovedCost rdf:type owl:DatatypeProperty ;
                           rdfs:subPropertyOf <https://w3id.org/italia/onto/MU/value> ;
                           rdfs:domain :CTNPRINAmount ;
                           rdfs:comment "Approved cost per individual expense item after valuation in itinere compared to the cost reported by the beneficiary to which the operation relates."@en ,
                                        "Costo approvato per singola voce di spesa dopo valutazione in itinere rispetto al costo rendicontato dal beneficiario a cui fa capo l'operazione."@it ;
                           rdfs:label "approved cost of CTN/PRIN amount"@en ,
                                      "costo approvato dell'importo CTN/PRIN"@it .


###  https://w3id.org/italia/onto/HER/ctnprinAmountCommittedContribution
:ctnprinAmountCommittedContribution rdf:type owl:DatatypeProperty ;
                                    rdfs:subPropertyOf <https://w3id.org/italia/onto/MU/value> ;
                                    rdfs:domain :CTNPRINAmount ;
                                    rdfs:comment "Contribution committed by the Ministry on the eligible costs per single expense item following ex-ante evaluation"@en ,
                                                 "Contributo impegnato dal Ministero sui costi ammessi per singola voce di spesa a seguito di valutazione ex-ante"@it ;
                                    rdfs:label "committed contribution of CTN/PRIN amount"@en ,
                                               "contributo impegnato dell'importo CTN/PRIN"@it .


###  https://w3id.org/italia/onto/HER/ctnprinAmountCommittedCredit
:ctnprinAmountCommittedCredit rdf:type owl:DatatypeProperty ;
                              rdfs:subPropertyOf <https://w3id.org/italia/onto/MU/value> ;
                              rdfs:domain :CTNPRINAmount ;
                              rdfs:comment """Credit committed by the Ministry on the eligible costs per single expense item following ex-ante evaluation
(for companies only)."""@en ,
                                           """Credito impegnato dal Ministero sui costi ammessi per singola voce di spesa a seguito di valutazione ex-ante
(solo per imprese)."""@it ;
                              rdfs:label "committed credit of CTN/PRIN amount"@en ,
                                         "credito impegnato dell'importo CTN/PRIN"@it .


###  https://w3id.org/italia/onto/HER/ctnprinAmountReportedCost
:ctnprinAmountReportedCost rdf:type owl:DatatypeProperty ;
                           rdfs:subPropertyOf <https://w3id.org/italia/onto/MU/value> ;
                           rdfs:domain :CTNPRINAmount ;
                           rdfs:comment "Cost reported by the beneficiary to which the operation relates by single expense item compared to the eligible costs"@en ,
                                        "Costo rendicontato dal beneficiaro a cui fa capo l'operazione per singola voce di spesa rispetto ai costi ammessi"@it ;
                           rdfs:label "costo rendicontato dell'importo CTN/PRIN"@it ,
                                      "reported cost of CTN/PRIN amount"@en .


###  https://w3id.org/italia/onto/HER/ctnprinAmountScope
:ctnprinAmountScope rdf:type owl:DatatypeProperty ;
                    rdfs:domain :CTNPRINAmount ;
                    rdfs:range rdfs:Literal ;
                    rdfs:comment """Ambito operativo a cui si riferisce l'importo tra quelli previsti dall'iniziativa:
- Ricerca di base
- Ricerca industriale
- Sviluppo
- Formazione"""@it ,
                                 """Operational scope to which the amount among those foreseen by the initiative refers:
- Basic research
- Industrial research
- Development
- Training"""@en ;
                    rdfs:isDefinedBy <https://w3id.org/italia/onto/HER> ;
                    rdfs:label "ambito di importo CTN/PRIN"@it ,
                               "scope of CTN/PRIN amount"@en ;
                    owl:versionInfo "provvisoria"@it ,
                                    "unstable"@en .


###  https://w3id.org/italia/onto/HER/ctnprinAvailableBudget
:ctnprinAvailableBudget rdf:type owl:DatatypeProperty ,
                                 owl:FunctionalProperty ;
                        rdfs:domain :CTNPRINFinancingFund ;
                        rdfs:range rdfs:Literal ;
                        rdfs:comment "Budget for the initiative available from the financing fund."@en ,
                                     "Budget per l'iniziativa in esame disponibile sul fondo di finanziamento."@it ;
                        rdfs:isDefinedBy <https://w3id.org/italia/onto/HER> ;
                        rdfs:label "available budget CTN/PRIN initiative's financing fund"@en ,
                                   "budget disponibile fondo di finanziamento iniziativa CTN/PRIN"@it ;
                        owl:versionInfo "stabile"@it ,
                                        "stable"@en .


###  https://w3id.org/italia/onto/HER/ctnprinInitiativeAdmittedCost
:ctnprinInitiativeAdmittedCost rdf:type owl:DatatypeProperty ;
                               rdfs:subPropertyOf <https://w3id.org/italia/onto/MU/value> ;
                               rdfs:domain :CTNPRINInitiative ;
                               rdfs:comment "Total admitted costs after evaluation of the costs indicated in the project proposals.  Calculated as the sum of the counterpart variable 'admittedCost' present at lower aggregation level (admittedCost_operations)"@en ,
                                            "Totale dei costi ammessi dopo la valutazione dei costi indicati nelle proposte di progetto.  Calcolati come somma dell'omologa variabile \"admittedCost\" presente a livello di aggregazione inferiore (admittedCost_operations)"@it ;
                               rdfs:label "admitted cost of CTN/PRIN initiative"@en ,
                                          "costi ammessi per iniziative CTN/PRIN"@it .


###  https://w3id.org/italia/onto/HER/ctnprinInitiativeApprovedCost
:ctnprinInitiativeApprovedCost rdf:type owl:DatatypeProperty ;
                               rdfs:subPropertyOf <https://w3id.org/italia/onto/MU/value> ;
                               rdfs:domain :CTNPRINInitiative ;
                               rdfs:comment "Total costs approved after in itinere evaluation compared to the costs reported by the beneficiaries. Calculated as the sum of the homologous 'approvedCost' variable present at the lower aggregation level (approvedCost_operations)"@en ,
                                            "Totale dei costi approvati dopo valutazione in itinere rispetto ai costi rendicontati dai beneficiari. Calcolati come somma dell'omologa variabile \"approvedCost\" presente a livello di aggregazione inferiore (approvedCost_operations)"@it ;
                               rdfs:label "approved cost of CTN/PRIN initiative"@en ,
                                          "costi approvati per iniziative CTN/PRIN"@it .


###  https://w3id.org/italia/onto/HER/ctnprinInitiativeCommittedContribution
:ctnprinInitiativeCommittedContribution rdf:type owl:DatatypeProperty ;
                                        rdfs:subPropertyOf <https://w3id.org/italia/onto/MU/value> ;
                                        rdfs:domain :CTNPRINInitiative ;
                                        rdfs:comment "Total contributions committed by the Ministry on eligible costs following ex-ante evaluation. Calculated as the sum of the homologous variable \"committedContribution\" present at the lower aggregation level (committedContribution_operations)"@en ,
                                                     "Totale dei contributi impegnati dal Ministero sui costi ammessi a seguito di valutazione ex-ante. Calcolati come somma dell'omologa variabile \"committedContribution\" presente a livello di aggregazione inferiore (committedContribution_operations)"@it ;
                                        rdfs:label "committed contribution of CTN/PRIN initiative"@en ,
                                                   "contributi impiegati per iniziative CTN/PRIN"@it .


###  https://w3id.org/italia/onto/HER/ctnprinInitiativeCommittedCredit
:ctnprinInitiativeCommittedCredit rdf:type owl:DatatypeProperty ;
                                  rdfs:subPropertyOf <https://w3id.org/italia/onto/MU/value> ;
                                  rdfs:domain :CTNPRINInitiative ;
                                  rdfs:comment "Total credits committed by the Ministry on eligible costs following ex-ante evaluation (only for companies). Calculated as the sum of the homologous variable 'committedCredit' present at the lower aggregation level (committedCredit_operations)."@en ,
                                               "Totale dei crediti impegnati dal Ministero sui costi ammessi a seguito di valutazione ex-ante (solo per imprese). Calcolati come somma dell'omologa variabile \"committedCredit\" presente a livello di aggregazione inferiore (committedCredit_operations)."@it ;
                                  rdfs:label "committed credit of CTN/PRIN initiative"@en ,
                                             "credito impegnato per iniziative CTN/PRIN"@it .


###  https://w3id.org/italia/onto/HER/ctnprinInitiativeGrantedContribution
:ctnprinInitiativeGrantedContribution rdf:type owl:DatatypeProperty ;
                                      rdfs:subPropertyOf <https://w3id.org/italia/onto/MU/value> ;
                                      rdfs:domain :CTNPRINInitiative ;
                                      rdfs:comment "Total contributions disbursed compared to approved costs. Calculated as the sum of the corresponding 'grantedContribution' variable at the lower aggregation level (grantedContribution_operations)."@en ,
                                                   "Totale dei contributi erogati rispetto ai costi approvati. Calcolati come somma dell'omologa variabile \"grantedContribution\" presente a livello di aggregazione inferiore (grantedContribution_operations)."@it ;
                                      rdfs:label "contributo erogato per iniziative CTN/PRIN"@it ,
                                                 "granted contribution of CTN/PRIN initiative"@en .


###  https://w3id.org/italia/onto/HER/ctnprinInitiativeReportedCost
:ctnprinInitiativeReportedCost rdf:type owl:DatatypeProperty ;
                               rdfs:subPropertyOf <https://w3id.org/italia/onto/MU/value> ;
                               rdfs:domain :CTNPRINInitiative ;
                               rdfs:comment "Total costs reported by beneficiaries compared to eligible costs. Calculated as the sum of the homologous variable 'reportedCost' present at the lower aggregation level (reportedCost_operations)"@en ,
                                            "Totale dei costi rendicontati dai beneficiari rispetto ai costi ammessi. Calcolati come somma dell'omologa variabile \"reportedCost\" presente a livello di aggregazione inferiore (reportedCost_operations)"@it ;
                               rdfs:label "costi rendicontati per iniziative CTN/PRIN"@it ,
                                          "reported cost of CTN/PRIN initiative"@en .


###  https://w3id.org/italia/onto/HER/ctnprinOperationAdmittedCost
:ctnprinOperationAdmittedCost rdf:type owl:DatatypeProperty ;
                              rdfs:subPropertyOf <https://w3id.org/italia/onto/MU/value> ;
                              rdfs:domain :CTNPRINOperation ;
                              rdfs:comment "Admitted costs after evaluation of the costs indicated in the project proposal. Calculated as the sum of the counterpart variable 'admittedCost' present at lower aggregation level (admittedCost_amounts)"@en ,
                                           "Costi ammessi dopo la valutazione dei costi indicati nella proposta di progetto. Calcolati come somma dell'omologa variabile \"admittedCost\" presente a livello di aggregazione inferiore (admittedCost_amounts)"@it ;
                              rdfs:label "admitted cost of CTN/PRIN operation"@en ,
                                         "costi amessi per operazioni CTN/PRIN"@it .


###  https://w3id.org/italia/onto/HER/ctnprinOperationApprovedCost
:ctnprinOperationApprovedCost rdf:type owl:DatatypeProperty ;
                              rdfs:subPropertyOf <https://w3id.org/italia/onto/MU/value> ;
                              rdfs:domain :CTNPRINOperation ;
                              rdfs:comment "Costi approvati dopo valutazione in itinere rispetto ai costi rendicontati dal beneficiario a cui fa capo l'operazione. Calcolati come somma dell'omologa variabile \"approvedCost\" presente a livello di aggregazione inferiore (approvedCost_amounts)"@it ,
                                           "Costs approved after evaluation in itinere compared to the costs reported by the beneficiary to which the operation belongs. Calculated as the sum of the approvedCost variable at the lower aggregation level (approvedCost_amounts)."@en ;
                              rdfs:label "approved cost of CTN/PRIN operation"@en ,
                                         "costi approvati per operazioni CTN/PRIN"@it .


###  https://w3id.org/italia/onto/HER/ctnprinOperationCommittedContribution
:ctnprinOperationCommittedContribution rdf:type owl:DatatypeProperty ;
                                       rdfs:subPropertyOf <https://w3id.org/italia/onto/MU/value> ;
                                       rdfs:domain :CTNPRINOperation ;
                                       rdfs:comment "Contributi impegnati dal Ministero sui costi ammessi a seguito di valutazione ex-ante. Calcolati come somma dell'omologa variabile \"committedContribution\" presente a livello di aggregazione inferiore (committedContribution_operations)"@it ,
                                                    "Contributions committed by the Ministry on eligible costs following ex-ante evaluation. Calculated as the sum of the corresponding 'committedContribution' variable at the lower aggregation level (committedContribution_operations)."@en ;
                                       rdfs:label "committed contribution of CTN/PRIN operation"@en ,
                                                  "contributi impegnati per operazioni CTN/PRIN"@it .


###  https://w3id.org/italia/onto/HER/ctnprinOperationCommittedCredit
:ctnprinOperationCommittedCredit rdf:type owl:DatatypeProperty ;
                                 rdfs:subPropertyOf <https://w3id.org/italia/onto/MU/value> ;
                                 rdfs:domain :CTNPRINOperation ;
                                 rdfs:comment "Crediti impegnati dal Ministero sui costi ammessi a seguito di valutazione ex-ante (solo per imprese). Calcolati come somma dell'omologa variabile \"committedCredit\" presente a livello di aggregazione inferiore (committedCredit_amounts)"@it ,
                                              "Credits committed by the Ministry on eligible costs following ex-ante evaluation (only for companies). Calculated as the sum of the homologous variable 'committedCredit' present at the lower aggregation level (committedCredit_amounts)"@en ;
                                 rdfs:label "committed credit of CTN/PRIN operation"@en ,
                                            "credito impegnato per operazioni CTN/PRIN"@it .


###  https://w3id.org/italia/onto/HER/ctnprinOperationGrantedContribution
:ctnprinOperationGrantedContribution rdf:type owl:DatatypeProperty ;
                                     rdfs:subPropertyOf <https://w3id.org/italia/onto/MU/value> ;
                                     rdfs:domain :CTNPRINOperation ;
                                     rdfs:comment "It represents the contributions disbursed in relation to the costs approved for the operation."@en ,
                                                  "Rappresenta i contributi erogati rispetto ai costi approvati per l'operazione."@it ;
                                     rdfs:label "contributo erogato per operazioni CTN/PRIN"@it ,
                                                "granted contribution of CTN/PRIN operation"@en .


###  https://w3id.org/italia/onto/HER/ctnprinOperationIdentifier
:ctnprinOperationIdentifier rdf:type owl:DatatypeProperty ;
                            rdfs:subPropertyOf l0:identifier ;
                            rdfs:domain :CTNPRINOperation ;
                            rdfs:range rdfs:Literal ;
                            rdfs:comment """ID univoco di una operazione.
E' ottenuto concatenando le seguenti variabili all'origine:
Codice locale progetto +  ambito + CF beneficiario
corrispondenti a: projectCode + scope_operations + fiscalcode_entity"""@it ,
                                         """Unique ID of an operation.
It is obtained by concatenating the following variables at the origin: \"Codice locale progetto +  ambito + CF beneficiario\"  corresponding to: projectCode + scope_operations + fiscalcode_entity"""@en ;
                            rdfs:label "CTN/PRIN operation identifier"@en ,
                                       "identificatore operazione CTN/PRIN"@it .


###  https://w3id.org/italia/onto/HER/ctnprinOperationReportedCost
:ctnprinOperationReportedCost rdf:type owl:DatatypeProperty ;
                              rdfs:subPropertyOf <https://w3id.org/italia/onto/MU/value> ;
                              rdfs:domain :CTNPRINOperation ;
                              rdfs:comment "Costi rendicontati dal beneficiario a cui fa capo l'operazione rispetto ai costi ammessi. Calcolati come somma dell'omologa variabile \"reportedCost\" presente a livello di aggregazione inferiore (reportedCost_amounts)"@it ,
                                           "Costs reported by the beneficiary to which the operation relates in relation to the eligible costs. Calculated as the sum of the homologous variable 'reportedCost' present at the lower aggregation level (reportedCost_amounts)"@en ;
                              rdfs:label "costi rendicontati da operazioni CTN/PRIN"@it ,
                                         "reported cost of CTN/PRIN operation"@en .


###  https://w3id.org/italia/onto/HER/ctnprinOperationScope
:ctnprinOperationScope rdf:type owl:DatatypeProperty ;
                       rdfs:domain :CTNPRINOperation ;
                       rdfs:range rdfs:Literal ;
                       rdfs:comment """Ambito operativo dell'operazione. Può essere:
- R&S
- Formazione
- Ricerca di base"""@it ,
                                    """Operational scope of the operation. Could be:
- R&D
- Training
- Basic research"""@en ;
                       rdfs:label "ambito operazione CTN/PRIN"@it ,
                                  "scope of CTN/PRIN operation"@en ;
                       owl:versionInfo "provvisoria"@it ,
                                       "unstable"@en .


###  https://w3id.org/italia/onto/HER/ctnprinSecondLevelSR
:ctnprinSecondLevelSR rdf:type owl:DatatypeProperty ;
                      rdfs:domain [ rdf:type owl:Class ;
                                    owl:unionOf ( :CTNPRINOperation
                                                  :CTNPRINProject
                                                )
                                  ] ;
                      rdfs:range rdfs:Literal ;
                      rdfs:comment "Area/settore di riferimento di secondo livello (se presente)"@it ,
                                   "Second level area/sector of reference (if any)"@en ;
                      rdfs:isDefinedBy <https://w3id.org/italia/onto/HER> ;
                      rdfs:label "second level CTN/PRIN sector of reference"@en ,
                                 "secondo livello settore riferimento CTN/PRIN"@it ;
                      owl:versionInfo "provvisoria"@it ,
                                      "unstable"@en .


###  https://w3id.org/italia/onto/HER/ctnprinSectorOfReference
:ctnprinSectorOfReference rdf:type owl:DatatypeProperty ;
                          rdfs:domain [ rdf:type owl:Class ;
                                        owl:unionOf ( :CTNPRINOperation
                                                      :CTNPRINProject
                                                    )
                                      ] ;
                          rdfs:range rdfs:Literal ;
                          rdfs:comment "Area/sector of reference of the project among those foreseen for the initiative that finances the project."@en ,
                                       "Area/settore di riferimento del progetto tra quelli previsti per l'iniziativa che finanzia il progetto."@it ;
                          rdfs:isDefinedBy <https://w3id.org/italia/onto/HER> ;
                          rdfs:label "CTN/PRIN sector of reference"@en ,
                                     "settore riferimento CTN/PRIN"@it ;
                          owl:versionInfo "provvisoria"@it ,
                                          "unstable"@en .


###  https://w3id.org/italia/onto/HER/cycleStartingYear
:cycleStartingYear rdf:type owl:DatatypeProperty ;
                   rdfs:subPropertyOf ti:year ;
                   rdfs:domain :ItalianPhDCourseByCycle ;
                   rdfs:range xsd:gYear ;
                   rdfs:comment "L'anno di inizio del ciclo accademico corrispondente."@it ,
                                "The start year of the corresponding academic cycle."@en ;
                   rdfs:isDefinedBy <https://w3id.org/italia/onto/HER> ;
                   rdfs:label "anno di inizio del ciclo"@it ,
                              "cycle starting year"@en .


###  https://w3id.org/italia/onto/HER/decreeDate
:decreeDate rdf:type owl:DatatypeProperty ;
            rdfs:subPropertyOf ti:date ;
            rdfs:domain :CTNPRINInitiative ;
            rdfs:range xsd:date ;
            rdfs:comment "Data di emissione del decreto MIUR (Ministero dell'Istruzione, dell'Università e della Ricerca) in cui è pubblicato il bando/avviso che definisce originariamente l'iniziativa in esame"@it ,
                         "Date of issue of the MIUR (Ministry of Education, University and Research) decree in which the call/notice originally defining the initiative in question is published"@en ;
            rdfs:isDefinedBy <https://w3id.org/italia/onto/HER> ;
            rdfs:label "data decreto"@it ,
                       "decree date"@en ;
            owl:versionInfo "stabile"@it ,
                            "stable"@en .


###  https://w3id.org/italia/onto/HER/decreeNumber
:decreeNumber rdf:type owl:DatatypeProperty ;
              rdfs:subPropertyOf l0:identifier ;
              rdfs:domain :CTNPRINInitiative ;
              rdfs:range rdfs:Literal ;
              rdfs:comment "Identification number of the MIUR (Ministry of Education, University and Research) decree in which the notice/warning/... which originally defines the initiative in question is published"@en ,
                           "Numero identificativo del decreto MIUR (Ministero dell'Istruzione, dell'Università e della Ricerca) in cui è pubblicato il bando/avviso/... che definisce originariamente l'iniziativa in esame"@it ;
              rdfs:isDefinedBy <https://w3id.org/italia/onto/HER> ;
              rdfs:label "decree number"@en ,
                         "numero decreto"@it ;
              owl:versionInfo "provvisoria"@it ,
                              "unstable"@en .


###  https://w3id.org/italia/onto/HER/departmentName
:departmentName rdf:type owl:DatatypeProperty ;
                rdfs:subPropertyOf l0:name ;
                rdfs:domain :ItalianPhDCourseByCycle ;
                rdfs:range rdfs:Literal ;
                rdfs:comment "Il nome del dipartimento universitario corrispondente."@it ,
                             "The corresponding university'a department name."@en ;
                rdfs:isDefinedBy <https://w3id.org/italia/onto/HER> ;
                rdfs:label "department"@en ,
                           "dipartimento"@it .


###  https://w3id.org/italia/onto/HER/dispositionFirstPostedDate
:dispositionFirstPostedDate rdf:type owl:DatatypeProperty ;
                            rdfs:subPropertyOf ti:date ;
                            rdfs:domain :AACTStudy ;
                            rdfs:range xsd:date ;
                            rdfs:comment "Il suffisso _posted indica la data in cui una presentazione è stata resa pubblica su ClinicalTrials.gov. In genere, l'invio avviene il giorno lavorativo successivo al completamento della revisione del qc. Abbiamo iniziato a raccogliere le date di pubblicazione all'inizio del 2017. Le date precedenti a tale data sono estmate. Tutte le date pubblicate includono un attributo di tipo Actual o Estimate."@it ,
                                         "The _posted suffix indicates the date that a submission was made public on ClinicalTrials.gov. Typically, posting occurs the business day after qc review was successfully completed. We began collecting posted dates in early 2017. Dates from before then are estmates. All posted dates include a type attribute of Actual or Estimate."@en ;
                            rdfs:isDefinedBy <https://w3id.org/italia/onto/HER> ;
                            rdfs:label "disposition first posted date"@en ,
                                       "disposizione prima data pubblicazione"@it ;
                            owl:versionInfo "stabile"@it ,
                                            "stable"@en .


###  https://w3id.org/italia/onto/HER/dispositionFirstPostedDateType
:dispositionFirstPostedDateType rdf:type owl:DatatypeProperty ;
                                rdfs:domain :AACTStudy ;
                                rdfs:comment "All posted dates include a type attribute of Actual or Estimate."@en ,
                                             "Tutte le date pubblicate includono un attributo di tipo Actual o Estimate."@it ;
                                rdfs:isDefinedBy <https://w3id.org/italia/onto/HER> ;
                                rdfs:label "disposition first posted date type"@en ,
                                           "disposizione prima data di pubblicazione tipo di data"@it ;
                                owl:versionInfo "provvisoria"@it ,
                                                "unstable"@en .


###  https://w3id.org/italia/onto/HER/dispositionFirstSubmittedDate
:dispositionFirstSubmittedDate rdf:type owl:DatatypeProperty ;
                               rdfs:subPropertyOf ti:date ;
                               rdfs:domain :AACTStudy ;
                               rdfs:range xsd:date ;
                               rdfs:comment "Data in cui uno sponsor indica che ritarderà la pubblicazione dei risultati (e sta certificando l'approvazione iniziale o il nuovo utilizzo), o quando richiede una proroga della scadenza. Il suffisso _submitted indica la data in cui il responsabile ha premuto il pulsante di rilascio nel sistema di invio dati di ClinicalTrials.gov, inviando così i dati per la revisione prima della pubblicazione."@it ,
                                            "Date when a sponsor indicates that they will be delaying posting of results (and are certifying initial approval or new use), or when they apply for an extension of the deadline. The _submitted suffix indicates the date that the responsible party pressed the release button in the ClinicalTrials.gov data submission system, thereby submitting the data for review prior to posting."@en ;
                               rdfs:isDefinedBy <https://w3id.org/italia/onto/HER> ;
                               rdfs:label "disposition first submitted date"@en ,
                                          "disposizione prima data presentazione"@it ;
                               owl:versionInfo "stabile"@it ,
                                               "stable"@en .


###  https://w3id.org/italia/onto/HER/dispositionFirstSubmittedQCDate
:dispositionFirstSubmittedQCDate rdf:type owl:DatatypeProperty ;
                                 rdfs:subPropertyOf ti:date ;
                                 rdfs:domain :AACTStudy ;
                                 rdfs:range xsd:date ;
                                 rdfs:comment "Il suffisso _submitted_qc indica la data di presentazione della versione del record che soddisfa i criteri di controllo della qualità. È comune che ci siano revisioni tra la prima presentazione e la presentazione che soddisfa i criteri qc. Si noti che questa non è la data in cui è stata completata la revisione qc"@it ,
                                              "The _submitted_qc suffix indicates the submission date of the version of the record that met quality control criteria. It is common for there to be revisions between the first submission and the submission that meets qc criteria. Note this is not the date that the qc review was completed.\""@en ;
                                 rdfs:isDefinedBy <https://w3id.org/italia/onto/HER> ;
                                 rdfs:label "disposition first submitted QC date"@en ,
                                            "disposizione prima data presentazione QC"@it ;
                                 owl:versionInfo "stabile"@it ,
                                                 "stable"@en .


###  https://w3id.org/italia/onto/HER/documentationURL
:documentationURL rdf:type owl:DatatypeProperty ;
                  rdfs:subPropertyOf <https://w3id.org/italia/onto/SM/URL> ;
                  rdfs:domain :CTNPRINInitiative ;
                  rdfs:range xsd:anyURI ;
                  rdfs:comment "Link a pagina web contenente il decreto del MIUR in cui è pubblicato il bando/avviso/... che prevede la concessione di finanziamenti per l'iniziativa in esame oltre ad eventuali allegati e decreti integrativi"@it ,
                               "Link to the web page containing the decree of the Ministry of Education, University and Research (MIUR) in which is published the call/announcement /... which provides for the granting of funding for the initiative in question, as well as any attachments and supplementary decrees."@en ;
                  rdfs:isDefinedBy <https://w3id.org/italia/onto/HER> ;
                  rdfs:label "URL documentazione"@it ,
                             "documentation URL"@en ;
                  owl:versionInfo "stabile"@it ,
                                  "stable"@en .


###  https://w3id.org/italia/onto/HER/downloadDateDescription
:downloadDateDescription rdf:type owl:DatatypeProperty ;
                         rdfs:domain :AACTStudy ;
                         rdfs:comment "Data in cui NLM ha reso disponibile lo studio tramite il suo API."@it ,
                                      "Date NLM made study available via their API."@en ;
                         rdfs:isDefinedBy <https://w3id.org/italia/onto/HER> ;
                         rdfs:label "Descrizione data di scarimento"@it ,
                                    "download date description"@en ;
                         owl:versionInfo "provvisoria"@it ,
                                         "unstable"@en .


###  https://w3id.org/italia/onto/HER/ecContribution
:ecContribution rdf:type owl:DatatypeProperty ;
                rdfs:subPropertyOf <https://w3id.org/italia/onto/MU/value> ;
                rdfs:domain [ rdf:type owl:Class ;
                              owl:unionOf ( :CHAFEAProject
                                            :ECParticipant
                                          )
                            ] ;
                rdfs:comment "Finanziamento concesso dall'Unione Europea. L'importo è espresso in euro."@it ,
                             "Funding granted by the European Union. The amount is expressed in euros."@en ;
                rdfs:isDefinedBy <https://w3id.org/italia/onto/HER> ;
                rdfs:label "EC contribution"@en ,
                           "contributo CE"@it .


###  https://w3id.org/italia/onto/HER/ecGrantAgreementNo
:ecGrantAgreementNo rdf:type owl:DatatypeProperty ;
                    rdfs:subPropertyOf l0:identifier ;
                    rdfs:domain [ rdf:type owl:Class ;
                                  owl:unionOf ( :ECProject
                                                :ERCProject
                                              )
                                ] ;
                    rdfs:range rdfs:Literal ;
                    rdfs:comment "Grant agreement identifier of an EC project."@en ,
                                 "Identificativo dell'accordo di finanziamento di un progetto CE."@it ;
                    rdfs:isDefinedBy <https://w3id.org/italia/onto/HER> ;
                    rdfs:label "ec grant agreement number"@en ,
                               "identificativo accordo finanziamento CE"@it ;
                    owl:versionInfo "stabile"@it ,
                                    "stable"@en .


###  https://w3id.org/italia/onto/HER/ecMaxContribution
:ecMaxContribution rdf:type owl:DatatypeProperty ;
                   rdfs:subPropertyOf <https://w3id.org/italia/onto/MU/value> ;
                   rdfs:domain [ rdf:type owl:Class ;
                                 owl:unionOf ( :ECProject
                                               :ERCProject
                                             )
                               ] ;
                   rdfs:comment "La parte di costo di un progetto CE finanziata dall'Unione Europea. L'importo è espresso in euro."@it ,
                                "The part of an EC project's cost that is funded by European Union. The amount is expressed in euros."@en ;
                   rdfs:isDefinedBy <https://w3id.org/italia/onto/HER> ;
                   rdfs:label "EC maximum contribution"@en ,
                              "massimo contributo CE"@it .


###  https://w3id.org/italia/onto/HER/ecObjective
:ecObjective rdf:type owl:DatatypeProperty ;
             rdfs:subPropertyOf l0:description ;
             rdfs:domain [ rdf:type owl:Class ;
                           owl:unionOf ( :ECProject
                                         :ERCProject
                                       )
                         ] ;
             rdfs:range rdfs:Literal ;
             rdfs:comment "Main objective(s) of the project. This serves as the project's abstract."@en ,
                          "Obiettivo(i) principale(i) del progetto. Questo serve come astratto del progetto."@it ;
             rdfs:isDefinedBy <https://w3id.org/italia/onto/HER> ;
             rdfs:label "ec objective"@en ,
                        "obiettivo CE"@it ;
             owl:versionInfo "provvisoria"@it ,
                             "unstable"@en .


###  https://w3id.org/italia/onto/HER/editionLabel
:editionLabel rdf:type owl:DatatypeProperty .


###  https://w3id.org/italia/onto/HER/endingYear
:endingYear rdf:type owl:DatatypeProperty ;
            rdfs:subPropertyOf ti:year ;
            rdfs:domain [ rdf:type owl:Class ;
                          owl:unionOf ( :CHAFEAProject
                                        :ECProject
                                        :ERCProject
                                        :EUREKAProject
                                        :ErasmusPlusProject
                                      )
                        ] ;
            rdfs:range xsd:gYear ;
            rdfs:comment "Ending year of the project"@en ,
                         "Indica l'anno di fine di un progetto"@it ;
            rdfs:isDefinedBy <https://w3id.org/italia/onto/HER> ;
            rdfs:label "anno di fine"@it ,
                       "ending year"@en .


###  https://w3id.org/italia/onto/HER/enrollmentType
:enrollmentType rdf:type owl:DatatypeProperty ;
                rdfs:domain :AACTStudy ;
                rdfs:range rdfs:Literal ;
                rdfs:comment "Il numero totale di partecipanti da iscrivere. Essi sono: la stima (numero target) o il numero totale effettivo di partecipanti che vengono arruolati nello studio clinico."@it ,
                             "The total number of participants to be enrolled. They are either: estimated (target number) or the actual total number of participants that are enrolled in the clinical study."@en ;
                rdfs:isDefinedBy <https://w3id.org/italia/onto/HER> ;
                rdfs:label "enrollment type"@en ,
                           "tipo di iscrizione"@it ;
                owl:versionInfo "provvisoria"@it ,
                                "unstable"@en .


###  https://w3id.org/italia/onto/HER/erasmusplusOrgType
:erasmusplusOrgType rdf:type owl:DatatypeProperty ;
                    rdfs:domain :ErasmusPlusParticipant ;
                    rdfs:range rdfs:Literal ;
                    rdfs:comment "Quando disponibile, si riferisce al tipo di organizzazione che partecipa al progetto Erasmus+."@it ,
                                 "When available, it refers to the type of the organization participating in the Erasmus+ project."@en ;
                    rdfs:isDefinedBy <https://w3id.org/italia/onto/HER> ;
                    rdfs:label "erasmus+ organization type"@en ,
                               "tipologia di organizzazione erasmus+"@it ;
                    owl:versionInfo "provvisoria"@it ,
                                    "unstable"@en .


###  https://w3id.org/italia/onto/HER/eurekaOrgType
:eurekaOrgType rdf:type owl:DatatypeProperty ;
               rdfs:domain :EUREKAParticipant ;
               rdfs:range rdfs:Literal ;
               rdfs:comment "Tipologia di organizzazione (Istituto di Ricerca, grande impresa, universitá, SME, R&D SME, altro)"@it ,
                            "Type of organization (Research institute, Large company, University, SME, R&D SME, Other)"@en ;
               rdfs:isDefinedBy <https://w3id.org/italia/onto/HER> ;
               rdfs:label "eureka's organization type"@en ,
                          "tipologia di organizzazione eureka"@it .


###  https://w3id.org/italia/onto/HER/eurekaProjectId
:eurekaProjectId rdf:type owl:DatatypeProperty ;
                 rdfs:subPropertyOf l0:identifier ;
                 rdfs:domain :EUREKAProject ;
                 rdfs:range rdfs:Literal ;
                 rdfs:comment "Codice univoco progetto EUREKA"@it ,
                              "EUREKA project unique identifier"@en ;
                 rdfs:isDefinedBy <https://w3id.org/italia/onto/HER> ;
                 rdfs:label "EUREKA project ID"@en ,
                            "ID del progetto EUREKA"@it ;
                 owl:versionInfo "provvisoria"@it ,
                                 "unstable"@en .


###  https://w3id.org/italia/onto/HER/expandedAccess
:expandedAccess rdf:type owl:DatatypeProperty ;
                rdfs:domain :AACTStudy ;
                rdfs:comment "Study has Expanded Access (A way for patients with serious diseases or conditions who cannot participate in a clinical trial to gain access to a medical product that has not been approved by the U.S. Food and Drug Administration (FDA). Also called compassionate use.)"@en ,
                             "Un modo per i pazienti con malattie o condizioni gravi che non possono partecipare a uno studio clinico di accedere a un prodotto medico che non è stato approvato dalla Food and Drug Administration (FDA) degli Stati Uniti. Chiamato anche uso compassionevole)."@it ;
                rdfs:isDefinedBy <https://w3id.org/italia/onto/HER> ;
                rdfs:label "accesso esteso"@it ,
                           "expanded access"@en .


###  https://w3id.org/italia/onto/HER/expandedAccessTypeIndividual
:expandedAccessTypeIndividual rdf:type owl:DatatypeProperty ;
                              rdfs:domain :AACTStudy ;
                              rdfs:comment "A way for patients with serious diseases or conditions who cannot participate in a clinical trial to gain access to a medical product that has not been approved by the U.S. Food and Drug Administration (FDA). Also called compassionate use. Individual Patients: Allows a single patient, with a serious disease or condition who cannot participate in a clinical trial, access to a drug or biological product that has not been approved by the FDA. This category also includes access in an emergency situation."@en ,
                                           "Un modo per i pazienti con malattie o condizioni gravi che non possono partecipare a uno studio clinico per avere accesso a un prodotto medico che non è stato approvato dalla Food and Drug Administration (FDA) degli Stati Uniti. Chiamato anche uso compassionevole. Pazienti individuali: Permette ad un singolo paziente, con una malattia o condizione grave che non può partecipare ad una sperimentazione clinica, di accedere ad un farmaco o ad un prodotto biologico che non è stato approvato dalla FDA. Questa categoria comprende anche l'accesso in una situazione di emergenza."@it ;
                              rdfs:isDefinedBy <https://w3id.org/italia/onto/HER> ;
                              rdfs:label "expanded access type individual"@en ,
                                         "tipo di accesso esteso individuale"@it .


###  https://w3id.org/italia/onto/HER/expandedAccessTypeIntermediate
:expandedAccessTypeIntermediate rdf:type owl:DatatypeProperty ;
                                rdfs:domain :AACTStudy ;
                                rdfs:comment "A way for patients with serious diseases or conditions who cannot participate in a clinical trial to gain access to a medical product that has not been approved by the U.S. Food and Drug Administration (FDA). Also called compassionate use. Intermediate-size Population: Allows more than one patient (but generally fewer patients than through a Treatment IND/Protocol) access to a drug or biological product that has not been approved by the FDA. This type of expanded access is used when multiple patients with the same disease or condition seek access to a specific drug or biological product that has not been approved by the FDA."@en ,
                                             "Un modo per i pazienti con malattie o condizioni gravi che non possono partecipare a uno studio clinico per avere accesso a un prodotto medico che non è stato approvato dalla Food and Drug Administration (FDA) degli Stati Uniti. Chiamato anche uso compassionevole. Popolazione di dimensioni intermedie: Permette a più di un paziente (ma generalmente meno pazienti rispetto a quelli che hanno accesso a un trattamento IND/Protocollo) di accedere a un farmaco o prodotto biologico che non è stato approvato dalla FDA. Questo tipo di accesso allargato viene utilizzato quando più pazienti con la stessa malattia o condizione cercano di accedere a un farmaco o prodotto biologico specifico che non è stato approvato dalla FDA."@it ;
                                rdfs:isDefinedBy <https://w3id.org/italia/onto/HER> ;
                                rdfs:label "expanded access type intermediate"@en ,
                                           "tipo di accesso esteso intermedio"@it .


###  https://w3id.org/italia/onto/HER/expandedAccessTypeTreatment
:expandedAccessTypeTreatment rdf:type owl:DatatypeProperty ;
                             rdfs:domain :AACTStudy ;
                             rdfs:comment "A way for patients with serious diseases or conditions who cannot participate in a clinical trial to gain access to a medical product that has not been approved by the U.S. Food and Drug Administration (FDA). Also called compassionate use. Treatment IND/Protocol: Allows a large, widespread population access to a drug or biological product that has not been approved by the FDA. This type of expanded access can only be provided if the product is already being developed for marketing for the same use as the expanded access use."@en ,
                                          "Un modo per i pazienti con malattie o condizioni gravi che non possono partecipare a uno studio clinico per avere accesso a un prodotto medico che non è stato approvato dalla Food and Drug Administration (FDA) degli Stati Uniti. Chiamato anche uso compassionevole. Trattamento IND/Protocollo: Permette a una vasta e diffusa popolazione di accedere a un farmaco o prodotto biologico che non è stato approvato dalla FDA. Questo tipo di accesso esteso può essere fornito solo se il prodotto è già in fase di sviluppo per la commercializzazione per lo stesso uso dell'accesso esteso."@it ;
                             rdfs:isDefinedBy <https://w3id.org/italia/onto/HER> ;
                             rdfs:label "expanded access type treatment"@en ,
                                        "trattamento del tipo di accesso esteso"@it .


###  https://w3id.org/italia/onto/HER/expenseType
:expenseType rdf:type owl:DatatypeProperty ;
             rdfs:domain :CTNPRINAmount ;
             rdfs:range rdfs:Literal ;
             rdfs:comment "Tipologia di spesa tra quelle previste dall'iniziativa (bando, avviso, …): - Personale - Strumentazione - Fabbricati - …."@it ,
                          "Type of expenditure among those foreseen by the initiative (call for proposals, notice, ...): - Personnel - Instrumentation - Buildings - ...."@en ;
             rdfs:isDefinedBy <https://w3id.org/italia/onto/HER> ;
             rdfs:label "expense type"@en ,
                        "tipo di spese"@it ;
             owl:versionInfo "provvisoria"@it ,
                             "unstable"@en .


###  https://w3id.org/italia/onto/HER/expireDate
:expireDate rdf:type owl:DatatypeProperty ;
            rdfs:subPropertyOf ti:date ;
            rdfs:domain :CTNPRINInitiative ;
            rdfs:range xsd:date ;
            rdfs:comment "Final deadline for submission of project proposals for CTN/PRIN initiative"@en ,
                         "Ultima data di scadenza utile per la presentazione di proposte di progetto per l'iniziativa di tipo CTN/PRIN in esame"@it ;
            rdfs:isDefinedBy <https://w3id.org/italia/onto/HER> ;
            rdfs:label "data scadenza"@it ,
                       "expiration date"@en ;
            owl:versionInfo "stabile"@it ,
                            "stable"@en .


###  https://w3id.org/italia/onto/HER/finalBalance
:finalBalance rdf:type owl:DatatypeProperty ;
              rdfs:subPropertyOf <https://w3id.org/italia/onto/MU/value> ;
              rdfs:domain :USTATContributionRevenue ;
              rdfs:range rdfs:Literal ;
              rdfs:comment "Amount of the final balance. The values are expressed in EURO. The final balance refers to the year (T-1)."@en ,
                           "Importo del conto consuntivo. I valori sono espressi in EURO. Il conto consuntivo fa riferimento all'anno (T-1)."@it ;
              rdfs:isDefinedBy <https://w3id.org/italia/onto/HER> ;
              rdfs:label "bilancio finale"@it ,
                         "final balance"@en .


###  https://w3id.org/italia/onto/HER/foundationProject
:foundationProject rdf:type owl:DatatypeProperty ;
                   rdfs:domain :Spinoff ;
                   rdfs:range rdfs:Literal ;
                   rdfs:comment "Fornisce una descrizione del progetto alla base della fondazione dello spin-off."@it ,
                                "It provides a description of the project behind the foundation of the spin-off."@en ;
                   rdfs:isDefinedBy <https://w3id.org/italia/onto/HER> ;
                   rdfs:label "foundation project"@en ,
                              "progetto di fondazione"@it ;
                   owl:versionInfo "provvisoria"@it ,
                                   "unstable"@en .


###  https://w3id.org/italia/onto/HER/founderCapital
:founderCapital rdf:type owl:DatatypeProperty ;
                rdfs:domain :Spinoff ;
                rdfs:range rdfs:Literal ;
                rdfs:comment "Indica il capitale dello spin-off al momento della sua fondazione."@it ,
                             "It indicates the capital of the spin-off at the time of its foundation."@en ;
                rdfs:isDefinedBy <https://w3id.org/italia/onto/HER> ;
                rdfs:label "capitale fondatore"@it ,
                           "founder capital"@en ;
                owl:versionInfo "provvisoria"@it ,
                                "unstable"@en .


###  https://w3id.org/italia/onto/HER/founderFaculty
:founderFaculty rdf:type owl:DatatypeProperty ;
                rdfs:domain :Spinoff ;
                rdfs:comment "It is used to link the spin-off to the faculty of the university of origin, or to a division of the research institution of origin."@en ,
                             "Viene utilizzato per collegare lo spin-off alla facoltà dell'ateneo di origine, o a una divisione dell'ente di ricerca di origine."@it ;
                rdfs:isDefinedBy <https://w3id.org/italia/onto/HER> ;
                rdfs:label "facoltá fondatrice"@it ,
                           "founder faculty"@en .


###  https://w3id.org/italia/onto/HER/founderPatent
:founderPatent rdf:type owl:DatatypeProperty ;
               rdfs:domain :Spinoff ;
               rdfs:comment "Indica se sono presenti dei brevetti collegati allo spin-off."@it ,
                            "It indicates if there are any patents related to the spin-off."@en ;
               rdfs:isDefinedBy <https://w3id.org/italia/onto/HER> ;
               rdfs:label "brevetto fondatore"@it ,
                          "founder patent"@en ;
               owl:versionInfo "provvisoria"@it ,
                               "unstable"@en .


###  https://w3id.org/italia/onto/HER/founderShareholding
:founderShareholding rdf:type owl:DatatypeProperty ;
                     rdfs:domain :Spinoff ;
                     rdfs:comment "Indica la participazione azionaria dell'Università o dell'ente di ricerca di origine al momento della fondazione dello spin-off."@it ,
                                  "It indicates the shareholding of the university or research institution of origin at the time of the foundation of the spin-off."@en ;
                     rdfs:isDefinedBy <https://w3id.org/italia/onto/HER> ;
                     rdfs:label "founder shareholding"@en ,
                                "partecipazione azionaria fondatore"@it ;
                     owl:versionInfo "provvisoria"@it ,
                                     "unstable"@en .


###  https://w3id.org/italia/onto/HER/grant
:grant rdf:type owl:DatatypeProperty ;
       rdfs:domain :EUREKAParticipant ;
       rdfs:comment "Contributo per i partecipanti"@it ,
                    "Participant grant"@en ;
       rdfs:isDefinedBy <https://w3id.org/italia/onto/HER> ;
       rdfs:label "contributo"@it ,
                  "grant"@en ;
       owl:versionInfo "provvisoria"@it ,
                       "unstable"@en .


###  https://w3id.org/italia/onto/HER/grantAgreementNo
:grantAgreementNo rdf:type owl:DatatypeProperty ;
                  rdfs:subPropertyOf l0:identifier ;
                  rdfs:range rdfs:Literal ;
                  rdfs:comment "Grant agreement identifier of an EC project."@en ,
                               "Identificativo dell'accordo di sovvenzione di un progetto CE."@it ;
                  rdfs:isDefinedBy <https://w3id.org/italia/onto/HER> ;
                  rdfs:label "grant agreement number"@en ,
                             "numero dell'accordo di sovvenzione"@it ;
                  owl:versionInfo "provvisoria"@it ,
                                  "unstable"@en .


###  https://w3id.org/italia/onto/HER/grantedCredit
:grantedCredit rdf:type owl:DatatypeProperty ;
               rdfs:domain [ rdf:type owl:Class ;
                             owl:unionOf ( :CTNPRINInitiative
                                           :CTNPRINOperation
                                         )
                           ] ;
               rdfs:isDefinedBy <https://w3id.org/italia/onto/HER> ;
               rdfs:label "credito concesso"@it ,
                          "granted credit"@en ;
               owl:versionInfo "provvisoria"@it ,
                               "unstable"@en .


###  https://w3id.org/italia/onto/HER/healthyVolunteers
:healthyVolunteers rdf:type owl:DatatypeProperty ;
                   rdfs:domain :AACTEligibility ;
                   rdfs:comment "I partecipanti che non hanno una malattia o una condizione, o condizioni o sintomi correlati"@it ,
                                "Participants do not have a disease or condition, or related conditions or symptoms"@en ;
                   rdfs:isDefinedBy <https://w3id.org/italia/onto/HER> ;
                   rdfs:label "Volontari sani"@it ,
                              "healthy volunteers"@en ;
                   owl:versionInfo "provvisoria"@it ,
                                   "unstable"@it .


###  https://w3id.org/italia/onto/HER/initiativeType
:initiativeType rdf:type owl:DatatypeProperty ;
                rdfs:domain :CTNPRINInitiative ;
                rdfs:range rdfs:Literal ;
                rdfs:comment "Tipologia dell'iniziativa. La Tipologia di una iniziativa può essere: - Ricerca di base - Ricerca industriale - Diffusione Cultura Scientifica - Antartide - Altro"@it ,
                             "Type of initiative. The typology of an initiative can be: - Basic research - Industrial research - Dissemination of Scientific culture - Antarctica - Other"@en ;
                rdfs:isDefinedBy <https://w3id.org/italia/onto/HER> ;
                rdfs:label "initiative type"@en ,
                           "tipi di iniziative"@it ;
                owl:versionInfo "provvisoria"@it ,
                                "unstable"@en .


###  https://w3id.org/italia/onto/HER/innovative
:innovative rdf:type owl:DatatypeProperty ,
                     owl:FunctionalProperty ;
            rdfs:domain :Spinoff ;
            rdfs:range xsd:boolean ;
            rdfs:comment "Indica se lo spin-off ha anche la qualifica di start-up innovativa ai sensi della L. 221/2012."@it ,
                         "It indicates whether the spin-off also qualifies as an innovative start-up under Law 221/2012."@en ;
            rdfs:isDefinedBy <https://w3id.org/italia/onto/HER> ;
            rdfs:label "innovativa"@it ,
                       "innovative"@en ;
            owl:versionInfo "stabile"@it ,
                            "stable"@en .


###  https://w3id.org/italia/onto/HER/interventionModel
:interventionModel rdf:type owl:DatatypeProperty ;
                   rdfs:domain :AACTDesign ;
                   rdfs:range rdfs:Literal ;
                   rdfs:comment """Il disegno generale della strategia per l'assegnazione degli interventi ai partecipanti ad uno studio clinico. I tipi di modelli di intervento includono:
Gruppo singolo: Studi clinici in una sola branca
Parallelo: I partecipanti sono assegnati a uno dei due o più gruppi in parallelo per tutta la durata dello studio
Crossover: I partecipanti ricevono uno dei due (o più) interventi alternativi durante la fase iniziale dello studio e ricevono l'altro intervento durante la seconda fase dello studio
Fattoriale: Due o più interventi, ciascuno da solo e in combinazione, sono valutati in parallelo rispetto ad un gruppo di controllo
Sequenziale: I gruppi di partecipanti sono assegnati a ricevere gli interventi in base alle tappe precedenti che vengono raggiunte nello studio, come ad esempio in alcuni studi di escalation di dose e di progettazione adattiva


"""@it ,
                                """The general design of the strategy for assigning interventions to participants in a clinical study. Types of intervention models include:
Single Group: Clinical trials with a single arm
Parallel: Participants are assigned to one of two or more groups in parallel for the duration of the study
Crossover: Participants receive one of two (or more) alternative interventions during the initial phase of the study and receive the other intervention during the second phase of the study
Factorial: Two or more interventions, each alone and in combination, are evaluated in parallel against a control group
Sequential: Groups of participants are assigned to receive interventions based on prior milestones being reached in the study, such as in some dose escalation and adaptive design studies
"""@en ;
                   rdfs:isDefinedBy <https://w3id.org/italia/onto/HER> ;
                   rdfs:label "Modello di Intervento"@it ,
                              "intervention model"@en ;
                   owl:versionInfo "provvisoria"@it ,
                                   "unstable"@en .


###  https://w3id.org/italia/onto/HER/interventionModelDescription
:interventionModelDescription rdf:type owl:DatatypeProperty ;
                              rdfs:subPropertyOf l0:description ;
                              rdfs:domain :AACTDesign ;
                              rdfs:range rdfs:Literal ;
                              rdfs:comment "Fornisce dettagli sul modello di studio utilizzato."@it ,
                                           "Provide details about the Interventional Study Model."@en ;
                              rdfs:isDefinedBy <https://w3id.org/italia/onto/HER> ;
                              rdfs:label "Descrizione modello intervento"@it ,
                                         "intervention model description"@en ;
                              owl:versionInfo "provvisoria"@it ,
                                              "unstable"@en .


###  https://w3id.org/italia/onto/HER/investigatorMasked
:investigatorMasked rdf:type owl:DatatypeProperty ,
                             owl:FunctionalProperty ;
                    rdfs:domain :AACTDesign ;
                    rdfs:range xsd:boolean ;
                    rdfs:comment "Gli sperimentatori sono le parti coinvolte nello studio clinico che non possono conoscere gli interventi assegnati ai singoli partecipanti."@it ,
                                 "Investigator is the party or parties involved in the clinical trial who are prevented from having knowledge of the interventions assigned to individual participants."@en ;
                    rdfs:isDefinedBy <https://w3id.org/italia/onto/HER> ;
                    rdfs:label "gli esaminatori coinvolti hanno conoscenza degli interventi?"@it ,
                               "investigator masked"@en ;
                    owl:versionInfo "provvisoria"@it ,
                                    "unstable"@en .


###  https://w3id.org/italia/onto/HER/investment
:investment rdf:type owl:DatatypeProperty ;
            rdfs:domain :EUREKAParticipant ;
            rdfs:comment "Investimento dei partecipanti"@it ,
                         "Participant investment"@en ;
            rdfs:isDefinedBy <https://w3id.org/italia/onto/HER> ;
            rdfs:label "investimento"@it ,
                       "investment"@en ;
            owl:versionInfo "provvisoria"@it ,
                            "unstable"@en .


###  https://w3id.org/italia/onto/HER/ipdAccessCriterion
:ipdAccessCriterion rdf:type owl:DatatypeProperty ;
                    rdfs:domain :AACTStudy ;
                    rdfs:range rdfs:Literal ;
                    rdfs:comment "Describe by what access criteria IPD and any additional supporting information will be shared, including with whom, for what types of analyses, and by what mechanism. Information about who will review requests and criteria for reviewing requests may also be provided."@en ,
                                 "Descrivere in base a quali criteri di accesso IPD ed eventuali informazioni di supporto aggiuntive saranno condivise, anche con chi, per quali tipi di analisi e con quale meccanismo. Possono essere fornite anche informazioni su chi esaminerà le richieste e sui criteri di revisione delle richieste."@it ;
                    rdfs:isDefinedBy <https://w3id.org/italia/onto/HER> ;
                    rdfs:label "IPD access criterion"@en ,
                               "criterio accesso IPD"@it ;
                    owl:versionInfo "provvisoria"@it ,
                                    "unstable"@en .


###  https://w3id.org/italia/onto/HER/ipdTimeFrame
:ipdTimeFrame rdf:type owl:DatatypeProperty ;
              rdfs:domain :AACTStudy ;
              rdfs:range rdfs:Literal ;
              rdfs:comment "A description of when the IPD and any additional supporting information will become available and for how long, including the start and end dates or period of availability. This may be provided as an absolute date (for example, starting in January 2025) or as a date relative to the time when summary data are published or otherwise made available (for example, starting 6 months after publication)."@en ,
                           "Una descrizione di quando il DPI ed eventuali informazioni aggiuntive di supporto saranno disponibili e per quanto tempo, incluse le date di inizio e fine o il periodo di disponibilità. Questa può essere fornita come data assoluta (ad esempio, a partire da gennaio 2025) o come data relativa al momento in cui i dati sintetici sono pubblicati o resi disponibili in altro modo (ad esempio, a partire da 6 mesi dopo la pubblicazione)."@it ;
              rdfs:isDefinedBy <https://w3id.org/italia/onto/HER> ;
              rdfs:label "IPD time frame"@en ,
                         "Intervallo di tempo IPD"@it ;
              owl:versionInfo "provvisoria"@it ,
                              "unstable"@en .


###  https://w3id.org/italia/onto/HER/ipdURL
:ipdURL rdf:type owl:DatatypeProperty ;
        rdfs:subPropertyOf <https://w3id.org/italia/onto/SM/URL> ;
        rdfs:domain :AACTStudy ;
        rdfs:range xsd:anyURI ;
        rdfs:comment "L'indirizzo web, se presente, utilizzato per trovare ulteriori informazioni sul piano di condivisione di IPD."@it ,
                     "The web address, if any, used to find additional information about the plan to share IPD."@en ;
        rdfs:isDefinedBy <https://w3id.org/italia/onto/HER> ;
        rdfs:label "IPD URL"@en ,
                   "IPD URL"@it ;
        owl:versionInfo "stabile"@it ,
                        "stable"@en .


###  https://w3id.org/italia/onto/HER/isFDARegulatedDevice
:isFDARegulatedDevice rdf:type owl:DatatypeProperty ,
                               owl:FunctionalProperty ;
                      rdfs:domain :AACTStudy ;
                      rdfs:range xsd:boolean ;
                      rdfs:comment "Indication that a clinical study is studying a device product subject to section 510(k), 515, or 520(m) of the Federal Food, Drug, and Cosmetic Act. Select Yes/No."@en ,
                                   "Indicazione che uno studio clinico sta studiando un prodotto per dispositivi soggetti alla sezione 510(k), 515, o 520(m) del Federal Food, Drug, and Cosmetic Act. Selezionare Sì/No."@it ;
                      rdfs:isDefinedBy <https://w3id.org/italia/onto/HER> ;
                      rdfs:label "is FDA regulated device"@en ,
                                 "è dispositivo regolamentato da FDA"@it ;
                      owl:versionInfo "stabile"@it ,
                                      "stable"@en .


###  https://w3id.org/italia/onto/HER/isFDARegulatedDrug
:isFDARegulatedDrug rdf:type owl:DatatypeProperty ;
                    rdfs:domain :AACTStudy ;
                    rdfs:comment "Indication that a clinical study is studying a drug product (including a biological product) subject to section 505 of the Federal Food, Drug, and Cosmetic Act or to section 351 of the Public Health Service Act. Select Yes/No."@en ,
                                 "Indicazione che uno studio clinico sta studiando un prodotto farmaceutico (incluso un prodotto biologico) soggetto alla sezione 505 del Federal Food, Drug, and Cosmetic Act o alla sezione 351 del Public Health Service Act. Selezionare Sì/No."@it ;
                    rdfs:isDefinedBy <https://w3id.org/italia/onto/HER> ;
                    rdfs:label "is FDA regulated drug?"@en ,
                               "è un farmaco regolamentato dalla FDA?"@it .


###  https://w3id.org/italia/onto/HER/isPPSD
:isPPSD rdf:type owl:DatatypeProperty ;
        rdfs:domain :AACTStudy ;
        rdfs:comment "Indication that a clinical study that includes a U.S. FDA-regulated device product is a pediatric postmarket surveillance of a device (PPSD) product ordered under section 522 of the Federal Food, Drug, and Cosmetic Act. Select Yes/No."@en ,
                     "Indicazione che uno studio clinico che include un prodotto per dispositivi regolamentato dalla FDA statunitense è una sorveglianza pediatrica post-vendita di un prodotto per dispositivi (PPSD) ordinato ai sensi della sezione 522 del Federal Food, Drug, and Cosmetic Act. Selezionare Sì/No."@it ;
        rdfs:isDefinedBy <https://w3id.org/italia/onto/HER> ;
        rdfs:label "is PPSD?"@en ,
                   "è PPSD?"@it .


###  https://w3id.org/italia/onto/HER/isUSExport
:isUSExport rdf:type owl:DatatypeProperty ;
            rdfs:domain :AACTStudy ;
            rdfs:comment "Se qualsiasi prodotto farmaceutico (incluso un prodotto biologico) o dispositivo studiato nello studio clinico viene fabbricato negli Stati Uniti o in uno dei suoi territori ed esportato per essere studiato in uno studio clinico in un altro paese. Richiesto se il farmaco regolamentato dalla FDA statunitense e/o il dispositivo regolamentato dalla FDA statunitense è \"Sì\", l'IND o l'IDE della FDA statunitense è \"No\", e le informazioni sulla struttura non includono almeno una sede negli Stati Uniti."@it ,
                         "Whether any drug product (including a biological product) or device product studied in the clinical study is manufactured in the United States or one of its territories and exported for study in a clinical study in another country. Required if U.S. FDA-regulated Drug and/or U.S. FDA-regulated Device is \"Yes,\" U.S. FDA IND or IDE is \"No\", and Facility Information does not include at least one U.S. location."@en ;
            rdfs:isDefinedBy <https://w3id.org/italia/onto/HER> ;
            rdfs:label "is US export?"@en ,
                       "è esportato dagli US?"@it .


###  https://w3id.org/italia/onto/HER/isUnapprovedDevice
:isUnapprovedDevice rdf:type owl:DatatypeProperty ;
                    rdfs:domain :AACTStudy ;
                    rdfs:comment "Indication that at least one device product studied in the clinical study has not been previously approved or cleared by the U.S. Food and Drug Administration (FDA) for one or more uses."@en ,
                                 "Indicazione che almeno un prodotto del dispositivo studiato nello studio clinico non è stato precedentemente approvato o approvato dalla Food and Drug Administration (FDA) degli Stati Uniti per uno o più usi."@it ;
                    rdfs:isDefinedBy <https://w3id.org/italia/onto/HER> ;
                    rdfs:label "is unapproved device?"@en ,
                               "è un dispositivo non regolamentato?"@it .


###  https://w3id.org/italia/onto/HER/lastKnownStatus
:lastKnownStatus rdf:type owl:DatatypeProperty ;
                 rdfs:domain :AACTStudy ;
                 rdfs:comment """Last registered study enrollment status. Enrollment status are: Not yet recruiting: The study has not started recruiting participants.
Recruiting: The study is currently recruiting participants.
Enrolling by invitation: The study is selecting its participants from a population, or group of people, decided on by the researchers in advance. These studies are not open to everyone who meets the eligibility criteria but only to people in that particular population, who are specifically invited to participate.
Active, not recruiting: The study is ongoing, and participants are receiving an intervention or being examined, but potential participants are not currently being recruited or enrolled.
Suspended: The study has stopped early but may start again.
Terminated: The study has stopped early and will not start again. Participants are no longer being examined or treated.
Completed: The study has ended normally, and participants are no longer being examined or treated (that is, the last participant's last visit has occurred).
Withdrawn: The study stopped early, before enrolling its first participant.
Unknown: A study on ClinicalTrials.gov whose last known status was recruiting; not yet recruiting; or active, not recruiting but that has passed its completion date, and the status has not been last verified within the past 2 years."""@en ,
                              """Ultimo stato di iscrizione allo studio registrato. Gli stati di iscrizione sono: Non ancora in fase di reclutamento: Lo studio non ha iniziato a reclutare partecipanti.
Reclutamento: Lo studio sta attualmente reclutando i partecipanti.
Iscrizione su invito: Lo studio sta selezionando i partecipanti da una popolazione, o gruppo di persone, decisa in anticipo dai ricercatori. Questi studi non sono aperti a tutti coloro che soddisfano i criteri di ammissibilità, ma solo alle persone di quella particolare popolazione, che sono specificamente invitate a partecipare.
Attivi, non reclutatori: Lo studio è in corso e i partecipanti ricevono un intervento o vengono esaminati, ma i potenziali partecipanti non sono attualmente reclutati o iscritti.
Sospeso: Lo studio è stato interrotto in anticipo ma potrebbe ricominciare.
Terminato: Lo studio si è interrotto anticipatamente e non inizierà di nuovo. I partecipanti non vengono più esaminati o trattati.
Completato: Lo studio è terminato normalmente e i partecipanti non vengono più esaminati o trattati (cioè si è verificata l'ultima visita dell'ultimo partecipante).
Ritirato: Lo studio si è interrotto anticipatamente, prima di iscrivere il primo partecipante.
Sconosciuto: Uno studio su ClinicalTrials.gov il cui ultimo stato conosciuto è stato il reclutamento; non ancora reclutamento; o attivo, non reclutamento ma che ha superato la data di completamento, e lo stato non è stato verificato per l'ultima volta negli ultimi 2 anni."""@it ;
                 rdfs:isDefinedBy <https://w3id.org/italia/onto/HER> ;
                 rdfs:label "Ultimo stato conosciuto"@it ,
                            "last known status"@en .


###  https://w3id.org/italia/onto/HER/lastUpdatePostedDate
:lastUpdatePostedDate rdf:type owl:DatatypeProperty ;
                      rdfs:subPropertyOf ti:modified ;
                      rdfs:domain :AACTStudy ;
                      rdfs:comment "La data più recente in cui sono state rese disponibili su ClinicalTrials.gov. Ci può essere un ritardo tra la data in cui le modifiche sono state inviate a ClinicalTrials.gov dallo sponsor o dallo sperimentatore dello studio (la data dell'ultimo aggiornamento inviato) e la data dell'ultimo aggiornamento pubblicato."@it ,
                                   "The most recent date on which changes to a study record were made available on ClinicalTrials.gov. There may be a delay between when the changes were submitted to ClinicalTrials.gov by the study's sponsor or investigator (the last update submitted date) and the last update posted date."@en ;
                      rdfs:isDefinedBy <https://w3id.org/italia/onto/HER> ;
                      rdfs:label "data dell'ultimo aggiornamento pubblicato"@it ,
                                 "last update posted date"@en .


###  https://w3id.org/italia/onto/HER/lastUpdatePostedDateType
:lastUpdatePostedDateType rdf:type owl:DatatypeProperty ;
                          rdfs:domain :AACTStudy ;
                          rdfs:comment "All posted dates include a type attribute of Actual or Estimate."@en ,
                                       "Tutte le date pubblicate includono un attributo di tipo Actual o Estimate."@it ;
                          rdfs:isDefinedBy <https://w3id.org/italia/onto/HER> ;
                          rdfs:label "last update posted date type"@en ,
                                     "tipo di data dell'ultimo aggiornamento pubblicato"@it .


###  https://w3id.org/italia/onto/HER/lastUpdateSubmittedDate
:lastUpdateSubmittedDate rdf:type owl:DatatypeProperty ;
                         rdfs:subPropertyOf ti:modified ;
                         rdfs:domain :AACTStudy ;
                         rdfs:comment "La data più recente in cui lo sponsor dello studio o lo sperimentatore ha presentato a ClinicalTrials.gov le modifiche al dossier dello studio. In genere c'è un ritardo di alcuni giorni tra la data dell'ultimo aggiornamento presentato e la data in cui le modifiche vengono pubblicate su ClinicalTrials.gov (la data dell'ultimo aggiornamento pubblicato)."@it ,
                                      "The most recent date on which the study sponsor or investigator submitted changes to a study record to ClinicalTrials.gov. There is typically a delay of a few days between the last update submitted date and when the date changes are posted on ClinicalTrials.gov (the last update posted date)."@en ;
                         rdfs:isDefinedBy <https://w3id.org/italia/onto/HER> ;
                         rdfs:label "data dell'ultimo aggiornamento presentato"@it ,
                                    "last update submitted date"@en .


###  https://w3id.org/italia/onto/HER/lastUpdateSubmittedQCDate
:lastUpdateSubmittedQCDate rdf:type owl:DatatypeProperty ;
                           rdfs:subPropertyOf ti:modified ;
                           rdfs:domain :AACTStudy ;
                           rdfs:comment "La data più recente in cui lo sponsor dello studio o lo sperimentatore ha presentato modifiche al registro dello studio che sono coerenti con i criteri di revisione del controllo di qualità (QC) della National Library of Medicine (NLM). È responsabilità dello sponsor o dello sperimentatore assicurarsi che la documentazione dello studio sia coerente con i criteri di revisione del controllo di qualità della NLM."@it ,
                                        "The most recent date on which the study sponsor or investigator submitted changes to a study record that are consistent with National Library of Medicine (NLM) quality control (QC) review criteria. It is the responsibility of the sponsor or investigator to ensure that the study record is consistent with the NLM QC review criteria."@en ;
                           rdfs:isDefinedBy <https://w3id.org/italia/onto/HER> ;
                           rdfs:label "data dell'ultimo aggiornamento presentato QC"@it ,
                                      "last update submitted QC date"@en .


###  https://w3id.org/italia/onto/HER/leadOrCollaborator
:leadOrCollaborator rdf:type owl:DatatypeProperty ;
                    rdfs:domain :AACTSponsor ;
                    rdfs:comment "If entity is considered to lead the trial or is a Collaborator (ie, other organizationsoproviding support; support may include funding, design, implementation, data analysis or reporting. The responsible party is responsible for confirming all collaborators)."@en ,
                                 "Se l'entità è considerata a capo della sperimentazione o è un Collaboratore (cioè un'altra organizzazione che fornisce supporto; il supporto può includere il finanziamento, la progettazione, l'implementazione, l'analisi dei dati o il reporting. Il responsabile è responsabile della conferma di tutti i collaboratori)."@it ;
                    rdfs:isDefinedBy <https://w3id.org/italia/onto/HER> ;
                    rdfs:label "capo o Collaboratore"@it ,
                               "lead or collaborator"@en .


###  https://w3id.org/italia/onto/HER/leaderName
:leaderName rdf:type owl:DatatypeProperty ;
            rdfs:subPropertyOf l0:name ;
            rdfs:domain :CHAFEAOutput ;
            rdfs:range rdfs:Literal ;
            rdfs:comment "Instrument leading Institution"@en ,
                         "Strumento che guida l'istituzione"@it ;
            rdfs:isDefinedBy <https://w3id.org/italia/onto/HER> ;
            rdfs:label "capo"@it ,
                       "leader"@en .


###  https://w3id.org/italia/onto/HER/limitationsAndCaveats
:limitationsAndCaveats rdf:type owl:DatatypeProperty ;
                       rdfs:domain :AACTStudy ;
                       rdfs:comment "Describe significant limitations of the study. Such limitations may include not reaching the target number of participants needed to achieve target power and statistically reliable results or technical problems with measurements leading to unreliable or uninterpretable data."@en ,
                                    "Descrive i limiti significativi dello studio. Tali limitazioni possono includere il mancato raggiungimento del numero di partecipanti necessario per raggiungere il potere target e risultati statisticamente affidabili o problemi tecnici con misurazioni che portano a dati inaffidabili o non interpretabili."@it ;
                       rdfs:isDefinedBy <https://w3id.org/italia/onto/HER> ;
                       rdfs:label "limitations and caveats"@en ,
                                  "limitazioni e avvertimenti"@it .


###  https://w3id.org/italia/onto/HER/masking
:masking rdf:type owl:DatatypeProperty ;
         rdfs:domain :AACTDesign ;
         rdfs:comment "Le parti coinvolte nello studio clinico che non possono conoscere gli interventi assegnati ai singoli partecipanti. I tipi di mascheramento comprendono: mascheramento aperto, mascheramento singolo cieco e mascheramento in doppio cieco."@it ,
                      "The party or parties involved in the clinical trial who are prevented from having knowledge of the interventions assigned to individual participants. Types of masking include: open label, single blind masking, and double-blind masking."@en ;
         rdfs:isDefinedBy <https://w3id.org/italia/onto/HER> ;
         rdfs:label "mascheramento"@it ,
                    "masking"@en .


###  https://w3id.org/italia/onto/HER/maskingDescription
:maskingDescription rdf:type owl:DatatypeProperty ;
                    rdfs:subPropertyOf l0:description ;
                    rdfs:domain :AACTDesign ;
                    rdfs:range rdfs:Literal ;
                    rdfs:comment "Fornisce informazioni su altri soggetti che potrebbero essere mascherati nello studio clinico, se presenti."@it ,
                                 "Provide information about other parties who may be masked in the clinical trial, if any."@en ;
                    rdfs:isDefinedBy <https://w3id.org/italia/onto/HER> ;
                    rdfs:label "description of masking"@en ,
                               "descrizione mascheramento"@it ;
                    owl:versionInfo "provvisoria"@it ,
                                    "unstable"@en .


###  https://w3id.org/italia/onto/HER/numberOfArms
:numberOfArms rdf:type owl:DatatypeProperty ;
              rdfs:domain :AACTStudy ;
              rdfs:range xsd:int ;
              rdfs:comment "number of pre-specified group or subgroup of participant(s) in a clinical trial assigned to receive specific intervention(s) (or no intervention) according to a protocol."@en ,
                           "numero di gruppi o sottogruppi predefiniti di partecipanti ad uno studio clinico assegnati a ricevere uno o più interventi specifici (o nessun intervento) secondo un protocollo."@it ;
              rdfs:isDefinedBy <https://w3id.org/italia/onto/HER> ;
              rdfs:label "number or arms"@en ,
                         "numero di bracci"@it .


###  https://w3id.org/italia/onto/HER/numberOfBeneficiaries
:numberOfBeneficiaries rdf:type owl:DatatypeProperty ;
                       rdfs:domain :CTNPRINInitiative ;
                       rdfs:range xsd:int ;
                       rdfs:comment "Numero totale di proponenti di proposte finanziate (beneficiari dei finanziamenti). NB: se un unico beneficiario è presente in più proposte finanziate viene contato tante volte quante sono le proposte in cui appare"@it ,
                                    "Total number of proposers of funded proposals (beneficiaries of funding). NB: if a single beneficiary is present in several funded proposals it is counted as many times as the number of proposals in which it appears"@en ;
                       rdfs:isDefinedBy <https://w3id.org/italia/onto/HER> ;
                       rdfs:label "number of beneficiaries"@en ,
                                  "numero di beneficiari"@it .


###  https://w3id.org/italia/onto/HER/numberOfEnrolledStudents
:numberOfEnrolledStudents rdf:type owl:DatatypeProperty ;
                          owl:equivalentProperty :totalEnrolledStudents ;
                          rdfs:domain [ rdf:type owl:Class ;
                                        owl:unionOf ( :MIURStudentsAggregate
                                                      :MIURStudentsByCitizenshipAggregate
                                                      :MIURStudentsByCitizenshipDegreeAggregate
                                                      :MIURStudentsByCitizenshipDegreeClassAggregate
                                                      :MIURStudentsByCitizenshipDegreeDegreeClassAggregate
                                                      :MIURStudentsByDegreeDegreeClassAggregate
                                                      :MIURStudentsByDiplomaAggregate
                                                      :MIURStudentsByDiplomaDegreeDegreeClassAggregate
                                                      :MIURStudentsByProvinceOfResidenceAggregate
                                                      :MIURStudentsByProvinceOfResidenceDegreeDegreeClassAggregate
                                                      :MIURStudentsByRegionOfResidenceAggregate
                                                      :MIURStudentsByRegionOfResidenceDegreeDegreeClassAggregate
                                                    )
                                      ] ;
                          rdfs:range xsd:int ;
                          rdfs:comment "Number of students enrolled in the Italian education system."@en ,
                                       "Numero di studenti iscritti al sistema educativo italiano."@it ;
                          rdfs:isDefinedBy <https://w3id.org/italia/onto/HER> ;
                          rdfs:label "number of enrolled students"@en ,
                                     "numero di studenti iscritti"@it .


###  https://w3id.org/italia/onto/HER/numberOfFinancedProposals
:numberOfFinancedProposals rdf:type owl:DatatypeProperty ;
                           rdfs:domain :CTNPRINInitiative ;
                           rdfs:range xsd:int ;
                           rdfs:comment "Numero totale delle proposte finanziate dall'iniziativa in esame"@it ,
                                        "Total number of proposals financed by the initiative under consideration"@en ;
                           rdfs:isDefinedBy <https://w3id.org/italia/onto/HER> ;
                           rdfs:label "number of financed proposals"@en ,
                                      "numero di proposte finanziate"@it .


###  https://w3id.org/italia/onto/HER/numberOfGraduatedStudents
:numberOfGraduatedStudents rdf:type owl:DatatypeProperty ;
                           owl:equivalentProperty :totalGraduatedStudents ;
                           rdfs:domain [ rdf:type owl:Class ;
                                         owl:unionOf ( :MIURStudentsAggregate
                                                       :MIURStudentsByCitizenshipAggregate
                                                       :MIURStudentsByCitizenshipDegreeAggregate
                                                       :MIURStudentsByCitizenshipDegreeClassAggregate
                                                       :MIURStudentsByCitizenshipDegreeDegreeClassAggregate
                                                       :MIURStudentsByDegreeDegreeClassAggregate
                                                       :MIURStudentsByDiplomaAggregate
                                                       :MIURStudentsByDiplomaDegreeDegreeClassAggregate
                                                       :MIURStudentsByProvinceOfResidenceAggregate
                                                       :MIURStudentsByProvinceOfResidenceDegreeDegreeClassAggregate
                                                       :MIURStudentsByRegionOfResidenceAggregate
                                                       :MIURStudentsByRegionOfResidenceDegreeDegreeClassAggregate
                                                     )
                                       ] ;
                           rdfs:range xsd:int ;
                           rdfs:comment "Number of students with a degree in the Italian education system."@en ,
                                        "Numero di studenti laureati nel sistema educativo italiano."@it ;
                           rdfs:isDefinedBy <https://w3id.org/italia/onto/HER> ;
                           rdfs:label "number of graduated students"@en ,
                                      "numero di studenti laureati"@it .


###  https://w3id.org/italia/onto/HER/numberOfGroups
:numberOfGroups rdf:type owl:DatatypeProperty ;
                rdfs:domain :AACTStudy ;
                rdfs:range xsd:int ;
                rdfs:comment "number of Group/cohorts (group or subgroup of participants in an observational study that is assessed for biomedical or health outcomes)."@en ,
                             "numero di gruppi/coorte (gruppo o sottogruppo di partecipanti ad uno studio osservazionale che viene valutato per i risultati biomedici o sanitari)."@it ;
                rdfs:isDefinedBy <https://w3id.org/italia/onto/HER> ;
                rdfs:label "number of groups"@en ,
                           "numero di gruppi"@it .


###  https://w3id.org/italia/onto/HER/numberOfProponents
:numberOfProponents rdf:type owl:DatatypeProperty ;
                    rdfs:domain :CTNPRINInitiative ;
                    rdfs:range xsd:int ;
                    rdfs:comment "Numero totale di persone giuridiche (soggetti) indicati come proponenti nelle proposte presentate. NB: se un unico soggetto è presente in più proposte viene contato tante volte quante sono le proposte in cui appare"@it ,
                                 "Total number of legal persons (entities) indicated as proposers in the proposals submitted. NB: if only one entity is present in more than one proposal, it is counted as many times as there are proposals where it appears"@en ;
                    rdfs:isDefinedBy <https://w3id.org/italia/onto/HER> ;
                    rdfs:label "number of proponents"@en ,
                               "numero di sostenitori"@it .


###  https://w3id.org/italia/onto/HER/numberOfRegisteredStudents
:numberOfRegisteredStudents rdf:type owl:DatatypeProperty ;
                            owl:equivalentProperty :totalRegisteredStudents ;
                            rdfs:domain [ rdf:type owl:Class ;
                                          owl:unionOf ( :MIURStudentsAggregate
                                                        :MIURStudentsByCitizenshipAggregate
                                                        :MIURStudentsByCitizenshipDegreeAggregate
                                                        :MIURStudentsByCitizenshipDegreeClassAggregate
                                                        :MIURStudentsByCitizenshipDegreeDegreeClassAggregate
                                                        :MIURStudentsByDegreeDegreeClassAggregate
                                                        :MIURStudentsByDiplomaAggregate
                                                        :MIURStudentsByDiplomaDegreeDegreeClassAggregate
                                                        :MIURStudentsByProvinceOfResidenceAggregate
                                                        :MIURStudentsByProvinceOfResidenceDegreeDegreeClassAggregate
                                                        :MIURStudentsByRegionOfResidenceAggregate
                                                        :MIURStudentsByRegionOfResidenceDegreeDegreeClassAggregate
                                                      )
                                        ] ;
                            rdfs:range xsd:int ;
                            rdfs:comment "Number of students registered in the Italian education system."@en ,
                                         "Numero di studenti immatricolati al sistema educativo italiano."@it ;
                            rdfs:isDefinedBy <https://w3id.org/italia/onto/HER> ;
                            rdfs:label "number of registered students"@en ,
                                       "numero di studenti immatricolati"@it .


###  https://w3id.org/italia/onto/HER/numberOfSubmittedProposals
:numberOfSubmittedProposals rdf:type owl:DatatypeProperty ;
                            rdfs:domain :CTNPRINInitiative ;
                            rdfs:range xsd:int ;
                            rdfs:comment "Numero totale delle proposte presentate per l'iniziativa in esame"@it ,
                                         "Total number of proposals submitted for the initiative under consideration"@en ;
                            rdfs:isDefinedBy <https://w3id.org/italia/onto/HER> ;
                            rdfs:label "number of submitted proposals"@en ,
                                       "numero di proposte inviate"@it .


###  https://w3id.org/italia/onto/HER/observationalModel
:observationalModel rdf:type owl:DatatypeProperty ;
                    rdfs:domain :AACTDesign ;
                    rdfs:range rdfs:Literal ;
                    rdfs:comment """Primary strategy for participant identification and follow-up. Types include:
Cohort: Group of individuals, initially defined and composed, with common characteristics (for example, condition, birth year), who are examined or traced over a given time period.
Case-Control: Group of individuals with specific characteristics (for example, conditions or exposures) compared to group(s) with different characteristics, but otherwise similar.
Case-Only: Single group of individuals with specific characteristics.
Case-Crossover: Characteristics of case immediately prior to disease onset (sometimes called the hazard period) compared to characteristics of same case at a prior time (that is, control period).
Ecologic or Community Studies: Geographically defined populations, such as countries or regions within a country, compared on a variety of environmental (for example, air pollution intensity, hours of sunlight) and/or global measures not reducible to individual level characteristics (for example, healthcare system, laws or policies median income, average fat intake, disease rate).
Family-Based: Studies conducted among family members, such as genetic studies within families or twin studies and studies of family environment.
Other: Explain in Detailed Description.
"""@en ,
                                 """Strategia primaria per l'identificazione dei partecipanti e il follow-up. I tipi includono:
Cohort: Gruppo di individui, inizialmente definiti e composti, con caratteristiche comuni (per esempio, condizione, anno di nascita), che vengono esaminati o tracciati in un determinato periodo di tempo.
Case-Control: Gruppo di individui con caratteristiche specifiche (ad esempio, condizioni o esposizioni) rispetto a gruppi con caratteristiche diverse, ma per il resto simili.
Case-Only: Singolo gruppo di individui con caratteristiche specifiche.
Case-Crossover: Caratteristiche del caso immediatamente prima dell'insorgenza della malattia (talvolta chiamato periodo di pericolo) rispetto alle caratteristiche dello stesso caso in un momento precedente (cioè, periodo di controllo).
Ecologic or Community Studies: Popolazioni geograficamente definite, come paesi o regioni all'interno di un paese, confrontate su una varietà di misure ambientali (ad esempio, intensità dell'inquinamento atmosferico, ore di luce solare) e/o globali non riducibili a caratteristiche di livello individuale (ad esempio, sistema sanitario, leggi o politiche di reddito mediano, assunzione media di grassi, tasso di malattia).
Family-Based: Studi condotti tra i membri della famiglia, come studi genetici all'interno delle famiglie o studi gemelli e studi sull'ambiente familiare.
Altro: Spiegato nella descrizione dettagliata.
"""@it ;
                    rdfs:isDefinedBy <https://w3id.org/italia/onto/HER> ;
                    rdfs:label "Modello osservativo"@it ,
                               "observational model"@en .


###  https://w3id.org/italia/onto/HER/outcomesAssessorMasked
:outcomesAssessorMasked rdf:type owl:DatatypeProperty ;
                        rdfs:domain :AACTDesign ;
                        rdfs:range rdfs:Literal ;
                        rdfs:comment "La persona che valuta gli esiti di interesse delle parti coinvolte nello studio clinico a cui viene impedito di avere conoscenza degli interventi assegnati ai singoli partecipanti."@it ,
                                     "The individual who evaluates the outcome(s) of interest is is the party or parties involved in the clinical trial who are prevented from having knowledge of the interventions assigned to individual participants."@en ;
                        rdfs:isDefinedBy <https://w3id.org/italia/onto/HER> ;
                        rdfs:label "outcomes assessor masked"@en ,
                                   "risultato esaminatore mascherato"@it .


###  https://w3id.org/italia/onto/HER/overallStatus
:overallStatus rdf:type owl:DatatypeProperty ;
               rdfs:domain :AACTStudy ;
               rdfs:comment "Indica lo stato di reclutamento attuale o lo stato di accesso ampliato."@it ,
                            "Indicates the current recruitment status or the expanded access status."@en ;
               rdfs:isDefinedBy <https://w3id.org/italia/onto/HER> ;
               rdfs:label "overall status"@en ,
                          "stato complessivo"@it .


###  https://w3id.org/italia/onto/HER/patentApplicationDate
:patentApplicationDate rdf:type owl:DatatypeProperty ;
                       rdfs:subPropertyOf ti:date ;
                       rdfs:domain :Patent ;
                       rdfs:range xsd:date ;
                       rdfs:comment "La data in cui è stata presentata la domanda di brevetto."@it ,
                                    "The data in which a patent's application was filled in."@en ;
                       rdfs:isDefinedBy <https://w3id.org/italia/onto/HER> ;
                       rdfs:label "data richiesta brevetto"@it ,
                                  "patent application date"@en ;
                       owl:versionInfo "stabile"@it ,
                                       "stable"@en .


###  https://w3id.org/italia/onto/HER/patentApplicationNo
:patentApplicationNo rdf:type owl:DatatypeProperty ;
                     rdfs:subPropertyOf l0:identifier ;
                     rdfs:domain :Patent ;
                     rdfs:range rdfs:Literal ;
                     rdfs:comment "Il numero di identificazione della domanda di brevetto."@it ,
                                  "The identification number of a patent application."@en ;
                     rdfs:isDefinedBy <https://w3id.org/italia/onto/HER> ;
                     rdfs:label "numero richiesta brevetto"@it ,
                                "patent application number"@en ;
                     owl:versionInfo "stabile"@it ,
                                     "stable"@en .


###  https://w3id.org/italia/onto/HER/patentApplicationYear
:patentApplicationYear rdf:type owl:DatatypeProperty ;
                       rdfs:subPropertyOf ti:year ;
                       rdfs:domain :Result ;
                       rdfs:range xsd:gYear ;
                       rdfs:comment "L'anno in cui è stata depositata la domanda di brevetto."@it ,
                                    "The year in which a patent application was filed."@en ;
                       rdfs:isDefinedBy <https://w3id.org/italia/onto/HER> ;
                       rdfs:label "anno della richiesta"@it ,
                                  "application year"@en .


###  https://w3id.org/italia/onto/HER/patentFamilyCode
:patentFamilyCode rdf:type owl:DatatypeProperty ;
                  rdfs:subPropertyOf l0:identifier ;
                  rdfs:domain :Patent ;
                  rdfs:range rdfs:Literal ;
                  rdfs:comment "Il codice identificativo di una famiglia di brevetti."@it ,
                               "The identification code of a patent family."@en ;
                  rdfs:isDefinedBy <https://w3id.org/italia/onto/HER> ;
                  rdfs:label "codice della famiglia di brevetti"@it ,
                             "patent family code"@en ;
                  owl:versionInfo "stabile"@it ,
                                  "stable"@en .


###  https://w3id.org/italia/onto/HER/patentKindCode
:patentKindCode rdf:type owl:DatatypeProperty ;
                rdfs:subPropertyOf l0:identifier ;
                rdfs:domain [ rdf:type owl:Class ;
                              owl:unionOf ( :PatentPublicationDetail
                                            :PatentPublicationStage
                                          )
                            ] ;
                rdfs:range rdfs:Literal ;
                rdfs:comment "I codici OMPI ST.16 standard (codici tipo) includono una lettera e, in molti casi, un numero, utilizzato per distinguere il tipo di documento di brevetto (ad esempio, pubblicazione di una domanda di brevetto di utilità (pubblicazione di una domanda di brevetto), brevetto, brevetto vegetale pubblicazione di domanda, brevetto di impianto o brevetto di progettazione) e il livello di pubblicazione (ad es. prima pubblicazione, seconda pubblicazione o pubblicazione corretta)."@it ,
                             "WIPO Standard ST.16 codes (kind codes) include a letter, and in many cases a number, used to distinguish the kind of patent document (e.g., publication of an application for a utility patent (patent application publication), patent, plant patent application publication, plant patent, or design patent) and the level of publication (e.g., first publication, second publication, or corrected publication)."@en ;
                rdfs:isDefinedBy <https://w3id.org/italia/onto/HER> ;
                rdfs:label "codice tipologia brevetto"@it ,
                           "patent kind code"@en ;
                owl:versionInfo "stabile"@it ,
                                "stable"@en .


###  https://w3id.org/italia/onto/HER/patentPriorityDate
:patentPriorityDate rdf:type owl:DatatypeProperty ;
                    rdfs:subPropertyOf ti:date ;
                    rdfs:domain :PatentPriorityDetail ;
                    rdfs:range xsd:date ;
                    rdfs:comment "La data di priorità della domanda di brevetto, corrispondente alla data del primo deposito della domanda"@it ,
                                 "The priority date of the patent application, corresponding to the date of the first application filing"@en ;
                    rdfs:isDefinedBy <https://w3id.org/italia/onto/HER> ;
                    rdfs:label "date prioritá"@it ,
                               "priority date"@en ;
                    owl:versionInfo "stabile"@it ,
                                    "stable"@en .


###  https://w3id.org/italia/onto/HER/patentPriorityNo
:patentPriorityNo rdf:type owl:DatatypeProperty ;
                  rdfs:subPropertyOf l0:identifier ;
                  rdfs:domain :PatentPriorityDetail ;
                  rdfs:range rdfs:Literal ;
                  rdfs:comment "Il numero della domanda per la quale viene richiesta una data di priorità. È quindi uguale al numero di domanda del documento di priorità richiesto. Il numero di priorità è costituito da un codice paese (due lettere), l'anno di deposito (quattro cifre) e un numero seriale (variabile, sette cifre)."@it ,
                               """The number of the application for which a priority date is claimed. It is therefore the same as the application number of the claimed priority document. The priority number is made up of a country code (two letters), the year of filing (four digits) and a serial number (variable, seven digits).
"""@en ;
                  rdfs:isDefinedBy <https://w3id.org/italia/onto/HER> ;
                  rdfs:label "numero di prioritá brevetto"@it ,
                             "patent priority number"@en ;
                  owl:versionInfo "provvisoria"@it ,
                                  "unstable"@en .


###  https://w3id.org/italia/onto/HER/patentPriorityYear
:patentPriorityYear rdf:type owl:DatatypeProperty ;
                    rdfs:subPropertyOf ti:year ;
                    rdfs:domain :PatentPriorityDetail ;
                    rdfs:range xsd:gYear ;
                    rdfs:comment "L'anno della data di priorità della domanda corrispondente"@it ,
                                 "The year of the priority date of the corresponding application"@en ;
                    rdfs:isDefinedBy <https://w3id.org/italia/onto/HER> ;
                    rdfs:label "anno di prioritá"@it ,
                               "priority year"@en .


###  https://w3id.org/italia/onto/HER/patentPublicationNumber
:patentPublicationNumber rdf:type owl:DatatypeProperty ;
                         rdfs:subPropertyOf l0:identifier ;
                         rdfs:domain :PatentPublicationDetail ;
                         rdfs:range rdfs:Literal ;
                         rdfs:comment "Il numero di riferimento incrociato assegnato a una domanda di brevetto al momento della pubblicazione"@it ,
                                      "The cross-reference number assigned to a patent application upon publication"@en ;
                         rdfs:isDefinedBy <https://w3id.org/italia/onto/HER> ;
                         rdfs:label "numero pubblicazione brevetto"@it ,
                                    "patent publication number"@en ;
                         owl:versionInfo "stabile"@it ,
                                         "stable"@en .


###  https://w3id.org/italia/onto/HER/patentPublishedAs
:patentPublishedAs rdf:type owl:DatatypeProperty ;
                   rdfs:subPropertyOf l0:identifier ;
                   rdfs:domain :Patent ;
                   rdfs:range rdfs:Literal ;
                   rdfs:comment "One of the (potentially multiple) publication numbers of a patent."@en ,
                                "Uno dei numeri di pubblicazione (potenzialmente multipli) di un brevetto."@it ;
                   rdfs:isDefinedBy <https://w3id.org/italia/onto/HER> ;
                   rdfs:label "brevetto pubblicato come"@it ,
                              "patent published as"@en ;
                   owl:versionInfo "provvisoria"@it ,
                                   "unstable"@en .


###  https://w3id.org/italia/onto/HER/phase
:phase rdf:type owl:DatatypeProperty ;
       rdfs:domain :AACTStudy ;
       rdfs:range rdfs:Literal ;
       rdfs:comment "La fase di uno studio clinico che studia un farmaco o un prodotto biologico, basato sulle definizioni sviluppate dalla Food and Drug Administration (FDA) degli Stati Uniti. La fase si basa sull'obiettivo dello studio, sul numero di partecipanti e su altre caratteristiche. Ci sono cinque fasi: Fase 1 iniziale (precedentemente elencata come Fase 0), Fase 1, Fase 2, Fase 3 e Fase 4. Non applicabile è utilizzato per descrivere studi senza fasi definite dall'FDA, compresi studi su dispositivi o interventi comportamentali."@it ,
                    "The stage of a clinical trial studying a drug or biological product, based on definitions developed by the U.S. Food and Drug Administration (FDA). The phase is based on the study's objective, the number of participants, and other characteristics. There are five phases: Early Phase 1 (formerly listed as Phase 0), Phase 1, Phase 2, Phase 3, and Phase 4. Not Applicable is used to describe trials without FDA-defined phases, including trials of devices or behavioral interventions."@en ;
       rdfs:isDefinedBy <https://w3id.org/italia/onto/HER> ;
       rdfs:label "Fase"@it ,
                  "phase"@en .


###  https://w3id.org/italia/onto/HER/picNumber
:picNumber rdf:type owl:DatatypeProperty ;
           rdfs:subPropertyOf l0:identifier ;
           rdfs:domain [ rdf:type owl:Class ;
                         owl:unionOf ( :ECParticipant
                                       :ErasmusPlusParticipant
                                     )
                       ] ;
           rdfs:range rdfs:Literal ;
           rdfs:comment "Numero di codice di identificazione del partecipante (PIC - Participant Identification Code). Si tratta di un numero a 9 cifre che serve come identificatore unico per le organizzazioni (soggetti giuridici) che partecipano a programmi di finanziamento / appalti dell'UE."@it ,
                        "Participant Identification Code (PIC) number. It is a 9-digit number serving as a unique identifier for organisations (legal entities) participating in EU funding programmes / procurement."@en ;
           rdfs:isDefinedBy <https://w3id.org/italia/onto/HER> ;
           rdfs:label "codice identificativo partecipante"@it ,
                      "pic number"@en ;
           owl:versionInfo "stabile"@it ,
                           "stable"@en .


###  https://w3id.org/italia/onto/HER/planToShareIPD
:planToShareIPD rdf:type owl:DatatypeProperty ;
                rdfs:domain :AACTStudy ;
                rdfs:comment """Define whether there is a plan to make individual participant data (IPD) collected in this study, including data dictionaries, available to other researchers (typically after the end of the study). Options are:
Yes: There is a plan to make IPD and related data dictionaries available.
No: There is not a plan to make IPD available.
Undecided: It is not yet known if there will be a plan to make IPD available.
"""@en ,
                             """Definire se esiste un piano per mettere a disposizione di altri ricercatori (in genere dopo la fine dello studio) i dati dei singoli partecipanti (IPD) raccolti in questo studio, compresi i dizionari dei dati. Le opzioni sono:
Sì: esiste un piano per rendere disponibili i dizionari IPD e i relativi dizionari di dati.
No: non esiste un piano per rendere disponibile l'IPD.
Indeciso: Non si sa ancora se ci sarà un piano per rendere disponibile l'IPD."""@it ;
                rdfs:isDefinedBy <https://w3id.org/italia/onto/HER> ;
                rdfs:label "piano per la condivisione di IPD"@it ,
                           "plan to share IPD"@en .


###  https://w3id.org/italia/onto/HER/planToShareIPDDescription
:planToShareIPDDescription rdf:type owl:DatatypeProperty ;
                           rdfs:subPropertyOf l0:description ;
                           rdfs:domain :AACTStudy ;
                           rdfs:range rdfs:Literal ;
                           rdfs:comment "If Plan to Share IPD is \"Yes,\" briefly describe what specific individual participant data sets are to be shared (for example, all collected IPD, all IPD that underlie results in a publication). If the Plan to Share IPD is \"No\" or \"Undecided,\" an explanation may be provided for why IPD will not be shared or why it is not yet decided."@en ,
                                        "Se Plan to Share IPD è \"Sì\", descrive brevemente quali specifici set di dati dei singoli partecipanti devono essere condivisi (ad esempio, tutti gli IPD raccolti, tutti gli IPD che sono alla base di una pubblicazione). Se l'IPD del Piano di condivisione è \"No\" o \"Indeciso\", può essere fornita una spiegazione del perché l'IPD non sarà condiviso o perché non è ancora stato deciso."@it ;
                           rdfs:isDefinedBy <https://w3id.org/italia/onto/HER> ;
                           rdfs:label "description of plan to share IPD"@en ,
                                      "descrizione del piano di condivisione del DPI"@it ;
                           owl:versionInfo "provvissoria"@it ,
                                           "unstable"@en .


###  https://w3id.org/italia/onto/HER/primaryCompletionDate
:primaryCompletionDate rdf:type owl:DatatypeProperty ;
                       rdfs:subPropertyOf ti:date ;
                       rdfs:domain :AACTStudy ;
                       rdfs:range xsd:date ;
                       rdfs:comment "La data di conclusione primaria dello studio (secondo la definizione di NLM) in un formato di tipo data, in modo da poterla utilizzare per trovare gli studi prima/dopo/indicatori di una o più date. Per gli studi che prevedono solo mese/anno, viene utilizzato l'ultimo giorno del mese."@it ,
                                    "The primary completion date for the study (as defined by NLM) in a date-type format so that it can be used to find studies before/after/inclusive of a date or dates. For studies that only provide month/year, the last day of the month is used."@en ;
                       rdfs:isDefinedBy <https://w3id.org/italia/onto/HER> ;
                       rdfs:label "data completamento principale"@it ,
                                  "primary completion date"@en ;
                       owl:versionInfo "provvisoria"@it ,
                                       "unstable"@en .


###  https://w3id.org/italia/onto/HER/primaryCompletionDateType
:primaryCompletionDateType rdf:type owl:DatatypeProperty ;
                           rdfs:domain :AACTStudy ;
                           rdfs:comment "All posted dates include a type attribute of Actual or Anticipated/ Estimate."@en ,
                                        "Tutte le date pubblicate includono un attributo di tipo Actual o Anticipated/ Estimate."@it ;
                           rdfs:isDefinedBy <https://w3id.org/italia/onto/HER> ;
                           rdfs:label "primary completion date type"@en ,
                                      "tipo di data primaria di completamento"@it .


###  https://w3id.org/italia/onto/HER/primaryCompletionMonthYear
:primaryCompletionMonthYear rdf:type owl:DatatypeProperty ;
                            rdfs:subPropertyOf ti:month ;
                            rdfs:domain :AACTStudy ;
                            rdfs:range xsd:gMonth ;
                            rdfs:comment "La data di conclusione primaria dello studio (secondo la definizione di NLM) in un formato di tipo data, in modo da poterla utilizzare per trovare gli studi prima/dopo/indicatori di una o più date. Per gli studi che prevedono solo mese/anno, viene utilizzato l'ultimo giorno del mese."@it ,
                                         "The primary completion date for the study (as defined by NLM) in a date-type format so that it can be used to find studies before/after/inclusive of a date or dates. For studies that only provide month/year, the last day of the month is used."@en ;
                            rdfs:isDefinedBy <https://w3id.org/italia/onto/HER> ;
                            rdfs:label "mese-anno di primario completamento"@it ,
                                       "primary completion month-year"@en .


###  https://w3id.org/italia/onto/HER/primaryPurpose
:primaryPurpose rdf:type owl:DatatypeProperty ;
                rdfs:domain :AACTDesign ;
                rdfs:range rdfs:Literal ;
                rdfs:comment """L'obiettivo principale degli interventi che vengono valutati dallo studio clinico. Gli scopi primari sono:
Trattamento: Uno o più interventi sono in fase di valutazione per il trattamento di una malattia, sindrome o condizione.
Prevenzione: Uno o più interventi sono in fase di valutazione per prevenire lo sviluppo di una specifica malattia o condizione di salute.
Diagnostica: Si stanno valutando uno o più interventi per identificare una malattia o una condizione di salute.
Cure di supporto: Uno o più interventi sono valutati per massimizzare il comfort, ridurre al minimo gli effetti collaterali o mitigare il declino della salute o della funzione del partecipante.
Screening: Uno o più interventi sono valutati o esaminati per identificare una condizione, o fattori di rischio per una condizione, in persone che non sono ancora note per avere la condizione o il fattore di rischio.
Ricerca sui servizi sanitari: Uno o più interventi per valutare la fornitura, i processi, la gestione, l'organizzazione o il finanziamento dell'assistenza sanitaria.
Scienza di base: Uno o più interventi per esaminare il meccanismo di base dell'azione (per esempio, la fisiologia o la biomeccanica di un intervento).
Fattibilità del dispositivo: Un intervento di un dispositivo viene valutato in un piccolo trial clinico (generalmente meno di 10 partecipanti) per determinare la fattibilità del prodotto; o un trial clinico per testare un prototipo di dispositivo per verificarne la fattibilità e non gli esiti sanitari. Tali studi sono condotti per confermare la progettazione e le specifiche operative di un dispositivo prima di iniziare una sperimentazione clinica completa.
Altro: Non si applica nessuna delle altre opzioni."""@it ,
                             """The main objective of the intervention(s) being evaluated by the clinical trial. Type os primary purpose are:
Treatment: One or more interventions are being evaluated for treating a disease, syndrome, or condition.
Prevention: One or more interventions are being assessed for preventing the development of a specific disease or health condition.
Diagnostic: One or more interventions are being evaluated for identifying a disease or health condition.
Supportive Care: One or more interventions are evaluated for maximizing comfort, minimizing side effects, or mitigating against a decline in the participant's health or function.
Screening: One or more interventions are assessed or examined for identifying a condition, or risk factors for a condition, in people who are not yet known to have the condition or risk factor.
Health Services Research: One or more interventions for evaluating the delivery, processes, management, organization, or financing of healthcare.
Basic Science: One or more interventions for examining the basic mechanism of action (for example, physiology or biomechanics of an intervention).
Device Feasibility: An intervention of a device product is being evaluated in a small clinical trial (generally fewer than 10 participants) to determine the feasibility of the product; or a clinical trial to test a prototype device for feasibility and not health outcomes. Such studies are conducted to confirm the design and operating specifications of a device before beginning a full clinical trial.
Other: None of the other options applies.
"""@en ;
                rdfs:isDefinedBy <https://w3id.org/italia/onto/HER> ;
                rdfs:label "Scopo primario"@it ,
                           "primary purpose"@en .


###  https://w3id.org/italia/onto/HER/projectCode
:projectCode rdf:type owl:DatatypeProperty ;
             rdfs:subPropertyOf l0:identifier ;
             rdfs:domain <https://w3id.org/italia/onto/Project/PublicInvestmentProject> ;
             rdfs:range rdfs:Literal ;
             rdfs:comment """Identification assigned to the Project to which the operation refers in the Information System of origin. To a single project can be assigned as many operations as there are subjects carrying out the project.
This id allows you to aggregate all the operations that are part of a project."""@en ,
                          """Identificativo assegnato al Progetto a cui si riferisce l'operazione nel Sistema Informatico di provenienza. Ad un unico progetto possono fanno capo tante operazioni quanti sono i soggetti che svolgono il progetto.
Questo id consente di aggregare tutte le operazioni che fanno capo ad un progetto."""@it ;
             rdfs:isDefinedBy <https://w3id.org/italia/onto/HER> ;
             rdfs:label "codice del progetto"@it ,
                        "project code"@en ;
             owl:versionInfo "provvisoria"@it ,
                             "unstable"@en .


###  https://w3id.org/italia/onto/HER/proposalsCost
:proposalsCost rdf:type owl:DatatypeProperty ;
               rdfs:domain :CTNPRINInitiative ;
               rdfs:comment "Somma dei costi totali indicati dai proponenti nelle proposte presentate"@it ,
                            "Sum of the total costs indicated by the proposers in the submitted proposals"@en ;
               rdfs:isDefinedBy <https://w3id.org/italia/onto/HER> ;
               rdfs:label "costo delle proposte"@it ,
                          "proposals cost"@en .


###  https://w3id.org/italia/onto/HER/publicationDate
:publicationDate rdf:type owl:DatatypeProperty ;
                 rdfs:subPropertyOf ti:date ;
                 rdfs:domain [ rdf:type owl:Class ;
                               owl:unionOf ( :PatentPublicationDetail
                                             :Result
                                           )
                             ] ;
                 rdfs:range xsd:date ;
                 rdfs:comment "La data di pubblicazione di un risultato"@it ,
                              "The date of publication of a result"@en ;
                 rdfs:isDefinedBy <https://w3id.org/italia/onto/HER> ;
                 rdfs:label "data pubblicazione"@it ,
                            "publication date"@en ;
                 owl:versionInfo "stabile"@it ,
                                 "stable"@en .


###  https://w3id.org/italia/onto/HER/publicationYear
:publicationYear rdf:type owl:DatatypeProperty ;
                 rdfs:subPropertyOf ti:year ;
                 rdfs:domain [ rdf:type owl:Class ;
                               owl:unionOf ( :PatentPublicationDetail
                                             :Result
                                           )
                             ] ;
                 rdfs:range xsd:gYear ;
                 rdfs:comment "L'anno di pubblicazione."@it ,
                              "The year of publication."@en ;
                 rdfs:isDefinedBy <https://w3id.org/italia/onto/HER> ;
                 rdfs:label "anno di pubblicazione"@it ,
                            "publication year"@en .


###  https://w3id.org/italia/onto/HER/pubmedId
:pubmedId rdf:type owl:DatatypeProperty ;
          rdfs:subPropertyOf l0:identifier ;
          rdfs:domain :Result ;
          rdfs:range rdfs:Literal ;
          rdfs:comment "Identificatore di una pubblicazione nel repository PubMed (https://pubmed.ncbi.nlm.nih.gov/)"@it ,
                       "Identifier of a publication in the PubMed repository (https://pubmed.ncbi.nlm.nih.gov/)"@en ;
          rdfs:isDefinedBy <https://w3id.org/italia/onto/HER> ;
          rdfs:label "PubMed ID"@en ,
                     "identificatore PubMed"@it .


###  https://w3id.org/italia/onto/HER/rcn
:rcn rdf:type owl:DatatypeProperty ;
     rdfs:subPropertyOf l0:identifier ;
     rdfs:domain :ECParticipant ;
     rdfs:range rdfs:Literal ;
     rdfs:comment "Record Control Number, used as a participant identifier in CORDIS."@en ,
                  "Record Control Number, utilizzato come identificativo del partecipante in CORDIS."@it ;
     rdfs:isDefinedBy <https://w3id.org/italia/onto/HER> ;
     rdfs:label "numero record di controllo"@it ,
                "record control number"@en ;
     owl:versionInfo "stabile"@it ,
                     "stable"@en .


###  https://w3id.org/italia/onto/HER/regionalExpense
:regionalExpense rdf:type owl:DatatypeProperty ;
                 rdfs:domain :USTATUniversityInterventionExpensesAggregate ;
                 rdfs:comment "Amount of expenditure financed with funds from the Region. Values already included in the column \"EXPENDITURE_TOTAL\". Data are related to the financial year per year (T-1)."@en ,
                              "Importo della spesa finanziata con fondi della Regione. Valori già ricompresi nella colonna \"SPESA_TOTALE\". I dati sono relativi all'esercizio finanziario all'anno (T-1)"@it ;
                 rdfs:isDefinedBy <https://w3id.org/italia/onto/HER> ;
                 rdfs:label "regional expense"@en ,
                            "spese regionali"@it .


###  https://w3id.org/italia/onto/HER/removedCountry
:removedCountry rdf:type owl:DatatypeProperty ,
                         owl:FunctionalProperty ;
                rdfs:domain :CountryInvolvement ;
                rdfs:range xsd:boolean ;
                rdfs:comment "Country where a facility conducting a clinical protocol was removed from study"@en ,
                             "Paese in cui una struttura che conduce un protocollo clinico è stata rimossa dallo studio"@it ;
                rdfs:isDefinedBy <https://w3id.org/italia/onto/HER> ;
                rdfs:label "country removed"@en ,
                           "paese rimosso"@it ;
                owl:versionInfo "stabile"@it ,
                                "stable"@en .


###  https://w3id.org/italia/onto/HER/requiredContribution
:requiredContribution rdf:type owl:DatatypeProperty ;
                      rdfs:domain :CTNPRINInitiative ;
                      rdfs:comment "Total contributions requested in the project proposals"@en ,
                                   "Totale dei contributi totali richiesti nelle proposte di progetto"@it ;
                      rdfs:isDefinedBy <https://w3id.org/italia/onto/HER> ;
                      rdfs:label "contributi richiesti"@it ,
                                 "required contributions"@en .


###  https://w3id.org/italia/onto/HER/resultType
:resultType rdf:type owl:DatatypeProperty ;
            rdfs:domain :Result ;
            rdfs:range rdfs:Literal ;
            rdfs:comment "Testo che indica il tipo di risultato/prodotto corrispondente. I valori possibili sono: \"Dimostratore, pilota, prototipo\", \"Documento, rapporti...\", \"Siti web, compilazione di brevetti, video ecc."@it ,
                         "Text denoting the corresponding type of result. Possible values are: \"Demonstrator, pilot, prototype\", \"Document, reports...\", \"Websites, patent filling, videos etc\" and \"Other\"."@en ;
            rdfs:isDefinedBy <https://w3id.org/italia/onto/HER> ;
            rdfs:label "result type"@en ,
                       "tipo di risultato"@it ;
            owl:versionInfo "stabile"@it ,
                            "stable"@en .


###  https://w3id.org/italia/onto/HER/resultsFirstPostedDate
:resultsFirstPostedDate rdf:type owl:DatatypeProperty ;
                        rdfs:subPropertyOf ti:date ;
                        rdfs:domain :AACTStudy ;
                        rdfs:range xsd:date ;
                        rdfs:comment "Data in cui i risultati sono stati resi pubblici per la prima volta su ClinicalTrials.gov"@it ,
                                     "Date on which results were first made public on ClinicalTrials.gov"@en ;
                        rdfs:isDefinedBy <https://w3id.org/italia/onto/HER> ;
                        rdfs:label "results first posted date"@en ,
                                   "risultati prima data pubblicazione"@it ;
                        owl:versionInfo "stabile"@it ,
                                        "stable"@en .


###  https://w3id.org/italia/onto/HER/resultsFirstPostedDateType
:resultsFirstPostedDateType rdf:type owl:DatatypeProperty ;
                            rdfs:domain :AACTStudy ;
                            rdfs:comment "All posted dates include a type attribute of Actual or Anticipated/ Estimate."@en ,
                                         "Tutte le date pubblicate includono un attributo di tipo Actual o Anticipated/ Estimate."@it ;
                            rdfs:isDefinedBy <https://w3id.org/italia/onto/HER> ;
                            rdfs:label "results first posted date type"@en ,
                                       "tipo di risultati prima data di pubblicazione"@it .


###  https://w3id.org/italia/onto/HER/resultsFirstSubmittedDate
:resultsFirstSubmittedDate rdf:type owl:DatatypeProperty ;
                           rdfs:subPropertyOf ti:date ;
                           rdfs:domain :AACTStudy ;
                           rdfs:range xsd:date ;
                           rdfs:comment "Date on which first results were submited"@en ,
                                        "La data in cui i primi risultati sono stati inviati."@it ;
                           rdfs:isDefinedBy <https://w3id.org/italia/onto/HER> ;
                           rdfs:label "results first submitted date"@en ,
                                      "risultati prima data invio"@it ;
                           owl:versionInfo "stabile"@it ,
                                           "stable"@en .


###  https://w3id.org/italia/onto/HER/resultsFirstSubmittedQCDate
:resultsFirstSubmittedQCDate rdf:type owl:DatatypeProperty ;
                             rdfs:subPropertyOf ti:date ;
                             rdfs:domain :AACTStudy ;
                             rdfs:range xsd:date ;
                             rdfs:comment "Il suffisso _submitted_qc indica la data di presentazione della versione del record che soddisfa i criteri di controllo della qualità. È comune che ci siano revisioni tra la prima presentazione e la presentazione che soddisfa i criteri qc. Si noti che questa non è la data in cui è stata completata la revisione qc."@it ,
                                          "The _submitted_qc suffix indicates the submission date of the version of the record that met quality control criteria. It is common for there to be revisions between the first submission and the submission that meets qc criteria. Note this is not the date that the qc review was completed."@en ;
                             rdfs:isDefinedBy <https://w3id.org/italia/onto/HER> ;
                             rdfs:label "results first submitted QC date"@en ,
                                        "risultati prima data invio QC"@it ;
                             owl:versionInfo "stabile"@it ,
                                             "stable"@en .


###  https://w3id.org/italia/onto/HER/revocationDate
:revocationDate rdf:type owl:DatatypeProperty ;
                rdfs:subPropertyOf ti:date ;
                rdfs:domain :CTNPRINOperation ;
                rdfs:range xsd:date ;
                rdfs:comment "Data di revoca nel contesto delle operazioni PRIN. La proprietà è valorizzata solo se la relativa proprietà revoca è utilizzata."@it ,
                             "Date of revocation of an operation in the context of PRIN. It is valorized only if the revoked property is used."@en ;
                rdfs:isDefinedBy <https://w3id.org/italia/onto/HER> ;
                rdfs:label "data revoca"@it ,
                           "revocation date"@en ;
                owl:versionInfo "stabile"@it ,
                                "stable"@en .


###  https://w3id.org/italia/onto/HER/revoked
:revoked rdf:type owl:DatatypeProperty ,
                  owl:FunctionalProperty ;
         rdfs:domain :CTNPRINOperation ;
         rdfs:range xsd:boolean ;
         rdfs:comment "Questa proprietà è vera solo se il progetto è stato revocato e può assumere i valori \"parzialmente\" o \"totalmente\""@it ,
                      "The value is true only if the project has been revoked and it can assume the values \"partially\" or \"totally\"."@en ;
         rdfs:isDefinedBy <https://w3id.org/italia/onto/HER> ;
         rdfs:label "revocata"@it ,
                    "revoked"@en .


###  https://w3id.org/italia/onto/HER/samplingMethod
:samplingMethod rdf:type owl:DatatypeProperty ;
                rdfs:domain :AACTEligibility ;
                rdfs:range rdfs:Literal ;
                rdfs:comment """Indicate the method used for the sampling approach and explain in the Detailed Description. Types are:
Probability Sample: Exclusively random process to guarantee that each participant or population has specified chance of selection, such as simple random sampling, systematic sampling, stratified random sampling, cluster sampling, and consecutive participant sampling
Non-Probability Sample: Any of a variety of other sampling processes, such as convenience sampling or invitation to volunteer
"""@en ,
                             """Indicazioni e spiegazioni riguardo il metodo utilizzato per l'approccio di campionamento I tipi sono:
Campione di probabilità: Processo esclusivamente casuale per garantire che ogni partecipante o popolazione abbia specificato la possibilità di selezione, come il campionamento casuale semplice, il campionamento sistematico, il campionamento casuale stratificato, il campionamento a grappolo e il campionamento consecutivo dei partecipanti.
Campione di nonrobabilità: Qualsiasi di una varietà di altri processi di campionamento, come il campionamento di convenienza o l'invito al volontariato"""@it ;
                rdfs:isDefinedBy <https://w3id.org/italia/onto/HER> ;
                rdfs:label "Metodo di campionamento"@it ,
                           "sampling method"@en .


###  https://w3id.org/italia/onto/HER/scopusAffiliationId
:scopusAffiliationId rdf:type owl:DatatypeProperty ;
                     rdfs:domain covapit:Organization ;
                     rdfs:range rdfs:Literal ;
                     rdfs:comment "L'identificatore dell'organizzazione in Scopus"@it ,
                                  "The identifier of the organization in Scopus"@en ;
                     rdfs:isDefinedBy <https://w3id.org/italia/onto/HER> ;
                     rdfs:label "identificativo affiliazione in Scopus"@it ,
                                "scopus affiliation identifier"@en .


###  https://w3id.org/italia/onto/HER/shortName
:shortName rdf:type owl:DatatypeProperty ;
           rdfs:subPropertyOf l0:name ;
           rdfs:range rdfs:Literal ;
           rdfs:isDefinedBy <https://w3id.org/italia/onto/HER> .


###  https://w3id.org/italia/onto/HER/shortTitle
:shortTitle rdf:type owl:DatatypeProperty ;
            rdfs:domain :AACTStudy ;
            rdfs:range rdfs:Literal ;
            rdfs:comment "A short title of the clinical study written in language intended for the lay public. The title should include, where possible, information on the participants, condition being evaluated, and intervention(s) studied."@en ,
                         "Un breve titolo dello studio clinico scritto in un linguaggio destinato al pubblico laico. Il titolo dovrebbe includere, ove possibile, informazioni sui partecipanti, sulla condizione in corso di valutazione e sugli interventi studiati."@it ;
            rdfs:isDefinedBy <https://w3id.org/italia/onto/HER> ;
            rdfs:label "short title"@en ,
                       "titolo breve"@it .


###  https://w3id.org/italia/onto/HER/sizeOfEntity
:sizeOfEntity rdf:type owl:DatatypeProperty ;
              rdfs:domain :CTNPRINEntity ;
              rdfs:range rdfs:Literal ;
              rdfs:comment "Dimensione dell'impresa secondo classificazione EU. N/A per soggetti pubblici."@it ,
                           "Enterprise size according to EU classification. N/A for public entities."@en ;
              rdfs:isDefinedBy <https://w3id.org/italia/onto/HER> ;
              rdfs:label "dimensione istituzione finanziata ctn/prin"@it ,
                         "size of ctn/prin funded institution"@en ;
              owl:versionInfo "provvisoria"@it ,
                              "unstable"@en .


###  https://w3id.org/italia/onto/HER/sponsorType
:sponsorType rdf:type owl:DatatypeProperty ;
             rdfs:domain :AACTSponsor ;
             rdfs:range rdfs:Literal ;
             rdfs:comment "Broad Category of sponsor. They can be: Other, Industry, NIH, US. Fed"@en ,
                          "Tipo di sponsor specificato con una stringa. Possono essere: Altro, Industria, NIH, USA. Fed"@it ;
             rdfs:isDefinedBy <https://w3id.org/italia/onto/HER> ;
             rdfs:label "sponsor type"@en ,
                        "tipo di sponsor"@it ;
             owl:versionInfo "stabile"@it ,
                             "stable"@en .


###  https://w3id.org/italia/onto/HER/startingDate
:startingDate rdf:type owl:DatatypeProperty ;
              rdfs:subPropertyOf ti:date ;
              rdfs:domain [ rdf:type owl:Class ;
                            owl:unionOf ( :AACTStudy
                                          :CTNPRINOperation
                                        )
                          ] ;
              rdfs:range xsd:date ;
              rdfs:comment "Data di inizio di uno studio o di un'operazione."@it ,
                           "Starting date of a study or operation."@en ;
              rdfs:isDefinedBy <https://w3id.org/italia/onto/HER> ;
              rdfs:label "data inizio"@it ,
                         "starting date"@en ;
              owl:versionInfo "stabile"@it ,
                              "stable"@en .


###  https://w3id.org/italia/onto/HER/startingDateType
:startingDateType rdf:type owl:DatatypeProperty ;
                  rdfs:domain :AACTStudy ;
                  rdfs:comment "La data effettiva in cui il primo partecipante è stato iscritto ad uno studio clinico. La data \"stimata\" di inizio dello studio è la data che i ricercatori ritengono essere la data di inizio dello studio."@it ,
                               "The actual date on which the first participant was enrolled in a clinical study. The \"estimated\" study start date is the date that the researchers think will be the study start date."@en ;
                  rdfs:isDefinedBy <https://w3id.org/italia/onto/HER> ;
                  rdfs:label "starting date type"@en ,
                             "tipo di data di inizio"@it .


###  https://w3id.org/italia/onto/HER/startingMonthYear
:startingMonthYear rdf:type owl:DatatypeProperty ;
                   rdfs:subPropertyOf ti:month ;
                   rdfs:domain :AACTStudy ;
                   rdfs:range xsd:gMonth ;
                   rdfs:comment "La data in cui il primo partecipante è stato iscritto / era previsto che si iscrivesse. La data effettiva di iscrizione del primo partecipante"@it ,
                                "The date on which the first participant was enrolled / was expected to enroll. The actual date on which the first participant was enrolled"@en ;
                   rdfs:isDefinedBy <https://w3id.org/italia/onto/HER> ;
                   rdfs:label "mese-anno di inizio"@it ,
                              "starting month-year"@en .


###  https://w3id.org/italia/onto/HER/startingYear
:startingYear rdf:type owl:DatatypeProperty ;
              rdfs:subPropertyOf ti:year ;
              rdfs:domain [ rdf:type owl:Class ;
                            owl:unionOf ( :CHAFEAProject
                                          :ECProject
                                          :ERCProject
                                          :EUREKAProject
                                          :ErasmusPlusProject
                                        )
                          ] ;
              rdfs:range xsd:gYear ;
              rdfs:comment "Indica l'anno di inizio di un progetto"@it ,
                           "Starting year of the project"@en ;
              rdfs:isDefinedBy <https://w3id.org/italia/onto/HER> ;
              rdfs:label "anno di inizio"@it ,
                         "starting year"@en .


###  https://w3id.org/italia/onto/HER/status
:status rdf:type owl:DatatypeProperty ;
        rdfs:domain [ rdf:type owl:Class ;
                      owl:unionOf ( :AACTFacility
                                    :EUREKAProject
                                    :ErasmusPlusProject
                                  )
                    ] ;
        rdfs:comment "Descrizione testuale dello stato di una struttura o progetto."@it ,
                     "Textual description of the status of a facility or project."@en ;
        rdfs:isDefinedBy <https://w3id.org/italia/onto/HER> ;
        rdfs:label "stato"@it ,
                   "status"@en .


###  https://w3id.org/italia/onto/HER/studyFirstPostedDate
:studyFirstPostedDate rdf:type owl:DatatypeProperty ;
                      rdfs:subPropertyOf ti:date ;
                      rdfs:domain :AACTStudy ;
                      rdfs:range xsd:date ;
                      rdfs:comment "La data in cui il record dello studio è stato disponibile per la prima volta su ClinicalTrials.gov. In genere c'è un ritardo di alcuni giorni tra la data in cui lo sponsor dello studio o lo sperimentatore ha presentato la cartella clinica e la prima data di pubblicazione."@it ,
                                   "The date on which the study record was first available on ClinicalTrials.gov. There is typically a delay of a few days between the date the study sponsor or investigator submitted the study record and the first posted date."@en ;
                      rdfs:isDefinedBy <https://w3id.org/italia/onto/HER> ;
                      rdfs:label "data inizio studio"@it ,
                                 "study first posted date"@en ;
                      owl:versionInfo "stabile"@it ,
                                      "stable"@en .


###  https://w3id.org/italia/onto/HER/studyFirstPostedDateType
:studyFirstPostedDateType rdf:type owl:DatatypeProperty ;
                          rdfs:domain :AACTStudy ;
                          rdfs:comment "All posted dates include a type attribute of Actual or Anticipated/ Estimate."@en ,
                                       "Tutte le date pubblicate includono un attributo di tipo Actual o Anticipated/ Estimate."@it ;
                          rdfs:isDefinedBy <https://w3id.org/italia/onto/HER> ;
                          rdfs:label "study first posted date type"@en ,
                                     "tipo di data di inizio dello studio"@it .


###  https://w3id.org/italia/onto/HER/studyFirstSubmittedDate
:studyFirstSubmittedDate rdf:type owl:DatatypeProperty ;
                         rdfs:subPropertyOf ti:date ;
                         rdfs:domain :AACTStudy ;
                         rdfs:range xsd:date ;
                         rdfs:comment "Il suffisso _submitted indica la data in cui il responsabile ha premuto il pulsante di rilascio nel sistema di invio dati di ClinicalTrials.gov, inviando così lo studio per la revisione prima della pubblicazione\"."@it ,
                                      "The _submitted suffix indicates the date that the responsible party pressed the release button in the ClinicalTrials.gov data submission system, thereby submitting the study for review prior to posting.\""@en ;
                         rdfs:isDefinedBy <https://w3id.org/italia/onto/HER> ;
                         rdfs:label "data presentazione primo studio"@it ,
                                    "study first submitted date"@en ;
                         owl:versionInfo "stabile"@it ,
                                         "stable"@en .


###  https://w3id.org/italia/onto/HER/studyFirstSubmittedQCDate
:studyFirstSubmittedQCDate rdf:type owl:DatatypeProperty ;
                           rdfs:subPropertyOf ti:date ;
                           rdfs:domain :AACTStudy ;
                           rdfs:range xsd:date ;
                           rdfs:comment "Il suffisso _submitted_qc indica la data di presentazione dello studio della versione del record che soddisfa i criteri di controllo di qualità. È comune che ci siano revisioni tra la prima presentazione dello studio e la presentazione che soddisfa i criteri qc. Si noti che questa non è la data in cui è stata completata la revisione qc\"."@it ,
                                        "The _submitted_qc suffix indicates the study submission date of the version of the record that met quality control criteria. It is common for there to be revisions between the first study submission and the submission that meets qc criteria. Note this is not the date that the qc review was completed.\""@en ;
                           rdfs:isDefinedBy <https://w3id.org/italia/onto/HER> ;
                           rdfs:label "data primo studio presentato QC"@it ,
                                      "study first submitted QC date"@en ;
                           owl:versionInfo "stabile"@it ,
                                           "stable"@en .


###  https://w3id.org/italia/onto/HER/studyType
:studyType rdf:type owl:DatatypeProperty ;
           rdfs:domain :AACTStudy ;
           rdfs:comment "Describes the nature of a clinical study. Study types include interventional studies (also called clinical trials), observational studies (including patient registries), and expanded access."@en ,
                        "Descrive la natura di uno studio clinico. I tipi di studio includono studi interventistici (chiamati anche studi clinici), studi osservazionali (inclusi i registri dei pazienti) e l'accesso esteso."@it ;
           rdfs:isDefinedBy <https://w3id.org/italia/onto/HER> ;
           rdfs:label "study type"@en ,
                      "tipo di studio"@it .


###  https://w3id.org/italia/onto/HER/subjectMasked
:subjectMasked rdf:type owl:DatatypeProperty ;
               rdfs:domain :AACTDesign ;
               rdfs:comment """L'obiettivo principale degli interventi che vengono valutati dallo studio clinico. Gli scopi primari sono:
Trattamento: Uno o più interventi sono in fase di valutazione per il trattamento di una malattia, sindrome o condizione.
Prevenzione: Uno o più interventi sono in fase di valutazione per prevenire lo sviluppo di una specifica malattia o condizione di salute.
Diagnostica: Si stanno valutando uno o più interventi per identificare una malattia o una condizione di salute.
Cure di supporto: Uno o più interventi sono valutati per massimizzare il comfort, ridurre al minimo gli effetti collaterali o mitigare il declino della salute o della funzione del partecipante.
Screening: Uno o più interventi sono valutati o esaminati per identificare una condizione, o fattori di rischio per una condizione, in persone che non sono ancora note per avere la condizione o il fattore di rischio.
Ricerca sui servizi sanitari: Uno o più interventi per valutare la fornitura, i processi, la gestione, l'organizzazione o il finanziamento dell'assistenza sanitaria.
Scienza di base: Uno o più interventi per esaminare il meccanismo di base dell'azione (per esempio, la fisiologia o la biomeccanica di un intervento).
Fattibilità del dispositivo: Un intervento di un dispositivo viene valutato in un piccolo trial clinico (generalmente meno di 10 partecipanti) per determinare la fattibilità del prodotto; o un trial clinico per testare un prototipo di dispositivo per verificarne la fattibilità e non gli esiti sanitari. Tali studi sono condotti per confermare la progettazione e le specifiche operative di un dispositivo prima di iniziare una sperimentazione clinica completa.
Altro: Non si applica nessuna delle altre opzioni."""@it ,
                            "Subject is the party or parties involved in the clinical trial who are prevented from having knowledge of the interventions assigned to individual participants."@en ;
               rdfs:isDefinedBy <https://w3id.org/italia/onto/HER> ;
               rdfs:label "is subject masked?"@en .


###  https://w3id.org/italia/onto/HER/targetDuration
:targetDuration rdf:type owl:DatatypeProperty ;
                rdfs:domain :AACTStudy ;
                rdfs:comment "expected number of months between start_date & primary_completion_date"@en ,
                             "numero di mesi previsti tra la data_di_inizio e la data_di_completamento_primaria"@it ;
                rdfs:isDefinedBy <https://w3id.org/italia/onto/HER> ;
                rdfs:label "durata del target"@it ,
                           "target duration"@en .


###  https://w3id.org/italia/onto/HER/timePerspective
:timePerspective rdf:type owl:DatatypeProperty ;
                 rdfs:domain :AACTDesign ;
                 rdfs:comment """Rapporto temporale tra il periodo di osservazione e il momento dell'iscrizione dei partecipanti. I tipi sono:
Retrospettiva: Osservazione retrospettiva basata su osservazioni raccolte prevalentemente prima della selezione dei soggetti e dell'iscrizione
Prospettiva: Osservazioni periodiche raccolte prevalentemente in seguito all'iscrizione al corso di studi.
Sezione trasversale: Osservazioni o misurazioni effettuate in un unico momento, di solito all'iscrizione del soggetto
Altro: Spiegato nella descrizione dettagliata"""@it ,
                              """Temporal relationship of observation period to time of participant enrollment. Types are:
Retrospective: Look back using observations collected predominantly prior to subject selection and enrollment
Prospective: Look forward using periodic observations collected predominantly following subject enrollment
Cross-sectional: Observations or measurements made at a single point in time, usually at subject enrollment
Other: Explain in Detailed Description
"""@en ;
                 rdfs:isDefinedBy <https://w3id.org/italia/onto/HER> ;
                 rdfs:label "prospettiva temporale"@it ,
                            "time perspective"@en .


###  https://w3id.org/italia/onto/HER/title
:title rdf:type owl:DatatypeProperty ;
       rdfs:domain [ rdf:type owl:Class ;
                     owl:unionOf ( :AACTStudy
                                   :CHAFEASummary
                                   :CHAFEAWorkpackage
                                   :CTNPRINOperation
                                   :ErasmusPlusFile
                                   :Result
                                 )
                   ] ;
       rdfs:range rdfs:Literal ;
       rdfs:comment "Testo del titolo di un progetto, risultato della ricerca, ecc."@it ,
                    "Text of the title of a project, research output, etc."@en ;
       rdfs:isDefinedBy <https://w3id.org/italia/onto/HER> ;
       rdfs:label "title"@en ,
                  "titolo"@it ;
       owl:versionInfo "stabile"@it ,
                       "stable"@en .


###  https://w3id.org/italia/onto/HER/total
:total rdf:type owl:DatatypeProperty ;
       rdfs:subPropertyOf <https://w3id.org/italia/onto/MU/value> ;
       rdfs:domain [ rdf:type owl:Class ;
                     owl:unionOf ( :DSUCanteenAndAccomodationsAggregate
                                   :USTATMealsProvidedAggregate
                                   :USTATPermanentStaff
                                   :USTATTemporaryStaff
                                   :USTATUniversityFacilitiesAggregate
                                 )
                   ] ;
       rdfs:comment "L'intero numero o importo."@it ,
                    "The whole number or amount."@en ;
       rdfs:isDefinedBy <https://w3id.org/italia/onto/HER> ;
       rdfs:label "total"@en ,
                  "totale"@it .


###  https://w3id.org/italia/onto/HER/totalDegree
:totalDegree rdf:type owl:DatatypeProperty ;
             rdfs:subPropertyOf <https://w3id.org/italia/onto/MU/value> ;
             rdfs:domain [ rdf:type owl:Class ;
                           owl:unionOf ( :DSURightToUniversityStudiesAggregate
                                         :USTATContributionByClass
                                         :USTATEnrolledStudentsAggregate
                                         :USTATInterventionExpensesAggregate
                                         :USTATInterventionsForStudentsByUniversitiesAggregate
                                         :USTATPartiallyExoneratedStudentsAggregate
                                         :USTATTotallyExoneratedStudentsAggregate
                                       )
                         ] ;
             rdfs:range rdfs:Literal ;
             rdfs:comment "Total with respect to undergraduate students: in this case, undergraduate students are considered to be students in good standing with the payment of tuition fees enrolled in undergraduate courses, master's degree courses, courses of the old system."@en ,
                          "Totale rispetto agli studenti di laurea: in questo caso, vengono considerati studenti di laurea gli studenti in regola con il pagamento delle tasse universitarie iscritti a corsi di laurea, corsi di laurea magistrale, corsi del vecchio ordinamento."@it ;
             rdfs:isDefinedBy <https://w3id.org/italia/onto/HER> ;
             rdfs:label "total degree"@en ,
                        "totale lauree"@it .


###  https://w3id.org/italia/onto/HER/totalDegreeExtraEU
:totalDegreeExtraEU rdf:type owl:DatatypeProperty ;
                    rdfs:subPropertyOf <https://w3id.org/italia/onto/MU/value> ;
                    rdfs:domain [ rdf:type owl:Class ;
                                  owl:unionOf ( :DSURightToUniversityStudiesAggregate
                                                :USTATInterventionsForStudentsByUniversitiesAggregate
                                              )
                                ] ;
                    rdfs:range rdfs:Literal ;
                    rdfs:comment "Total with respect to students from outside the European Union who are beneficiaries of interventions enrolled in degree courses, master's degree courses, courses of the old system. Students in good standing with the payment of tuition fees are considered."@en ,
                                 "Totale rispetto agli studenti di nazionalità extra Unione Europea beneficiari di interventi iscritti a corsi di laurea, corsi di laurea magistrale, corsi del vecchio ordinamento. Vengono considerati gli studenti in regola con il pagamento delle tasse universitarie."@it ;
                    rdfs:isDefinedBy <https://w3id.org/italia/onto/HER> ;
                    rdfs:label "total degree extra-EU"@en ,
                               "totale lauree extra-UE"@it .


###  https://w3id.org/italia/onto/HER/totalDoctorate
:totalDoctorate rdf:type owl:DatatypeProperty ;
                rdfs:subPropertyOf <https://w3id.org/italia/onto/MU/value> ;
                rdfs:domain [ rdf:type owl:Class ;
                              owl:unionOf ( :DSURightToUniversityStudiesAggregate
                                            :USTATContributionByClass
                                            :USTATEnrolledStudentsAggregate
                                            :USTATInterventionExpensesAggregate
                                            :USTATInterventionsForStudentsByUniversitiesAggregate
                                            :USTATPartiallyExoneratedStudentsAggregate
                                            :USTATTotallyExoneratedStudentsAggregate
                                          )
                            ] ;
                rdfs:range rdfs:Literal ;
                rdfs:comment "Total with respect to students enrolled in PhD courses."@en ,
                             "Totale rispetto agli iscritti a corsi di dottorato di ricerca."@it ;
                rdfs:isDefinedBy <https://w3id.org/italia/onto/HER> ;
                rdfs:label "total doctorate"@en ,
                           "totali dottorati"@it .


###  https://w3id.org/italia/onto/HER/totalEnrolledStudents
:totalEnrolledStudents rdf:type owl:DatatypeProperty ;
                       rdfs:subPropertyOf <https://w3id.org/italia/onto/MU/value> ;
                       rdfs:isDefinedBy <https://w3id.org/italia/onto/HER> ;
                       rdfs:label "total enrolled students"@en ,
                                  "totale di studenti iscritti"@it .


###  https://w3id.org/italia/onto/HER/totalExpense
:totalExpense rdf:type owl:DatatypeProperty ;
              rdfs:subPropertyOf <https://w3id.org/italia/onto/MU/value> ;
              rdfs:domain :USTATUniversityInterventionExpensesAggregate ;
              rdfs:comment "Amount of total expenditure. The values are expressed in EURO. The data relate to the financial year per year (T-1)."@en ,
                           "Importo della spesa totale. I valori sono espressi in EURO. I dati sono relativi all'esercizio finanziario all'anno (T-1)."@it ;
              rdfs:isDefinedBy <https://w3id.org/italia/onto/HER> ;
              rdfs:label "spese totali"@it ,
                         "total expense"@en .


###  https://w3id.org/italia/onto/HER/totalFemale
:totalFemale rdf:type owl:DatatypeProperty ;
             rdfs:subPropertyOf <https://w3id.org/italia/onto/MU/value> ;
             rdfs:domain [ rdf:type owl:Class ;
                           owl:unionOf ( :USTATPostgraduateAggregateOfEnrolled
                                         :USTATPostgraduateAggregateOfGraduated
                                         :USTATPostgraduateAggregateOfRegistered
                                         :USTATStaffByGender
                                         :USTATTAStaffByGender
                                       )
                         ] ;
             rdfs:comment "Total with respect to the female population of the sample considered."@en ,
                          "Totale rispetto alla popolazione di sesso femminile del campione considerato."@it ;
             rdfs:isDefinedBy <https://w3id.org/italia/onto/HER> ;
             rdfs:label "total female"@en ,
                        "totale genere femminile"@it .


###  https://w3id.org/italia/onto/HER/totalFemaleDoctorateGraduated
:totalFemaleDoctorateGraduated rdf:type owl:DatatypeProperty ;
                               rdfs:subPropertyOf <https://w3id.org/italia/onto/MU/value> ;
                               rdfs:domain :USTATStudentsBySexAggregate ;
                               rdfs:comment "Information on women PhDs, disaggregated by gender, university, geographical area, course type and field of education and training (ISCED-F 2013). Data available as of calendar year 2012."@en ,
                                            "Informazioni sui dottori di ricerca di genere femminile, disaggregate per genere, ateneo, area geografica, tipo di corso e field of education and training (ISCED-F 2013). Dati disponibili a partire dall’anno solare 2012."@it ;
                               rdfs:isDefinedBy <https://w3id.org/italia/onto/HER> ;
                               rdfs:label "total female doctorate graduated"@en ,
                                          "totale di laurati ad un dottorato di genere famminile"@it .


###  https://w3id.org/italia/onto/HER/totalFemaleDoctorateStudents
:totalFemaleDoctorateStudents rdf:type owl:DatatypeProperty ;
                              rdfs:subPropertyOf <https://w3id.org/italia/onto/MU/value> ;
                              rdfs:domain :USTATStudentsBySexAggregate ;
                              rdfs:comment """Information on women enrolled in PhD courses, broken down by gender, university, geographical area, course type and field of education and training (ISCED-F 2013). Data available from the academic year 2012/2013. Students at ISCED Level 8 2011.
From 2015-2016 onwards, data are collected by the National Register of Students and Graduates (ANS_PL), which could lead to a discontinuity in the historical series.
Elaborations on ANS-PL data extracted on 2/10/2019."""@en ,
                                           """Informazioni sulle donne iscritte ai corsi di dottorato, disaggregate per genere, ateneo, area geografica, tipo di corso e field of education and training (ISCED-F 2013). Dati disponibili a partire dall’anno accademico 2012/2013. Studenti del livello 8 della ISCED 2011.
A partire dall'a.a. 2015-2016 i dati sono rilevati dall'Anagrafe Nazionale degli Studenti e dei Laureati (ANS_PL), ciò potrebbe determinare una discontinuità nella serie storica.
Elaborazioni su dati ANS-PL estratti alla data del 2/10/2019."""@it ;
                              rdfs:isDefinedBy <https://w3id.org/italia/onto/HER> ;
                              rdfs:label "total female doctorate students"@en ,
                                         "totale degli studenti di dottorato di genere famminile"@it .


###  https://w3id.org/italia/onto/HER/totalFemaleEnrolled
:totalFemaleEnrolled rdf:type owl:DatatypeProperty ;
                     rdfs:subPropertyOf <https://w3id.org/italia/onto/MU/value> ;
                     rdfs:domain :USTATStudentsBySexAggregate ;
                     rdfs:comment "Number of registered female students corresponding to the selected combination of variables. In particular: number of female students who, with reference to a.a. (t) - (t+1), are enrolled on July 31st of the year (t+1). Notes: Students of levels 6 and 7 of ISCED 2011. For the year 2018-2019: elaborations on ANS data - extraction December 2019."@en ,
                                  "Numero di studentesse di genere femminile iscritte corrispondente alla combinazione di variabili selezionata. In particolare: numero di studentesse che, con riferimento all' a.a. (t) - (t+1), risultano iscritte alla data del 31 luglio dell'anno (t+1). Note: Studentesse dei livelli 6 e 7 della ISCED 2011. Per l'anno 2018-2019: elaborazioni su dati ANS - estrazione Dicembre 2019."@it ;
                     rdfs:isDefinedBy <https://w3id.org/italia/onto/HER> ;
                     rdfs:label "total female enrolled"@en ,
                                "totale di genere femminile iscritto"@it .


###  https://w3id.org/italia/onto/HER/totalFemaleGraduated
:totalFemaleGraduated rdf:type owl:DatatypeProperty ;
                      rdfs:subPropertyOf <https://w3id.org/italia/onto/MU/value> ;
                      rdfs:domain :USTATStudentsBySexAggregate ;
                      rdfs:comment """Number of female graduates corresponding to the selected combination of variables. In particular: Number of female students who graduated in the reference calendar year. Students of levels 6 and 7 of ISCED 2011.
For the year 2018: elaborations on ANS data - extraction December 2019."""@en ,
                                   "Numero di laureate di genere femminile corrispondente alla combinazione di variabili selezionata. In particolare: Numero di studentesse che si sono laureate nell’anno solare di riferimento. Studentesse dei livelli 6 e 7 della ISCED 2011. Per l'anno 2018: elaborazioni su dati ANS - estrazione Dicembre 2019."@it ;
                      rdfs:isDefinedBy <https://w3id.org/italia/onto/HER> ;
                      rdfs:label "total female graduated"@en ,
                                 "totale di genere femminile laureato"@it .


###  https://w3id.org/italia/onto/HER/totalForeignFemale
:totalForeignFemale rdf:type owl:DatatypeProperty ;
                    rdfs:subPropertyOf <https://w3id.org/italia/onto/MU/value> ;
                    rdfs:domain [ rdf:type owl:Class ;
                                  owl:unionOf ( :USTATPostgraduateAggregateOfEnrolled
                                                :USTATPostgraduateAggregateOfGraduated
                                                :USTATPostgraduateAggregateOfRegistered
                                              )
                                ] ;
                    rdfs:comment "Total with respect to the population of women with foreign citizenship of the sample considered."@en ,
                                 "Totale rispetto alla popolazione di sesso femminile e con cittadinanza straniera del campione considerato."@it ;
                    rdfs:isDefinedBy <https://w3id.org/italia/onto/HER> ;
                    rdfs:label "total foreign female"@en ,
                               "totale di genere femminile straniero"@it .


###  https://w3id.org/italia/onto/HER/totalForeignMale
:totalForeignMale rdf:type owl:DatatypeProperty ;
                  rdfs:subPropertyOf <https://w3id.org/italia/onto/MU/value> ;
                  rdfs:domain [ rdf:type owl:Class ;
                                owl:unionOf ( :USTATPostgraduateAggregateOfEnrolled
                                              :USTATPostgraduateAggregateOfGraduated
                                              :USTATPostgraduateAggregateOfRegistered
                                            )
                              ] ;
                  rdfs:comment "Total with respect to the population of men with foreign citizenship of the sample considered."@en ,
                               "Totale rispetto alla popolazione di sesso maschile e con cittadinanza straniera del campione considerato."@it ;
                  rdfs:isDefinedBy <https://w3id.org/italia/onto/HER> ;
                  rdfs:label "total foreign male"@en ,
                             "totale di genere maschile straniero"@it .


###  https://w3id.org/italia/onto/HER/totalGraduatedStudents
:totalGraduatedStudents rdf:type owl:DatatypeProperty ;
                        rdfs:subPropertyOf <https://w3id.org/italia/onto/MU/value> ;
                        rdfs:isDefinedBy <https://w3id.org/italia/onto/HER> .


###  https://w3id.org/italia/onto/HER/totalGrant
:totalGrant rdf:type owl:DatatypeProperty ;
            rdfs:subPropertyOf <https://w3id.org/italia/onto/MU/value> ;
            rdfs:domain [ rdf:type owl:Class ;
                          owl:unionOf ( :EUREKAProject
                                        :ErasmusPlusProject
                                      )
                        ] ;
            rdfs:comment "Project total grant"@en ,
                         "Totale contributo progetto"@it ;
            rdfs:isDefinedBy <https://w3id.org/italia/onto/HER> ;
            rdfs:label "total grant"@en ,
                       "totale contributo"@it .


###  https://w3id.org/italia/onto/HER/totalInvestment
:totalInvestment rdf:type owl:DatatypeProperty ;
                 rdfs:subPropertyOf <https://w3id.org/italia/onto/MU/value> ;
                 rdfs:domain :EUREKAProject ;
                 rdfs:comment "Project total investment"@en ,
                              "Totale investimento del progetto"@it ;
                 rdfs:isDefinedBy <https://w3id.org/italia/onto/HER> ;
                 rdfs:label "investimento totale"@it ,
                            "total investment"@en .


###  https://w3id.org/italia/onto/HER/totalMale
:totalMale rdf:type owl:DatatypeProperty ;
           rdfs:subPropertyOf <https://w3id.org/italia/onto/MU/value> ;
           rdfs:domain [ rdf:type owl:Class ;
                         owl:unionOf ( :USTATPostgraduateAggregateOfEnrolled
                                       :USTATPostgraduateAggregateOfGraduated
                                       :USTATPostgraduateAggregateOfRegistered
                                       :USTATStaffByGender
                                       :USTATTAStaffByGender
                                     )
                       ] ;
           rdfs:comment "Total with respect to the male population of the sample considered."@en ,
                        "Totale rispetto alla popolazione di sesso maschile del campione considerato."@it ;
           rdfs:isDefinedBy <https://w3id.org/italia/onto/HER> ;
           rdfs:label "total male"@en ,
                      "totale generemaschile"@it .


###  https://w3id.org/italia/onto/HER/totalMaleDoctorateGraduated
:totalMaleDoctorateGraduated rdf:type owl:DatatypeProperty ;
                             rdfs:subPropertyOf <https://w3id.org/italia/onto/MU/value> ;
                             rdfs:domain :USTATStudentsBySexAggregate ;
                             rdfs:comment "Information on men PhDs, disaggregated by gender, university, geographical area, course type and field of education and training (ISCED-F 2013). Data available as of calendar year 2012."@en ,
                                          "Informazioni sui dottori di ricerca di genere maschile, disaggregate per genere, ateneo, area geografica, tipo di corso e field of education and training (ISCED-F 2013). Dati disponibili a partire dall’anno solare 2012."@it ;
                             rdfs:isDefinedBy <https://w3id.org/italia/onto/HER> ;
                             rdfs:label "total male doctorate graduated"@en ,
                                        "totale di laurati ad un dottorato di genere maschile"@it .


###  https://w3id.org/italia/onto/HER/totalMaleDoctorateStudents
:totalMaleDoctorateStudents rdf:type owl:DatatypeProperty ;
                            rdfs:subPropertyOf <https://w3id.org/italia/onto/MU/value> ;
                            rdfs:domain :USTATStudentsBySexAggregate ;
                            rdfs:range rdfs:Literal ;
                            rdfs:comment """Information on men enrolled in PhD courses, broken down by gender, university, geographical area, course type and field of education and training (ISCED-F 2013). Data available from the academic year 2012/2013. Students at ISCED Level 8 2011.
From 2015-2016 onwards, data are collected by the National Register of Students and Graduates (ANS_PL), which could lead to a discontinuity in the historical series.
Elaborations on ANS-PL data extracted on 2/10/2019."""@en ,
                                         """Informazioni sugli uomini iscritti ai corsi di dottorato, disaggregate per genere, ateneo, area geografica, tipo di corso e field of education and training (ISCED-F 2013). Dati disponibili a partire dall’anno accademico 2012/2013. Studenti del livello 8 della ISCED 2011.
A partire dall'a.a. 2015-2016 i dati sono rilevati dall'Anagrafe Nazionale degli Studenti e dei Laureati (ANS_PL), ciò potrebbe determinare una discontinuità nella serie storica. Elaborazioni su dati ANS-PL estratti alla data del 2/10/2019."""@it ;
                            rdfs:isDefinedBy <https://w3id.org/italia/onto/HER> ;
                            rdfs:label "total male doctorate students"@en ,
                                       "totale degli studenti di dottorato di genere maschile"@it .


###  https://w3id.org/italia/onto/HER/totalMaleEnrolled
:totalMaleEnrolled rdf:type owl:DatatypeProperty ;
                   rdfs:subPropertyOf <https://w3id.org/italia/onto/MU/value> ;
                   rdfs:domain :USTATStudentsBySexAggregate ;
                   rdfs:comment "Number of registered male students corresponding to the selected combination of variables. In particular: number of male students who, with reference to a.a. (t) - (t+1), are enrolled on July 31st of the year (t+1). Notes: Students of levels 6 and 7 of ISCED 2011. For the year 2018-2019: elaborations on ANS data - extraction December 2019."@en ,
                                "Numero di studenti di genere maschile iscritti, corrispondente alla combinazione di variabili selezionata. In particolare: numero di studenti di genere maschile che, con riferimento all' a.a. (t) - (t+1), risultano iscritti alla data del 31 luglio dell'anno (t+1). Note: Studenti dei livelli 6 e 7 della ISCED 2011. Per l'anno 2018-2019: elaborazioni su dati ANS - estrazione Dicembre 2019."@it ;
                   rdfs:isDefinedBy <https://w3id.org/italia/onto/HER> ;
                   rdfs:label "total male enrolled"@en ,
                              "totale di generemaschile iscritto"@it .


###  https://w3id.org/italia/onto/HER/totalMaleGraduated
:totalMaleGraduated rdf:type owl:DatatypeProperty ;
                    rdfs:subPropertyOf <https://w3id.org/italia/onto/MU/value> ;
                    rdfs:domain :USTATStudentsBySexAggregate ;
                    rdfs:comment """Number of male graduates corresponding to the selected combination of variables. In particular: Number of male students who graduated in the reference calendar year. Students of levels 6 and 7 of ISCED 2011.
For the year 2018: elaborations on ANS data - extraction December 2019."""@en ,
                                 """Numero di laureati di genere maschile corrispondente alla combinazione di variabili selezionata. In particolare: Numero di studenti di genere maschile che si sono laureati nell’anno solare di riferimento. Studenti dei livelli 6 e 7 della ISCED 2011.
Per l'anno 2018: elaborazioni su dati ANS - estrazione Dicembre 2019."""@it ;
                    rdfs:isDefinedBy <https://w3id.org/italia/onto/HER> ;
                    rdfs:label "total male graduated"@en ,
                               "totale di genere maschile laureato"@it .


###  https://w3id.org/italia/onto/HER/totalMaster
:totalMaster rdf:type owl:DatatypeProperty ;
             rdfs:subPropertyOf <https://w3id.org/italia/onto/MU/value> ;
             rdfs:domain [ rdf:type owl:Class ;
                           owl:unionOf ( :USTATContributionByClass
                                         :USTATEnrolledStudentsAggregate
                                         :USTATInterventionsForStudentsByUniversitiesAggregate
                                         :USTATPartiallyExoneratedStudentsAggregate
                                         :USTATTotallyExoneratedStudentsAggregate
                                       )
                         ] ;
             rdfs:comment "Total with respect to students in good standing with the payment of tuition fees enrolled in Level I and Level II master's courses."@en ,
                          "Totale rispetto agli studenti in regola con il pagamento delle tasse universitarie iscritti a corsi di master di I e II livello."@it ;
             rdfs:isDefinedBy <https://w3id.org/italia/onto/HER> ;
             rdfs:label "total master"@en ,
                        "totale lauree magistrali"@it .


###  https://w3id.org/italia/onto/HER/totalPerfectioningMaster
:totalPerfectioningMaster rdf:type owl:DatatypeProperty ;
                          rdfs:subPropertyOf <https://w3id.org/italia/onto/MU/value> ;
                          rdfs:domain [ rdf:type owl:Class ;
                                        owl:unionOf ( :USTATContributionByClass
                                                      :USTATInterventionsForStudentsByUniversitiesAggregate
                                                      :USTATPartiallyExoneratedStudentsAggregate
                                                      :USTATTotallyExoneratedStudentsAggregate
                                                    )
                                      ] ;
                          rdfs:comment "Total with respect to students enrolled in 1st and 2nd level master's courses and perfectioning courses. Disaggregation criterion used for data from 2009 to 2013, both included."@en ,
                                       "Totale rispetto agli studenti iscritti a corsi di master di I e II livello e a corsi di perfezionamento. Criterio di disaggregazione utilizzato per dati dal 2009 al 2013, entrambi inclusi."@it ;
                          rdfs:isDefinedBy <https://w3id.org/italia/onto/HER> ;
                          rdfs:label "total perfectioning master"@en ,
                                     "totale corsi di perfezionamento"@it .


###  https://w3id.org/italia/onto/HER/totalRegisteredStudents
:totalRegisteredStudents rdf:type owl:DatatypeProperty ;
                         rdfs:subPropertyOf <https://w3id.org/italia/onto/MU/value> ;
                         rdfs:isDefinedBy <https://w3id.org/italia/onto/HER> .


###  https://w3id.org/italia/onto/HER/totalSpecialization
:totalSpecialization rdf:type owl:DatatypeProperty ;
                     rdfs:subPropertyOf <https://w3id.org/italia/onto/MU/value> ;
                     rdfs:domain [ rdf:type owl:Class ;
                                   owl:unionOf ( :DSURightToUniversityStudiesAggregate
                                                 :USTATContributionByClass
                                                 :USTATEnrolledStudentsAggregate
                                                 :USTATInterventionExpensesAggregate
                                                 :USTATInterventionsForStudentsByUniversitiesAggregate
                                                 :USTATPartiallyExoneratedStudentsAggregate
                                                 :USTATTotallyExoneratedStudentsAggregate
                                               )
                                 ] ;
                     rdfs:comment "Total with respect to students in good standing with the payment of tuition fees enrolled in specialized courses."@en ,
                                  "Totale rispetto agli studenti in regola con il pagamento delle tasse universitarie iscritti a corsi di specializzazione."@it ;
                     rdfs:isDefinedBy <https://w3id.org/italia/onto/HER> ;
                     rdfs:label "total specialization"@en ,
                                "totale specializzazioni"@it .


###  https://w3id.org/italia/onto/HER/transmissionDate
:transmissionDate rdf:type owl:DatatypeProperty ;
                  rdfs:subPropertyOf ti:date ;
                  rdfs:domain :CTNPRINOperation ;
                  rdfs:range xsd:date ;
                  rdfs:comment "Data di presentazione della proposta progettuale associata all'operazione"@it ,
                               "Date of submission of the project proposal associated with the operation"@en ;
                  rdfs:isDefinedBy <https://w3id.org/italia/onto/HER> ;
                  rdfs:label "data trasmissione"@it ,
                             "transmission date"@en ;
                  owl:versionInfo "stabile"@it ,
                                  "stable"@en .


###  https://w3id.org/italia/onto/HER/unicsId
:unicsId rdf:type owl:DatatypeProperty ;
         rdfs:subPropertyOf l0:identifier ;
         rdfs:domain [ rdf:type owl:Class ;
                       owl:unionOf ( :ECParticipant
                                     :ECProject
                                     :ERCProject
                                     :EUREKAProject
                                   )
                     ] ;
         rdfs:range rdfs:Literal ;
         rdfs:comment "Identificativo all'interno della piattaforma UNiCS"@it ,
                      "Identifier in the UNiCS platform."@en ;
         rdfs:isDefinedBy <https://w3id.org/italia/onto/HER> ;
         rdfs:label "identificativo in unics"@it ,
                    "unics identifier"@en ;
         owl:versionInfo "stabile"@it ,
                         "stable"@en .


###  https://w3id.org/italia/onto/HER/ustatCourseType
:ustatCourseType rdf:type owl:DatatypeProperty ;
                 rdfs:domain :USTATReportedPostgraduateCourse ;
                 rdfs:range rdfs:Literal ;
                 rdfs:comment "Name of the postgraduate education course; in this dataset, it can be referred to Postgraduate Schools/Level I Masters/Level II Masters/Research Doctorates."@en ,
                              "Nome del corso di studio di formazione Post-Laurea; in questo dataset, si può riferire a Scuole di specializzazione/Master di I livello/Master di II livello/Dottorati di ricerca."@it ;
                 rdfs:isDefinedBy <https://w3id.org/italia/onto/HER> ;
                 rdfs:label "course type"@en ,
                            "tipologia di corso"@it .


###  https://w3id.org/italia/onto/HER/verificationDate
:verificationDate rdf:type owl:DatatypeProperty ;
                  rdfs:subPropertyOf ti:date ;
                  rdfs:domain :AACTStudy ;
                  rdfs:range xsd:date ;
                  rdfs:comment "Numero totale di partecipanti allo studio"@it ,
                               "The date the study was last verified in a date-type format so that it can be used to find studies before/after/inclusive of a date or dates. For studies that only provide month/year, the last day of the month is used."@en ;
                  rdfs:isDefinedBy <https://w3id.org/italia/onto/HER> ;
                  rdfs:label "data verifica"@it ,
                             "verification date"@en ;
                  owl:versionInfo "stabile"@it ,
                                  "stable"@en .


###  https://w3id.org/italia/onto/HER/verificationMonthYear
:verificationMonthYear rdf:type owl:DatatypeProperty ;
                       rdfs:subPropertyOf ti:year ;
                       rdfs:domain :AACTStudy ;
                       rdfs:range xsd:gYear ;
                       rdfs:comment "La data in cui lo studio è stato verificato per l'ultima volta in un formato di tipo data, in modo da poterlo utilizzare per trovare gli studi prima/dopo/conclusiva di una o più date. Per gli studi che forniscono solo mese/anno, viene utilizzato l'ultimo giorno del mese."@it ,
                                    "The date the study was last verified in a date-type format so that it can be used to find studies before/after/inclusive of a date or dates. For studies that only provide month/year, the last day of the month is used."@en ;
                       rdfs:isDefinedBy <https://w3id.org/italia/onto/HER> ;
                       rdfs:label "mese-anno di verifica"@it ,
                                  "verification month-year"@en .


###  https://w3id.org/italia/onto/HER/whyStopped
:whyStopped rdf:type owl:DatatypeProperty ;
            rdfs:domain :AACTStudy ;
            rdfs:range rdfs:Literal ;
            rdfs:comment "A brief explanation of the reason(s) why such clinical study was stopped (for a clinical study that is \"Suspended,\" \"Terminated,\" or \"Withdrawn\" prior to its planned completion as anticipated by the protocol)."@en ,
                         "Una breve spiegazione delle ragioni per cui tale studio clinico è stato interrotto (per uno studio clinico \"Sospeso\", \"Terminato\" o \"Ritirato\" prima del suo completamento previsto, come previsto dal protocollo)."@it ;
            rdfs:isDefinedBy <https://w3id.org/italia/onto/HER> ;
            rdfs:label "perchè bloccato"@it ,
                       "why stopped"@en ;
            owl:versionInfo "stabile"@it ,
                            "stable"@en .


###  https://w3id.org/italia/onto/Project/anticipatedCompletionDate
<https://w3id.org/italia/onto/Project/anticipatedCompletionDate> rdf:type owl:DatatypeProperty ;
                                                                 rdfs:subPropertyOf ti:date ;
                                                                 rdfs:domain :AACTStudy ;
                                                                 rdfs:range xsd:date ;
                                                                 rdfs:comment "La data prevista di completamento dello studio AACT."@it ,
                                                                              "The date estimated for the completion of the AACT study."@en ;
                                                                 rdfs:isDefinedBy <https://w3id.org/italia/onto/HER> ;
                                                                 rdfs:label "data prevista completamento"@it ,
                                                                            "estimated completion date"@en ;
                                                                 owl:versionInfo "provvisoria"@it ,
                                                                                 "unstable"@en .


###  https://w3id.org/italia/onto/Project/projectAcronym
<https://w3id.org/italia/onto/Project/projectAcronym> rdf:type owl:DatatypeProperty ;
                                                      rdfs:label "acronimo di project"@it ,
                                                                 "acronym of project"@en .


###  https://w3id.org/italia/onto/SM/URL
<https://w3id.org/italia/onto/SM/URL> rdf:type owl:DatatypeProperty .


#################################################################
#    Classes
#################################################################

###  https://w3id.org/italia/onto/COV/Employment
covapit:Employment rdf:type owl:Class .


###  https://w3id.org/italia/onto/COV/Group
covapit:Group rdf:type owl:Class .


###  https://w3id.org/italia/onto/COV/Office
covapit:Office rdf:type owl:Class .


###  https://w3id.org/italia/onto/COV/PrivateOrganization
covapit:PrivateOrganization rdf:type owl:Class .


###  https://w3id.org/italia/onto/COV/PublicOrganization
covapit:PublicOrganization rdf:type owl:Class .


###  https://w3id.org/italia/onto/COV/SupportUnit
covapit:SupportUnit rdf:type owl:Class .


###  https://w3id.org/italia/onto/CPV/Person
<https://w3id.org/italia/onto/CPV/Person> rdf:type owl:Class ;
                                          rdfs:subClassOf [ rdf:type owl:Restriction ;
                                                            owl:onProperty :birthyear ;
                                                            owl:maxQualifiedCardinality "1"^^xsd:nonNegativeInteger ;
                                                            owl:onDataRange xsd:gYear
                                                          ] .


###  https://w3id.org/italia/onto/CPV/Sex
<https://w3id.org/italia/onto/CPV/Sex> rdf:type owl:Class .


###  https://w3id.org/italia/onto/HER/AACTCondition
:AACTCondition rdf:type owl:Class ;
               rdfs:subClassOf l0:Characteristic ;
               rdfs:comment "La malattia, il disturbo, la sindrome, o la lesione che si sta studiando. Su ClinicalTrials.gov, le condizioni possono includere anche altre questioni relative alla salute, come la durata della vita, la qualità della vita e i rischi per la salute. Il nome della condizione può includere lettere maiuscolo o minuscole."@it ,
                            "The disease, disorder, syndrome, illness, or injury that is being studied. On ClinicalTrials.gov, conditions may also include other health-related issues, such as lifespan, quality of life, and health risks. The name of the condition may include upper or lower case letters."@en ;
               rdfs:isDefinedBy <https://w3id.org/italia/onto/HER> ;
               rdfs:label "Condition"@en ,
                          "Condizione"@it .


###  https://w3id.org/italia/onto/HER/AACTConditionMeshTerm
:AACTConditionMeshTerm rdf:type owl:Class ;
                       rdfs:subClassOf :AACTMeshTerm ;
                       rdfs:comment """I nomi della malattia o delle condizioni studiate nello studio clinico, o il focus dello studio clinico. I dati vengono descritti da NLM (Medical Subject Headings - MeSH) - thesaurus del vocabolario controllato o termini da un altro vocabolario, come la Nomenclatura sistematica dei termini medico-clinici (SNOMED CT), che è stato mappato al MeSH all'interno del Metathesaurus Unified Medical Language System (UMLS).

Tradotto con www.DeepL.com/Translator (versione gratuita)"""@it ,
                                    "The name(s) of the disease(s) or condition(s) studied in the clinical study, or the focus of the clinical study appropriate descriptors from NLM's Medical Subject Headings (MeSH)-controlled vocabulary thesaurus or terms from another vocabulary, such as the Systematized Nomenclature of Medicine—Clinical Terms (SNOMED CT), that has been mapped to MeSH within the Unified Medical Language System (UMLS) Metathesaurus."@en ;
                       rdfs:isDefinedBy <https://w3id.org/italia/onto/HER> ;
                       rdfs:label "Condition Mesh Term"@en ,
                                  "Termine MeSH di Condizione"@it .


###  https://w3id.org/italia/onto/HER/AACTDesign
:AACTDesign rdf:type owl:Class ;
            rdfs:subClassOf l0:Description ,
                            [ rdf:type owl:Restriction ;
                              owl:onProperty l0:description ;
                              owl:someValuesFrom rdfs:Literal
                            ] ,
                            [ rdf:type owl:Restriction ;
                              owl:onProperty :allocation ;
                              owl:maxCardinality "1"^^xsd:nonNegativeInteger
                            ] ;
            rdfs:comment "I metodi di indagine e le strategie utilizzate nello studio clinico. Una descrizione delle modalità di conduzione dello studio clinico"@it ,
                         "The investigative methods and strategies used in the clinical study. A description of the manner in which the clinical trial will be conducted"@en ;
            rdfs:isDefinedBy <https://w3id.org/italia/onto/HER> ;
            rdfs:label "AACT Design"@en ,
                       "Progettazione AACT"@it ;
            owl:versionInfo "stabile"@it ,
                            "stable"@en .


###  https://w3id.org/italia/onto/HER/AACTEligibility
:AACTEligibility rdf:type owl:Class ;
                 rdfs:subClassOf l0:Characteristic ,
                                 [ rdf:type owl:Restriction ;
                                   owl:onProperty :aactCriterion ;
                                   owl:someValuesFrom rdfs:Literal
                                 ] ,
                                 [ rdf:type owl:Restriction ;
                                   owl:onProperty :aactPopulation ;
                                   owl:allValuesFrom rdfs:Literal
                                 ] ,
                                 [ rdf:type owl:Restriction ;
                                   owl:onProperty :aactEligibleSex ;
                                   owl:maxCardinality "1"^^xsd:nonNegativeInteger
                                 ] ,
                                 [ rdf:type owl:Restriction ;
                                   owl:onProperty :aactMaximumAge ;
                                   owl:maxQualifiedCardinality "1"^^xsd:nonNegativeInteger ;
                                   owl:onDataRange xsd:integer
                                 ] ,
                                 [ rdf:type owl:Restriction ;
                                   owl:onProperty :aactMinimumAge ;
                                   owl:maxQualifiedCardinality "1"^^xsd:nonNegativeInteger ;
                                   owl:onDataRange xsd:integer
                                 ] ;
                 rdfs:comment "I requisiti chiave che le persone che vogliono partecipare a uno studio clinico devono soddisfare o le caratteristiche che devono avere."@it ,
                              "The key requirements that people who want to participate in a clinical study must meet or the characteristics they must have."@en ;
                 rdfs:isDefinedBy <https://w3id.org/italia/onto/HER> ;
                 rdfs:label "Eligibility"@en ,
                            "Idoneitá"@it .


###  https://w3id.org/italia/onto/HER/AACTFacility
:AACTFacility rdf:type owl:Class ;
              rdfs:subClassOf <https://w3id.org/italia/onto/CLV/SpatialObject> ,
                              [ rdf:type owl:Restriction ;
                                owl:onProperty covapit:hasOrganization ;
                                owl:someValuesFrom covapit:Organization
                              ] ;
              rdfs:comment "conduzione del sito/partecipazione ad uno studio"@it ,
                           "site conducting/participating in a study"@en ;
              rdfs:isDefinedBy <https://w3id.org/italia/onto/HER> ;
              rdfs:label "Facility of Clinical Trial"@en ,
                         "Struttura di sperimentazione clinica"@it .


###  https://w3id.org/italia/onto/HER/AACTIntervention
:AACTIntervention rdf:type owl:Class ;
                  rdfs:subClassOf l0:Activity ;
                  rdfs:comment "A process or action that is the focus of a clinical study. Interventions include drugs, medical devices, procedures, vaccines, and other products that are either investigational or already available. Interventions can also include noninvasive approaches, such as education or modifying diet and exercise."@en ,
                               "Un processo o un'azione che è il fulcro di uno studio clinico. Gli interventi comprendono farmaci, dispositivi medici, procedure, vaccini e altri prodotti che sono in fase di sperimentazione o già disponibili. Gli interventi possono anche includere approcci non invasivi, come l'educazione o la modifica della dieta e dell'esercizio fisico."@it ;
                  rdfs:isDefinedBy <https://w3id.org/italia/onto/HER> ;
                  rdfs:label "AACT Intervention"@en ,
                             "Intervento AACT"@it .


###  https://w3id.org/italia/onto/HER/AACTInterventionMeshTerm
:AACTInterventionMeshTerm rdf:type owl:Class ;
                          rdfs:subClassOf :AACTMeshTerm ;
                          rdfs:comment "Interventi di studio clinico documentati da NLM's Medical Subject Headings (MeSH) - thesaurus del vocabolario controllato da NLM's Medical Subject Headings (MeSH)"@it ,
                                       "clinical study intervention appropriate descriptors from NLM's Medical Subject Headings (MeSH)-controlled vocabulary thesaurus"@en ;
                          rdfs:isDefinedBy <https://w3id.org/italia/onto/HER> ;
                          rdfs:label "AACT Intervention Mesh Term"@en ,
                                     "Termine MeSH di Intervento AACT"@it .


###  https://w3id.org/italia/onto/HER/AACTMeshTerm
:AACTMeshTerm rdf:type owl:Class ;
              rdfs:subClassOf l0:Concept ,
                              [ rdf:type owl:Restriction ;
                                owl:onProperty l0:identifier ;
                                owl:allValuesFrom rdfs:Literal
                              ] ,
                              [ rdf:type owl:Restriction ;
                                owl:onProperty l0:name ;
                                owl:allValuesFrom rdfs:Literal
                              ] ;
              rdfs:comment "descriptors from NLM's Medical Subject Headings (MeSH)-controlled vocabulary thesaurus"@en ,
                           "descrittori del thesaurus del vocabolario controllato dalla NLM \"Medical Subject Headings (MeSH)\" (MeSH)"@it ;
              rdfs:isDefinedBy <https://w3id.org/italia/onto/HER> ;
              rdfs:label "Condition/Intervention Mesh Term"@en ,
                         "Termine Mesh di Condizione/Interventi"@it ;
              prov:wasDerivedFrom skos:Concept .


###  https://w3id.org/italia/onto/HER/AACTResponsibleParty
:AACTResponsibleParty rdf:type owl:Class ;
                      rdfs:subClassOf <https://w3id.org/italia/onto/CPV/Person> ;
                      rdfs:comment "La persona responsabile dell'invio di informazioni su uno studio clinico a ClinicalTrials.gov e dell'aggiornamento di tali informazioni. Di solito lo sponsor dello studio o lo sperimentatore."@it ,
                                   "The person responsible for submitting information about a clinical study to ClinicalTrials.gov and updating that information. Usually the study sponsor or investigator."@en ;
                      rdfs:isDefinedBy <https://w3id.org/italia/onto/HER> ;
                      rdfs:label "Responsible Party"@en ,
                                 "parte responsabile"@it .


###  https://w3id.org/italia/onto/HER/AACTSponsor
:AACTSponsor rdf:type owl:Class ;
             rdfs:subClassOf covapit:PrivateOrganization ,
                             [ rdf:type owl:Restriction ;
                               owl:onProperty :sponsorType ;
                               owl:maxCardinality "1"^^xsd:nonNegativeInteger
                             ] ;
             rdfs:comment "L'organizzazione o la persona che avvia lo studio e che ha autorità e controllo sullo studio."@it ,
                          "The organization or person who initiates the study and who has authority and control over the study."@en ;
             rdfs:isDefinedBy <https://w3id.org/italia/onto/HER> ;
             rdfs:label "Sponsor"@en ,
                        "sponsor"@it .


###  https://w3id.org/italia/onto/HER/AACTStudy
:AACTStudy rdf:type owl:Class ;
           rdfs:subClassOf l0:Activity ,
                           [ rdf:type owl:Restriction ;
                             owl:onProperty :hasCountryInvolvement ;
                             owl:someValuesFrom :CountryInvolvement
                           ] ,
                           [ rdf:type owl:Restriction ;
                             owl:onProperty :biospecDescription ;
                             owl:someValuesFrom rdfs:Literal
                           ] ,
                           [ rdf:type owl:Restriction ;
                             owl:onProperty :title ;
                             owl:someValuesFrom rdfs:Literal
                           ] ,
                           [ rdf:type owl:Restriction ;
                             owl:onProperty :whyStopped ;
                             owl:allValuesFrom rdfs:Literal
                           ] ,
                           [ rdf:type owl:Restriction ;
                             owl:onProperty :studyFirstPostedDate ;
                             owl:qualifiedCardinality "1"^^xsd:nonNegativeInteger ;
                             owl:onDataRange xsd:date
                           ] ,
                           [ rdf:type owl:Restriction ;
                             owl:onProperty :studyFirstSubmittedDate ;
                             owl:qualifiedCardinality "1"^^xsd:nonNegativeInteger ;
                             owl:onDataRange xsd:date
                           ] ,
                           [ rdf:type owl:Restriction ;
                             owl:onProperty :actualCompletionDate ;
                             owl:maxQualifiedCardinality "1"^^xsd:nonNegativeInteger ;
                             owl:onDataRange xsd:date
                           ] ,
                           [ rdf:type owl:Restriction ;
                             owl:onProperty :biospecRetention ;
                             owl:maxCardinality "1"^^xsd:nonNegativeInteger
                           ] ,
                           [ rdf:type owl:Restriction ;
                             owl:onProperty :dispositionFirstPostedDate ;
                             owl:maxQualifiedCardinality "1"^^xsd:nonNegativeInteger ;
                             owl:onDataRange xsd:date
                           ] ,
                           [ rdf:type owl:Restriction ;
                             owl:onProperty :dispositionFirstSubmittedDate ;
                             owl:maxQualifiedCardinality "1"^^xsd:nonNegativeInteger ;
                             owl:onDataRange xsd:date
                           ] ,
                           [ rdf:type owl:Restriction ;
                             owl:onProperty :dispositionFirstSubmittedQCDate ;
                             owl:maxQualifiedCardinality "1"^^xsd:nonNegativeInteger ;
                             owl:onDataRange xsd:date
                           ] ,
                           [ rdf:type owl:Restriction ;
                             owl:onProperty :ipdURL ;
                             owl:maxQualifiedCardinality "1"^^xsd:nonNegativeInteger ;
                             owl:onDataRange xsd:anyURI
                           ] ,
                           [ rdf:type owl:Restriction ;
                             owl:onProperty :isFDARegulatedDevice ;
                             owl:maxQualifiedCardinality "1"^^xsd:nonNegativeInteger ;
                             owl:onDataRange xsd:boolean
                           ] ,
                           [ rdf:type owl:Restriction ;
                             owl:onProperty :primaryCompletionDate ;
                             owl:maxQualifiedCardinality "1"^^xsd:nonNegativeInteger ;
                             owl:onDataRange xsd:date
                           ] ,
                           [ rdf:type owl:Restriction ;
                             owl:onProperty :resultsFirstPostedDate ;
                             owl:maxQualifiedCardinality "1"^^xsd:nonNegativeInteger ;
                             owl:onDataRange xsd:date
                           ] ,
                           [ rdf:type owl:Restriction ;
                             owl:onProperty :resultsFirstSubmittedDate ;
                             owl:maxQualifiedCardinality "1"^^xsd:nonNegativeInteger ;
                             owl:onDataRange xsd:date
                           ] ,
                           [ rdf:type owl:Restriction ;
                             owl:onProperty :resultsFirstSubmittedQCDate ;
                             owl:maxQualifiedCardinality "1"^^xsd:nonNegativeInteger ;
                             owl:onDataRange xsd:date
                           ] ,
                           [ rdf:type owl:Restriction ;
                             owl:onProperty :startingDate ;
                             owl:maxQualifiedCardinality "1"^^xsd:nonNegativeInteger ;
                             owl:onDataRange xsd:date
                           ] ,
                           [ rdf:type owl:Restriction ;
                             owl:onProperty :studyFirstSubmittedQCDate ;
                             owl:maxQualifiedCardinality "1"^^xsd:nonNegativeInteger ;
                             owl:onDataRange xsd:date
                           ] ,
                           [ rdf:type owl:Restriction ;
                             owl:onProperty :verificationDate ;
                             owl:maxQualifiedCardinality "1"^^xsd:nonNegativeInteger ;
                             owl:onDataRange xsd:date
                           ] ,
                           [ rdf:type owl:Restriction ;
                             owl:onProperty <https://w3id.org/italia/onto/Project/anticipatedCompletionDate> ;
                             owl:maxQualifiedCardinality "1"^^xsd:nonNegativeInteger ;
                             owl:onDataRange xsd:date
                           ] ,
                           [ rdf:type owl:Restriction ;
                             owl:onProperty <https://w3id.org/italia/onto/Project/projectAcronym> ;
                             owl:maxCardinality "1"^^xsd:nonNegativeInteger
                           ] ;
           rdfs:comment "Studio clinico"@it ,
                        "clinical study"@en ;
           rdfs:isDefinedBy <https://w3id.org/italia/onto/HER> ;
           rdfs:label "Studio"@it ,
                      "Study"@en .


###  https://w3id.org/italia/onto/HER/ASJC
:ASJC rdf:type owl:Class ;
      rdfs:subClassOf :HERClassification ;
      rdfs:isDefinedBy <https://w3id.org/italia/onto/HER> ;
      rdfs:label "All Science Journal Classification"@en ,
                 "Classificazione  Scopus"@it ,
                 "Scopus Classification"@en ;
      prov:wasDerivedFrom skos:ConceptScheme ;
      l0:controlledVocabulary <https://w3id.org/italia/controlled-vocabulary/classifications-for-universities/all-science-journal> .


###  https://w3id.org/italia/onto/HER/ASJCField
:ASJCField rdf:type owl:Class ;
           rdfs:subClassOf :ASJC ;
           rdfs:comment "Journals are assigned to 27 major thematic categories as well as to 313 specific subject categories according to Scopus® Classification."@en ;
           rdfs:isDefinedBy <https://w3id.org/italia/onto/HER> ;
           prov:wasDerivedFrom skos:Concept ;
           l0:controlledVocabulary <https://w3id.org/italia/controlled-vocabulary/classifications-for-universities/all-science-journal> .


###  https://w3id.org/italia/onto/HER/ASJCSubjectArea
:ASJCSubjectArea rdf:type owl:Class ;
                 rdfs:subClassOf :ASJC ;
                 rdfs:comment """The SCOPUS classification scheme contains 27 subject areas: Agricultural and Biological Sciences; Arts and Humanities; Biochemistry; Genetics and Molecular Biology; Business; Management and Accounting; Chemical Engineering; Chemistry; Computer Science; Decision Sciences; Dentistry; Earth and Planetary Science; Economics; Econometrics and Finance; Energy
Engineering; Environmental Science; Health Professions; Immunology and Microbiology; Materials Science; Mathematics; Medicine; Multidisciplinary; Neuroscience; Nursing; Pharmacology, Toxicology and Pharmaceutics; Physics and Astronomy; Psychology; Social Sciences; Veterinary

Attributes:
:name
:scopusSubjectAreaCode"""@en ;
                 rdfs:isDefinedBy <https://w3id.org/italia/onto/HER> ;
                 prov:wasDerivedFrom skos:Concept ;
                 l0:controlledVocabulary <https://w3id.org/italia/controlled-vocabulary/classifications-for-universities/all-science-journal> .


###  https://w3id.org/italia/onto/HER/ASJCSupergroup
:ASJCSupergroup rdf:type owl:Class ;
                rdfs:subClassOf :ASJC ;
                rdfs:isDefinedBy <https://w3id.org/italia/onto/HER> ;
                prov:wasDerivedFrom skos:Concept ;
                l0:controlledVocabulary <https://w3id.org/italia/controlled-vocabulary/classifications-for-universities/all-science-journal> .


###  https://w3id.org/italia/onto/HER/AcademicAffiliation
:AcademicAffiliation rdf:type owl:Class ;
                     rdfs:subClassOf covapit:Employment ;
                     rdfs:comment "Rappresenta l'affiliazione di una persona a un'organizzazione con un determinato ruolo per un periodo di tempo."@it ,
                                  "Represents the affiliation of a person to an organization with a certain role for a period of time."@en ;
                     rdfs:isDefinedBy <https://w3id.org/italia/onto/HER> ;
                     rdfs:label "Academic Affiliation"@en ,
                                "Affilizazione accademica"@it .


###  https://w3id.org/italia/onto/HER/AcademicDegree
:AcademicDegree rdf:type owl:Class ;
                rdfs:subClassOf l0:Object ,
                                [ rdf:type owl:Restriction ;
                                  owl:onProperty l0:name ;
                                  owl:someValuesFrom xsd:boolean
                                ] ;
                rdfs:comment "Il principale titolo accademico post-secondario in Italia."@it ,
                             "The main post-secondary academic degree in Italy."@en ;
                rdfs:isDefinedBy <https://w3id.org/italia/onto/HER> ;
                rdfs:label "Academic Degree"@en ,
                           "Laurea"@it .


###  https://w3id.org/italia/onto/HER/AcademicDiscipline
:AcademicDiscipline rdf:type owl:Class ;
                    rdfs:subClassOf :HERClassification ,
                                    [ rdf:type owl:Restriction ;
                                      owl:onProperty l0:name ;
                                      owl:someValuesFrom rdfs:Literal
                                    ] ;
                    rdfs:isDefinedBy <https://w3id.org/italia/onto/HER> ;
                    rdfs:label "Classification of Academic Disciplines"@en ,
                               "Classificazione Settori Sicentifico Disciplinari"@it ;
                    prov:wasDerivedFrom skos:ConceptScheme ;
                    l0:controlledVocabulary <https://w3id.org/italia/controlled-vocabulary/classifications-for-universities/academic-disciplines> .


###  https://w3id.org/italia/onto/HER/AcademicRecruitementField
:AcademicRecruitementField rdf:type owl:Class ;
                           rdfs:subClassOf :AcademicDiscipline ;
                           rdfs:isDefinedBy <https://w3id.org/italia/onto/HER> ;
                           prov:wasDerivedFrom skos:Concept ;
                           l0:controlledVocabulary <https://w3id.org/italia/controlled-vocabulary/classifications-for-universities/academic-disciplines> .


###  https://w3id.org/italia/onto/HER/AcademicRole
:AcademicRole rdf:type owl:Class ;
              rdfs:subClassOf <https://w3id.org/italia/onto/RO/Role> ;
              rdfs:comment "Il ruolo che una persona svolge in un'organizzazione accademica."@it ,
                           "The role a person plays in an academic organization."@en ;
              rdfs:isDefinedBy <https://w3id.org/italia/onto/HER> ;
              rdfs:label "Academic role"@en ,
                         "Ruolo Accademico"@it ;
              owl:versionInfo "provvisoria"@it ,
                              "unstable"@en .


###  https://w3id.org/italia/onto/HER/Area
:Area rdf:type owl:Class ;
      rdfs:subClassOf :AcademicDiscipline ;
      rdfs:comment """It refers to the areas set up by the National University Council (CUN).
Currently, there are fourteen areas. (Gelmin Law 240/2010)
- Area 01 Mathematics and informatics
- Area 02 Physics
- Area 03 Chemistry
- Area 04 Earth Science
- Area 05 Biology
- Area 06 Medicine
- Area 07 Agricultural and veterinary science
- Area 08 Civil engineering and architecture
- Area 09 Industrial and information engineering
- Area 10 Antiquities, philology, literary studies, art history
- Area 11 History, philosophy, pedagogy and psychology
- Area 12 Law
- Area 13 Economics and statistics
- Area 14 Political and social science"""@en ,
                   """Si riferisce alle aree istituite dal Consiglio Universitario Nazionale (CUN).
Attualmente le aree sono quattordici. (Legge Gelmin 240/2010)
- Area 01 Matematica e informatica
- Area 02 Fisica
- Area 03 Chimica
- Area 04 Scienze della Terra
- Area 05 Biologia
- Area 06 Medicina
- Area 07 Scienze agrarie e veterinarie
- Area 08 Ingegneria civile e architettura
- Area 09 Ingegneria industriale e dell'informazione
- Area 10 Antichità, filologia, studi letterari, storia dell'arte
- Area 11 Storia, filosofia, pedagogia e psicologia
- Area 12 Legge
- Area 13 Economia e statistica
- Area 14 Scienze politiche e sociali"""@it ;
      rdfs:isDefinedBy <https://w3id.org/italia/onto/HER> ;
      rdfs:label "Area CUN"@it ,
                 "CUN Area"@en ;
      prov:wasDerivedFrom skos:Concept ;
      l0:controlledVocabulary <https://w3id.org/italia/controlled-vocabulary/classifications-for-universities/academic-disciplines> .


###  https://w3id.org/italia/onto/HER/CHAFEACall
:CHAFEACall rdf:type owl:Class ;
            rdfs:subClassOf :Call ;
            rdfs:comment "Bando specifico per il quale è stato concesso il finanziamento di ogni attività"@it ,
                         "Specific call unders which each activity was granted funding"@en ;
            rdfs:isDefinedBy <https://w3id.org/italia/onto/HER> ;
            rdfs:label "Bando CHAFEA"@it ,
                       "CHAFEA Call"@en .


###  https://w3id.org/italia/onto/HER/CHAFEAInstrument
:CHAFEAInstrument rdf:type owl:Class ;
                  rdfs:subClassOf l0:Concept ;
                  rdfs:comment "Tipo di attività finanziata. I tipi sono: Progetti, Conferenza, Azioni congiunte, Sovvenzione di funzionamento, Accordo quadro di partenariato"@it ,
                               "Type of activity funded. Types are: Projects, Conference, Joint Actions, Operating Grant, Framework Partnership Agreement"@en ;
                  rdfs:isDefinedBy <https://w3id.org/italia/onto/HER> ;
                  rdfs:label "CHAFEA Instrument"@en ,
                             "Strumento CHAFEA"@it ;
                  prov:wasDerivedFrom skos:Concept .


###  https://w3id.org/italia/onto/HER/CHAFEAOutput
:CHAFEAOutput rdf:type owl:Class ;
              rdfs:subClassOf :Result ;
              rdfs:comment "Ouput prodotto da un'attività finanziata. I diversi tipi di output sono: \"Dimostratore, pilota, prototipo\", \"Documento, rapporti...\", \"Siti web, compilazione di brevetti, video ecc."@it ,
                           "Ouput produced by a funded activity. The different types of outputs are: \"Demonstrator, pilot, prototype\", \"Document, reports...\", \"Websites, patent filling, videos etc\" and \"Other\"."@en ;
              rdfs:isDefinedBy <https://w3id.org/italia/onto/HER> ;
              rdfs:label "CHAFEA Project's Output"@en ,
                         "Risultato progetto CHAFEA"@it .


###  https://w3id.org/italia/onto/HER/CHAFEAParticipant
:CHAFEAParticipant rdf:type owl:Class ;
                   rdfs:subClassOf <https://w3id.org/italia/onto/RO/TimeIndexedRole> ,
                                   [ rdf:type owl:Restriction ;
                                     owl:onProperty :hasParticipationCountry ;
                                     owl:allValuesFrom <https://w3id.org/italia/onto/CLV/Country>
                                   ] ;
                   rdfs:comment "Involved Institutions"@en ,
                                "Istituzioni coinvolte"@it ;
                   rdfs:isDefinedBy <https://w3id.org/italia/onto/HER> ;
                   rdfs:label "CHAFEA Participant"@en ,
                              "Partecipanti CHAFEA"@it .


###  https://w3id.org/italia/onto/HER/CHAFEAProgramme
:CHAFEAProgramme rdf:type owl:Class ;
                 rdfs:subClassOf :Programme ;
                 rdfs:comment "Funding programme of an activity. Possible values are: \"First Programme of Community action in the field of public health (2003-2008)\", \"Second Programme of Community action in the Field of Health 2008-2013\", and \"3rd Health Programme (2014-2020)\"."@en ,
                              "Programma di finanziamento di un'attività. I valori possibili sono: \"Primo programma d'azione comunitaria nel campo della sanità pubblica (2003-2008)\", \"Secondo programma d'azione comunitaria in materia di salute 2008-2013\" e \"Terzo programma in materia di salute (2014-2020)\"."@it ;
                 rdfs:isDefinedBy <https://w3id.org/italia/onto/HER> ;
                 rdfs:label "CHAFEA Programme"@en ,
                            "Programma CHAFEA"@it ;
                 prov:wasDerivedFrom skos:Concept .


###  https://w3id.org/italia/onto/HER/CHAFEAProject
:CHAFEAProject rdf:type owl:Class ;
               rdfs:subClassOf <https://w3id.org/italia/onto/Project/PublicResearchProject> ;
               rdfs:comment "Attività finanziata pubblicata dall'Agenzia esecutiva per i consumatori, la salute, l'agricoltura e l'alimentazione (CHAFEA)"@it ,
                            "Funded activity published by the Consumers, Health, Agriculture and Food Executive Agency (CHAFEA)"@en ;
               rdfs:isDefinedBy <https://w3id.org/italia/onto/HER> ;
               rdfs:label "CHAFEA Project"@en ,
                          "Progetto CHAFEA"@it .


###  https://w3id.org/italia/onto/HER/CHAFEASummary
:CHAFEASummary rdf:type owl:Class ;
               rdfs:subClassOf l0:Object ,
                               [ rdf:type owl:Restriction ;
                                 owl:onProperty l0:description ;
                                 owl:allValuesFrom rdfs:Literal
                               ] ;
               rdfs:comment "Description of funded activity."@en ,
                            "Descrizione dell'attività finanziata."@it ;
               rdfs:isDefinedBy <https://w3id.org/italia/onto/HER> ;
               rdfs:label "CHAFEA Project's Summary"@en ,
                          "Sommario progetto CHAFEA"@it .


###  https://w3id.org/italia/onto/HER/CHAFEATopic
:CHAFEATopic rdf:type owl:Class ;
             rdfs:subClassOf :HERClassification ;
             rdfs:comment "Classification of funded activities published by the Consumers, Health, Agriculture and Food Executive Agency (CHAFEA)"@en ,
                          "Classificazione delle attività finanziate pubblicata dall'Agenzia esecutiva per i consumatori, la salute, l'agricoltura e l'alimentazione (CHAFEA)"@it ;
             rdfs:isDefinedBy <https://w3id.org/italia/onto/HER> ;
             rdfs:label "Argomento CHAFEA"@it ,
                        "CHAFEA Topic"@en ;
             prov:wasDerivedFrom skos:Concept .


###  https://w3id.org/italia/onto/HER/CHAFEAWorkpackage
:CHAFEAWorkpackage rdf:type owl:Class ;
                   rdfs:subClassOf l0:Description ;
                   rdfs:comment "Pacchetto di lavoro che fa parte di un'attività finanziata."@it ,
                                "Workpackage that is part of a funded activity."@en ;
                   rdfs:isDefinedBy <https://w3id.org/italia/onto/HER> ;
                   rdfs:label "CHAFEA Project's Workpackage"@en ,
                              "Paino di lavoro progetto CHAFEA"@it .


###  https://w3id.org/italia/onto/HER/CPCClassification
:CPCClassification rdf:type owl:Class ;
                   rdfs:subClassOf :HERClassification ,
                                   [ rdf:type owl:Restriction ;
                                     owl:onProperty l0:name ;
                                     owl:someValuesFrom rdfs:Literal
                                   ] ,
                                   [ rdf:type owl:Restriction ;
                                     owl:onProperty l0:identifier ;
                                     owl:cardinality "1"^^xsd:nonNegativeInteger
                                   ] ;
                   rdfs:isDefinedBy <https://w3id.org/italia/onto/HER> ;
                   rdfs:label "Classificazione dei brevetti cooperativi"@it ,
                              "Cooperative Patent Classification"@en ;
                   prov:wasDerivedFrom skos:ConceptScheme .


###  https://w3id.org/italia/onto/HER/CTNPRINAmount
:CTNPRINAmount rdf:type owl:Class ;
               rdfs:subClassOf <https://w3id.org/italia/onto/MU/Value> ,
                               [ rdf:type owl:Restriction ;
                                 owl:onProperty :ctnprinAmountScope ;
                                 owl:maxCardinality "1"^^xsd:nonNegativeInteger
                               ] ,
                               [ rdf:type owl:Restriction ;
                                 owl:onProperty :expenseType ;
                                 owl:maxCardinality "1"^^xsd:nonNegativeInteger
                               ] ;
               rdfs:comment "Importi monetari allegati a un'operazione CTN/PRIN"@it ,
                            "Monetary amounts attached to a CTN/PRIN operation"@en ;
               rdfs:isDefinedBy <https://w3id.org/italia/onto/HER> ;
               rdfs:label "Ammontare CTN/PRIN"@it ,
                          "CTN/PRIN Amount"@en ;
               owl:versionInfo "stabile"@it ,
                               "stable"@en .


###  https://w3id.org/italia/onto/HER/CTNPRINEntity
:CTNPRINEntity rdf:type owl:Class ;
               rdfs:subClassOf covapit:Organization ;
               rdfs:comment "Soggetti beneficiari dell'iniziativa. I dati integrati in ToscanaOpenResearch sono stati ottenuti nel contesto di un protocollo di intesa tra il Ministero dell'Istruzione, dell'Università e della Ricerca e la Regione toscana, e sono relativi a progetti aventi almeno un beneficiario con sede legale o operativa in Toscana."@it ,
                            "Subjects that are beneficiaries of the initiative. The data integrated in ToscanaOpenResearch were obtained in the context of a memorandum of understanding between the Ministry of Education, University and Research and the Region of Tuscany, and are related to projects with at least one beneficiary with registered or operational headquarters in Tuscany."@en ;
               rdfs:isDefinedBy <https://w3id.org/italia/onto/HER> ;
               rdfs:label "CTN/PRIN Funded Institution"@en ,
                          "Istituzione finanziata da CTN/PRIN"@it .


###  https://w3id.org/italia/onto/HER/CTNPRINFinancingFund
:CTNPRINFinancingFund rdf:type owl:Class ;
                      rdfs:subClassOf l0:Object ,
                                      [ rdf:type owl:Restriction ;
                                        owl:onProperty :ctnprinAvailableBudget ;
                                        owl:maxCardinality "1"^^xsd:nonNegativeInteger
                                      ] ;
                      rdfs:comment "Financing fund from which the initiative draws its economic resources"@en ,
                                   "Fondo di finanziamento da cui l'iniziativa attinge le sue risorse economiche"@it ;
                      rdfs:isDefinedBy <https://w3id.org/italia/onto/HER> ;
                      rdfs:label "CTN/PRIN Financing Fund"@en ,
                                 "Fondo di finanziamento CTN/PRIN"@it .


###  https://w3id.org/italia/onto/HER/CTNPRINInitiative
:CTNPRINInitiative rdf:type owl:Class ;
                   rdfs:subClassOf l0:Activity ,
                                   [ rdf:type owl:Restriction ;
                                     owl:onProperty :decreeDate ;
                                     owl:qualifiedCardinality "1"^^xsd:nonNegativeInteger ;
                                     owl:onDataRange xsd:date
                                   ] ,
                                   [ rdf:type owl:Restriction ;
                                     owl:onProperty :decreeNumber ;
                                     owl:cardinality "1"^^xsd:nonNegativeInteger
                                   ] ,
                                   [ rdf:type owl:Restriction ;
                                     owl:onProperty :documentationURL ;
                                     owl:qualifiedCardinality "1"^^xsd:nonNegativeInteger ;
                                     owl:onDataRange xsd:anyURI
                                   ] ,
                                   [ rdf:type owl:Restriction ;
                                     owl:onProperty :expireDate ;
                                     owl:qualifiedCardinality "1"^^xsd:nonNegativeInteger ;
                                     owl:onDataRange xsd:date
                                   ] ,
                                   [ rdf:type owl:Restriction ;
                                     owl:onProperty :initiativeType ;
                                     owl:maxCardinality "1"^^xsd:nonNegativeInteger
                                   ] ;
                   rdfs:comment "An initiative in this context is a funding action that can be associated with a call, a notice, an invitation, a campaign, etc. The data integrated in ToscanaOpenResearch have been obtained in the context of a memorandum of understanding between the Ministry of Education, University and Research and the Tuscan Region, and are related to the initiatives CTN2012, CTN20916 and PRIN 2012, and to projects with at least one beneficiary with legal or operational headquarters in Tuscany."@en ,
                                "Un'iniziativa in questo contesto è un'azione di finanziamento che può essere associata ad un bando, un avviso, un invito, una campagna, etc. I dati integrati in ToscanaOpenResearch sono stati ottenuti nel contesto di un protocollo di intesa tra il Ministero dell'Istruzione, dell'Università e della Ricerca e la Regione toscana, e sono relativi alle iniziative CTN2012, CTN20916 e PRIN 2012, e a progetti aventi almeno un beneficiario con sede legale o operativa in Toscana."@it ;
                   rdfs:isDefinedBy <https://w3id.org/italia/onto/HER> ;
                   rdfs:label "CTN/PRIN Initiative"@en ,
                              "iniziativa CTN/PRIN"@it ;
                   owl:versionInfo "stabile"@it ,
                                   "stable"@en .


###  https://w3id.org/italia/onto/HER/CTNPRINOperation
:CTNPRINOperation rdf:type owl:Class ;
                  rdfs:subClassOf l0:Activity ,
                                  [ rdf:type owl:Restriction ;
                                    owl:onProperty :allocatesFundsTo ;
                                    owl:someValuesFrom :CTNPRINEntity
                                  ] ,
                                  [ rdf:type owl:Restriction ;
                                    owl:onProperty :hasCTNPRINAmount ;
                                    owl:allValuesFrom :CTNPRINAmount
                                  ] ,
                                  [ rdf:type owl:Restriction ;
                                    owl:onProperty :refersToProject ;
                                    owl:allValuesFrom :CTNPRINProject
                                  ] ,
                                  [ rdf:type owl:Restriction ;
                                    owl:onProperty :ctnprinOperationScope ;
                                    owl:someValuesFrom rdfs:Literal
                                  ] ,
                                  [ rdf:type owl:Restriction ;
                                    owl:onProperty :ctnprinSecondLevelSR ;
                                    owl:someValuesFrom rdfs:Literal
                                  ] ,
                                  [ rdf:type owl:Restriction ;
                                    owl:onProperty :ctnprinSectorOfReference ;
                                    owl:someValuesFrom rdfs:Literal
                                  ] ,
                                  [ rdf:type owl:Restriction ;
                                    owl:onProperty :abstract ;
                                    owl:allValuesFrom rdfs:Literal
                                  ] ,
                                  [ rdf:type owl:Restriction ;
                                    owl:onProperty :admissionDate ;
                                    owl:qualifiedCardinality "1"^^xsd:nonNegativeInteger ;
                                    owl:onDataRange xsd:date
                                  ] ,
                                  [ rdf:type owl:Restriction ;
                                    owl:onProperty :ctnprinOperationIdentifier ;
                                    owl:cardinality "1"^^xsd:nonNegativeInteger
                                  ] ,
                                  [ rdf:type owl:Restriction ;
                                    owl:onProperty :startingDate ;
                                    owl:qualifiedCardinality "1"^^xsd:nonNegativeInteger ;
                                    owl:onDataRange xsd:date
                                  ] ,
                                  [ rdf:type owl:Restriction ;
                                    owl:onProperty :transmissionDate ;
                                    owl:qualifiedCardinality "1"^^xsd:nonNegativeInteger ;
                                    owl:onDataRange xsd:date
                                  ] ,
                                  [ rdf:type owl:Restriction ;
                                    owl:onProperty :revocationDate ;
                                    owl:maxQualifiedCardinality "1"^^xsd:nonNegativeInteger ;
                                    owl:onDataRange xsd:date
                                  ] ,
                                  [ rdf:type owl:Restriction ;
                                    owl:onProperty :revoked ;
                                    owl:maxCardinality "1"^^xsd:nonNegativeInteger
                                  ] ,
                                  [ rdf:type owl:Restriction ;
                                    owl:onProperty <https://w3id.org/italia/onto/Project/projectAcronym> ;
                                    owl:maxCardinality "1"^^xsd:nonNegativeInteger
                                  ] ;
                  rdfs:comment "Accounting operation, related to Local code project, scope, beneficiary"@en ,
                               "Operazione contabile, relativa a Codice locale progetto, ambito, beneficiario"@it ;
                  rdfs:isDefinedBy <https://w3id.org/italia/onto/HER> ;
                  rdfs:label "CTN/PRIN Operation"@en ,
                             "Operazione CTN/PRIN"@it ;
                  owl:versionInfo "stabile"@it ,
                                  "stable"@en .


###  https://w3id.org/italia/onto/HER/CTNPRINProject
:CTNPRINProject rdf:type owl:Class ;
                rdfs:subClassOf <https://w3id.org/italia/onto/Project/PublicResearchProject> ,
                                [ rdf:type owl:Restriction ;
                                  owl:onProperty :ctnprinSecondLevelSR ;
                                  owl:someValuesFrom rdfs:Literal
                                ] ,
                                [ rdf:type owl:Restriction ;
                                  owl:onProperty :ctnprinSectorOfReference ;
                                  owl:someValuesFrom rdfs:Literal
                                ] ;
                rdfs:comment "Progetto finanziato da CTN (Cluster Tecnologici Nazionali) o PRIN (Progetti di Ricerca di Interesse Nazionale)"@it ,
                             "Project funded by CTN (Cluster Tecnologici Nazionali) or PRIN (Progetti di Ricerca di Interesse Nazionale)"@en ;
                rdfs:isDefinedBy <https://w3id.org/italia/onto/HER> ;
                rdfs:label "CTN/PRIN Project"@en ,
                           "Progetto CTN/PRIN"@it .


###  https://w3id.org/italia/onto/HER/Call
:Call rdf:type owl:Class ;
      rdfs:subClassOf l0:Object ;
      rdfs:comment "A call for projects."@en ,
                   "Un invito a presentare progetti."@it ;
      rdfs:isDefinedBy <https://w3id.org/italia/onto/HER> ;
      rdfs:label "Bando"@it ,
                 "Call"@en .


###  https://w3id.org/italia/onto/HER/CountryInvolvement
:CountryInvolvement rdf:type owl:Class ;
                    rdfs:subClassOf l0:EventOrSituation ,
                                    [ rdf:type owl:Restriction ;
                                      owl:onProperty :hasAACTStudy ;
                                      owl:qualifiedCardinality "1"^^xsd:nonNegativeInteger ;
                                      owl:onClass :AACTStudy
                                    ] ,
                                    [ rdf:type owl:Restriction ;
                                      owl:onProperty :withCountry ;
                                      owl:qualifiedCardinality "1"^^xsd:nonNegativeInteger ;
                                      owl:onClass <https://w3id.org/italia/onto/CLV/Country>
                                    ] ,
                                    [ rdf:type owl:Restriction ;
                                      owl:onProperty :removedCountry ;
                                      owl:maxQualifiedCardinality "1"^^xsd:nonNegativeInteger ;
                                      owl:onDataRange xsd:boolean
                                    ] ;
                    rdfs:comment "Country where the facility conducting a clinical protocol is located"@en ,
                                 "Paese in cui si trova la struttura che conduce un protocollo clinico"@it ;
                    rdfs:isDefinedBy <https://w3id.org/italia/onto/HER> ;
                    rdfs:label "Coinvolgimento del paese"@it ,
                               "Country Involvement"@en .


###  https://w3id.org/italia/onto/HER/DSUCanteenAndAccomodationsAggregate
:DSUCanteenAndAccomodationsAggregate rdf:type owl:Class ;
                                     rdfs:subClassOf :StatisticalDataAggregation ;
                                     rdfs:comment "Information on accommodation and canteens active at 1/11 of the reference year."@en ,
                                                  "Informazioni sui posti alloggio e mense attive all'1/11 dell'anno di riferimento."@it ;
                                     rdfs:isDefinedBy <https://w3id.org/italia/onto/HER> ;
                                     rdfs:label "Aggregazione degli alloggi e mense riportate da DSU"@it ,
                                                "DSU Aggregate of Canteen And Accommodations"@en .


###  https://w3id.org/italia/onto/HER/DSUInterventionType
:DSUInterventionType rdf:type owl:Class ;
                     rdfs:subClassOf l0:Characteristic ,
                                     [ rdf:type owl:Restriction ;
                                       owl:onProperty l0:description ;
                                       owl:someValuesFrom rdfs:Literal
                                     ] ,
                                     [ rdf:type owl:Restriction ;
                                       owl:onProperty l0:identifier ;
                                       owl:cardinality "1"^^xsd:nonNegativeInteger
                                     ] ;
                     rdfs:comment "Information (code and description) on interventions in favor of students for the Academic Year (T-1)/(T)."@en ,
                                  "Informazioni (codice e descrizione) sugli interventi a favore degli studenti per l'Anno Accademico (T-1)/(T)"@it ;
                     rdfs:isDefinedBy <https://w3id.org/italia/onto/HER> ;
                     rdfs:label "DSU Intervention Type"@en ,
                                "Tipo (o classe) di intervento DSU"@it ;
                     owl:versionInfo "stabile"@it ,
                                     "stable"@en .


###  https://w3id.org/italia/onto/HER/DSURightToUniversityStudiesAggregate
:DSURightToUniversityStudiesAggregate rdf:type owl:Class ;
                                      rdfs:subClassOf :StatisticalDataAggregation ;
                                      rdfs:comment "Interventi concessi a studenti per ciascun Ateneo/Istituto gestito da ciascun ente per il DSU/ufficio, per l'anno accademico di riferimento."@it ,
                                                   "Interventions granted to students for each University/Institute managed by each institution for the Right to University Studies - DSU/Office, for the academic year of reference."@en ;
                                      rdfs:isDefinedBy <https://w3id.org/italia/onto/HER> ;
                                      rdfs:label "Aggregazione Diritto allo studio universitario riportato da USTAT"@it ,
                                                 "DSU Aggregate of Right to University Studies"@en .


###  https://w3id.org/italia/onto/HER/DegreeArea
:DegreeArea rdf:type owl:Class ;
            rdfs:subClassOf :HERClassification ;
            rdfs:comment """According to http://anagrafe.miur.it/, the areas are the following:

- Sanitaria
- Scientifica
- Sociale
- Umanistica

Each faculty is gruped under one of the previous areas."""@en ;
            rdfs:isDefinedBy <https://w3id.org/italia/onto/HER> ;
            rdfs:label "Area di laurea italiana"@it ,
                       "Italian Degree Area"@en ;
            prov:wasDerivedFrom skos:Concept .


###  https://w3id.org/italia/onto/HER/DegreeClass
:DegreeClass rdf:type owl:Class ;
             rdfs:subClassOf :HERClassification ;
             rdfs:comment """http://www.miur.it/0002Univer/0021Offert/index_cf2.htm

- Determinazione delle classi delle lauree universitarie (1-42)
http://www.miur.it/UserFiles/521.pdf

- Determinazione delle classi delle lauree specialistiche (1-104)"""@it ;
             rdfs:isDefinedBy <https://w3id.org/italia/onto/HER> ;
             rdfs:label "Italian Degree Class"@en ,
                        "Tipo di laurea italiana"@it ;
             prov:wasDerivedFrom skos:Concept .


###  https://w3id.org/italia/onto/HER/Diploma
:Diploma rdf:type owl:Class ;
         rdfs:subClassOf l0:Object ;
         rdfs:comment "A maturity diploma that can be awarded upon successful completion of secondary education."@en ,
                      "Un diploma di maturità che può essere rilasciato al termine del ciclo di studi secondari."@it ;
         rdfs:isDefinedBy <https://w3id.org/italia/onto/HER> ;
         rdfs:label "Diploma"@en ,
                    "diploma"@it .


###  https://w3id.org/italia/onto/HER/ECActivityType
:ECActivityType rdf:type owl:Class ;
                rdfs:subClassOf :ECClassification ;
                rdfs:comment "Tipologia di attività dell'organizzazione che partecipa a un progetto CE. Le seguenti descrizioni e codici di convenzione sono utilizzati per distinguere tra i diversi tipi di organizzazioni: società private a scopo di lucro (PRC), enti pubblici (esclusi ricerca e istruzione) (PUB), organizzazioni di ricerca (esclusa l'istruzione) (REC), istituti di istruzione secondaria e superiore (HES) e altri enti (OTH)."@it ,
                             "Type of activity performed by the organisation participating in a EC project. The following descriptions and convention codes are used for distinguishing between the different types of organisations according to their nature/activity: private for profit companies (PRC), public bodies (excluding research and education) (PUB), research organisations (excluding education) (REC), secondary and higher education establishments (HES), and other entities (OTH)."@en ;
                rdfs:isDefinedBy <https://w3id.org/italia/onto/HER> ;
                rdfs:label "EC Activity Type of Organization"@en ,
                           "Tipologia CE di attivitá dell'organizzazione"@it ;
                owl:versionInfo "stabile"@it ,
                                "stable"@en .


###  https://w3id.org/italia/onto/HER/ECCall
:ECCall rdf:type owl:Class ;
        rdfs:subClassOf :Call ,
                        :ECClassification ;
        rdfs:comment "Procedura per invitare i candidati a presentare proposte di progetti, con l'obiettivo di ricevere un finanziamento UE."@it ,
                     "Procedure for inviting applicants to submit project proposals, with the aim of receiving EU funding."@en ;
        rdfs:isDefinedBy <https://w3id.org/italia/onto/HER> ;
        rdfs:label "Bando CE"@it ,
                   "EC Call"@en ;
        prov:wasDerivedFrom skos:Concept .


###  https://w3id.org/italia/onto/HER/ECClassification
:ECClassification rdf:type owl:Class ;
                  rdfs:subClassOf :HERClassification ;
                  rdfs:isDefinedBy <https://w3id.org/italia/onto/HER> ;
                  prov:wasDerivedFrom skos:ConceptScheme .


###  https://w3id.org/italia/onto/HER/ECFrameworkProgramme
:ECFrameworkProgramme rdf:type owl:Class ;
                      rdfs:subClassOf :ECClassification ;
                      owl:disjointWith :ECProgramme ;
                      rdfs:comment "I framework program, o in forma abbreviata dal FP1 a FP7 - \"FP8\" è stato chiamato \"Horizon 2020\" - sono programmi di finanziamento creati dall'Unione Europea e dalla Commissione Europea per sostenere e promuovere la ricerca nello Spazio Europeo della Ricerca (ERA)."@it ,
                                   "The Framework Programmes, or abbreviated FP1 to FP7 with \"FP8\" being named \"Horizon 2020\", are funding programmes created by the European Union/European Commission to support and foster research in the European Research Area (ERA)."@en ;
                      rdfs:isDefinedBy <https://w3id.org/italia/onto/HER> ;
                      rdfs:label "EC Framework Program"@en ,
                                 "Programma quadro CE"@it ;
                      prov:wasDerivedFrom skos:Concept .


###  https://w3id.org/italia/onto/HER/ECFundingScheme
:ECFundingScheme rdf:type owl:Class ;
                 rdfs:subClassOf :ECClassification ,
                                 l0:Concept ;
                 rdfs:comment "Funding scheme (or \"Types of action\" in Horizon 2020) are the types of projects funded under a EC Framework Programme. In Horizon 2020, the existing types of action are the following: Research and innovation actions (RIA), Innovation actions (IA), Coordination and support actions (CSA), ERA-NET Cofund actions, European Joint Programme (EJP) Cofund actions, Pre-Commercial Procurement (PCP) actions, Public Procurement of Innovative Solutions (PPI) actions and Prizes."@en ,
                              """Gli schemi di finanziamento (o \"Tipi di azione\" in Horizon 2020) sono i tipi di progetti finanziati nell'ambito di un programma quadro CE. In Horizon 2020, i tipi di azione esistenti sono i seguenti: Azioni di ricerca e innovazione (RIA), azioni di innovazione (IA), azioni di coordinamento e sostegno (CSA), azioni Cofund ERA-NET, azioni Cofund del programma comune europeo (EJP), azioni Cofund del programma europeo congiunto (EJP), azioni di appalti pre-commerciali (PCP), azioni di appalti pubblici di soluzioni innovative (PPI) e premi.
"""@it ;
                 rdfs:isDefinedBy <https://w3id.org/italia/onto/HER> ;
                 rdfs:label "EC Funding Scheme"@en ,
                            "Piano di finanziamento CE"@it ;
                 prov:wasDerivedFrom skos:Concept .


###  https://w3id.org/italia/onto/HER/ECParticipant
:ECParticipant rdf:type owl:Class ;
               rdfs:subClassOf <https://w3id.org/italia/onto/RO/TimeIndexedRole> ,
                               [ rdf:type owl:Restriction ;
                                 owl:onProperty <https://w3id.org/italia/onto/CLV/hasSpatialCoverage> ;
                                 owl:allValuesFrom <https://w3id.org/italia/onto/CLV/Feature>
                               ] ,
                               [ rdf:type owl:Restriction ;
                                 owl:onProperty :hasParticipationCountry ;
                                 owl:allValuesFrom <https://w3id.org/italia/onto/CLV/Country>
                               ] ,
                               [ rdf:type owl:Restriction ;
                                 owl:onProperty ti:hasYear ;
                                 owl:maxQualifiedCardinality "1"^^xsd:nonNegativeInteger ;
                                 owl:onClass ti:Year
                               ] ,
                               [ rdf:type owl:Restriction ;
                                 owl:onProperty covapit:VATnumber ;
                                 owl:allValuesFrom rdfs:Literal
                               ] ,
                               [ rdf:type owl:Restriction ;
                                 owl:onProperty :rcn ;
                                 owl:cardinality "1"^^xsd:nonNegativeInteger
                               ] ,
                               [ rdf:type owl:Restriction ;
                                 owl:onProperty :unicsId ;
                                 owl:cardinality "1"^^xsd:nonNegativeInteger
                               ] ,
                               [ rdf:type owl:Restriction ;
                                 owl:onProperty :picNumber ;
                                 owl:maxCardinality "1"^^xsd:nonNegativeInteger
                               ] ;
               rdfs:comment "Partecipante ad un progetto CE. Questa classe è una reificazione del rapporto che coinvolge un progetto con un'organizzazione partecipante. Questa classe reificata memorizza informazioni aggiuntive come il finanziamento concesso dall'UE al partecipante specifico."@it ,
                            "Participant in a EC project. This class is a reification of the relationship that involves a project with a participating organization. This reified class stores additional information such as the funding granted by the EU to the specific participant."@en ;
               rdfs:isDefinedBy <https://w3id.org/italia/onto/HER> ;
               rdfs:label "EC Participant"@en ,
                          "Partecipante CE"@it .


###  https://w3id.org/italia/onto/HER/ECProgramme
:ECProgramme rdf:type owl:Class ;
             rdfs:subClassOf :ECClassification ,
                             :Programme ;
             rdfs:comment "Programma di finanziamento specifico di un progetto all'interno di una gerarchia a più livelli che rientra in un programma quadro."@it ,
                          "Specific funding programme of a project within a multi-level hierarchy that falls under a framework programme."@en ;
             rdfs:isDefinedBy <https://w3id.org/italia/onto/HER> ;
             rdfs:label "EC Programme"@en ,
                        "Programma CE"@it ;
             prov:wasDerivedFrom skos:Concept .


###  https://w3id.org/italia/onto/HER/ECProject
:ECProject rdf:type owl:Class ;
           rdfs:subClassOf <https://w3id.org/italia/onto/Project/PublicResearchProject> ,
                           [ rdf:type owl:Restriction ;
                             owl:onProperty :cordisRef ;
                             owl:cardinality "1"^^xsd:nonNegativeInteger
                           ] ,
                           [ rdf:type owl:Restriction ;
                             owl:onProperty :ecGrantAgreementNo ;
                             owl:cardinality "1"^^xsd:nonNegativeInteger
                           ] ;
           rdfs:comment "Progetto finanziato dai programmi quadro dell'UE per la ricerca e l'innovazione (dal 1° PQ1 a Horizon 2020) e pubblicato dalla Commissione europea sul servizio comunitario di informazione per la ricerca e lo sviluppo (CORDIS)."@it ,
                        "Project funded by the EU's framework programmes for research and innovation (FP1 to Horizon 2020) and published by the European Comission on the Community Research and Development Information Service (CORDIS)."@en ;
           rdfs:isDefinedBy <https://w3id.org/italia/onto/HER> ;
           rdfs:label "EC Project"@en ,
                      "Progetto CE"@it .


###  https://w3id.org/italia/onto/HER/ECSubjectArea
:ECSubjectArea rdf:type owl:Class ;
               rdfs:subClassOf :ECClassification ;
               rdfs:comment "Categorizzazione tematica utilizzata nel 7° Programma Quadro. Non disponibile in H2020."@it ,
                            "Thematic categorisation used in the 7th Framework Programme. Not available in H2020."@en ;
               rdfs:isDefinedBy <https://w3id.org/italia/onto/HER> ;
               rdfs:label "Area tematica CE"@it ,
                          "EC Subject Area"@en ;
               prov:wasDerivedFrom skos:Concept .


###  https://w3id.org/italia/onto/HER/ECTopic
:ECTopic rdf:type owl:Class ;
         rdfs:subClassOf :ECClassification ;
         rdfs:comment "Calls for proposals are subdivided into topics. A topic defines a specific subject or area for which applicants are invited to submit proposals. The description of a topic comprises its specific scope, the type of action, evaluation criteria and deadline for submission of proposals."@en ,
                      "Gli inviti a presentare proposte sono suddivisi per argomenti. Un argomento definisce un argomento o un settore specifico per il quale i candidati sono invitati a presentare proposte. La descrizione di un argomento comprende il suo ambito specifico, il tipo di azione, i criteri di valutazione e la scadenza per la presentazione delle proposte."@it ;
         rdfs:isDefinedBy <https://w3id.org/italia/onto/HER> ;
         rdfs:label "Argomento di ricerca CE"@it ,
                    "EC Topic"@en ;
         prov:wasDerivedFrom skos:Concept .


###  https://w3id.org/italia/onto/HER/ERCClassification
:ERCClassification rdf:type owl:Class ;
                   rdfs:subClassOf :ECClassification ;
                   rdfs:isDefinedBy <https://w3id.org/italia/onto/HER> ;
                   prov:wasDerivedFrom skos:ConceptScheme .


###  https://w3id.org/italia/onto/HER/ERCGrantType
:ERCGrantType rdf:type owl:Class ;
              rdfs:subClassOf l0:Characteristic ;
              rdfs:comment "Tipo di finanziamento dell'European Research Council - ERC. Le sovvenzioni dell'ERC sono suddivise in 6 tipi: Sovvenzione di avviamento, Sovvenzione per la sinergia, Sovvenzione per il consolidamento, Sovvenzione per il sostegno, Sovvenzione per la prova di un concetto e Sovvenzione per la fase avanzata. Si tratta di contributi finanziari diretti donati dal bilancio del ERC per finanziare le attività."@it ,
                           "Type of ERC funding. ERC grants are divided in 6 types: Starting Grant, Synergy Grant, Consolidator Grant, Support, Proof of Concept Grant and Advanced Grant. These are direct financial contributions donated from the ERC budget in order to finance activities."@en ;
              rdfs:isDefinedBy <https://w3id.org/italia/onto/HER> ;
              rdfs:label "ERC Grant Type"@en ,
                         "Tipo Contributo ERC"@it .


###  https://w3id.org/italia/onto/HER/ERCPanel
:ERCPanel rdf:type owl:Class ;
          rdfs:subClassOf :ERCClassification ;
          rdfs:comment """English: http://www.unipr.it/sites/default/files/allegatiparagrafo/01-08-2013/settori_erc.pdf
Italian: https://it.wikipedia.org/wiki/Settori_ERC""" ;
          rdfs:isDefinedBy <https://w3id.org/italia/onto/HER> ;
          rdfs:label "ERC Panel"@en ,
                     "Pannello ERC"@it ;
          prov:wasDerivedFrom skos:Concept ;
          l0:controlledVocabulary <https://w3id.org/italia/controlled-vocabulary/classifications-for-her/erc-panel-h2020-fp> .


###  https://w3id.org/italia/onto/HER/ERCProject
:ERCProject rdf:type owl:Class ;
            rdfs:subClassOf <https://w3id.org/italia/onto/Project/PublicResearchProject> ,
                            [ rdf:type owl:Restriction ;
                              owl:onProperty :cordisRef ;
                              owl:cardinality "1"^^xsd:nonNegativeInteger
                            ] ,
                            [ rdf:type owl:Restriction ;
                              owl:onProperty :ecGrantAgreementNo ;
                              owl:cardinality "1"^^xsd:nonNegativeInteger
                            ] ;
            rdfs:comment "Progetto finanziato dal Consiglio Europeo della Ricerca"@it ,
                         "Project funded by the European Research Council"@en ;
            rdfs:isDefinedBy <https://w3id.org/italia/onto/HER> ;
            rdfs:label "ERC Project"@en ,
                       "Progetto ERC"@it .


###  https://w3id.org/italia/onto/HER/ERCResearchDomain
:ERCResearchDomain rdf:type owl:Class ;
                   rdfs:subClassOf :ERCClassification ;
                   rdfs:comment "Scientific domains to which the 25 ERC panels -used for the planning and operation of the evaluation of ERC grant proposals- are assigned to. They cover all fields of science, engineering and scholarship which, concretely: Social Sciences and Humanities (6 Panels, SH1–SH6), Physical Sciences and Engineering (10 Panels, PE1–PE10), Life Sciences (9 Panels, LS1–LS9)."@en ,
                                "Settori scientifici ai quali sono assegnati i 25 gruppi di esperti scientifici del CER - utilizzati per la pianificazione e il funzionamento della valutazione delle proposte di sovvenzione del CER -. Essi coprono tutti i campi della scienza, dell'ingegneria e delle borse di studio che, in concreto: Scienze sociali e umanistiche (6 gruppi, SH1-SH6), Scienze fisiche e ingegneria (10 gruppi, PE1-PE10), Scienze della vita (9 gruppi, LS1-LS9)."@it ;
                   rdfs:isDefinedBy <https://w3id.org/italia/onto/HER> ;
                   rdfs:label "Dominio di ricerca ERC"@it ,
                              "ERC Research Domain"@en ;
                   prov:wasDerivedFrom skos:Concept ;
                   l0:controlledVocabulary <https://w3id.org/italia/controlled-vocabulary/classifications-for-her/erc-panel-h2020-fp> .


###  https://w3id.org/italia/onto/HER/ERCSubpanel
:ERCSubpanel rdf:type owl:Class ;
             rdfs:subClassOf :ERCClassification ;
             rdfs:isDefinedBy <https://w3id.org/italia/onto/HER> ;
             prov:wasDerivedFrom skos:Concept ;
             l0:controlledVocabulary <https://w3id.org/italia/controlled-vocabulary/classifications-for-her/erc-panel-h2020-fp> .


###  https://w3id.org/italia/onto/HER/EUREKACluster
:EUREKACluster rdf:type owl:Class ;
               rdfs:subClassOf l0:Concept ,
                               [ rdf:type owl:Restriction ;
                                 owl:onProperty <https://w3id.org/italia/onto/CLV/hasSpatialCoverage> ;
                                 owl:allValuesFrom <https://w3id.org/italia/onto/CLV/Feature>
                               ] ;
               rdfs:comment "EUREKA Clusters are strategic initiatives proposed and led by industry, developing generic technologies of key importance for European competitiveness"@en ,
                            "I Cluster EUREKA sono iniziative strategiche proposte e guidate dall'industria, che sviluppano tecnologie generiche di importanza fondamentale per la competitività europea"@it ;
               rdfs:isDefinedBy <https://w3id.org/italia/onto/HER> ;
               rdfs:label "EUREKA Cluster"@en ,
                          "Gruppo EUREKA"@it ;
               prov:wasDerivedFrom skos:Concept .


###  https://w3id.org/italia/onto/HER/EUREKAInstrument
:EUREKAInstrument rdf:type owl:Class ;
                  rdfs:subClassOf :HERClassification ;
                  rdfs:comment "EUREKA financial instrument. EUREKA instruments are of several kinds, and their choice depends mainly on the type of research project to be developed (Eurostars, Clusters, Network projects and InvestHorizon)."@en ,
                               "Strumento finanziario EUREKA. Gli strumenti EUREKA sono di vario tipo e la loro scelta dipende principalmente dal tipo di progetto di ricerca da sviluppare (Eurostars, Clusters, progetti di rete e InvestHorizon)."@it ;
                  rdfs:isDefinedBy <https://w3id.org/italia/onto/HER> ;
                  rdfs:label "EUREKA Instrument"@en ,
                             "Strumento EUREKA"@it ;
                  prov:wasDerivedFrom skos:Concept .


###  https://w3id.org/italia/onto/HER/EUREKAMarketArea
:EUREKAMarketArea rdf:type owl:Class ;
                  rdfs:subClassOf :HERClassification ;
                  rdfs:comment "Area di mercato EUREKA (Prodotti industriali / Produzione; Medicina / Salute; Trasporti; Consumer Related)"@it ,
                               "EUREKA Market area (Industrial Products / Manufacturing; Medical / Health Related; Transportation; Consumer Related)"@en ;
                  rdfs:isDefinedBy <https://w3id.org/italia/onto/HER> ;
                  rdfs:label "Area di mercato EUREKA"@it ,
                             "EUREKA Market Area"@en ;
                  prov:wasDerivedFrom skos:Concept .


###  https://w3id.org/italia/onto/HER/EUREKAParticipant
:EUREKAParticipant rdf:type owl:Class ;
                   rdfs:subClassOf <https://w3id.org/italia/onto/RO/TimeIndexedRole> ,
                                   [ rdf:type owl:Restriction ;
                                     owl:onProperty :hasParticipationCountry ;
                                     owl:allValuesFrom <https://w3id.org/italia/onto/CLV/Country>
                                   ] ;
                   rdfs:comment "Partecipanti in progetto EUREKA"@it ,
                                "Participant in a EUREKA project"@en ;
                   rdfs:isDefinedBy <https://w3id.org/italia/onto/HER> ;
                   rdfs:label "EUREKA Participant"@en ,
                              "Partecipante EUREKA"@it .


###  https://w3id.org/italia/onto/HER/EUREKAProject
:EUREKAProject rdf:type owl:Class ;
               rdfs:subClassOf <https://w3id.org/italia/onto/Project/PublicResearchProject> ,
                               [ rdf:type owl:Restriction ;
                                 owl:onProperty :eurekaProjectId ;
                                 owl:cardinality "1"^^xsd:nonNegativeInteger
                               ] ;
               rdfs:comment "Project funded by the EUREKA network."@en ,
                            "Project funded by the EUREKA network."@it ;
               rdfs:isDefinedBy <https://w3id.org/italia/onto/HER> ;
               rdfs:label "EUREKA Project"@en ,
                          "Progetto EUREKA"@it .


###  https://w3id.org/italia/onto/HER/EUREKATechArea
:EUREKATechArea rdf:type owl:Class ;
                rdfs:subClassOf :HERClassification ;
                rdfs:comment "Area tecnologica EUREKA (Elettronica, IT e tecnologia delle telecomunicazioni; Produzione industriale, materiali e trasporti; Scienze / tecnologie biologiche; Tecnologia per la protezione dell'uomo e dell'ambiente; Tecnologia energetica)"@it ,
                             "EUREKA Tecnological area (Electronics, IT and Telecoms Technology; Industrial Manufacturing, Material and Transport; Biological Sciences / Technologies; Technology for Protecting Man and the Environment; Energy Technology)"@en ;
                rdfs:isDefinedBy <https://w3id.org/italia/onto/HER> ;
                rdfs:label "Area tecnica EUREKA"@it ,
                           "EUREKA Tech Area"@en ;
                prov:wasDerivedFrom skos:Concept .


###  https://w3id.org/italia/onto/HER/ErasmusPlusActionType
:ErasmusPlusActionType rdf:type owl:Class ;
                       rdfs:subClassOf :ErasmusPlusClassification ;
                       rdfs:comment "It refers to the specific action type within each Key action."@en ,
                                    "Si riferisce al tipo di azione specifica all'interno di ogni azione chiave."@it ;
                       rdfs:isDefinedBy <https://w3id.org/italia/onto/HER> ;
                       rdfs:label "Erasmus+ Action Type"@en ,
                                  "Tipo di azione Erasmus+"@it ;
                       prov:wasDerivedFrom skos:Concept .


###  https://w3id.org/italia/onto/HER/ErasmusPlusClassification
:ErasmusPlusClassification rdf:type owl:Class ;
                           rdfs:subClassOf :ECClassification ;
                           rdfs:comment "It is used to classify the erasmus plus projects under the European Commission classification."@en ,
                                        "Viene utilizzato per classificare i progetti erasmus plus nella classificazione della Commissione Europea."@it ;
                           rdfs:isDefinedBy <https://w3id.org/italia/onto/HER> ;
                           rdfs:label "Erasmus+ Classification"@en ,
                                      "classificazione Erasmus+"@it ;
                           prov:wasDerivedFrom skos:ConceptScheme .


###  https://w3id.org/italia/onto/HER/ErasmusPlusFile
:ErasmusPlusFile rdf:type owl:Class ;
                 rdfs:subClassOf l0:Object ,
                                 [ rdf:type owl:Restriction ;
                                   owl:onProperty <https://w3id.org/italia/onto/SM/URL> ;
                                   owl:allValuesFrom xsd:anyURI
                                 ] ,
                                 [ rdf:type owl:Restriction ;
                                   owl:onProperty l0:name ;
                                   owl:allValuesFrom rdfs:Literal
                                 ] ,
                                 [ rdf:type owl:Restriction ;
                                   owl:onProperty l0:identifier ;
                                   owl:cardinality "1"^^xsd:nonNegativeInteger
                                 ] ;
                 rdfs:comment """It refers to the output result file of an erasmus plus project.
The file tipycally is available by an url provided by the European Commission."""@en ,
                              """Si riferisce al file dei risultati di un progetto erasmus plus.
Il file è tipicamente disponibile tramite un url fornito dalla Commissione Europea."""@it ;
                 rdfs:isDefinedBy <https://w3id.org/italia/onto/HER> ;
                 rdfs:label "Erasmus+ File"@en ,
                            "File Erasmus+"@it .


###  https://w3id.org/italia/onto/HER/ErasmusPlusKeyAction
:ErasmusPlusKeyAction rdf:type owl:Class ;
                      rdfs:subClassOf :ErasmusPlusClassification ;
                      rdfs:comment """It refers to the collective name for activities and projects that can be funded under Erasmus+.
There are three Key Action areas which can be summarised as:
- Key Action 1 (Mobility)
- Key Action 2 (Cooperation for Innovation and Exchange of Good Practices)
- Key Action 3 (Support for Policy Reform)"""@en ,
                                   """Si riferisce al nome collettivo per le attività e i progetti che possono essere finanziati nell'ambito di Erasmus+.
Ci sono tre aree di azione chiave che possono essere riassunte come:
- Azione chiave 1 (Mobilità)
- Azione chiave 2 (Cooperazione per l'innovazione e lo scambio di buone pratiche)
- Azione chiave 3 (Sostegno alla riforma delle politiche)"""@it ;
                      rdfs:isDefinedBy <https://w3id.org/italia/onto/HER> ;
                      rdfs:label "Azione chiave Erasmus+"@it ,
                                 "Erasmus+ Key Action"@en ;
                      prov:wasDerivedFrom skos:Concept .


###  https://w3id.org/italia/onto/HER/ErasmusPlusParticipant
:ErasmusPlusParticipant rdf:type owl:Class ;
                        rdfs:subClassOf <https://w3id.org/italia/onto/RO/TimeIndexedRole> ,
                                        [ rdf:type owl:Restriction ;
                                          owl:onProperty <https://w3id.org/italia/onto/CLV/hasSpatialCoverage> ;
                                          owl:allValuesFrom <https://w3id.org/italia/onto/CLV/Feature>
                                        ] ,
                                        [ rdf:type owl:Restriction ;
                                          owl:onProperty :hasParticipationCountry ;
                                          owl:allValuesFrom <https://w3id.org/italia/onto/CLV/Country>
                                        ] ,
                                        [ rdf:type owl:Restriction ;
                                          owl:onProperty :picNumber ;
                                          owl:cardinality "1"^^xsd:nonNegativeInteger
                                        ] ;
                        rdfs:comment """It refers to the entities which are involved in the Erasmus+ projects.
The entities could be both universities and private organizations."""@en ,
                                     """Si riferisce alle entità coinvolte nei progetti Erasmus+.
Le entità potrebbero essere sia università che organizzazioni private."""@it ;
                        rdfs:isDefinedBy <https://w3id.org/italia/onto/HER> ;
                        rdfs:label "Erasmus+ Participant"@en ,
                                   "Partecipante Erasmus+"@it .


###  https://w3id.org/italia/onto/HER/ErasmusPlusProgramme
:ErasmusPlusProgramme rdf:type owl:Class ;
                      rdfs:subClassOf :ECProgramme ,
                                      :ErasmusPlusClassification ;
                      rdfs:comment "It refers to the funding programme (for example, Erasmus)."@en ,
                                   "Si riferisce al programma di finanziamento (per esempio, Erasmus)."@it ;
                      rdfs:isDefinedBy <https://w3id.org/italia/onto/HER> ;
                      rdfs:label "Erasmus+ Programme"@en ,
                                 "Programma Erasmus+"@it ;
                      prov:wasDerivedFrom skos:Concept .


###  https://w3id.org/italia/onto/HER/ErasmusPlusProject
:ErasmusPlusProject rdf:type owl:Class ;
                    rdfs:subClassOf <https://w3id.org/italia/onto/Project/PublicInvestmentProject> ;
                    rdfs:comment "It refers to projects under the funding scheme \"Erasmus+\" from the European Union for education, training, youth and sport in Europe."@en ,
                                 "Si riferisce a progetti nell'ambito del programma di finanziamento \"Erasmus+\" dell'Unione Europea per l'istruzione, la formazione, la gioventù e lo sport in Europa."@it ;
                    rdfs:isDefinedBy <https://w3id.org/italia/onto/HER> ;
                    rdfs:label "Erasmus+ Project"@en ,
                               "Progetto Erasmus+"@it .


###  https://w3id.org/italia/onto/HER/ErasmusPlusProjectResult
:ErasmusPlusProjectResult rdf:type owl:Class ;
                          rdfs:subClassOf :Result ,
                                          [ rdf:type owl:Restriction ;
                                            owl:onProperty :distributedInErasumplusFile ;
                                            owl:maxQualifiedCardinality "1"^^xsd:nonNegativeInteger ;
                                            owl:onClass :ErasmusPlusFile
                                          ] ;
                          rdfs:comment "It is used to address results for erasmus plus projects that have ended."@en ,
                                       "Viene utilizzato per indicare i risultati dei progetti erasmus plus che si sono conclusi."@it ;
                          rdfs:isDefinedBy <https://w3id.org/italia/onto/HER> ;
                          rdfs:label "Erasmus+ Project Result"@en ,
                                     "Risultato progetto Erasmus+"@it .


###  https://w3id.org/italia/onto/HER/ErasmusPlusTopic
:ErasmusPlusTopic rdf:type owl:Class ;
                  rdfs:subClassOf :ErasmusPlusClassification ;
                  rdfs:comment "Quando disponibile, si riferisce all'argomento o agli argomenti principali del progetto."@it ,
                               "When available, it refers to the main topic(s) of the project."@en ;
                  rdfs:isDefinedBy <https://w3id.org/italia/onto/HER> ;
                  rdfs:label "Argomento Erasmus+"@it ,
                             "Erasmus+ Topic"@en ;
                  prov:wasDerivedFrom skos:Concept .


###  https://w3id.org/italia/onto/HER/FORDClassification
:FORDClassification rdf:type owl:Class ;
                    rdfs:subClassOf :HERClassification ;
                    rdfs:comment "La classificazione Fields of research and development (FORD) viene utilizzata per classificare le unità e le risorse di R&S in base ai campi di indagine, vale a dire ampi domini di conoscenza basati principalmente sul contenuto della materia di R&S. (Fonte: http://uis.unesco.org/en/glossary-term/fields-research-and-development-ford)"@it ,
                                 "The Fields of research and development (FORD) classification is used to classify R&D units and resources by fields of enquiry, namely, broad knowledge domains based primarily on the content of the R&D subject matter. (Source: http://uis.unesco.org/en/glossary-term/fields-research-and-development-ford)"@en ;
                    rdfs:isDefinedBy <https://w3id.org/italia/onto/HER> ;
                    rdfs:label "Classificazione FORD"@it ,
                               "FORD Classification"@en ;
                    prov:wasDerivedFrom skos:Concept ;
                    l0:controlledVocabulary <https://w3id.org/italia/controlled-vocabulary/classifications-for-her/fields-of-research-development> .


###  https://w3id.org/italia/onto/HER/HERClassification
:HERClassification rdf:type owl:Class ;
                   rdfs:subClassOf l0:Topic ;
                   rdfs:isDefinedBy <https://w3id.org/italia/onto/HER> ;
                   prov:wasDerivedFrom skos:ConceptScheme .


###  https://w3id.org/italia/onto/HER/ISCEDFClassification
:ISCEDFClassification rdf:type owl:Class ;
                      rdfs:subClassOf :HERClassification ;
                      rdfs:comment "La classificazione internazionale standard dell'istruzione (ISCED) è un quadro per l'assemblaggio, la compilazione e l'analisi di statistiche comparabili a livello transnazionale sull'istruzione. (Fonte: https://unesdoc.unesco.org/ark:/48223/pf0000228085)"@it ,
                                   "The International Standard Classification of Education (ISCED) is a framework for assembling, compiling and analysing cross-nationally comparable statistics on education. (Source: https://unesdoc.unesco.org/ark:/48223/pf0000228085)"@en ;
                      rdfs:isDefinedBy <https://w3id.org/italia/onto/HER> ;
                      rdfs:label "Classificazione ISCED-F"@it ,
                                 "ISCED-F Classification"@en ;
                      prov:wasDerivedFrom skos:Concept .


###  https://w3id.org/italia/onto/HER/InternationalPatentClassification
:InternationalPatentClassification rdf:type owl:Class ;
                                   rdfs:subClassOf l0:Topic ;
                                   rdfs:comment "La classificazione internazionale dei brevetti (IPC), istituita dall'accordo di Strasburgo del 1971, prevede un sistema gerarchico di simboli indipendenti dal linguaggio per la classificazione dei brevetti e dei modelli di utilità in base alle diverse aree tecnologiche a cui si riferiscono."@it ,
                                                "The International Patent Classification (IPC), established by the Strasbourg Agreement 1971, provides for a hierarchical system of language independent symbols for the classification of patents and utility models according to the different areas of technology to which they pertain."@en ;
                                   rdfs:isDefinedBy <https://w3id.org/italia/onto/HER> ;
                                   rdfs:label "Classificazione internazionale dei brevetti"@it ,
                                              "International Patent Classification"@en ;
                                   prov:wasDerivedFrom skos:ConceptScheme .


###  https://w3id.org/italia/onto/HER/ItalianAcademicRole
:ItalianAcademicRole rdf:type owl:Class ;
                     rdfs:subClassOf :AcademicRole ;
                     rdfs:comment """It refers to the academic position held. In the Italian university system,
there are the following academic roles:
- Full professor (or first-tier professor) who is admitted after a competition;
- Associate professor (or second level professor) to whom access is granted following a competition;
- Adjunct professor;
- Temporary lecturer;
- Assistant Professor;
- Research fellow;
- Assistant Professor (tenure track);
- Postdoctoral Researcher
- Professor Emeritus"""@en ,
                                  """Si riferisce alla posizione accademica ricoperta. Nel sistema universitario italiano,
ci sono i seguenti ruoli accademici:
- Professore ordinario (o professore di primo livello) che viene ammesso dopo un concorso;
- Professore associato (o professore di secondo livello) al quale viene concesso l'accesso a seguito di un concorso;
- Professore aggiunto;
- Docente temporaneo;
- Professore assistente;
- Ricercatore;
- Professore assistente (cattedra di ruolo);
- Ricercatore post-dottorato
- Professore emerito"""@it ;
                     rdfs:isDefinedBy <https://w3id.org/italia/onto/HER> ;
                     rdfs:label "Italian Academic Role"@en ,
                                "Ruolo accademico italiano"@it ;
                     prov:wasDerivedFrom skos:Concept ;
                     l0:controlledVocabulary <https://w3id.org/italia/controlled-vocabulary/classifications-for-universitites/italian-academic-roles> .


###  https://w3id.org/italia/onto/HER/ItalianDegree
:ItalianDegree rdf:type owl:Class ;
               rdfs:subClassOf :AcademicDegree ;
               rdfs:comment "It is refers to Italian degree qualification that students can award upon successful completion of a course of study in higher education, usually at a college or university."@en ,
                            "Si riferisce al titolo di studio di laurea italiano che gli studenti possono rilasciare al termine di un corso di studi nell'ambito dell'istruzione superiore, di solito presso un college o un'università."@it ;
               rdfs:isDefinedBy <https://w3id.org/italia/onto/HER> ;
               rdfs:label "Italian Degree"@en ,
                          "Laurea italiana"@it .


###  https://w3id.org/italia/onto/HER/ItalianDiploma
:ItalianDiploma rdf:type owl:Class ;
                rdfs:subClassOf :Diploma ;
                rdfs:comment "It is refers to the Italian maturity diploma that can be award upon successful completion of secondary education"@en ,
                             "Si riferisce al diploma di maturità italiano che può essere rilasciato al termine del ciclo di studi secondari."@it ;
                rdfs:isDefinedBy <https://w3id.org/italia/onto/HER> ;
                rdfs:label "Diploma italiano"@it ,
                           "Italian Diploma"@en .


###  https://w3id.org/italia/onto/HER/ItalianPhDCourse
:ItalianPhDCourse rdf:type owl:Class ;
                  rdfs:subClassOf :PhDCourse ;
                  rdfs:comment "A PhD courses provided by an Italian university."@en ,
                               "Un corso di dottorato di ricerca previsot da un'universitá italiana."@it ;
                  rdfs:isDefinedBy <https://w3id.org/italia/onto/HER> ;
                  rdfs:label "Corso di Dottorato Italiano"@it ,
                             "Italian PhD Course"@en .


###  https://w3id.org/italia/onto/HER/ItalianPhDCourseByCycle
:ItalianPhDCourseByCycle rdf:type owl:Class ;
                         rdfs:subClassOf l0:EventOrSituation ;
                         rdfs:comment "Rapporti con i corsi di dottorato di ricerca che offre ogni anno."@it ,
                                      "Reified relationship that related an university with the PhD courses it offers each cycle year."@en ;
                         rdfs:isDefinedBy <https://w3id.org/italia/onto/HER> ;
                         rdfs:label "Corsi di PHD italian per ciclo accademico"@it ,
                                    "Italian PhD Course By Academic Cycle"@en .


###  https://w3id.org/italia/onto/HER/ItalianStudentType
:ItalianStudentType rdf:type owl:Class ;
                    rdfs:subClassOf <https://w3id.org/italia/onto/RO/Role> ;
                    rdfs:comment "Tipo di studente nel sistema accademico italiano (Immatricolato, Iscritto, Laureato, Dottorato, ...)"@it ,
                                 "Type of student in the Italian academic system."@en ;
                    rdfs:isDefinedBy <https://w3id.org/italia/onto/HER> ;
                    rdfs:label "Italian Student Type"@en ,
                               "Tipo di studente italiano"@it .


###  https://w3id.org/italia/onto/HER/MIURStudentsAggregate
:MIURStudentsAggregate rdf:type owl:Class ;
                       rdfs:subClassOf :StatisticalDataAggregation ;
                       rdfs:comment "Aggregated data on Italian students filed in the MIUR system, grouped by year and university."@en ,
                                    "Dati aggregati sugli studenti italiani archiviati nel sistema MIUR, raggruppati per anno e per università."@it ;
                       rdfs:isDefinedBy <https://w3id.org/italia/onto/HER> ;
                       rdfs:label "Aggregate of Italian Students"@en ,
                                  "Aggregazione dei studenti italiani"@it .


###  https://w3id.org/italia/onto/HER/MIURStudentsByCitizenshipAggregate
:MIURStudentsByCitizenshipAggregate rdf:type owl:Class ;
                                    rdfs:subClassOf :StatisticalDataAggregation ;
                                    rdfs:comment "Aggregated data on Italian students filed in the MIUR system, grouped by year, university and citizenship."@en ,
                                                 "Dati aggregati sugli studenti italiani archiviati nel sistema MIUR, raggruppati per anno, università e cittadinanza."@it ;
                                    rdfs:isDefinedBy <https://w3id.org/italia/onto/HER> ;
                                    rdfs:label "Aggregate of Italian Students By Citizenship"@en ,
                                               "Aggregazione dei studenti italiani per cittadinanza"@it .


###  https://w3id.org/italia/onto/HER/MIURStudentsByCitizenshipDegreeAggregate
:MIURStudentsByCitizenshipDegreeAggregate rdf:type owl:Class ;
                                          rdfs:subClassOf :StatisticalDataAggregation ;
                                          rdfs:comment "Aggregated data on Italian students filed in the MIUR system, grouped by year, university, citizenship and degree."@en ,
                                                       "Dati aggregati sugli studenti italiani archiviati nel sistema MIUR, raggruppati per anno, università, cittadinanza e laurea."@it ;
                                          rdfs:isDefinedBy <https://w3id.org/italia/onto/HER> ;
                                          rdfs:label "Aggregate of Italian Students By Citizenship and Degree"@en ,
                                                     "Aggregazione dei studenti italiani per cittadinanza e laurea"@it .


###  https://w3id.org/italia/onto/HER/MIURStudentsByCitizenshipDegreeClassAggregate
:MIURStudentsByCitizenshipDegreeClassAggregate rdf:type owl:Class ;
                                               rdfs:subClassOf :StatisticalDataAggregation ;
                                               rdfs:comment "Aggregated data on Italian students filed in the MIUR system, grouped by year, university, citizenship, degree and degree class."@en ,
                                                            "Dati aggregati sugli studenti italiani archiviati nel sistema MIUR, raggruppati per anno, università, cittadinanza, laurea e classe di laurea."@it ;
                                               rdfs:isDefinedBy <https://w3id.org/italia/onto/HER> ;
                                               rdfs:label "Aggregate of Italian Students By Citizenship, Degree and Degree Class"@en ,
                                                          "Aggregazione dei studenti italiani per cittadinanza, laurea e classe di laurea"@it .


###  https://w3id.org/italia/onto/HER/MIURStudentsByCitizenshipDegreeDegreeClassAggregate
:MIURStudentsByCitizenshipDegreeDegreeClassAggregate rdf:type owl:Class ;
                                                     rdfs:subClassOf :StatisticalDataAggregation ;
                                                     rdfs:comment "Aggregated data on Italian students filed in the MIUR system, grouped by year, university, citizenship and degree class."@en ,
                                                                  "Dati aggregati sugli studenti italiani archiviati nel sistema MIUR, raggruppati per anno, università, cittadinanza e classe di laurea."@it ;
                                                     rdfs:isDefinedBy <https://w3id.org/italia/onto/HER> ;
                                                     rdfs:label "Aggregate of Italian Students By Citizenship and Degree Class"@en ,
                                                                "Aggregazione dei studenti italiani per cittadinanza e classe di laurea"@it .


###  https://w3id.org/italia/onto/HER/MIURStudentsByDegreeDegreeClassAggregate
:MIURStudentsByDegreeDegreeClassAggregate rdf:type owl:Class ;
                                          rdfs:subClassOf :StatisticalDataAggregation ;
                                          rdfs:comment "Aggregated data on Italian students filed in the MIUR system, grouped by year, university, citizenship and degree class."@en ,
                                                       "Dati aggregati sugli studenti italiani archiviati nel sistema MIUR, raggruppati per anno, università, cittadinanza e classe di laurea."@it ;
                                          rdfs:isDefinedBy <https://w3id.org/italia/onto/HER> ;
                                          rdfs:label "Aggregate of Italian Students By Degree and Degree Class"@en ,
                                                     "Aggregazione dei studenti italiani per laurea e classe di laurea"@it .


###  https://w3id.org/italia/onto/HER/MIURStudentsByDiplomaAggregate
:MIURStudentsByDiplomaAggregate rdf:type owl:Class ;
                                rdfs:subClassOf :StatisticalDataAggregation ;
                                rdfs:comment "Aggregated data on Italian students filed in the MIUR system, grouped by year, university and diploma."@en ,
                                             "Dati aggregati sugli studenti italiani archiviati nel sistema MIUR, raggruppati per anno, università e diploma."@it ;
                                rdfs:isDefinedBy <https://w3id.org/italia/onto/HER> ;
                                rdfs:label "Aggregate of Italian Students By Diploma"@en ,
                                           "Aggregazione dei studenti italiani per diploma"@it .


###  https://w3id.org/italia/onto/HER/MIURStudentsByDiplomaDegreeDegreeClassAggregate
:MIURStudentsByDiplomaDegreeDegreeClassAggregate rdf:type owl:Class ;
                                                 rdfs:subClassOf :StatisticalDataAggregation ;
                                                 rdfs:comment "Aggregated data on Italian students filed in the MIUR system, grouped by year, university, diploma, degree and degree class."@en ,
                                                              "Dati aggregati sugli studenti italiani archiviati nel sistema MIUR, raggruppati per anno, università, diploma, laurea e classe di laurea."@it ;
                                                 rdfs:isDefinedBy <https://w3id.org/italia/onto/HER> ;
                                                 rdfs:label "Aggregate of Italian Students By Diploma, Degree and Degree Class"@en ,
                                                            "Aggregazione dei studenti italiani per diploma, laurea e classe di laurea"@it .


###  https://w3id.org/italia/onto/HER/MIURStudentsByProvinceOfResidenceAggregate
:MIURStudentsByProvinceOfResidenceAggregate rdf:type owl:Class ;
                                            rdfs:subClassOf :StatisticalDataAggregation ,
                                                            [ rdf:type owl:Restriction ;
                                                              owl:onProperty <https://w3id.org/italia/onto/CLV/hasSpatialCoverage> ;
                                                              owl:someValuesFrom <https://w3id.org/italia/onto/CLV/Province>
                                                            ] ;
                                            rdfs:comment "Aggregated data on Italian students filed in the MIUR system, grouped by year, university and Italian province of residence."@en ,
                                                         "Dati aggregati sugli studenti italiani archiviati nel sistema MIUR, raggruppati per anno, università e provincia di residenza italiana."@it ;
                                            rdfs:isDefinedBy <https://w3id.org/italia/onto/HER> ;
                                            rdfs:label "Aggregate of Italian Students By Province of Residence"@en ,
                                                       "Aggregazione dei studenti italiani per provincia di residenza"@it .


###  https://w3id.org/italia/onto/HER/MIURStudentsByProvinceOfResidenceDegreeDegreeClassAggregate
:MIURStudentsByProvinceOfResidenceDegreeDegreeClassAggregate rdf:type owl:Class ;
                                                             rdfs:subClassOf :StatisticalDataAggregation ,
                                                                             [ rdf:type owl:Restriction ;
                                                                               owl:onProperty <https://w3id.org/italia/onto/CLV/hasSpatialCoverage> ;
                                                                               owl:someValuesFrom <https://w3id.org/italia/onto/CLV/Province>
                                                                             ] ;
                                                             rdfs:comment "Aggregated data on Italian students filed in the MIUR system, grouped by year, university, Italian province of residence, degree and degree class."@en ,
                                                                          "Dati aggregati sugli studenti italiani archiviati nel sistema MIUR, raggruppati per anno, università, provincia di residenza italiana, laurea e classe di laurea."@it ;
                                                             rdfs:isDefinedBy <https://w3id.org/italia/onto/HER> ;
                                                             rdfs:label "Aggregate of Italian Students By Province of Residence, Degree and Degree Class"@en ,
                                                                        "Aggregazione dei studenti italiani per provincia di residenza, laurea e classe di laurea"@it .


###  https://w3id.org/italia/onto/HER/MIURStudentsByRegionOfResidenceAggregate
:MIURStudentsByRegionOfResidenceAggregate rdf:type owl:Class ;
                                          rdfs:subClassOf :StatisticalDataAggregation ,
                                                          [ rdf:type owl:Restriction ;
                                                            owl:onProperty <https://w3id.org/italia/onto/CLV/hasSpatialCoverage> ;
                                                            owl:someValuesFrom <https://w3id.org/italia/onto/CLV/Region>
                                                          ] ;
                                          rdfs:comment "Aggregated data on Italian students filed in the MIUR system, grouped by year, university and Italian region of residence."@en ,
                                                       "Dati aggregati sugli studenti italiani archiviati nel sistema MIUR, raggruppati per anno, università e regione di residenza italiana."@it ;
                                          rdfs:isDefinedBy <https://w3id.org/italia/onto/HER> ;
                                          rdfs:label "Aggregate of Italian Students By Region of Residence"@en ,
                                                     "Aggregazione dei studenti italiani per regione di residenza"@it .


###  https://w3id.org/italia/onto/HER/MIURStudentsByRegionOfResidenceDegreeDegreeClassAggregate
:MIURStudentsByRegionOfResidenceDegreeDegreeClassAggregate rdf:type owl:Class ;
                                                           rdfs:subClassOf :StatisticalDataAggregation ,
                                                                           [ rdf:type owl:Restriction ;
                                                                             owl:onProperty <https://w3id.org/italia/onto/CLV/hasSpatialCoverage> ;
                                                                             owl:someValuesFrom <https://w3id.org/italia/onto/CLV/Region>
                                                                           ] ;
                                                           rdfs:comment "Aggregated data on Italian students filed in the MIUR system, grouped by year, university, Italian region of residence, degree and degree class."@en ,
                                                                        "Dati aggregati sugli studenti italiani archiviati nel sistema MIUR, raggruppati per anno, università, regione di residenza italiana, laurea e classe di laurea."@it ;
                                                           rdfs:isDefinedBy <https://w3id.org/italia/onto/HER> ;
                                                           rdfs:label "Aggregate of Italian Students By Region of Residence, Degree and Degree Class"@en ,
                                                                      "Aggregazione dei studenti italiani per regione di residenza, laurea e classe di laurea"@it .


###  https://w3id.org/italia/onto/HER/MacroSector
:MacroSector rdf:type owl:Class ;
             rdfs:subClassOf :AcademicDiscipline ;
             rdfs:isDefinedBy <https://w3id.org/italia/onto/HER> ;
             prov:wasDerivedFrom skos:Concept ;
             l0:controlledVocabulary <https://w3id.org/italia/controlled-vocabulary/classifications-for-universities/academic-disciplines> .


###  https://w3id.org/italia/onto/HER/Patent
:Patent rdf:type owl:Class ;
        rdfs:subClassOf :Result ,
                        [ rdf:type owl:Restriction ;
                          owl:onProperty :hasPatentPriorityDetail ;
                          owl:someValuesFrom :PatentPriorityDetail
                        ] ,
                        [ rdf:type owl:Restriction ;
                          owl:onProperty :hasIPC ;
                          owl:allValuesFrom :InternationalPatentClassification
                        ] ,
                        [ rdf:type owl:Restriction ;
                          owl:onProperty :patentApplicationNo ;
                          owl:cardinality "1"^^xsd:nonNegativeInteger
                        ] ,
                        [ rdf:type owl:Restriction ;
                          owl:onProperty :patentFamilyCode ;
                          owl:cardinality "1"^^xsd:nonNegativeInteger
                        ] ,
                        [ rdf:type owl:Restriction ;
                          owl:onProperty :patentApplicationDate ;
                          owl:maxQualifiedCardinality "1"^^xsd:nonNegativeInteger ;
                          owl:onDataRange xsd:date
                        ] ;
        rdfs:comment "A granted patent, i.e. an intellectual property right for the owner to exclude others from making, using, selling and importing an invention"@en ,
                     "Un brevetto concesso, ovvero un diritto di proprietà intellettuale per il proprietario di escludere altri dal fare, utilizzare, vendere e importare un'invenzione"@it ;
        rdfs:isDefinedBy <https://w3id.org/italia/onto/HER> ;
        rdfs:label "Brevetto"@it ,
                   "Patent"@en .


###  https://w3id.org/italia/onto/HER/PatentPriorityDetail
:PatentPriorityDetail rdf:type owl:Class ;
                      rdfs:subClassOf l0:Description ,
                                      [ rdf:type owl:Restriction ;
                                        owl:onProperty :patentPriorityDate ;
                                        owl:qualifiedCardinality "1"^^xsd:nonNegativeInteger ;
                                        owl:onDataRange xsd:date
                                      ] ,
                                      [ rdf:type owl:Restriction ;
                                        owl:onProperty :patentPriorityNo ;
                                        owl:cardinality "1"^^xsd:nonNegativeInteger
                                      ] ;
                      rdfs:comment "A priority right or right of priority is a time-limited right, triggered by the first filing of an application for a patent. It allows the claimant to file a subsequent application in another country for the same invention as of the date of filing the first application."@en ,
                                   "Un diritto o diritto di priorità prioritario è un diritto limitato nel tempo, innescato dal primo deposito di una domanda di brevetto. Consente al richiedente di presentare una domanda successiva in un altro paese per la stessa invenzione a partire dalla data di deposito della prima domanda."@it ;
                      rdfs:isDefinedBy <https://w3id.org/italia/onto/HER> ;
                      rdfs:label "Dettagli sulla priorità dei brevetti"@it ,
                                 "Patent Priority Details"@en .


###  https://w3id.org/italia/onto/HER/PatentPublicationDetail
:PatentPublicationDetail rdf:type owl:Class ;
                         rdfs:subClassOf l0:Description ,
                                         [ rdf:type owl:Restriction ;
                                           owl:onProperty :patentKindCode ;
                                           owl:cardinality "1"^^xsd:nonNegativeInteger
                                         ] ,
                                         [ rdf:type owl:Restriction ;
                                           owl:onProperty :patentPublicationNumber ;
                                           owl:cardinality "1"^^xsd:nonNegativeInteger
                                         ] ,
                                         [ rdf:type owl:Restriction ;
                                           owl:onProperty :publicationDate ;
                                           owl:qualifiedCardinality "1"^^xsd:nonNegativeInteger ;
                                           owl:onDataRange xsd:date
                                         ] ;
                         rdfs:comment "Details of the patent publication (e.g. publication number, year, etc.)"@en ,
                                      "Dettagli della pubblicazione del brevetto (ad es. Numero di pubblicazione, anno, ecc.)"@it ;
                         rdfs:isDefinedBy <https://w3id.org/italia/onto/HER> ;
                         rdfs:label "Dettagli della pubblicazione del brevetto"@it ,
                                    "Patent Publication Details"@en .


###  https://w3id.org/italia/onto/HER/PatentPublicationStage
:PatentPublicationStage rdf:type owl:Class ;
                        rdfs:subClassOf l0:Object ,
                                        [ rdf:type owl:Restriction ;
                                          owl:onProperty :patentKindCode ;
                                          owl:cardinality "1"^^xsd:nonNegativeInteger
                                        ] ;
                        rdfs:comment "La fase in cui è attualmente in corso il processo di pubblicazione dei brevetti."@it ,
                                     "The stage in which the patent publication process is currently on."@en ;
                        rdfs:isDefinedBy <https://w3id.org/italia/onto/HER> ;
                        rdfs:label "Fase di pubblicazione del brevetto"@it ,
                                   "Patent Publication Stage"@en .


###  https://w3id.org/italia/onto/HER/PhDCourse
:PhDCourse rdf:type owl:Class ;
           rdfs:subClassOf l0:Object ;
           rdfs:comment "A PhD course."@en ,
                        "Un corso di dottorato di ricerca."@it ;
           rdfs:isDefinedBy <https://w3id.org/italia/onto/HER> ;
           rdfs:label "Corso di dottorato"@it ,
                      "PhD Course"@en .


###  https://w3id.org/italia/onto/HER/Programme
:Programme rdf:type owl:Class ;
           rdfs:subClassOf :HERClassification ,
                           l0:Description ,
                           [ rdf:type owl:Restriction ;
                             owl:onProperty l0:description ;
                             owl:someValuesFrom rdfs:Literal
                           ] ,
                           [ rdf:type owl:Restriction ;
                             owl:onProperty l0:name ;
                             owl:someValuesFrom rdfs:Literal
                           ] ,
                           [ rdf:type owl:Restriction ;
                             owl:onProperty l0:identifier ;
                             owl:maxCardinality "1"^^xsd:nonNegativeInteger
                           ] ;
           rdfs:comment "Questa classe raggruppa le classificazioni specifiche del progetto in base ai programmi."@it ,
                        "This class groups project-specific classifications based on programs."@en ;
           rdfs:isDefinedBy <https://w3id.org/italia/onto/HER> ;
           rdfs:label "Programma"@it ,
                      "Programme"@en ;
           prov:wasDerivedFrom skos:Concept .


###  https://w3id.org/italia/onto/HER/ReportedCitizenship
:ReportedCitizenship rdf:type owl:Class ;
                     rdfs:subClassOf l0:Characteristic ;
                     rdfs:comment """It refers to the citenzship of where a person was born. The possible values are:
- Italian
- Non italian"""@en ,
                                  """Si riferisce alla cittadinanza del luogo di nascita di una persona. I valori possibili sono:
- Italiano
- Non italiano"""@it ;
                     rdfs:isDefinedBy <https://w3id.org/italia/onto/HER> ;
                     rdfs:label "Cittadinanza riportata in sistemi nazionali scolastici"@it ,
                                "Reported Citizenship"@en .


###  https://w3id.org/italia/onto/HER/ResearcherSeniorityGrade
:ResearcherSeniorityGrade rdf:type owl:Class ;
                          rdfs:subClassOf <https://w3id.org/italia/onto/RO/Role> ;
                          rdfs:comment "La classificazione dell'UNESCO di professionisti impegnati nella concezione o nella creazione di nuove conoscenze (che conducono ricerche e migliorano o sviluppano concetti, teorie, modelli, tecniche di strumentazione, software o metodi operativi) in base ai livelli di anzianità. Si propone di utilizzare la seguente classificazione dei gradi / livelli di anzianità: Categoria A: il singolo voto / posto più alto in cui viene normalmente condotta la ricerca. Esempi: \"Direttore della ricerca\" o \"Professore ordinario\" Categoria B: Ricercatori che lavorano in posizioni non più alte della posizione più alta (A) ma più senior rispetto ai neolaureati qualificati (livello ISCED 8). Esempi: \"Ricercatore senior\" o \"Ricercatore principale\" o \"Professore associato\". Categoria C: il primo grado / posto in cui verrebbe normalmente assunto un dottorato di ricerca appena qualificato. Esempi: \"Ricercatore\" o \"Investigatore\" o \"Ricercatore\" o \"Dottorando post-dottorato\". Categoria D: Studenti di dottorato di livello CITE 8 impegnati come ricercatori o ricercatori che lavorano in posti che normalmente non richiedono un dottorato. Esempi: \"dottorandi\" o \"ricercatori junior\" (senza dottorato di ricerca). Anche gli studenti del Master che sono considerati ricercatori rientrerebbero in questa categoria."@it ,
                                       "UNESCO's clasification of professionals engaged in the conception or creation of new knowledge (who conduct research and improve or develop concepts, theories, models, techniques instrumentation, software or operational methods) by the seniority levels. It is proposed to use the following classification of seniority grades/levels: Category A: The single highest grade/post at which research is normally conducted. Examples: \"Director of research\" or \"Full professor\" Category B: Researchers working in positions not as senior as top position (A) but more senior than newly qualified doctoral graduates (ISCED level 8). Examples: \"Senior researcher\" or \"Principal investigator\" or \"Associate professor\". Category C: The first grade/post into which a newly qualified doctoral graduate would normally be recruited. Examples: \"Researcher\" or \"Investigator\" or \"Assistant professor\" or \"Post-doctoral fellow\". Category D: Either doctoral students at the ISCED level 8 who are engaged as researchers, or researchers working in posts that do not normally require a doctorate degree. Examples: \"Ph.D. students\" or \"Junior researchers\" (without a Ph.D.). Master’s students who are counted as researchers would also fall under this category."@en ;
                          rdfs:isDefinedBy <https://w3id.org/italia/onto/HER> ;
                          rdfs:label "Anzianità del ricercatore"@it ,
                                     "Researcher Seniority Grade"@en .


###  https://w3id.org/italia/onto/HER/Result
:Result rdf:type owl:Class ;
        rdfs:subClassOf l0:Object ,
                        [ rdf:type owl:Restriction ;
                          owl:onProperty :abstract ;
                          owl:someValuesFrom rdfs:Literal
                        ] ,
                        [ rdf:type owl:Restriction ;
                          owl:onProperty :title ;
                          owl:someValuesFrom rdfs:Literal
                        ] ,
                        [ rdf:type owl:Restriction ;
                          owl:onProperty :publicationDate ;
                          owl:qualifiedCardinality "1"^^xsd:nonNegativeInteger ;
                          owl:onDataRange xsd:date
                        ] ,
                        [ rdf:type owl:Restriction ;
                          owl:onProperty :resultType ;
                          owl:maxCardinality "1"^^xsd:nonNegativeInteger
                        ] ;
        rdfs:isDefinedBy <https://w3id.org/italia/onto/HER> .


###  https://w3id.org/italia/onto/HER/ScientificDisciplinarySector
:ScientificDisciplinarySector rdf:type owl:Class ;
                              rdfs:subClassOf :AcademicDiscipline ;
                              rdfs:isDefinedBy <https://w3id.org/italia/onto/HER> ;
                              prov:wasDerivedFrom skos:Concept ;
                              l0:controlledVocabulary <https://w3id.org/italia/controlled-vocabulary/classifications-for-universities/academic-disciplines> .


###  https://w3id.org/italia/onto/HER/Spinoff
:Spinoff rdf:type owl:Class ;
         rdfs:subClassOf covapit:PrivateOrganization ,
                         [ rdf:type owl:Restriction ;
                           owl:onProperty :foundedBy ;
                           owl:allValuesFrom covapit:Organization
                         ] ,
                         [ rdf:type owl:Restriction ;
                           owl:onProperty :hasOperationalSpinoffAddress ;
                           owl:allValuesFrom <https://w3id.org/italia/onto/CLV/Address>
                         ] ,
                         [ rdf:type owl:Restriction ;
                           owl:onProperty :additionalInfo ;
                           owl:allValuesFrom rdfs:Literal
                         ] ,
                         [ rdf:type owl:Restriction ;
                           owl:onProperty :foundationProject ;
                           owl:allValuesFrom rdfs:Literal
                         ] ,
                         [ rdf:type owl:Restriction ;
                           owl:onProperty :active ;
                           owl:qualifiedCardinality "1"^^xsd:nonNegativeInteger ;
                           owl:onDataRange xsd:boolean
                         ] ,
                         [ rdf:type owl:Restriction ;
                           owl:onProperty :innovative ;
                           owl:qualifiedCardinality "1"^^xsd:nonNegativeInteger ;
                           owl:onDataRange xsd:boolean
                         ] ;
         rdfs:comment "Enterprise created from a pre-existing entity or unit; in this specific dataset are included the spin-offs of public research: adopting the definition of the Netval 2014 report, an \"enterprise operating in high-tech sectors constituted by (at least) a university professor/researcher or a doctoral candidate/fellow/student who has carried out multiannual research activities on a specific theme, object of creation of the enterprise itself\".The data are obtained from Spin-off Italia, the spin-off database of public research in Italy: https://www.spinoffitalia.it/. As indicated by the website Spin-off Italia (https://www.spinoffitalia.it/?q=about), \"The database (Spin-off Italia, Editor's note) is the result of the collaboration between the Centre for Innovation and Entrepreneurship of the Polytechnic University of Marche, NetVal and the Management Institute of the Scuola Superiore Sant'Anna. The database contains information on the companies that the research group considered to associate with the spin-off concept of public research. In particular, in the database it is possible to select the companies that have been accredited as spin-offs by the research institutions of origin\"."@en ,
                      "Impresa creata a partire da un ente o un’unità preesistente; in questo specifico dataset vengono inclusi gli spin-off della ricerca pubblica: adottando la definizione del rapporto Netval 2014, una “impresa operante in settori high-tech costituita da (almeno) un professore/ricercatore universitario o da un dottorando/contrattista/studente che abbia effettuato attività di ricerca pluriennale su un tema specifico, oggetto di creazione dell’impresa stessa”. I dati sono ottenuti da Spin-off Italia, il database degli spin-off della ricerca pubblica in Italia: https://www.spinoffitalia.it/. Come indicato dal sito Spin-off Italia (https://www.spinoffitalia.it/?q=about), \"Il database (Spin-off Italia, NdR) è frutto della collaborazione fra il Centro per l'Innovazione e l'Imprenditorialità dell'Università Politecnica delle Marche, NetVal e l'Istituto di Management della Scuola Superiore Sant'Anna. Il database contiene informazioni sulle imprese che il gruppo di ricerca ha ritenuto di associare al concetto di spin-off della ricerca pubblica. In particolare, nel database è possibile selezionare le imprese che sono state accreditate come spin-off dagli enti di ricerca di provenienza.\""@it ;
         rdfs:isDefinedBy <https://w3id.org/italia/onto/HER> ;
         rdfs:label "Spinoff"@en ,
                    "Spinoff"@it .


###  https://w3id.org/italia/onto/HER/StatisticalDataAggregation
:StatisticalDataAggregation rdf:type owl:Class ;
                            rdfs:subClassOf l0:Collection ,
                                            [ rdf:type owl:Restriction ;
                                              owl:onProperty covapit:hasOrganization ;
                                              owl:maxQualifiedCardinality "1"^^xsd:nonNegativeInteger ;
                                              owl:onClass covapit:Organization
                                            ] ;
                            rdfs:isDefinedBy <https://w3id.org/italia/onto/HER> .


###  https://w3id.org/italia/onto/HER/USTATAverageContributionsAggregate
:USTATAverageContributionsAggregate rdf:type owl:Class ;
                                    rdfs:subClassOf :StatisticalDataAggregation ,
                                                    [ rdf:type owl:Restriction ;
                                                      owl:onProperty covapit:hasOrganization ;
                                                      owl:maxQualifiedCardinality "1"^^xsd:nonNegativeInteger ;
                                                      owl:onClass covapit:Organization
                                                    ] ;
                                    rdfs:comment "Information on the average contribution for students enrolled in I and II level degree courses (including single cycle courses) calculated on the basis of the fees actually paid (net of the regional tax for the DSU and stamp duty where applicable) ."@en ,
                                                 "Informazioni sulla contribuzione media per gli studenti iscritti a corsi di laurea di I e II livello (inclusi i corsi a ciclo unico) calcolata sulla base delle tasse realmente pagate (al netto della tassa regionale per il DSU e dell’imposta di bollo dove previste)."@it ;
                                    rdfs:isDefinedBy <https://w3id.org/italia/onto/HER> ;
                                    rdfs:label "Aggregazione della contribuzione media riportata da USTAT"@it ,
                                               "USTAT Aggregate of Average Contributions"@en .


###  https://w3id.org/italia/onto/HER/USTATCanteenServiceClass
:USTATCanteenServiceClass rdf:type owl:Class ;
                          rdfs:subClassOf l0:Characteristic ;
                          rdfs:comment """Information on accommodation and catering services at 1/11 of the reference year (T). In particular, the service provided is described through the identification code and description of the service: the possible values for codes and description are:
1 : Accommodation places in residences
2a: Accommodation in residences - of which assigned to eligible students (scholarship holders and non-scholarship holders)
4 : Accommodation in residences - of which allocated to non-eligible students
5 : Accommodation in residences - of which reserved for mobility students (e.g. Erasmus)
6 : Accommodation in residences - of which reserved for guest house use
7 : Directly managed canteens
8 : Seats in directly managed canteens
9 : Canteens under indirect management
10: Seats in indirectly managed canteens

When using the data take special care to avoid duplication, after carefully reading the code descriptions.
In particular, pay attention to the values indicated as \"\"of which...\"\", already included in the main entry."""@en ,
                                       """Informazioni sui posti alloggio e servizi di ristorazione all'1/11 dell'anno di riferimento (T). In particolare, il servizio erogato viene descritto tramite il codice identificativo e la descrizione del servizio: i valori possibili per codici e descrizione sono:
1 : Posti alloggio in residenze
2a: Posti alloggio in residenze - di cui assegnati a studenti idonei (borsisti e non borsisti)
4 : Posti alloggio in residenze - di cui assegnati a studenti non idonei
5 : Posti alloggio in residenze - di cui riservati a studenti in mobilità (es. Erasmus)
6 : Posti alloggio in residenze - di cui riservati ad uso foresteria
7 : Mense attive a gestione diretta
8 : Posti a sedere in mense a gestione diretta
9 : Mense attive a gestione indiretta
10: Posti a sedere in mense a gestione indiretta

Nell'utilizzo dei dati porre particolare attenzione ad evitare duplicazioni, dopo aver letto accuratamente le descrizioni dei codici.
In particolare fare attenzione ai valori indicati come \"\"di cui…\"\", già ricompresi nella voce principale.

"""@it ;
                          rdfs:isDefinedBy <https://w3id.org/italia/onto/HER> ;
                          rdfs:label "Classe di servizio mensa riportata da USTAT"@it ,
                                     "USTAT Reported Canteen Service Class"@en .


###  https://w3id.org/italia/onto/HER/USTATContributionByClass
:USTATContributionByClass rdf:type owl:Class ;
                          rdfs:subClassOf :StatisticalDataAggregation ;
                          rdfs:comment "Data relating to the contribution classes of university students. Indicates the distribution of students by class of contribution amount per capita, per Academic year (T-1)/(T)."@en ,
                                       "Dati relativi alle classi di contribuzione degli studenti universitari. Indica la distribuzione degli studenti per classe di importo della contribuzione pro-capite, per anno Accademico (T-1)/(T)"@it ;
                          rdfs:isDefinedBy <https://w3id.org/italia/onto/HER> ;
                          rdfs:label "Aggregazione dei contributi per classe riportati da USTAT"@it ,
                                     "USTAT Aggregate of Contributions By Class"@en .


###  https://w3id.org/italia/onto/HER/USTATContributionClass
:USTATContributionClass rdf:type owl:Class ;
                        rdfs:subClassOf l0:Characteristic ,
                                        [ rdf:type owl:Restriction ;
                                          owl:onProperty covapit:hasOrganization ;
                                          owl:maxQualifiedCardinality "1"^^xsd:nonNegativeInteger ;
                                          owl:onClass covapit:Organization
                                        ] ;
                        rdfs:comment "Data on university student contribution classes."@en ,
                                     "Dati relativi alle classi di contribuzione degli studenti universitari."@it ;
                        rdfs:isDefinedBy <https://w3id.org/italia/onto/HER> ;
                        rdfs:label "Classe di contribuzione USTAT"@it ,
                                   "USTAT Reported Contribution Class"@en .


###  https://w3id.org/italia/onto/HER/USTATContributionRevenue
:USTATContributionRevenue rdf:type owl:Class ;
                          rdfs:subClassOf :StatisticalDataAggregation ,
                                          [ rdf:type owl:Restriction ;
                                            owl:onProperty covapit:hasOrganization ;
                                            owl:maxQualifiedCardinality "1"^^xsd:nonNegativeInteger ;
                                            owl:onClass covapit:Organization
                                          ] ;
                          rdfs:comment "Data on the revenue from the student contribution of the universities, in particular the student contribution and other income from students, the final balance sheet and the established budget. The balance sheet refers to the year (T-1)."@en ,
                                       "Dati relativi al gettito della contribuzione studentesca degli atenei, in particolare alla contribuzione studentesca e alle altre entrate provenienti dagli studenti, al conto consuntivo e al bilancio di previsione assestato. Conto consuntivo: riferimento all'anno (T-1)."@it ;
                          rdfs:isDefinedBy <https://w3id.org/italia/onto/HER> ;
                          rdfs:label "Aggregazione dei ricavi del contributo riportato da USTAT"@it ,
                                     "USTAT Aggregate of Contribution Revenue"@en .


###  https://w3id.org/italia/onto/HER/USTATContributionRevenueClass
:USTATContributionRevenueClass rdf:type owl:Class ;
                               rdfs:subClassOf l0:Characteristic ;
                               rdfs:comment """Information on the source of the student contribution revenue. In particular, the identifier/extended name shows the code/description of the revenue, respectively, which may consist of the values:
01 : Revenue related to degree courses, master's degree courses, courses of the old system
02 : Revenue related to PhD courses
03 : Revenue related to specialisation courses;
040: Revenue related to first and second level master's courses
041: Revenue related to courses for the purpose of teaching qualification
04a: Revenue related to other course fees
04b: Revenue related to improvement courses
05 : Regional tax for the Right to University Study - DSU (if collected by the university)
06a: Revenue related to state exams, internships and pre-registration tests
07 : Other income not required for registration
08 : Other from students, not constituent revenue.
"""@en ,
                                            """Informazioni sulla fonte del gettito della contribuzione studentesca. In particolare, l'identificativo/nome esteso riportano il codice/la descrizione del gettito, rispettivamente, e possono essumere i valori:
01 : Gettito relativo a corsi di laurea, corsi di laurea magistrale, corsi del vecchio ordinamento
02 : Gettito relativo a corsi di dottorato
03 : Gettito relativo a corsi di specializzazione
040: Gettito relativo a corsi di master di primo e secondo livello
041: Gettito relativo a corsi finalizzati all'abilitazione all'insegnamento
04a: Gettito relativo ad altri corsi
04b: Gettito relativo a corsi di perfezionamento
05 : Tassa regionale per il DSU (se riscossa da università)
06a: Gettito esami di stato, tirocini e test pre-immatricolazioni
07 : Altre entrate non necessarie per l'iscrizione
08 : Altro da studenti, non costituente gettito"""@it ;
                               rdfs:isDefinedBy <https://w3id.org/italia/onto/HER> ;
                               rdfs:label "Classe di contribuzione riportata da USTAT"@it ,
                                          "USTAT Reported Contribution Revenue Class"@en .


###  https://w3id.org/italia/onto/HER/USTATEnrolledStudentsAggregate
:USTATEnrolledStudentsAggregate rdf:type owl:Class ;
                                rdfs:subClassOf :StatisticalDataAggregation ,
                                                [ rdf:type owl:Restriction ;
                                                  owl:onProperty covapit:hasOrganization ;
                                                  owl:maxQualifiedCardinality "1"^^xsd:nonNegativeInteger ;
                                                  owl:onClass covapit:Organization
                                                ] ;
                                rdfs:comment "Data on university students' enrolled at universities in good standing with the payment of tuition fees."@en ,
                                             "Dati relativi agli iscritti degli atenei in regola con il pagamento delle tasse universitarie."@it ;
                                rdfs:isDefinedBy <https://w3id.org/italia/onto/HER> ;
                                rdfs:label "Aggregazione degli studenti iscritt riportati da USTAT"@it ,
                                           "USTAT Aggregate of Enrolled Students"@en .


###  https://w3id.org/italia/onto/HER/USTATEnrollment
:USTATEnrollment rdf:type owl:Class ;
                 rdfs:subClassOf :StatisticalDataAggregation ;
                 rdfs:comment """Information on the types of enrollment of the enrolled students of the universities in good standing with the payment of tuition fees. In particular, the identification/extended name shows the code/description of the type of enrollment, respectively and may consist of values:
T1: Total enrolled students
T1a: Total enrolled students - of which PhD students with financial support
T1b: Total enrolled students - of which students with partial coverage of fees from external bodies
T1c: Total number of enrolled students - of which students enrolled part-time"""@en ,
                              """Informazioni sulle tipologie di iscrizione degli iscritti degli atenei in regola con il pagamento delle tasse universitarie. In particolare, l'identificativo/nome esteso riportano il codice/la descrizione della tipologia di iscrizione , rispettivamente, e possono essumere i valori:
T1: Totale iscritti
T1a: Totale iscritti - di cui dottorandi con supporto finanziario
T1b: Totale iscritti - di cui studenti con parziale copertura delle tasse da enti esterni
T1c: Totale iscritti - di cui studenti iscritti a tempo parziale"""@it ;
                 rdfs:isDefinedBy <https://w3id.org/italia/onto/HER> ;
                 rdfs:label "Iscrizioni riportate da USTAT"@it ,
                            "USTAT Reported Enrollment"@en .


###  https://w3id.org/italia/onto/HER/USTATExonerationType
:USTATExonerationType rdf:type owl:Class ;
                      rdfs:subClassOf l0:Characteristic ;
                      rdfs:comment """Information on the type of exemption.
In the case of partial exemption, the exemption types are characterised by the following codes/descriptions:

09: Students with a disability of less than 66% (Legislative Decree 68/12 art. 9, c. 7a)
19: Other disability situations not included in the previous ones
15: Other types not included under the above entries

In the case of total exemption, the types of exemption are characterised by the following codes/descriptions:

01: Scholarship recipients (Legislative Decree 68/12 art. 9, c. 2)
02: Eligible non-beneficiaries of scholarships (Legislative Decree 68/12 art. 9, c. 2)
03: Disabled students with disabilities over 66% (Legislative Decree 68/12 art. 9, c. 2)
16: Students who meet the requirements for NO TAX AREA (Law 232/2016, c. 255 and 256) and Beneficiaries of scholarships d.lgs. 68/12
17: Students who meet the requirements for NO TAX AREA (Law 232/2016, c. 255 and 256) and eligibility for a scholarship d.lgs. 68/12
18: Students with requirements for NO TAX AREA (L. 232/2016, c. 255 and 256)
19: Other disability situations not included in the previous ones
20: Doctoral student holder of a PhD scholarship
21: Doctoral student not holding a PhD scholarship (Law 232/2016, c. 262)
15: Other types not included under the above headings"""@en ,
                                   """Informazioni sulla tipologia di esonero.
Nel caso di esonero parziale, le tipologie di esonero sono caratterizzate dai codici/descrizioni seguenti:

09: Studenti in situazione di disabilità con invalidità inferiore al 66% (d.lgs. 68/12 art. 9, c. 7a)
19: Altre situazioni di disabilità non incluse nelle precedenti
15: Altre tipologie non comprese nelle precedenti voci

Nel caso di esonero totale, le tipologie di esonero sono caratterizzate dai codici/descrizioni seguenti:

01: Beneficiari borse studio (d.lgs. 68/12 art. 9, c. 2)
02: Idonei non beneficiari borse di studio (d.lgs. 68/12 art. 9, c. 2)
03: Studenti in situazione di disabilità con invalidità oltre il 66% (d.lgs. 68/12 art. 9, c. 2)
16: Studenti con compresenza di requisiti per NO TAX AREA (L. 232/2016, c. 255 e 256) e Beneficiari di borsa di studio d.lgs. 68/12
17: Studenti con compresenza di requisiti per NO TAX AREA (L. 232/2016, c. 255 e 256) e Idoneità per borsa di studio d.lgs. 68/12
18: Studenti con requisiti per NO TAX AREA (L. 232/2016, c. 255 e 256)
19: Altre situazioni di disabilità non incluse nelle precedenti
20: Dottorando titolare di borsa di studio di dottorato di ricerca
21: Dottorando non beneficiario di borsa (L. 232/2016, c. 262)
15: Altre tipologie non comprese nelle precedenti voci"""@it ;
                      rdfs:isDefinedBy <https://w3id.org/italia/onto/HER> ;
                      rdfs:label "Tipo (o classe) di esonero riportata da USTAT"@it ,
                                 "USTAT Reported Exoneration Class"@en .


###  https://w3id.org/italia/onto/HER/USTATExpenseClass
:USTATExpenseClass rdf:type owl:Class ;
                   rdfs:subClassOf l0:Characteristic ;
                   rdfs:comment """Codice della spesa per tipologia di intervento. Corrispondono alle tipologie di intervento secondo le relazioni:
1 : Borse di studio - Spesa per borse concesse
2 : Borse di studio - Spesa per borse concesse - di cui Fondo Sociale Europeo
3 : Prestiti di onore e altri prestiti agevolati - Spesa per prestiti concessi
4 : Mobilità internazionale - Spesa per contributi concessi
5 : Interventi a favore di studenti in situazione di handicap - Spesa per interventi concessi
6 : Attività di collaborazione a tempo parziale - Spesa per attività di collaborazioni a tempo parziale
7 : Posti alloggio e contributi-alloggio - Spesa per contributi-alloggio assegnati
8 : Posti alloggio e contributi-alloggio - Spesa per contributi-alloggio assegnati - di cui spesa per contributi a borsisti (non beneficiari di alloggio)
9 : Posti alloggio e contributi-alloggio - Spesa per contributi-alloggio assegnati - di cui spesa per contributi a idonei non borsisti (non beneficiari di alloggio)
10 : Posti alloggio e contributi-alloggio - Spesa per contributi-alloggio assegnati - di cui spesa per contributi a studenti non idonei alla borsa
11 : Altri interventi di tipo finanziario - Spesa per premi per il conseguimento del titolo
12 : Altri interventi di tipo finanziario - Spesa per contributi finanziari per il trasporto
13 : Altri interventi di tipo finanziario - Spesa per contributi straordinari
14 : Altri interventi di tipo finanziario - Spesa per altri sussidi concessi"""@it ,
                                """Spending code by type of intervention. They correspond to the types of intervention according to the reports:
1 : Scholarships - Expenditure for scholarships awarded
2 : Scholarships - Expenditure for grants - of which European Social Fund (Fondo Sociale Europeo)
3 : Honour loans and other subsidised loans - Expenditure on loans granted
4 : International mobility - Expenditure on granted contributions
5 : Interventions in favour of students with disabilities - Expenditure for interventions granted
6 : Part-time collaboration activities - Expenditure for part-time collaboration activities
7 : Accommodation places and accommodation contributions - Expenditure for allocated accommodation contributions
8 : Accommodation and accommodation grants - Expenditure for allocated accommodation grants - of which expenditure for grants to scholarship holders (not beneficiaries of accommodation)
9 : Accommodation and accommodation grants - Expenditure for allocated accommodation grants - of which expenditure for grants to eligible non-scholarship holders (non-beneficiaries of accommodation)
10 : Accommodation places and accommodation contributions - Expenditure for assigned accommodation contributions - of which expenditure for contributions to students not eligible for the grant
11 : Other financial measures - Expenditure on bonuses for obtaining the title
12 : Other financial interventions - Expenditure on financial contributions for transport
13 : Other financial interventions - Expenditure on extraordinary contributions
14 : Other financial interventions - Expenditure on other subsidies granted.
"""@en ;
                   rdfs:isDefinedBy <https://w3id.org/italia/onto/HER> ;
                   rdfs:label "Classe di spese riportata da USTAT"@it ,
                              "USTAT Reported Expense Class"@en .


###  https://w3id.org/italia/onto/HER/USTATFunctionalArea
:USTATFunctionalArea rdf:type owl:Class ;
                     rdfs:subClassOf :HERClassification ;
                     rdfs:comment "Indica l'area a cui fanno riferimento le funzioni del gruppo di personale tecnico-amministrativo considerato. Rappresenta una delle variabili di disaggregazione dei dati sulle carriere del personale tecnico-amministrativo. Attualmente può assumere i seguenti valori: 01-Dirigenza amministrativa; 02-Amministrativa ed Amministrativa-gestionale; 03-Biblioteche; 04-Servizi generali e tecnici; 05-Socio sanitaria; 06-Tecnica; 07-Area non individuata."@it ,
                                  "It indicates the area to which the functions of the technical-administrative staff group considered refer. Represents one of the variables of disaggregation of the career data of technical-administrative staff. Currently it can take on the following values: 01-Dirigenza amministrativa; 02-Amministrativa ed Amministrativa-gestionale; 03-Biblioteche; 04-Servizi generali e tecnici; 05-Socio sanitaria; 06-Tecnica; 07-Area non individuata."@en ;
                     rdfs:isDefinedBy <https://w3id.org/italia/onto/HER> ;
                     rdfs:label "Area funzionale"@it ,
                                "Functional Area"@en ;
                     prov:wasDerivedFrom skos:Concept .


###  https://w3id.org/italia/onto/HER/USTATInterventionExpensesAggregate
:USTATInterventionExpensesAggregate rdf:type owl:Class ;
                                    rdfs:subClassOf :StatisticalDataAggregation ;
                                    rdfs:comment "Information on the expenditure committed for interventions granted to students for each University/Institute managed by each institution for the Right to University Studies (DSU)/Office, for the calendar year of reference."@en ,
                                                 "Informazione sulla spesa impegnata per interventi concessi a studenti per ciascun Ateneo/Istituto gestito da ciascun ente per il DSU/ufficio, per l'anno solare di riferimento."@it ;
                                    rdfs:isDefinedBy <https://w3id.org/italia/onto/HER> ;
                                    rdfs:label "Aggregazione degli interventi di spese universitarie riportate da USTAT"@it ,
                                               "USTAT Aggregate of University Intervention Expenses"@en .


###  https://w3id.org/italia/onto/HER/USTATInterventionsForStudentsByUniversitiesAggregate
:USTATInterventionsForStudentsByUniversitiesAggregate rdf:type owl:Class ;
                                                      rdfs:subClassOf :StatisticalDataAggregation ,
                                                                      [ rdf:type owl:Restriction ;
                                                                        owl:onProperty covapit:hasOrganization ;
                                                                        owl:maxQualifiedCardinality "1"^^xsd:nonNegativeInteger ;
                                                                        owl:onClass covapit:Organization
                                                                      ] ;
                                                      rdfs:comment "Data related to the number of interventions in favour of students (excluding the Right to Study by the regions) carried out by the universities."@en ,
                                                                   "Dati relativi al numero di interventi a favore degli studenti (escluso il Diritto allo Studio regionale) effettuati dagli atenei."@it ;
                                                      rdfs:isDefinedBy <https://w3id.org/italia/onto/HER> ;
                                                      rdfs:label "Aggregazione degli interventi universitari per gli studenti riportati da USTAT"@it ,
                                                                 "USTAT Aggregate of University Interventions For Students"@en .


###  https://w3id.org/italia/onto/HER/USTATMealsProvidedAggregate
:USTATMealsProvidedAggregate rdf:type owl:Class ;
                             rdfs:subClassOf :StatisticalDataAggregation ;
                             rdfs:comment "Meals provided and students who used the canteens in the calendar year of reference."@en ,
                                          "Pasti erogati e studenti che hanno usufruito delle mense nell'anno solare di riferimento."@it ;
                             rdfs:isDefinedBy <https://w3id.org/italia/onto/HER> ;
                             rdfs:label "Aggregazione dei pasti forniti riportati da USTAT"@it ,
                                        "USTAT Aggregate of Meals Provided"@en .


###  https://w3id.org/italia/onto/HER/USTATMeasureOfMealsProvided
:USTATMeasureOfMealsProvided rdf:type owl:Class ;
                             rdfs:subClassOf <https://w3id.org/italia/onto/MU/MeasureType> ;
                             rdfs:comment """Information (code, description and number) on meals provided in the calendar year (T-1). The types are represented by the following codes and descriptions:
11: Meals provided in directly managed canteens
12: Meals provided in indirectly managed canteens
13: Meals provided in contracted catering services
14: Students who use canteens"""@en ,
                                          """Informazioni (codice, descrizione e numero) sui pasti erogati nell'anno solare (T-1). Le tipologie sono rappresentate dai seguenti codici e descrizioni:
11: Pasti erogati in mense a gestione diretta
12: Pasti erogati in mense a gestione indiretta
13: Pasti erogati in servizi di ristorazione convenzionati
14: Studenti che usufruiscono delle mense"""@it ;
                             rdfs:isDefinedBy <https://w3id.org/italia/onto/HER> ;
                             rdfs:label "Misura dei pasti forniti riportati da USTAT"@it ,
                                        "USTAT Reported Measure of Meals Provided"@en .


###  https://w3id.org/italia/onto/HER/USTATPartiallyExoneratedStudentsAggregate
:USTATPartiallyExoneratedStudentsAggregate rdf:type owl:Class ;
                                           rdfs:subClassOf :StatisticalDataAggregation ,
                                                           [ rdf:type owl:Restriction ;
                                                             owl:onProperty covapit:hasOrganization ;
                                                             owl:maxQualifiedCardinality "1"^^xsd:nonNegativeInteger ;
                                                             owl:onClass covapit:Organization
                                                           ] ;
                                           rdfs:comment "Data on students with partial exemption of universities."@en ,
                                                        "Dati relativi agli studenti con esonero parziale degli atenei"@it ;
                                           rdfs:isDefinedBy <https://w3id.org/italia/onto/HER> ;
                                           rdfs:label "Aggregazione degli studenti parzialmente esonerati riportati da USTAT"@it ,
                                                      "USTAT Aggregate of Partially Exonerated Students"@en .


###  https://w3id.org/italia/onto/HER/USTATPermanentStaff
:USTATPermanentStaff rdf:type owl:Class ;
                     rdfs:subClassOf covapit:Group ,
                                     [ rdf:type owl:Restriction ;
                                       owl:onProperty <https://w3id.org/italia/onto/CLV/hasSpatialCoverage> ;
                                       owl:allValuesFrom <https://w3id.org/italia/onto/CLV/Feature>
                                     ] ;
                     rdfs:comment "Personale in servizio a tempo indeterminato negli Enti e negli Uffici per il Diritto allo Studio Universitario - DSU al 31/12 dell'anno di riferimento, aggregato per Regione."@it ,
                                  "Personnel in permanent service in the Entities and Offices for the Right to University Studies - DSU at 31/12 of the year of reference, aggregated by Region."@en ;
                     rdfs:isDefinedBy <https://w3id.org/italia/onto/HER> ;
                     rdfs:label "Permanent Staff"@en ,
                                "Personale Indeterminato"@it .


###  https://w3id.org/italia/onto/HER/USTATPostgraduateAggregateOfEnrolled
:USTATPostgraduateAggregateOfEnrolled rdf:type owl:Class ;
                                      rdfs:subClassOf :StatisticalDataAggregation ,
                                                      [ rdf:type owl:Restriction ;
                                                        owl:onProperty covapit:hasOrganization ;
                                                        owl:maxQualifiedCardinality "1"^^xsd:nonNegativeInteger ;
                                                        owl:onClass covapit:Organization
                                                      ] ;
                                      rdfs:comment "Information about the students enrolled in [Specialisation Schools / Level I Master / Level II Master / Research Doctorates] by university and by course of study (time series)."@en ,
                                                   "Informazioni sugli iscritti a [Scuole di specializzazione/Master di I livello/Master di II livello/Dottorati di ricerca] per ateneo e per corso di studio (serie storica)."@it ;
                                      rdfs:isDefinedBy <https://w3id.org/italia/onto/HER> ;
                                      rdfs:label "Aggregazione USTAT Postgraduate - Iscritti"@it ,
                                                 "USTAT Postgraduate Aggregate of Enrolled"@en .


###  https://w3id.org/italia/onto/HER/USTATPostgraduateAggregateOfGraduated
:USTATPostgraduateAggregateOfGraduated rdf:type owl:Class ;
                                       rdfs:subClassOf :StatisticalDataAggregation ,
                                                       [ rdf:type owl:Restriction ;
                                                         owl:onProperty covapit:hasOrganization ;
                                                         owl:maxQualifiedCardinality "1"^^xsd:nonNegativeInteger ;
                                                         owl:onClass covapit:Organization
                                                       ] ;
                                       rdfs:comment "Information on graduates (of specialization schools, Masters of I and II level, PhDs) by university and by course of study (time series)."@en ,
                                                    "Informazioni sui diplomati di [Scuole di specializzazione/Master di I livello/Master di II livello/Dottorati di ricerca] per corso di studio."@it ;
                                       rdfs:isDefinedBy <https://w3id.org/italia/onto/HER> ;
                                       rdfs:label "Aggregazione USTAT Postgraduate - Diplomati"@it ,
                                                  "USTAT Postgraduate Aggregate of Graduated"@en .


###  https://w3id.org/italia/onto/HER/USTATPostgraduateAggregateOfRegistered
:USTATPostgraduateAggregateOfRegistered rdf:type owl:Class ;
                                        rdfs:subClassOf :StatisticalDataAggregation ,
                                                        [ rdf:type owl:Restriction ;
                                                          owl:onProperty covapit:hasOrganization ;
                                                          owl:maxQualifiedCardinality "1"^^xsd:nonNegativeInteger ;
                                                          owl:onClass covapit:Organization
                                                        ] ;
                                        rdfs:comment "A partire dal XXXI ciclo, i dati sono desunti dall'Anagrafe Nazionale degli Studenti universitari: in questo caso, l'informazione riportata è relativa agli studenti iscritti per ciclo al primo anno del dottorato di ricerca. Fino al XXX ciclo incluso, la fonte dei dati è la \"Rilevazione sull'Istruzione Universititaria\", e l'informazione riportata è relativa al numero di studenti vincitori di concorso, a prescindere dal fatto che si siano in seguito iscritti. Fonte dell'informazione: Informazioni sui file relativi ai Dottorati di Ricerca, sito USTAT-MIUR (http://dati.ustat.miur.it/dataset/formazione-post-laurea/resource/fdee4043-0011-43ef-9f44-ef00e484f0d8) e comunciazione dell'Ufficio di Statistica e Studi - settore Università e Ricerca."@it ,
                                                     "Starting from the XXXI cycle, the data are derived from the National Register of University Students: in this case, the information reported is related to students enrolled per cycle in the first year of the PhD. Up to and including the XXXth cycle, the data source is the \"Universities Education Survey\", and the information reported is related to the number of students who have won the exam, regardless of whether they have subsequently enrolled. Source of information: Information on PhD files, USTAT-MIUR website (http://dati.ustat.miur.it/dataset/formazione-post-laurea/resource/fdee4043-0011-43ef-9f44-ef00e484f0d8) and communication from the Office of Statistics and Studies - University and Research sector."@en ;
                                        rdfs:isDefinedBy <https://w3id.org/italia/onto/HER> ;
                                        rdfs:label "Aggregazione USTAT Postgraduate - Accessi"@it ,
                                                   "USTAT Postgraduate Aggregate of Registered"@en .


###  https://w3id.org/italia/onto/HER/USTATReportedHERInstitution
:USTATReportedHERInstitution rdf:type owl:Class ;
                             rdfs:subClassOf covapit:PublicOrganization ;
                             rdfs:comment "Information (identification code, name, typology) of the Institute under consideration (University, Istituto Alta Formazione Artistica e Musicale - AFAM, Scuola Superiore per Mediatori Linguistici, Other)."@en ,
                                          "Informazioni (codice identificativo, nome, tipologia) dell'Istituto in questione (Ateneo, Istituto Alta Formazione Artistica e Musicale - AFAM, Scuola Superiore per Mediatori Linguistici, Altro)."@it ;
                             rdfs:isDefinedBy <https://w3id.org/italia/onto/HER> ;
                             rdfs:label "Istituzione HER riportate da USTAT"@it ,
                                        "USTAT Reported HER Institution"@en .


###  https://w3id.org/italia/onto/HER/USTATReportedPostgraduateCourse
:USTATReportedPostgraduateCourse rdf:type owl:Class ;
                                 rdfs:subClassOf l0:Object ,
                                                 [ rdf:type owl:Restriction ;
                                                   owl:onProperty :ustatCourseType ;
                                                   owl:maxCardinality "1"^^xsd:nonNegativeInteger
                                                 ] ;
                                 rdfs:comment "Corsi di studio di formazione Post-Laurea; in questo dataset, si può riferire a Scuole di specializzazione/Master di I livello/Master di II livello/Dottorati di ricerca."@it ,
                                              "Postgraduate education courses; in this dataset, it can be referred to Specialization Schools / Masters of I Level / Masters of II Level / Research Doctorates."@en ;
                                 rdfs:isDefinedBy <https://w3id.org/italia/onto/HER> ;
                                 rdfs:label "Corsi di specializzazione riportati da USTAT"@it ,
                                            "USTAT Reported Postgraduate Course"@en ;
                                 owl:versionInfo "stabile"@it ,
                                                 "stable"@en .


###  https://w3id.org/italia/onto/HER/USTATReportedUniversityFacilityType
:USTATReportedUniversityFacilityType rdf:type owl:Class ;
                                     rdfs:subClassOf l0:Characteristic ,
                                                     [ rdf:type owl:Restriction ;
                                                       owl:onProperty l0:description ;
                                                       owl:someValuesFrom rdfs:Literal
                                                     ] ,
                                                     [ rdf:type owl:Restriction ;
                                                       owl:onProperty l0:identifier ;
                                                       owl:someValuesFrom rdfs:Literal
                                                     ] ;
                                     rdfs:comment "Strutture degli atenei: mense e posti alloggio direttamente gestiti dagli Atenei."@it ,
                                                  "University structures: canteens and accommodation places directly managed by the universities."@en ;
                                     rdfs:isDefinedBy <https://w3id.org/italia/onto/HER> ;
                                     rdfs:label "Tipo struttura universitá riportata da USTAT"@it ,
                                                "USTAT Reported Facility of University Type"@en .


###  https://w3id.org/italia/onto/HER/USTATStaffByGender
:USTATStaffByGender rdf:type owl:Class ;
                    rdfs:subClassOf :StatisticalDataAggregation ,
                                    [ rdf:type owl:Restriction ;
                                      owl:onProperty covapit:hasOrganization ;
                                      owl:maxQualifiedCardinality "1"^^xsd:nonNegativeInteger ;
                                      owl:onClass covapit:Organization
                                    ] ,
                                    [ rdf:type owl:Restriction ;
                                      owl:onProperty :ageClass ;
                                      owl:maxCardinality "1"^^xsd:nonNegativeInteger
                                    ] ;
                    rdfs:comment """Data on the careers of teaching and research staff from a gender perspective. The data concern full professors, associate professors, researchers and research grant holders and are disaggregated by gender, age group, university, geographical area, field of research and development and grade. Data are available as of 2012. Whenever possible, the descriptions have been derived from the Record Sheet for the time series on university staff provided by USTAT - Open data.

Data at the 31/12 of the reference year."""@en ,
                                 """Dati sulle carriere del personale docente e ricercatore in un'ottica di genere. I dati riguardano professori ordinari, professori associati, ricercatori e titolari di assegni di ricerca e sono disaggregati per genere, classe di età, ateneo, area geografica, field of research and development e grade. I dati sono disponibili a partire dal 2012. Quando possibile, le descrizioni sono state derivate dal Tracciato record per la serie storica sul personale universitario fornito dal USTAT - Open data.

Dati al 31/12 dell'anno di riferimento."""@it ;
                    rdfs:isDefinedBy <https://w3id.org/italia/onto/HER> ;
                    rdfs:label "Aggrazione per genere dello Staff riportata da USTAT"@it ,
                               "USTAT Reported Aggregate of Staff By Sex"@en .


###  https://w3id.org/italia/onto/HER/USTATStaffType
:USTATStaffType rdf:type owl:Class ;
                rdfs:subClassOf <https://w3id.org/italia/onto/RO/Role> ;
                rdfs:comment """Information on the personnel in service in the Entities and Offices for the Right to University Studies - DSU, aggregated by Region. In particular:
- information on personnel on permanent service in the entities and offices for the DSU as of 31/12 of the year of reference, aggregated by Region;
- information on staff serving on a fixed-term contract in the entities and offices for the DSU in the reference year, aggregated by Region."""@en ,
                             """Informazioni sul personale in servizio negli Enti e negli Uffici per il DSU, aggregato per Regione. In particolare:
- informazioni sul personale in servizio a tempo indeterminato negli Enti e negli Uffici per il DSU al 31/12 dell'anno di riferimento, aggregato per Regione;
- informazioni sul personale che ha prestato servizio a tempo determinato negli Enti e negli Uffici per il DSU nell'anno di riferimento, aggregato per Regione"""@it ;
                rdfs:isDefinedBy <https://w3id.org/italia/onto/HER> ;
                rdfs:label "Italian University Staff Role"@en ,
                           "Ruolo del personale universitario italiano"@it ;
                prov:wasDerivedFrom skos:Concept .


###  https://w3id.org/italia/onto/HER/USTATStudentsBySexAggregate
:USTATStudentsBySexAggregate rdf:type owl:Class ;
                             rdfs:subClassOf :StatisticalDataAggregation ,
                                             [ rdf:type owl:Restriction ;
                                               owl:onProperty covapit:hasOrganization ;
                                               owl:maxQualifiedCardinality "1"^^xsd:nonNegativeInteger ;
                                               owl:onClass covapit:Organization
                                             ] ;
                             rdfs:comment "Data on the student population from a gender perspective. The data concern students, graduates, PhDs and PhDs. The data are available from the academic year 2012/2013. Where possible, the descriptions have been derived from the Record Sheet for the Student time Series provided by USTAT - Open data."@en ,
                                          "Dati sulla popolazione studentesca in un'ottica di genere. I dati riguardano student-i/-esse, laureat-i/-e, dottorand-i/-e e dottori di ricerca. I dati sono disponibili a partire dall'anno accademico 2012/2013. Quando possibile, le descrizioni sono state derivate dal Tracciato record per la serie storica sugli studenti fornito dal USTAT - Open data."@it ;
                             rdfs:isDefinedBy <https://w3id.org/italia/onto/HER> ;
                             rdfs:label "Aggregazione degli studenti per genere riportati da USTAT"@it ,
                                        "USTAT Aggregate of Students By Sex"@en .


###  https://w3id.org/italia/onto/HER/USTATTAStaffByGender
:USTATTAStaffByGender rdf:type owl:Class ;
                      rdfs:subClassOf :StatisticalDataAggregation ;
                      rdfs:comment "Data on the careers of technical-administrative staff from a gender perspective. The data concern technical-administrative personnel with permanent and fixed-term contracts and are broken down by gender, university, geographical area, type of contract and functional area. The data are available from 2012."@en ,
                                   "Dati sulle carriere del personale tecnico-amministrativo in un'ottica di genere. I dati riguardano il personale tecnico-amministrativo con contratto a tempo indeterminato e determinato e sono disaggregati per genere, ateneo, area geografica, tipologia di contratto e area funzionale. I dati sono disponibili a partire dal 2012."@it ;
                      rdfs:isDefinedBy <https://w3id.org/italia/onto/HER> ;
                      rdfs:label "Aggregazione di Staff TA per genere riportato da USTAT"@it ,
                                 "USTAT Reported Aggregate of TA Staff By Sex"@en .


###  https://w3id.org/italia/onto/HER/USTATTemporaryStaff
:USTATTemporaryStaff rdf:type owl:Class ;
                     rdfs:subClassOf covapit:Group ,
                                     [ rdf:type owl:Restriction ;
                                       owl:onProperty <https://w3id.org/italia/onto/CLV/hasSpatialCoverage> ;
                                       owl:allValuesFrom <https://w3id.org/italia/onto/CLV/Feature>
                                     ] ;
                     rdfs:comment "Personale che ha prestato servizio a tempo determinato negli Enti e negli Uffici per il Diritto allo Studio Universitario - DSU nell'anno di riferimento, aggregato per Regione."@it ,
                                  "Personnel who have served on a temporary basis in the Bodies and Offices for the Right to University Studies - DSU in the year of reference, aggregated by Region."@en ;
                     rdfs:isDefinedBy <https://w3id.org/italia/onto/HER> ;
                     rdfs:label "Personale Determinato"@it ,
                                "Temporary Staff"@en .


###  https://w3id.org/italia/onto/HER/USTATTotallyExoneratedStudentsAggregate
:USTATTotallyExoneratedStudentsAggregate rdf:type owl:Class ;
                                         rdfs:subClassOf :StatisticalDataAggregation ,
                                                         [ rdf:type owl:Restriction ;
                                                           owl:onProperty covapit:hasOrganization ;
                                                           owl:maxQualifiedCardinality "1"^^xsd:nonNegativeInteger ;
                                                           owl:onClass covapit:Organization
                                                         ] ;
                                         rdfs:comment "Data on totally exempted students by type of exemption. Data referring to the Academic year (T-1)/(T)."@en ,
                                                      "Dati relativi agli studenti esonerati totalmente per tipologia di esonero. Dati riferiti all'anno Accademico (T-1)/(T)."@it ;
                                         rdfs:isDefinedBy <https://w3id.org/italia/onto/HER> ;
                                         rdfs:label "Aggregazione degli studenti totalmente esonerati riportati da USTAT"@it ,
                                                    "USTAT Aggregate of Totally Exonerated Students"@en .


###  https://w3id.org/italia/onto/HER/USTATUniversityExpenseClass
:USTATUniversityExpenseClass rdf:type owl:Class ;
                             rdfs:subClassOf l0:Characteristic ;
                             rdfs:comment """Information on the expenditure for interventions in favor of students (student loans only) of the universities by type. Data are related to the financial year (T-1). The types of intervention are classified according to the following code/descriptions:
51 : SECTION 3 - LOANS PROVIDED BY CONVENTIONED CREDIT INSTITUTIONS - Amount of loans
52 : SECTION 3 - LOANS PROVIDED BY CONVENTIONED CREDIT INSTITUTIONS - Guarantee Fund
53 : section 3 - loans provided by conventioned credit institutions - amount of interest and/or capital contributions to be paid by the University"""@en ,
                                          """Informazioni sulla spesa per interventi a favore degli studenti (solo prestiti a studenti) degli atenei per tipologia. I dati sono relativi all'esercizio finanziario all'anno (T-1). Le tipologie di intervento sono classificate secondo i codici/descrizioni seguenti:
51    : SEZIONE 3 - PRESTITI EROGATI DA ISTITUTI DI CREDITO CONVENZIONATI - Ammontare dei prestiti
52    : SEZIONE 3 - PRESTITI EROGATI DA ISTITUTI DI CREDITO CONVENZIONATI - Fondo di garanzia
53    : SEZIONE 3 - PRESTITI EROGATI DA ISTITUTI DI CREDITO CONVENZIONATI - Ammontare contributi in conto interesse e/o conto capitale a carico dell'Ateneo"""@it ;
                             rdfs:isDefinedBy <https://w3id.org/italia/onto/HER> ;
                             rdfs:label "Classe di spese universitarie riportate da USTAT"@it ,
                                        "USTAT Reported University Expense Class"@en .


###  https://w3id.org/italia/onto/HER/USTATUniversityFacilitiesAggregate
:USTATUniversityFacilitiesAggregate rdf:type owl:Class ;
                                    rdfs:subClassOf :StatisticalDataAggregation ,
                                                    [ rdf:type owl:Restriction ;
                                                      owl:onProperty :availableSlot ;
                                                      owl:maxCardinality "1"^^xsd:nonNegativeInteger
                                                    ] ;
                                    rdfs:comment "Data on the facilities of the universities: canteens and accommodation places directly managed by the universities."@en ,
                                                 "Dati relativi alle strutture degli atenei: mense e posti alloggio direttamente gestiti dagli Atenei."@it ;
                                    rdfs:label "Aggregato USTAT delle strutture universitarie"@it ,
                                               "USTAT Aggregate of University Facilities"@en .


###  https://w3id.org/italia/onto/HER/USTATUniversityInterventionExpensesAggregate
:USTATUniversityInterventionExpensesAggregate rdf:type owl:Class ;
                                              rdfs:subClassOf :StatisticalDataAggregation ,
                                                              [ rdf:type owl:Restriction ;
                                                                owl:onProperty covapit:hasOrganization ;
                                                                owl:maxQualifiedCardinality "1"^^xsd:nonNegativeInteger ;
                                                                owl:onClass covapit:Organization
                                                              ] ;
                                              rdfs:comment "Data on expenditure on interventions in favour of university students (student loans only)."@en ,
                                                           "Dati relativi alla spesa per interventi a favore degli studenti degli atenei (solo prestiti a studenti)."@it ;
                                              rdfs:isDefinedBy <https://w3id.org/italia/onto/HER> ;
                                              rdfs:label "Aggregazione delle spese di interventi universitari riportati da USTAT"@it ,
                                                         "USTAT Aggregate of University Intervention Expenses"@en .


###  https://w3id.org/italia/onto/HER/USTATUniversityInterventionType
:USTATUniversityInterventionType rdf:type owl:Class ;
                                 rdfs:subClassOf l0:Characteristic ,
                                                 [ rdf:type owl:Restriction ;
                                                   owl:onProperty l0:description ;
                                                   owl:cardinality "1"^^xsd:nonNegativeInteger
                                                 ] ,
                                                 [ rdf:type owl:Restriction ;
                                                   owl:onProperty l0:identifier ;
                                                   owl:cardinality "1"^^xsd:nonNegativeInteger
                                                 ] ;
                                 rdfs:comment """Tipologia di intervento effettuato dall'ateneo. La tipologia è definita dai codici/descrizioni di seguito:
030 : Borse di studio - N. borse di studio concesse con fondi dell'ATENEO (escluse le borse post-laurea riportate nell'apposita sezione)
061 : Mobilità internazionale - N. iscritti nell'ateneo coinvolti in programmi di mobilità internazionale (studenti in uscita)
061c : Mobilità internazionale - N. iscritti nell'ateneo coinvolti in programmi di mobilità internazionale (studenti in uscita) - di cui studenti SENZA borsa
061m : Mobilità internazionale - N. iscritti nell'ateneo coinvolti in programmi di mobilità internazionale (studenti in uscita) - di cui studenti in mobilità extraeuropea
061p : Mobilità internazionale - N. iscritti nell'ateneo coinvolti in programmi di mobilità internazionale (studenti in uscita) - di cui dottorandi percettori di borsa che usufruiscono della maggiorazione del 50%
063 : Mobilità internazionale - N. iscritti in atenei esteri coinvolti in programmi di mobilità internazionale presso l'ateneo italiano (studenti in entrata)
063c : Mobilità internazionale - N. iscritti in atenei esteri coinvolti in programmi di mobilità internazionale presso l'ateneo italiano (studenti in entrata) - di cui studenti con borsa dell'Ateneo italiano
064 : Mobilità internazionale - N. iscritti in atenei esteri coinvolti in programmi di mobilità internazionale presso l'ateneo italiano (studenti in entrata) - di cui studenti provenienti da Paesi extraeuropei
073 : Interventi a favore di studenti in situazione di disabilità - N. contributi finanziari
074 : Interventi a favore di studenti in situazione di disabilità - N. interventi non finanziari
081 : Attività di collaborazione a tempo parziale - N. collaborazioni
091 : Posti alloggio e contributi-alloggio - N. domande posti alloggio
092 : Posti alloggio e contributi-alloggio - N. posti alloggio assegnati
092c : Posti alloggio e contributi-alloggio - N. posti alloggio assegnati - di cui assegnati in strutture convenzionate o private
093 : Posti alloggio e contributi-alloggio - N. domande contributi-alloggio
094 : Posti alloggio e contributi-alloggio - N. contributi-alloggio assegnati
101 : Altri interventi di tipo finanziario - N. prestiti agevolati concessi da istituti di credito convenzionati
101a : Altri interventi di tipo finanziario - N. prestiti agevolati concessi da istituti di credito convenzionati - di cui con contributo in conto interesse e/o in conto capitale a carico dell'Ateneo
104 : Altri interventi di tipo finanziario - N. altri sussidi erogati
111a : Borse di studio post-lauream - N. borse finanziate con fondi MIUR
111b : Borse di studio post-lauream - N. borse finanziate da altri Ministeri
112 : Borse di studio post-lauream - N. borse finanziate dall'Ateneo con fondi propri
113 : Borse di studio post-lauream - N. borse finanziate mediante convenzione con altri Atenei
114 : Borse di studio post-lauream - N. borse finanziate con fondi UE
115 : Borse di studio post-lauream - N. borse finanziate mediante convenzione con altri enti pubblici
116 : Borse di studio post-lauream - N. borse finanziate mediante convenzione con enti privati"""@it ,
                                              """Type of intervention carried out by the university. The typology is defined by the codes/descriptions below:
030 : Scholarships - No. of scholarships awarded with funds from the University (excluding post-graduate scholarships listed in the appropriate section)
061 : International mobility - No. of students enrolled at the university involved in international mobility programmes (outgoing students)
061c : International mobility - No. enrolled at the university involved in international mobility programmes (outgoing students) - of which students WITHOUT a grant
061m : International mobility - No. of students enrolled at the university involved in international mobility programmes (outgoing students) - of which students on mobility outside Europe
061p : International mobility - No. of students enrolled at the university involved in international mobility programmes (outgoing students) - of which PhD students who are grant recipients benefiting from the 50% surcharge
063 : International mobility - No. enrolled in foreign universities involved in international mobility programs at the Italian university (incoming students)
063c : International mobility - No. enrolled in foreign universities involved in international mobility programs at the Italian athenaeum (incoming students) - of which students with a scholarship from the Italian university
064 : International mobility - No. enrolled in foreign universities involved in international mobility programs at the Italian university (incoming students) - of which students from non-European countries
073 : Interventions in favour of students with disabilities - No. of financial contributions
074 : Interventions in favour of students with disabilities - No. of non-financial interventions
081 : Part-time collaboration activities - No. of collaborations
091 : Accommodation places and accommodation contributions - No. of applications for accommodation places
092 : Accommodation and accommodation contributions - No. of accommodation places allocated
092c : Accommodation places and accommodation contributions - No. of accommodation places allocated - of which allocated in contracted or private facilities
093 : Accommodation places and accommodation contributions - No. of accommodation contributions applications
094 : Accommodation and accommodation contributions - No. of accommodation contributions allocated
101 : Other financial measures - No. of subsidised loans granted by credit institutions under agreement
101a : Other financial measures - No. of subsidized loans granted by credit institutions - of which with an interest rate and/or capital contribution borne by the University
104 : Other financial interventions - No. of other subsidies granted
111a : Post-graduate scholarships - No. of scholarships financed by MIUR funds
111b : Post-graduate scholarships - No. of scholarships funded by other Ministries
112 : Post-graduate scholarships - No. of scholarships financed by the University from its own funds
113 : Post-graduate scholarships - No. of scholarships financed by agreement with other universities
114 : Post-graduate scholarships - No. of EU-funded scholarships
115 : Post-graduate scholarships - No. of grants financed by agreement with other public bodies
116 : Post-graduate scholarships - No. of scholarships financed by agreement with private bodies"""@en ;
                                 rdfs:isDefinedBy <https://w3id.org/italia/onto/HER> ;
                                 rdfs:label "Tipo (o classe) di interventi universitari riportati da USTAT"@it ,
                                            "USTAT Reported University Intervention Class"@en ;
                                 owl:versionInfo "stabile"@it ,
                                                 "stable"@en .


###  https://w3id.org/italia/onto/HER/WIPOIPCClass
:WIPOIPCClass rdf:type owl:Class ;
              rdfs:subClassOf :InternationalPatentClassification ;
              rdfs:comment "In each classification symbol, the section (first letter) combined with a two digit number represents the \"class\"."@en ,
                           "In ogni simbolo di classificazione, la sezione (prima lettera) combinata con un numero di due cifre rappresenta la \"classe\"."@it ;
              rdfs:isDefinedBy <https://w3id.org/italia/onto/HER> ;
              rdfs:label "Classe IPC WIPO"@it ,
                         "WIPO IPC Class"@en ;
              prov:wasDerivedFrom skos:Concept .


###  https://w3id.org/italia/onto/HER/WIPOIPCMainGroup
:WIPOIPCMainGroup rdf:type owl:Class ;
                  rdfs:subClassOf :InternationalPatentClassification ;
                  rdfs:comment "La sottoclasse è seguita da un numero di \"gruppo\" composto da una a tre cifre, un tratto obliquo e un numero di almeno due cifre che rappresentano un \"gruppo principale\" o \"sottogruppo\"."@it ,
                               "The subclass is followed by a one-to-three-digit \"group\" number, an oblique stroke and a number of at least two digits representing a \"main group\" or \"subgroup\"."@en ;
                  rdfs:isDefinedBy <https://w3id.org/italia/onto/HER> ;
                  rdfs:label "Gruppo principale WIPO ipc"@it ,
                             "WIPO IPC Main Group"@en ;
                  prov:wasDerivedFrom skos:Concept .


###  https://w3id.org/italia/onto/HER/WIPOIPCSection
:WIPOIPCSection rdf:type owl:Class ;
                rdfs:subClassOf :InternationalPatentClassification ;
                rdfs:comment "La prima lettera di ogni simbolo di classificazione rappresenta la \"sezione\" costituita da una lettera da A (\"Necessità umane\") a H (\"Elettricità\")."@it ,
                             "The first letter of each classification symbol represents the \"section\" consisting of a letter from A (\"Human Necessities\") to H (\"Electricity\")."@en ;
                rdfs:isDefinedBy <https://w3id.org/italia/onto/HER> ;
                rdfs:label "Sezione IPC WIPO"@it ,
                           "WIPO IPC Section"@en ;
                prov:wasDerivedFrom skos:Concept .


###  https://w3id.org/italia/onto/HER/WIPOIPCSubclass
:WIPOIPCSubclass rdf:type owl:Class ;
                 rdfs:subClassOf :InternationalPatentClassification ;
                 rdfs:comment "In each classification symbol, the letter following the class (two digit number after the initial letter) makes up the \"subclass\"."@en ,
                              "In ogni simbolo di classificazione, la lettera che segue la classe (numero di due cifre dopo la lettera iniziale) costituisce la \"sottoclasse\"."@it ;
                 rdfs:isDefinedBy <https://w3id.org/italia/onto/HER> ;
                 rdfs:label "Sottoclasse WIPO IPC"@it ,
                            "WIPO IPC Subclass"@en ;
                 prov:wasDerivedFrom skos:Concept .


###  https://w3id.org/italia/onto/HER/WIPOIPCSubgroup
:WIPOIPCSubgroup rdf:type owl:Class ;
                 rdfs:subClassOf :InternationalPatentClassification ;
                 rdfs:comment "La sottoclasse è seguita da un numero di \"gruppo\" composto da una a tre cifre, un tratto obliquo e un numero di almeno due cifre che rappresentano un \"gruppo principale\" o \"sottogruppo\"."@it ,
                              "The subclass is followed by a one-to-three-digit \"group\" number, an oblique stroke and a number of at least two digits representing a \"main group\" or \"subgroup\"."@en ;
                 rdfs:isDefinedBy <https://w3id.org/italia/onto/HER> ;
                 rdfs:label "Sottogruppo WIPO IPC"@it ,
                            "WIPO IPC Subgroup"@en ;
                 prov:wasDerivedFrom skos:Concept .


###  https://w3id.org/italia/onto/POI/PointOfInterest
<https://w3id.org/italia/onto/POI/PointOfInterest> rdf:type owl:Class .


###  https://w3id.org/italia/onto/Project/PublicInvestmentProject
<https://w3id.org/italia/onto/Project/PublicInvestmentProject> rdf:type owl:Class .


###  https://w3id.org/italia/onto/Project/PublicResearchProject
<https://w3id.org/italia/onto/Project/PublicResearchProject> rdf:type owl:Class ;
                                                             rdfs:subClassOf [ rdf:type owl:Restriction ;
                                                                               owl:onProperty :abstract ;
                                                                               owl:allValuesFrom rdfs:Literal
                                                                             ] .


###  https://w3id.org/italia/onto/RO/Role
<https://w3id.org/italia/onto/RO/Role> rdf:type owl:Class .


###  https://w3id.org/italia/onto/RO/TimeIndexedRole
<https://w3id.org/italia/onto/RO/TimeIndexedRole> rdf:type owl:Class .


###  https://w3id.org/italia/onto/l0/Activity
l0:Activity rdf:type owl:Class .


###  https://w3id.org/italia/onto/l0/Collection
l0:Collection rdf:type owl:Class .


###  https://w3id.org/italia/onto/l0/Concept
l0:Concept rdf:type owl:Class .


###  https://w3id.org/italia/onto/l0/Description
l0:Description rdf:type owl:Class .


###  https://w3id.org/italia/onto/l0/Object
l0:Object rdf:type owl:Class .


###  https://w3id.org/italia/onto/l0/Topic
l0:Topic rdf:type owl:Class .


#################################################################
#    Individuals
#################################################################

###  https://w3id.org/italia/data/contact-point/onto-agid
<https://w3id.org/italia/data/contact-point/onto-agid> rdf:type owl:NamedIndividual ,
                                                                dcatapit:Organization ,
                                                                vcard:Kind ,
                                                                vcard:Organization ;
                                                       vcard:fn "banche dati e open data" ;
                                                       vcard:hasEmail <mailto:info@dati.gov.it> .


###  https://w3id.org/italia/data/distribution/HERAPIT-JSON-LD
<https://w3id.org/italia/data/distribution/HERAPIT-JSON-LD> rdf:type owl:NamedIndividual ,
                                                                     admsapit:SemanticAssetDistribution ;
                                                            dct:description "Questa è la distribuzione JSON-LD dell'ontologia della Ricerca Pubblica"@it ,
                                                                            "This is the distribution in JSON-LD of the Public Research ontology"@en ;
                                                            dct:format <http://publications.europa.eu/resource/authority/file-type/JSON_LD> ;
                                                            dct:license <https://w3id.org/italia/controlled-vocabulary/licences/A21_CCBY40> ;
                                                            dct:title "Distribuzione JSON-LD ontologia PublicReseach-AP_IT"@it ,
                                                                      "JSON-LD distribution of PublicReseach-AP_IT Ontology"@en ;
                                                            dcat:accessURL <https://raw.githubusercontent.com/italia/daf-ontologie-vocabolari-controllati/master/Ontologie/HER/latest> ;
                                                            dcat:downloadURL <https://raw.githubusercontent.com/italia/daf-ontologie-vocabolari-controllati/master/Ontologie/HER/latest/HER-AP_IT.jsonld> .


###  https://w3id.org/italia/data/distribution/HERAPIT-RDF-TURTLE
<https://w3id.org/italia/data/distribution/HERAPIT-RDF-TURTLE> rdf:type owl:NamedIndividual ,
                                                                        admsapit:SemanticAssetDistribution ;
                                                               dct:description "Questa è la distribuzione RDF/Turtle dell'ontologia della Ricerca Pubblica"@it ,
                                                                               "This is the distribution in RDF/turtle of the Public Research ontology"@en ;
                                                               dct:format <http://publications.europa.eu/resource/authority/file-type/RDF_TURTLE> ;
                                                               dct:license <https://w3id.org/italia/controlled-vocabulary/licences/A21_CCBY40> ;
                                                               dct:title "Distribuzione RDF/Turtle ontologia PublicReseach-AP_IT"@it ,
                                                                         "RDF/Turtle distribution of PublicReseach-AP_IT Ontology"@en ;
                                                               dcat:accessURL <https://raw.githubusercontent.com/italia/daf-ontologie-vocabolari-controllati/master/Ontologie/HER/latest> ;
                                                               dcat:downloadURL <https://raw.githubusercontent.com/italia/daf-ontologie-vocabolari-controllati/master/Ontologie/HER/latest/HER-AP_IT.ttl> .


###  https://w3id.org/italia/data/distribution/HERAPIT-RDF-XML
<https://w3id.org/italia/data/distribution/HERAPIT-RDF-XML> rdf:type owl:NamedIndividual ,
                                                                     admsapit:SemanticAssetDistribution ;
                                                            dct:description "Questa è la distribuzione RDF/XML dell'ontologia della Ricerca Pubblica"@it ,
                                                                            "This is the distribution in RDF/XML of the Public Research ontology"@en ;
                                                            dct:format <http://publications.europa.eu/resource/authority/file-type/RDF_XML> ;
                                                            dct:license <https://w3id.org/italia/controlled-vocabulary/licences/A21_CCBY40> ;
                                                            dct:title "Distribuzione RDF/XML ontologia PublicReseach-AP_IT"@it ,
                                                                      "RDF/XML distribution of PublicReseach-AP_IT Ontology"@en ;
                                                            dcat:accessURL <https://raw.githubusercontent.com/italia/daf-ontologie-vocabolari-controllati/master/Ontologie/HER/latest> ;
                                                            dcat:downloadURL <https://raw.githubusercontent.com/italia/daf-ontologie-vocabolari-controllati/master/Ontologie/HER/latest/HER-AP_IT.rdf> .


###  https://w3id.org/italia/data/private-organization/siris
<https://w3id.org/italia/data/private-organization/siris> rdf:type owl:NamedIndividual ,
                                                                   dcatapit:Agent ,
                                                                   foaf:Agent ;
                                                          dct:identifier "siris" ;
                                                          foaf:name "SIRIS"@en ,
                                                                    "SIRIS"@it .


###  https://w3id.org/italia/data/private-organization/03033080213
<https://w3id.org/italia/data/private-organization/03033080213> rdf:type owl:NamedIndividual ,
                                                                         dcatapit:Agent ,
                                                                         foaf:Agent ;
                                                                dct:identifier "03033080213" ;
                                                                foaf:name "ONTOPIC"@en ,
                                                                          "ONTOPIC"@it .


###  https://w3id.org/italia/data/project/OntoPiA
<https://w3id.org/italia/data/project/OntoPiA> rdf:type owl:NamedIndividual ,
                                                        admsapit:Project ;
                                               l0:name "OntoPiA - la rete di ontologie della pubblica amministrazione italiana"@it .


###  https://w3id.org/italia/data/project/toscana-open-research
<https://w3id.org/italia/data/project/toscana-open-research> rdf:type owl:NamedIndividual ,
                                                                      admsapit:Project ;
                                                             l0:name "Toscana Open Research"@it .


###  https://w3id.org/italia/data/public-organization/agid
<https://w3id.org/italia/data/public-organization/agid> rdf:type owl:NamedIndividual ,
                                                                 dcatapit:Agent ,
                                                                 foaf:Agent ;
                                                        dct:identifier "agid" ;
                                                        foaf:name "Agenzia per l'Italia Digitale"@it ,
                                                                  "Italian Digital Agency"@en .


###  https://w3id.org/italia/data/public-organization/r_toscan
<https://w3id.org/italia/data/public-organization/r_toscan> rdf:type owl:NamedIndividual ,
                                                                     dcatapit:Agent ,
                                                                     foaf:Agent ;
                                                            dct:identifier "r_toscan" ;
                                                            foaf:name "Regione Toscana"@it ,
                                                                      "Toscany Region"@en .


###  https://w3id.org/italia/onto/HER
<https://w3id.org/italia/onto/HER> rdf:type owl:NamedIndividual ,
                                            admsapit:SemanticAsset .


###  https://w3id.org/italia/onto/HER/HES
:HES rdf:type owl:NamedIndividual ,
              :ECActivityType ;
     rdfs:isDefinedBy <https://w3id.org/italia/onto/HER> ;
     rdfs:label "Higher or Secondary Education Establishments"@en ;
     owl:versionInfo "stabile"@it ,
                     "stable"@en .


###  https://w3id.org/italia/onto/HER/Italian
:Italian rdf:type owl:NamedIndividual ,
                  :ReportedCitizenship ;
         rdfs:isDefinedBy <https://w3id.org/italia/onto/HER> ;
         rdfs:label "Italian"@en ,
                    "Italiana"@it ;
         owl:versionInfo "stabile"@it ,
                         "stable"@en .


###  https://w3id.org/italia/onto/HER/NotItalian
:NotItalian rdf:type owl:NamedIndividual ,
                     :ReportedCitizenship ;
            rdfs:isDefinedBy <https://w3id.org/italia/onto/HER> ;
            rdfs:label "Non Italiana"@it ,
                       "Not Italian"@en ;
            owl:versionInfo "stabile"@it ,
                            "stable"@en .


###  https://w3id.org/italia/onto/HER/OTH
:OTH rdf:type owl:NamedIndividual ,
              :ECActivityType ;
     rdfs:isDefinedBy <https://w3id.org/italia/onto/HER> ;
     rdfs:label "Other"@en ;
     owl:versionInfo "stabile"@it ,
                     "stable"@en .


###  https://w3id.org/italia/onto/HER/PRC
:PRC rdf:type owl:NamedIndividual ,
              :ECActivityType ;
     rdfs:isDefinedBy <https://w3id.org/italia/onto/HER> ;
     rdfs:label "Private for-profit entities (excluding Higher or Secondary Education Establishments)"@en ;
     owl:versionInfo "stabile"@it ,
                     "stable"@en .


###  https://w3id.org/italia/onto/HER/PUB
:PUB rdf:type owl:NamedIndividual ,
              :ECActivityType ;
     rdfs:isDefinedBy <https://w3id.org/italia/onto/HER> ;
     rdfs:label "Public bodies (excluding Research Organisations and Secondary or Higher Education Establishments)"@en ;
     owl:versionInfo "stabile"@it ,
                     "stable"@en .


###  https://w3id.org/italia/onto/HER/REC
:REC rdf:type owl:NamedIndividual ,
              :ECActivityType ;
     rdfs:isDefinedBy <https://w3id.org/italia/onto/HER> ;
     rdfs:label "Research Organisations"@en ;
     owl:versionInfo "stabile"@it ,
                     "stable"@en .


[ owl:maxQualifiedCardinality "1"^^xsd:nonNegativeInteger
] .

#################################################################
#    Annotations
#################################################################

:CTNMIUREntity rdfs:label "Istituzione finanziata CTN/PRIN"@it .


:CTNMIURExpense rdfs:label "Spese"@it .


:CTNMIURInitiative rdfs:label "iniziative"@it .


:CTNMIURLocation rdfs:label "ubicazione dell'istituzione finanziata CTN/PRIN"@it .


:CTNMIUROffice rdfs:label "Ufficio dell'istituzione finanziata CTN/PRIN"@it .


:CTNMIUROperation rdfs:label "Operazione"@it .


:CTNMIURProject rdfs:label "Progetto CTN/PRIN"@it .


:CooperativePatentClassification rdfs:label "Classificazione dei brevetti cooperativi"@it ;
                                 rdfs:comment "La Cooperative Patent Classification (CPC) è un'estensione dell'IPC ed è gestita congiuntamente dall'EPO e dall'Ufficio brevetti e marchi degli Stati Uniti. È diviso in nove sezioni, A-H e Y, che a loro volta sono suddivise in classi, sottoclassi, gruppi e sottogruppi. (Fonte: https://www.epo.org/searching-for-patents/helpful-resources/first-time-here/classification/cpc.html)"@it ;
                                 rdfs:label "Cooperative Patent Classification"@en ;
                                 rdfs:comment "The Cooperative Patent Classification (CPC) is an extension of the IPC and is jointly managed by the EPO and the US Patent and Trademark Office. It is divided into nine sections, A-H and Y, which in turn are sub-divided into classes, sub-classes, groups and sub-groups. (Source: https://www.epo.org/searching-for-patents/helpful-resources/first-time-here/classification/cpc.html)"@en .


:DataVoc rdfs:comment "Questa classe raggruppa i vocabolari specifici del set di dati."@it ,
                      "This class groups dataset-specific vocabularies."@en ;
         rdfs:label "Data Vocabulary"@en ,
                    "Vocabolario dei dati"@it .


:DisplinaryClassification rdfs:label "Disciplinary Classification"@en ,
                                     "Classificazione disciplinaria"@it ;
                          rdfs:comment "This class groups different discipline-based classifications."@en ,
                                       "Questa classe raggruppa diverse classificazioni basate sulla disciplina."@it .


:EC-Classification rdfs:label "Classificazione CE"@it ,
                              "EC Classification"@en .


:EC-ResearchTopic rdfs:label "EC Research Topic"@en ,
                             "argomento di ricerca CE"@it .


:FoundationDate rdfs:comment "It indicates the year of foundation of the spin-off."@en ,
                             "Indica l'anno di fondazione dello spin-off."@it .


:KeywordInProject rdfs:comment "A keyword attached to a project."@en ;
                  rdfs:label "Keyword"@en ,
                             "Parola chiave"@it ;
                  rdfs:comment "Una parola chiave allegata a un progetto."@it .


:MIUR-Classification rdfs:label "MIUR Classification"@en ;
                     rdfs:comment "Questa classe raggruppa le classificazioni pubblicate dal MIUR."@it ;
                     rdfs:label "Classificazione del MIUR"@it ;
                     rdfs:comment "This class groups classifications published by the MIUR."@en .


:MIUR-DegreeArea rdfs:label "Italian Degree Area"@en ,
                            "Area di laurea italiana"@it .


:MIUR-DegreeClass rdfs:label "Classe di laurea italiana"@it ;
                  rdfs:comment "A group of several university courses that share same knowledge goals."@en ;
                  rdfs:label "Italian Degree Class"@en ;
                  rdfs:comment "Un gruppo di diversi corsi universitari che condividono gli stessi obiettivi di conoscenza."@it .


:MIUR-MacroSector rdfs:comment """Distinzione disciplinare utilizzata in Italia per organizzare l'istruzione superiore,
Secondo il decreto ministeriale 855 del 30 ottobre 2015, i macrosettori sono 88."""@it ,
                               """Disciplinary distinction used in Italy to organize higher education,
According to the Ministerial Decree 855 of 30 October 2015, there are 88 macro-sectors."""@en .


:MIUR-Reified rdfs:label "MIUR Reported Aggregate"@en ;
              rdfs:comment "Raggruppa tutti i diversi dati aggregati del MIUR."@it ;
              rdfs:label "Aggregato riportato dal MIUR"@it ;
              rdfs:comment "Groups together all the different aggregated data from the MIUR."@en .


:MIUR-SSD rdfs:comment """Si riferisce ai Settori Scientifici Disciplinari (SSD). Questi settori sono raggruppati in diverse aree di \"concorrenza\".
Secondo il decreto ministeriale 855 del 30 ottobre 2015, 367 settori scientifico-disciplinari."""@it ,
                       """It refers to Disciplinary Scientific Sectors (SSD). These sectors are grouped in several “competition” areas.
According to the Ministerial Decree 855 of 30 October 2015, 367 scientific-disciplinary sectors."""@en .


:PatentClassification rdfs:label "Classificazione dei brevetti"@it ,
                                 "Patent Classification"@en .


:PersonInResearch rdfs:comment "Una persona coinvolta in attività di ricerca."@it ,
                               "A person involved in research activities."@en ;
                  rdfs:label "Person in Research"@en ,
                             "Persona nella ricerca"@it .


:ResearchOutput rdfs:label "Risultato della ricerca"@it ,
                           "Research Output"@en ;
                rdfs:comment "Un risultato di un'attività di ricerca. Ad esempio: una pubblicazione, un brevetto, ecc."@it ,
                             "A result of a research activity. For instance: a publication, a patent, etc."@en .


:SCOPUS-Category rdfs:label "Scopus Category"@en ,
                            "Categoria di Scopus"@it .


:SCOPUS-Classification rdfs:label "Scopus Classification"@en ,
                                  "Classificazione di Scopus"@it .


:SCOPUS-SpecificSubject rdfs:label "Scopus Specific Subject"@en ,
                                   "Soggetto specifico di Scopus"@it .


:SCOPUS-SubjectArea rdfs:label "Scopus Subject Area"@en ,
                               "Area del soggetto di Scopus"@it .


:SpinoffFacility rdfs:label "Struttura della spinoff"@it .


:StaffRole rdfs:comment "The role a staff member plays within an organization."@en ,
                        "Il ruolo di un membro dello staff all'interno di un'organizzazione."@it .


:Student rdfs:comment "Questa classe raggruppa diverse classificazioni nazionali degli studenti."@it ;
         rdfs:label "Studente italiano"@it ,
                    "Student"@en ;
         rdfs:comment "This class groups different national classifications of students."@en .


:USTAT-UniversityFacilities rdfs:label "Aggregazione delle strutture universitarie riportate da USTAT"@it ;
                            rdfs:comment "Dati relativi alle strutture degli atenei: mense e posti alloggio direttamente gestiti dagli Atenei."@it ;
                            rdfs:label "USTAT Reported Aggregate of University Facilities"@en ;
                            rdfs:comment "Data on the facilities of the universities: canteens and accommodation places directly managed by the universities."@en .


:USTATAverageContribution rdfs:label "Contribuzione media"@it .


:USTATCanteenAccommodation rdfs:label "Alloggi mensa"@it .


:USTATEnrolledStudent rdfs:label "Aggregazione di studenti iscritti riportati da USTAT"@it .


:USTATEntity rdfs:label "Agente di finanziamento segnalato dall'USTAT"@it .


:USTATFacility rdfs:label "Struttura dell'universitá"@it .


:USTATInstitution rdfs:label "Istituzione riportata da USTAT"@it .


:USTATInstitutionStudentByGender rdfs:label "Aggregazione per genere degli studenti riportata da USTAT"@it .


:USTATIntervention rdfs:label "Intervento universitario"@it .


:USTATInterventionClass rdfs:label "Classe di intervento USTAT"@it .


:USTATInterventionExpense rdfs:label "Spese di intervento universitario"@it .


:USTATPartiallyExoneratedStudent rdfs:label "Studenti parzialmente esonerati"@it .


:USTATProvidedMeal rdfs:label "Pasti forniti"@it .


:USTATStudentByGender rdfs:label "Aggregato di studenti segnalati dall'USTAT per genere"@it .


:USTATTotallyExoneratedStudent rdfs:label "Aggregazione degli studenti totalemente esonerati riportati da USTAT"@it .


:USTATUniversityIntervention rdfs:label "Aggregazione degli interventi universitari riportati da USTAT"@it .


:USTATUniversityIterventionExpense rdfs:label "Aggregazione delle spese di inteventi universitari riportati da USTAT"@it .


:WOS-Category rdfs:label "Categoria WOS"@it ,
                         "WOS Category"@en .


:admissibleCost rdfs:label "costi di ammissione"@it .


:approvedCost rdfs:label "costi approvati"@it .


:committedContribution rdfs:label "contributo impegnato"@it .


:committedCredit rdfs:label "credito impegnato"@it .


:cpcLevel rdfs:label "livello cpcp"@it ;
          rdfs:comment "The numerical value of the level within the CPC hierarchy of a particular classification label."@en ;
          rdfs:label "cpcp level"@en ;
          rdfs:comment "Il valore numerico del livello all'interno della gerarchia CPC di una particolare etichetta di classificazione."@it .


:cpcParent rdfs:comment "The parent of a classification label within the CPC hierarchy. Both the label and its parent are instances of CPC-Classification."@en ,
                        "Genitore di un'etichetta di classificazione nella gerarchia CPC. Sia l'etichetta che il suo genitore sono esempi di classificazione CPC."@it ;
           rdfs:label "has cpc parent classification"@en ,
                      "ha una classificazione brevettuale cpc"@it .


:cunArea rdfs:comment "Questa proprietà è collegata ad un'area disciplinare secondo la classificazione del Consiglio Universitario Nazionale (CUN)."@it ;
         rdfs:label "area CUN"@it ;
         rdfs:comment "This property links to a disciplinary area according to the classification by Consiglio Universitario Nazionale (CUN)."@en ;
         rdfs:label "cun area"@en .


:ecProgramme-ancestorOrSelf rdfs:label "programma EC antenato o autoprogramma CE"@it ;
                            rdfs:comment "Questa proprietà collega ogni programma di finanziamento a entrambi i suoi antenati all'interno della gerarchia del framework program e a se stesso."@it ,
                                         "This property links each funding programme to both its ancestors within the framework's programme hierarchy and itself."@en ;
                            rdfs:label "ancestor-or-self EC programme"@en .


:ercResearchDomain rdfs:comment "Scientific domains to which the 25 ERC panels -used for the planning and operation of the evaluation of ERC grant proposals- are assigned to. They cover all fields of science, engineering and scholarship which, concretely: Social Sciences and Humanities (6 Panels, SH1–SH6), Physical Sciences and Engineering (10 Panels, PE1–PE10), Life Sciences (9 Panels, LS1–LS9)."@en ,
                                """Settori scientifici ai quali sono assegnati i 25 comitati ERC (European Research council) - utilizzati per la pianificazione e il funzionamento della valutazione delle proposte di sovvenzione dell'ERC. Essi coprono tutti i campi della scienza, dell'ingegneria e delle borse di studio che sono, in concreto: Scienze sociali e umanistiche (6 gruppi, SH1-SH6), scienze fisiche e ingegneria (10 gruppi, PE1-PE10), scienze della vita (9 gruppi, LS1-LS9).
"""@it ;
                   rdfs:label "erc research domain"@en ,
                              "dominio di ricerca erc"@it .


:framework rdfs:label "struttura"@it ,
                      "framework"@en .


:hasExpense rdfs:label "ha una spesa"@it .


:hasSpinoffFacility rdfs:label "la spinoff ha una struttura?"@it .


:hasTopic rdfs:comment "Questa proprietà collega un progetto di ricerca a un argomento."@it ;
          rdfs:label "ha un topic"@it ,
                     "has topic"@en ;
          rdfs:comment "This property links a research project with a topic."@en .


:internationalClassificationLabel rdfs:label "international classification label"@en ;
                                  rdfs:comment "The IPC classification symbol."@en ,
                                               "Il simbolo di classificazione IPC."@it ;
                                  rdfs:label "etichetta classificazione internazionale"@it .


:iscedFLevel rdfs:label "isced-f level"@en ;
             rdfs:comment "The numerical value of the level within the ISCED-F classification of a particular classification label."@en ;
             rdfs:label "livello isced-f"@it ;
             rdfs:comment "Il valore numerico del livello all'interno della classificazione ISCED-F di una particolare etichetta di classificazione."@it .


:keyword rdfs:label "parola chiave"@it ,
                    "keyword"@en ;
         rdfs:comment "Questa proprietà collega un'attività finanziata con lo strumento corrispondente."@it ,
                      "This property conects a funded activity with one of its keywords."@en .


:lowercaseTextualValue rdfs:comment "Textual information provided in lower case."@en ,
                                    "Informazioni testuali fornite in minuscolo."@it ;
                       rdfs:label "valore testuale minuscolo"@it ,
                                  "lowercase textual value"@en .


:mapsTo rdfs:comment "Questa proprietà collega due classificazioni correlate."@it ;
        rdfs:label "mappato a"@it ;
        rdfs:comment "This property connects two related classifications."@en ;
        rdfs:label "maps to"@en .


:miurDegreeClass rdfs:comment "Questa proprietà si collega alla corrispondente classe di laurea del sistema educativo italiano."@it ,
                              "This property links to the corresponding degree class in the Italian education system."@en ;
                 rdfs:label "classe di laurea italiana"@it ,
                            "italian degree class"@en .


:miurSSD rdfs:comment "Questa proprietà è collegata ad uno dei \"settori scientifico-disciplinari\" del MIUR."@it ;
         rdfs:label "miur ssd"@en ,
                    "settore scientifico disciplinare del MIUR"@it ;
         rdfs:comment "This property links to one of the MIUR's \"settori scientifico-disciplinari\"."@en .


:officeTypeName rdfs:label "tipo di ufficio"@it .


:organization rdfs:label "organization"@en ;
              rdfs:comment "This property links to an Organization."@en ;
              rdfs:label "organizzazione"@it ;
              rdfs:comment "Questa proprietà si collega a un'organizzazione."@it .


:person rdfs:label "persona"@it ;
        rdfs:comment "This property connects an Academic Affiliation with the corresponding Person."@en ;
        rdfs:label "person"@en ;
        rdfs:comment "Questa proprietà collega un'affiliazione accademica con la persona corrispondente."@it .


:province rdfs:comment "Questa proprietà si collega alla provincia corrispondente."@it ,
                       "This property links to the corresponding province."@en ;
          rdfs:label "province"@en ,
                     "provincia"@it .


:region rdfs:comment "This property links to the corresponding region."@en ;
        rdfs:label "regione"@it ,
                   "region"@en ;
        rdfs:comment "Questa proprietà si collega alla regione corrispondente."@it .


:roleContext rdfs:label "role context"@en ,
                        "contesto di ruolo"@it .


:scopusSpecificSubject rdfs:label "oggetto specifico dello scopus"@it ;
                       rdfs:comment "La classificazione delle materie di Scopus è composta da 295 aree tematiche specifiche raggruppate in 26 aree tematiche"@it ;
                       rdfs:label "scopus specific subject"@en ;
                       rdfs:comment "Scopus' subject classification consisting of 295 specific subject areas grouped into 26 subject areas"@en .


:scopusSubjectAreaCode rdfs:label "codice scopus dell'argomento"@it ,
                                  "scopus subject area code"@en .


:textualValue rdfs:comment "Testo di un termine mesh o parola chiave."@it ,
                           "Text of a mesh term or keyword."@en ;
              rdfs:label "valore testuale"@it ,
                         "textual value"@en .


:totalCost rdfs:comment "Somma di tutti i costi ammissibili sostenuti per il progetto. I costi ammissibili comprendono di norma le seguenti categorie di costi: costi di personale, costi di subappalto, costi di viaggio e di soggiorno, costi di attrezzature e costi di altri beni e servizi. L'importo è espresso in euro."@it ;
           rdfs:label "total cost"@en ,
                      "costi totali"@it ;
           rdfs:comment "Sum of all eligible costs incurred for the project. Eligible costs usually include the following cost categories: personnel costs, sub-contracting costs, travel and subsistence costs, equipment costs and costs of other goods and services. The amount is expressed in euros."@en .


:totalEnrolled rdfs:label "totale iscritti"@it .


:ustatEntity rdfs:label "ha un agente finanziatore riportato in USTAT"@it .


:ustatFacility rdfs:label "l'univesitá ha una struttura"@it .


:ustatInstitution rdfs:label "ha una istituzione riportata da USTAT"@it .


:ustatInterventionClass rdfs:label "ha una classe di inteventi"@it .


:ustatInterventionCode rdfs:label "codice di intervento universitario"@it .


:wipo-ipc-class rdfs:comment "This property connects to the corresponding IPC class."@en ;
                rdfs:label "classe ipc wipo"@it ,
                           "wipo ipc class"@en ;
                rdfs:comment "Questa proprietà si connette alla classe IPC corrispondente."@it .


:wipo-ipc-mainGroup rdfs:comment "Questa proprietà si connette al gruppo principale IPC corrispondente."@it ;
                    rdfs:label "wipo ipc main group"@en ;
                    rdfs:comment "This property connects to the corresponding IPC main group."@en ;
                    rdfs:label "gruppo principale wipo ipc"@it .


:wipo-ipc-section rdfs:comment "This property connects to the corresponding IPC section."@en ,
                               "Questa proprietà si collega alla sezione IPC corrispondente."@it ;
                  rdfs:label "wipo ipc section"@en ,
                             "sezione wipo ipc"@it .


:wipo-ipc-subclass rdfs:comment "This property connects to the corresponding IPC subclass."@en ;
                   rdfs:label "sottoclasse wipo ipc"@it ,
                              "wipo ipc subclass"@en ;
                   rdfs:comment "Questa proprietà si connette alla sottoclasse IPC corrispondente."@it .


:year rdfs:comment "Reference year. Enrolled and PhD students are per academic year (t) - (t+1). Graduates and PhD students are by calendar year (t). The data on Enrolled students refer to the date of July 31st of the year (t+1)."@en ,
                   "Anno di riferimento. Gli Iscritti ed i Dottorandi sono per anno accademico (t) - (t+1). I Laureati ed i Dottori di ricerca sono per anno solare (t). I dati sugli Iscritti sono riferiti alla data del 31 luglio dell'anno (t+1)."@it .


###  Generated by the OWL API (version 4.5.9.2019-02-01T07:24:44Z) https://github.com/owlcs/owlapi
